<?xml version="1.0"?>
<rdf:RDF xmlns="https://purl.archive.org/oquo#"
     xml:base="https://purl.archive.org/oquo"
     xmlns:dc="http://purl.org/dc/elements/1.1/"
     xmlns:obo="http://purl.obolibrary.org/obo/"
     xmlns:owl="http://www.w3.org/2002/07/owl#"
     xmlns:rdf="http://www.w3.org/1999/02/22-rdf-syntax-ns#"
     xmlns:xml="http://www.w3.org/XML/1998/namespace"
     xmlns:xsd="http://www.w3.org/2001/XMLSchema#"
     xmlns:om-1="http://www.wurvoc.org/vocabularies/om-1.8/"
     xmlns:rdf1="http://www.cropontology.org/rdf/"
     xmlns:rdfs="http://www.w3.org/2000/01/rdf-schema#"
     xmlns:skos="http://www.w3.org/2004/02/skos/core#"
     xmlns:vann="http://purl.org/vocab/vann/"
     xmlns:terms="http://purl.org/dc/terms/"
     xmlns:oboInOwl="http://www.geneontology.org/formats/oboInOwl#"
     xmlns:QualityModel="http://purl.org/net/QualityModel#">
    <owl:Ontology rdf:about="https://purl.archive.org/oquo"/>
    


    <!-- 
    ///////////////////////////////////////////////////////////////////////////////////////
    //
    // Annotation properties
    //
    ///////////////////////////////////////////////////////////////////////////////////////
     -->

    


    <!-- http://purl.obolibrary.org/obo/IAO_0000111 -->

    <owl:AnnotationProperty rdf:about="http://purl.obolibrary.org/obo/IAO_0000111">
        <obo:IAO_0000111 xml:lang="en">editor preferred term</obo:IAO_0000111>
        <obo:IAO_0000114 rdf:resource="http://purl.obolibrary.org/obo/IAO_0000122"/>
        <obo:IAO_0000115 xml:lang="en">The concise, meaningful, and human-friendly name for a class or property preferred by the ontology developers. (US-English)</obo:IAO_0000115>
        <obo:IAO_0000117 xml:lang="en">PERSON:Daniel Schober</obo:IAO_0000117>
        <obo:IAO_0000119 xml:lang="en">GROUP:OBI:&lt;http://purl.obolibrary.org/obo/obi&gt;</obo:IAO_0000119>
        <rdfs:isDefinedBy rdf:resource="http://purl.obolibrary.org/obo/iao.owl"/>
        <rdfs:label xml:lang="en">editor preferred term</rdfs:label>
    </owl:AnnotationProperty>
    


    <!-- http://purl.obolibrary.org/obo/IAO_0000112 -->

    <owl:AnnotationProperty rdf:about="http://purl.obolibrary.org/obo/IAO_0000112">
        <obo:IAO_0000111 xml:lang="en">example of usage</obo:IAO_0000111>
        <obo:IAO_0000114 rdf:resource="http://purl.obolibrary.org/obo/IAO_0000122"/>
        <obo:IAO_0000115 xml:lang="en">A phrase describing how a term should be used and/or a citation to a work which uses it. May also include other kinds of examples that facilitate immediate understanding, such as widely know prototypes or instances of a class, or cases where a relation is said to hold.</obo:IAO_0000115>
        <obo:IAO_0000117 xml:lang="en">PERSON:Daniel Schober</obo:IAO_0000117>
        <obo:IAO_0000119 xml:lang="en">GROUP:OBI:&lt;http://purl.obolibrary.org/obo/obi&gt;</obo:IAO_0000119>
        <rdfs:isDefinedBy rdf:resource="http://purl.obolibrary.org/obo/iao.owl"/>
        <rdfs:label xml:lang="en">example of usage</rdfs:label>
    </owl:AnnotationProperty>
    


    <!-- http://purl.obolibrary.org/obo/IAO_0000114 -->

    <owl:AnnotationProperty rdf:about="http://purl.obolibrary.org/obo/IAO_0000114">
        <obo:IAO_0000111 xml:lang="en">has curation status</obo:IAO_0000111>
        <obo:IAO_0000117 xml:lang="en">PERSON:Alan Ruttenberg</obo:IAO_0000117>
        <obo:IAO_0000117 xml:lang="en">PERSON:Bill Bug</obo:IAO_0000117>
        <obo:IAO_0000117 xml:lang="en">PERSON:Melanie Courtot</obo:IAO_0000117>
        <rdfs:label xml:lang="en">has curation status</rdfs:label>
    </owl:AnnotationProperty>
    


    <!-- http://purl.obolibrary.org/obo/IAO_0000115 -->

    <owl:AnnotationProperty rdf:about="http://purl.obolibrary.org/obo/IAO_0000115">
        <obo:IAO_0000111 xml:lang="en">definition</obo:IAO_0000111>
        <obo:IAO_0000114 rdf:resource="http://purl.obolibrary.org/obo/IAO_0000122"/>
        <obo:IAO_0000115 xml:lang="en">The official definition, explaining the meaning of a class or property. Shall be Aristotelian, formalized and normalized. Can be augmented with colloquial definitions.</obo:IAO_0000115>
        <obo:IAO_0000116 xml:lang="en">2012-04-05: 
Barry Smith

The official OBI definition, explaining the meaning of a class or property: &apos;Shall be Aristotelian, formalized and normalized. Can be augmented with colloquial definitions&apos;  is terrible.

Can you fix to something like:

A statement of necessary and sufficient conditions explaining the meaning of an expression referring to a class or property.

Alan Ruttenberg

Your proposed definition is a reasonable candidate, except that it is very common that necessary and sufficient conditions are not given. Mostly they are necessary, occasionally they are necessary and sufficient or just sufficient. Often they use terms that are not themselves defined and so they effectively can&apos;t be evaluated by those criteria. 

On the specifics of the proposed definition:

We don&apos;t have definitions of &apos;meaning&apos; or &apos;expression&apos; or &apos;property&apos;. For &apos;reference&apos; in the intended sense I think we use the term &apos;denotation&apos;. For &apos;expression&apos;, I think we you mean symbol, or identifier. For &apos;meaning&apos; it differs for class and property. For class we want documentation that let&apos;s the intended reader determine whether an entity is instance of the class, or not. For property we want documentation that let&apos;s the intended reader determine, given a pair of potential relata, whether the assertion that the relation holds is true. The &apos;intended reader&apos; part suggests that we also specify who, we expect, would be able to understand the definition, and also generalizes over human and computer reader to include textual and logical definition. 

Personally, I am more comfortable weakening definition to documentation, with instructions as to what is desirable. 

We also have the outstanding issue of how to aim different definitions to different audiences. A clinical audience reading chebi wants a different sort of definition documentation/definition from a chemistry trained audience, and similarly there is a need for a definition that is adequate for an ontologist to work with.  </obo:IAO_0000116>
        <obo:IAO_0000117 xml:lang="en">PERSON:Daniel Schober</obo:IAO_0000117>
        <obo:IAO_0000119 xml:lang="en">GROUP:OBI:&lt;http://purl.obolibrary.org/obo/obi&gt;</obo:IAO_0000119>
        <rdfs:isDefinedBy rdf:resource="http://purl.obolibrary.org/obo/iao.owl"/>
        <rdfs:label xml:lang="en">definition</rdfs:label>
    </owl:AnnotationProperty>
    


    <!-- http://purl.obolibrary.org/obo/IAO_0000116 -->

    <owl:AnnotationProperty rdf:about="http://purl.obolibrary.org/obo/IAO_0000116">
        <obo:IAO_0000111 xml:lang="en">editor note</obo:IAO_0000111>
        <obo:IAO_0000114 rdf:resource="http://purl.obolibrary.org/obo/IAO_0000122"/>
        <obo:IAO_0000115 xml:lang="en">An administrative note intended for its editor. It may not be included in the publication version of the ontology, so it should contain nothing necessary for end users to understand the ontology.</obo:IAO_0000115>
        <obo:IAO_0000117 xml:lang="en">PERSON:Daniel Schober</obo:IAO_0000117>
        <obo:IAO_0000119 xml:lang="en">GROUP:OBI:&lt;http://purl.obofoundry.org/obo/obi&gt;</obo:IAO_0000119>
        <rdfs:isDefinedBy rdf:resource="http://purl.obolibrary.org/obo/iao.owl"/>
        <rdfs:label xml:lang="en">editor note</rdfs:label>
    </owl:AnnotationProperty>
    


    <!-- http://purl.obolibrary.org/obo/IAO_0000117 -->

    <owl:AnnotationProperty rdf:about="http://purl.obolibrary.org/obo/IAO_0000117">
        <obo:IAO_0000111 xml:lang="en">term editor</obo:IAO_0000111>
        <obo:IAO_0000114 rdf:resource="http://purl.obolibrary.org/obo/IAO_0000122"/>
        <obo:IAO_0000115 xml:lang="en">Name of editor entering the term in the file. The term editor is a point of contact for information regarding the term. The term editor may be, but is not always, the author of the definition, which may have been worked upon by several people</obo:IAO_0000115>
        <obo:IAO_0000116 xml:lang="en">20110707, MC: label update to term editor and definition modified accordingly. See https://github.com/information-artifact-ontology/IAO/issues/115.</obo:IAO_0000116>
        <obo:IAO_0000117 xml:lang="en">PERSON:Daniel Schober</obo:IAO_0000117>
        <obo:IAO_0000119 xml:lang="en">GROUP:OBI:&lt;http://purl.obolibrary.org/obo/obi&gt;</obo:IAO_0000119>
        <rdfs:isDefinedBy rdf:resource="http://purl.obolibrary.org/obo/iao.owl"/>
        <rdfs:label xml:lang="en">term editor</rdfs:label>
    </owl:AnnotationProperty>
    


    <!-- http://purl.obolibrary.org/obo/IAO_0000119 -->

    <owl:AnnotationProperty rdf:about="http://purl.obolibrary.org/obo/IAO_0000119">
        <obo:IAO_0000111 xml:lang="en">definition source</obo:IAO_0000111>
        <obo:IAO_0000114 rdf:resource="http://purl.obolibrary.org/obo/IAO_0000122"/>
        <obo:IAO_0000115 xml:lang="en">Formal citation, e.g. identifier in external database to indicate / attribute source(s) for the definition. Free text indicate / attribute source(s) for the definition. EXAMPLE: Author Name, URI, MeSH Term C04, PUBMED ID, Wiki uri on 31.01.2007</obo:IAO_0000115>
        <obo:IAO_0000117 xml:lang="en">PERSON:Daniel Schober</obo:IAO_0000117>
        <obo:IAO_0000119 xml:lang="en">Discussion on obo-discuss mailing-list, see http://bit.ly/hgm99w</obo:IAO_0000119>
        <obo:IAO_0000119 xml:lang="en">GROUP:OBI:&lt;http://purl.obolibrary.org/obo/obi&gt;</obo:IAO_0000119>
        <rdfs:isDefinedBy rdf:resource="http://purl.obolibrary.org/obo/iao.owl"/>
        <rdfs:label xml:lang="en">definition source</rdfs:label>
    </owl:AnnotationProperty>
    


    <!-- http://purl.org/dc/elements/1.1/creator -->

    <owl:AnnotationProperty rdf:about="http://purl.org/dc/elements/1.1/creator"/>
    


    <!-- http://purl.org/dc/elements/1.1/description -->

    <owl:AnnotationProperty rdf:about="http://purl.org/dc/elements/1.1/description"/>
    


    <!-- http://purl.org/dc/elements/1.1/title -->

    <owl:AnnotationProperty rdf:about="http://purl.org/dc/elements/1.1/title"/>
    


    <!-- http://purl.org/dc/terms/created -->

    <owl:AnnotationProperty rdf:about="http://purl.org/dc/terms/created"/>
    


    <!-- http://purl.org/dc/terms/license -->

    <owl:AnnotationProperty rdf:about="http://purl.org/dc/terms/license"/>
    


    <!-- http://purl.org/vocab/vann/preferredNamespacePrefix -->

    <owl:AnnotationProperty rdf:about="http://purl.org/vocab/vann/preferredNamespacePrefix"/>
    


    <!-- http://purl.org/vocab/vann/preferredNamespaceUri -->

    <owl:AnnotationProperty rdf:about="http://purl.org/vocab/vann/preferredNamespaceUri"/>
    


    <!-- http://www.cropontology.org/rdf/acronym -->

    <owl:AnnotationProperty rdf:about="http://www.cropontology.org/rdf/acronym">
        <rdfs:label>acronym</rdfs:label>
    </owl:AnnotationProperty>
    


    <!-- http://www.geneontology.org/formats/oboInOwl#hasDbXref -->

    <owl:AnnotationProperty rdf:about="http://www.geneontology.org/formats/oboInOwl#hasDbXref">
        <oboInOwl:hasDbXref>
            <rdf:Description/>
        </oboInOwl:hasDbXref>
        <rdfs:label xml:lang="en">has_dbxref</rdfs:label>
    </owl:AnnotationProperty>
    


    <!-- http://www.geneontology.org/formats/oboInOwl#hasDefinition -->

    <owl:AnnotationProperty rdf:about="http://www.geneontology.org/formats/oboInOwl#hasDefinition">
        <oboInOwl:hasDbXref>
            <rdf:Description/>
        </oboInOwl:hasDbXref>
        <oboInOwl:hasDefinition>
            <rdf:Description/>
        </oboInOwl:hasDefinition>
        <rdfs:comment>we are forced to use the n-ary relation pattern in OWL1.0. For OWL2 we may make this a direct axiom between a class and the string</rdfs:comment>
        <rdfs:label xml:lang="en">has_definition</rdfs:label>
    </owl:AnnotationProperty>
    


    <!-- http://www.geneontology.org/formats/oboInOwl#hasExactSynonym -->

    <owl:AnnotationProperty rdf:about="http://www.geneontology.org/formats/oboInOwl#hasExactSynonym">
        <oboInOwl:hasDbXref>
            <rdf:Description/>
        </oboInOwl:hasDbXref>
        <oboInOwl:hasDbXref>
            <rdf:Description/>
        </oboInOwl:hasDbXref>
        <oboInOwl:hasDefinition>
            <rdf:Description/>
        </oboInOwl:hasDefinition>
        <oboInOwl:hasDefinition>
            <rdf:Description/>
        </oboInOwl:hasDefinition>
        <rdfs:label xml:lang="en">has_exact_synonym</rdfs:label>
    </owl:AnnotationProperty>
    


    <!-- http://www.w3.org/2000/01/rdf-schema#comment -->

    <rdf:Description rdf:about="http://www.w3.org/2000/01/rdf-schema#comment">
        <rdfs:comment>A description of the subject resource.</rdfs:comment>
        <rdfs:isDefinedBy rdf:resource="http://www.w3.org/2000/01/rdf-schema#"/>
        <rdfs:label>comment</rdfs:label>
    </rdf:Description>
    


    <!-- http://www.w3.org/2000/01/rdf-schema#isDefinedBy -->

    <rdf:Description rdf:about="http://www.w3.org/2000/01/rdf-schema#isDefinedBy">
        <rdfs:comment>The defininition of the subject resource.</rdfs:comment>
        <rdfs:isDefinedBy rdf:resource="http://www.w3.org/2000/01/rdf-schema#"/>
        <rdfs:label>isDefinedBy</rdfs:label>
    </rdf:Description>
    


    <!-- http://www.w3.org/2000/01/rdf-schema#label -->

    <rdf:Description rdf:about="http://www.w3.org/2000/01/rdf-schema#label">
        <rdfs:comment>A human-readable name for the subject.</rdfs:comment>
        <rdfs:isDefinedBy rdf:resource="http://www.w3.org/2000/01/rdf-schema#"/>
        <rdfs:label>label</rdfs:label>
    </rdf:Description>
    


    <!-- http://www.w3.org/2004/02/skos/core#definition -->

    <owl:AnnotationProperty rdf:about="http://www.w3.org/2004/02/skos/core#definition">
        <rdfs:isDefinedBy rdf:resource="http://www.w3.org/2004/02/skos/core"/>
        <rdfs:label xml:lang="en">definition</rdfs:label>
        <skos:definition xml:lang="en">A statement or formal explanation of the meaning of a concept.</skos:definition>
    </owl:AnnotationProperty>
    


    <!-- http://www.w3.org/2004/02/skos/core#editorialNote -->

    <owl:AnnotationProperty rdf:about="http://www.w3.org/2004/02/skos/core#editorialNote">
        <rdfs:isDefinedBy rdf:resource="http://www.w3.org/2004/02/skos/core"/>
        <rdfs:label xml:lang="en">editorial note</rdfs:label>
        <skos:definition xml:lang="en">A note for an editor, translator or maintainer of the vocabulary.</skos:definition>
    </owl:AnnotationProperty>
    


    <!-- http://www.w3.org/2004/02/skos/core#note -->

    <owl:AnnotationProperty rdf:about="http://www.w3.org/2004/02/skos/core#note">
        <rdfs:isDefinedBy rdf:resource="http://www.w3.org/2004/02/skos/core"/>
        <rdfs:label xml:lang="en">note</rdfs:label>
        <skos:definition xml:lang="en">A general note, for any purpose.</skos:definition>
        <skos:scopeNote xml:lang="en">This property may be used directly, or as a super-property for more specific note types.</skos:scopeNote>
    </owl:AnnotationProperty>
    


    <!-- http://www.w3.org/2004/02/skos/core#scopeNote -->

    <owl:AnnotationProperty rdf:about="http://www.w3.org/2004/02/skos/core#scopeNote">
        <rdfs:isDefinedBy rdf:resource="http://www.w3.org/2004/02/skos/core"/>
        <rdfs:label xml:lang="en">scope note</rdfs:label>
        <skos:definition xml:lang="en">A note that helps to clarify the meaning and/or the use of a concept.</skos:definition>
    </owl:AnnotationProperty>
    


    <!-- http://www.wurvoc.org/vocabularies/om-1.8/alternative_label -->

    <owl:AnnotationProperty rdf:about="http://www.wurvoc.org/vocabularies/om-1.8/alternative_label">
        <rdfs:label xml:lang="en">alternative label</rdfs:label>
    </owl:AnnotationProperty>
    


    <!-- 
    ///////////////////////////////////////////////////////////////////////////////////////
    //
    // Object Properties
    //
    ///////////////////////////////////////////////////////////////////////////////////////
     -->

    


    <!-- http://ecoinformatics.org/oboe/oboe.1.2/oboe-core.owl#hasMeasurement -->

    <owl:ObjectProperty rdf:about="http://ecoinformatics.org/oboe/oboe.1.2/oboe-core.owl#hasMeasurement">
        <owl:inverseOf rdf:resource="http://ecoinformatics.org/oboe/oboe.1.2/oboe-core.owl#measurementFor"/>
        <rdf:type rdf:resource="http://www.w3.org/2002/07/owl#InverseFunctionalProperty"/>
        <rdfs:domain rdf:resource="http://ecoinformatics.org/oboe/oboe.1.2/oboe-core.owl#Observation"/>
        <rdfs:range rdf:resource="http://ecoinformatics.org/oboe/oboe.1.2/oboe-core.owl#Measurement"/>
        <rdfs:comment>The hasMeasurement property gives the measurements of the observed entity.</rdfs:comment>
        <rdfs:label xml:lang="en">has measurement</rdfs:label>
    </owl:ObjectProperty>
    


    <!-- http://ecoinformatics.org/oboe/oboe.1.2/oboe-core.owl#hasValue -->

    <owl:ObjectProperty rdf:about="http://ecoinformatics.org/oboe/oboe.1.2/oboe-core.owl#hasValue">
        <rdf:type rdf:resource="http://www.w3.org/2002/07/owl#FunctionalProperty"/>
        <rdfs:domain rdf:resource="http://ecoinformatics.org/oboe/oboe.1.2/oboe-core.owl#Measurement"/>
        <rdfs:range rdf:resource="http://ecoinformatics.org/oboe/oboe.1.2/oboe-core.owl#MeasuredValue"/>
        <rdfs:comment>The hasValue property gives the value of the measurement.</rdfs:comment>
        <rdfs:label xml:lang="en">has value</rdfs:label>
    </owl:ObjectProperty>
    


    <!-- http://ecoinformatics.org/oboe/oboe.1.2/oboe-core.owl#measurementFor -->

    <owl:ObjectProperty rdf:about="http://ecoinformatics.org/oboe/oboe.1.2/oboe-core.owl#measurementFor">
        <rdf:type rdf:resource="http://www.w3.org/2002/07/owl#FunctionalProperty"/>
        <rdfs:domain rdf:resource="http://ecoinformatics.org/oboe/oboe.1.2/oboe-core.owl#Measurement"/>
        <rdfs:range rdf:resource="http://ecoinformatics.org/oboe/oboe.1.2/oboe-core.owl#Observation"/>
        <rdfs:comment>The measurementFor property gives the observation (observed entitiy) that a measurement is associated with. Each measurement is for exactly one observation. </rdfs:comment>
        <rdfs:label xml:lang="en">measurement for</rdfs:label>
    </owl:ObjectProperty>
    


    <!-- http://ecoinformatics.org/oboe/oboe.1.2/oboe-core.owl#ofCharacteristic -->

    <owl:ObjectProperty rdf:about="http://ecoinformatics.org/oboe/oboe.1.2/oboe-core.owl#ofCharacteristic">
        <rdf:type rdf:resource="http://www.w3.org/2002/07/owl#FunctionalProperty"/>
        <rdfs:domain rdf:resource="http://ecoinformatics.org/oboe/oboe.1.2/oboe-core.owl#Measurement"/>
        <rdfs:range rdf:resource="http://ecoinformatics.org/oboe/oboe.1.2/oboe-core.owl#Characteristic"/>
        <rdfs:comment>The ofCharacteristic property gives the entity characteristic measured by a measurement.</rdfs:comment>
        <rdfs:label xml:lang="en">of characteristic</rdfs:label>
    </owl:ObjectProperty>
    


    <!-- http://ecoinformatics.org/oboe/oboe.1.2/oboe-core.owl#ofEntity -->

    <owl:ObjectProperty rdf:about="http://ecoinformatics.org/oboe/oboe.1.2/oboe-core.owl#ofEntity">
        <rdf:type rdf:resource="http://www.w3.org/2002/07/owl#FunctionalProperty"/>
        <rdfs:domain rdf:resource="http://ecoinformatics.org/oboe/oboe.1.2/oboe-core.owl#Observation"/>
        <rdfs:range rdf:resource="http://ecoinformatics.org/oboe/oboe.1.2/oboe-core.owl#Entity"/>
        <rdfs:comment>The ofEntity property gives the observed entity of an observation.</rdfs:comment>
        <rdfs:label xml:lang="en">of entity</rdfs:label>
    </owl:ObjectProperty>
    


    <!-- http://purl.org/ipo/core#assetOf -->

    <owl:ObjectProperty rdf:about="http://purl.org/ipo/core#assetOf">
        <rdfs:comment xml:lang="en">Indicates a IssueEntity that is related to the Asset.
This property can be used to facilitate retrieval records of problems related to the Asset.</rdfs:comment>
        <rdfs:isDefinedBy rdf:resource="http://purl.org/ipo/core"/>
        <rdfs:label xml:lang="en">assetOf</rdfs:label>
    </owl:ObjectProperty>
    


    <!-- http://purl.org/ipo/core#causativeAssetOf -->

    <owl:ObjectProperty rdf:about="http://purl.org/ipo/core#causativeAssetOf">
        <rdfs:subPropertyOf rdf:resource="http://purl.org/ipo/core#assetOf"/>
        <owl:inverseOf rdf:resource="http://purl.org/ipo/core#hasCausativeAsset"/>
        <rdfs:comment xml:lang="en">This property relates a Asset with a Issue caused by this Asset. For example, a virus associated with a disease caused by it.</rdfs:comment>
        <rdfs:isDefinedBy rdf:resource="http://purl.org/ipo/core"/>
        <rdfs:label xml:lang="en">causativeAssetOf</rdfs:label>
    </owl:ObjectProperty>
    


    <!-- http://purl.org/ipo/core#hasAsset -->

    <owl:ObjectProperty rdf:about="http://purl.org/ipo/core#hasAsset">
        <rdfs:comment xml:lang="en">Indicates an Asset to IssueEntity, i.e., any &quot;thing&quot; which is related to IssueEntity.</rdfs:comment>
        <rdfs:isDefinedBy rdf:resource="http://purl.org/ipo/core"/>
        <rdfs:label xml:lang="en">hasAsset</rdfs:label>
    </owl:ObjectProperty>
    


    <!-- http://purl.org/ipo/core#hasCausativeAsset -->

    <owl:ObjectProperty rdf:about="http://purl.org/ipo/core#hasCausativeAsset">
        <rdfs:subPropertyOf rdf:resource="http://purl.org/ipo/core#hasAsset"/>
        <rdfs:domain rdf:resource="http://purl.org/ipo/core#Issue"/>
        <rdfs:comment xml:lang="en">Indicates an Asset that is the causer of the Issue.</rdfs:comment>
        <rdfs:isDefinedBy rdf:resource="http://purl.org/ipo/core"/>
        <rdfs:label xml:lang="en">hasCausativeAsset</rdfs:label>
    </owl:ObjectProperty>
    


    <!-- http://purl.org/ipo/core#hasHostAsset -->

    <owl:ObjectProperty rdf:about="http://purl.org/ipo/core#hasHostAsset">
        <rdfs:subPropertyOf rdf:resource="http://purl.org/ipo/core#hasAsset"/>
        <owl:inverseOf rdf:resource="http://purl.org/ipo/core#hostAssetOf"/>
        <rdfs:domain rdf:resource="http://purl.org/ipo/core#Issue"/>
        <rdfs:comment xml:lang="en">Indicates an Asset that is the host (harbourer) of the Issue.</rdfs:comment>
        <rdfs:isDefinedBy rdf:resource="http://purl.org/ipo/core"/>
        <rdfs:label xml:lang="en">hasHostAsset</rdfs:label>
    </owl:ObjectProperty>
    


    <!-- http://purl.org/ipo/core#hostAssetOf -->

    <owl:ObjectProperty rdf:about="http://purl.org/ipo/core#hostAssetOf">
        <rdfs:subPropertyOf rdf:resource="http://purl.org/ipo/core#assetOf"/>
        <rdfs:comment xml:lang="en">Relates an Asset with a Issue that occurs in it.
This property can be used to relate a person with a disease whose the person is where the disease occurs.</rdfs:comment>
        <rdfs:isDefinedBy rdf:resource="http://purl.org/ipo/core"/>
        <rdfs:label xml:lang="en">hostAssetOf</rdfs:label>
    </owl:ObjectProperty>
    


    <!-- http://purl.org/ipo/core#indicatedBy -->

    <owl:ObjectProperty rdf:about="http://purl.org/ipo/core#indicatedBy">
        <owl:inverseOf rdf:resource="http://purl.org/ipo/core#indicates"/>
        <rdfs:comment xml:lang="en">Indicates a Symptom of this Issue.</rdfs:comment>
        <rdfs:isDefinedBy rdf:resource="http://purl.org/ipo/core"/>
        <rdfs:label xml:lang="en">indicatedBy</rdfs:label>
    </owl:ObjectProperty>
    


    <!-- http://purl.org/ipo/core#indicates -->

    <owl:ObjectProperty rdf:about="http://purl.org/ipo/core#indicates">
        <rdfs:domain rdf:resource="http://purl.org/ipo/core#Symptom"/>
        <rdfs:range rdf:resource="http://purl.org/ipo/core#Issue"/>
        <rdfs:comment xml:lang="en">This property relates a Issue indicated by this Symptom.
A Symptom may indicate many Issues, such as a Symptom of fever can indicate many diseases.</rdfs:comment>
        <rdfs:isDefinedBy rdf:resource="http://purl.org/ipo/core"/>
        <rdfs:label xml:lang="en">indicates</rdfs:label>
    </owl:ObjectProperty>
    


    <!-- http://purl.org/net/EvaluationResult#belongsToCategory -->

    <owl:ObjectProperty rdf:about="http://purl.org/net/EvaluationResult#belongsToCategory">
        <rdfs:domain rdf:resource="http://purl.org/net/EvaluationResult#EvaluationSubject"/>
        <rdfs:range rdf:resource="http://purl.org/net/EvaluationResult#SubjectCategory"/>
        <rdfs:comment>Denotes a category of an evaluation subject.</rdfs:comment>
        <rdfs:label>belongsToCategory</rdfs:label>
    </owl:ObjectProperty>
    


    <!-- http://purl.org/net/EvaluationResult#evaluatedSubject -->

    <owl:ObjectProperty rdf:about="http://purl.org/net/EvaluationResult#evaluatedSubject">
        <rdfs:domain rdf:resource="http://purl.org/net/EvaluationResult#Evaluation"/>
        <rdfs:range rdf:resource="http://purl.org/net/EvaluationResult#EvaluationSubject"/>
        <rdfs:comment>Denotes an evaluation subject that is evaluated.</rdfs:comment>
        <rdfs:label>evaluatedSubject</rdfs:label>
    </owl:ObjectProperty>
    


    <!-- http://purl.org/net/EvaluationResult#forMeasure -->

    <owl:ObjectProperty rdf:about="http://purl.org/net/EvaluationResult#forMeasure">
        <rdfs:domain rdf:resource="http://purl.org/net/EvaluationResult#QualityValue"/>
        <rdfs:range rdf:resource="http://purl.org/net/QualityModel#QualityMeasure"/>
        <rdfs:comment>Denotes a quality measure for which a quality value is produced.</rdfs:comment>
        <rdfs:label>forMeasure</rdfs:label>
    </owl:ObjectProperty>
    


    <!-- http://purl.org/net/EvaluationResult#hasSubCategory -->

    <owl:ObjectProperty rdf:about="http://purl.org/net/EvaluationResult#hasSubCategory">
        <rdfs:domain rdf:resource="http://purl.org/net/EvaluationResult#SubjectCategory"/>
        <rdfs:range rdf:resource="http://purl.org/net/EvaluationResult#SubjectCategory"/>
        <rdfs:comment>Denotes a subcategory of a category.</rdfs:comment>
        <rdfs:label>hasSubCategory</rdfs:label>
    </owl:ObjectProperty>
    


    <!-- http://purl.org/net/EvaluationResult#inputData -->

    <owl:ObjectProperty rdf:about="http://purl.org/net/EvaluationResult#inputData">
        <rdfs:domain rdf:resource="http://purl.org/net/EvaluationResult#Evaluation"/>
        <rdfs:range rdf:resource="http://purl.org/net/EvaluationResult#EvaluationData"/>
        <rdfs:comment>Denotes inout data that is used in an evaluation.</rdfs:comment>
        <rdfs:label>inputData</rdfs:label>
    </owl:ObjectProperty>
    


    <!-- http://purl.org/net/EvaluationResult#isMeasuredInUnit -->

    <owl:ObjectProperty rdf:about="http://purl.org/net/EvaluationResult#isMeasuredInUnit">
        <rdfs:domain rdf:resource="http://purl.org/net/EvaluationResult#QualityValue"/>
        <rdfs:range rdf:resource="http://www.wurvoc.org/vocabularies/om-1.8/Unit_of_measure"/>
        <rdfs:comment>Denotes a unit of measure in which a quality value is measured.</rdfs:comment>
        <rdfs:label>isMeasuredInUnit</rdfs:label>
    </owl:ObjectProperty>
    


    <!-- http://purl.org/net/EvaluationResult#isMeasuredOnScale -->

    <owl:ObjectProperty rdf:about="http://purl.org/net/EvaluationResult#isMeasuredOnScale">
        <rdfs:domain rdf:resource="http://purl.org/net/EvaluationResult#QualityValue"/>
        <rdfs:range rdf:resource="http://www.wurvoc.org/vocabularies/om-1.8/Measurement_scale"/>
        <rdfs:comment>Denotes a scale on which a quality value is measured on.</rdfs:comment>
        <rdfs:label>isMeasuredOnScale</rdfs:label>
    </owl:ObjectProperty>
    


    <!-- http://purl.org/net/EvaluationResult#obtainedFrom -->

    <owl:ObjectProperty rdf:about="http://purl.org/net/EvaluationResult#obtainedFrom">
        <rdfs:domain rdf:resource="http://purl.org/net/EvaluationResult#QualityValue"/>
        <rdfs:range rdf:resource="http://purl.org/net/EvaluationResult#Evaluation"/>
        <rdfs:comment>Denotes a quality evaluation from which a quality value is obtained.</rdfs:comment>
        <rdfs:label>obtainedFrom</rdfs:label>
    </owl:ObjectProperty>
    


    <!-- http://purl.org/net/EvaluationResult#performedOn -->

    <owl:ObjectProperty rdf:about="http://purl.org/net/EvaluationResult#performedOn">
        <rdfs:domain rdf:resource="http://purl.org/net/EvaluationResult#Evaluation"/>
        <rdfs:range rdf:resource="http://www.w3.org/2006/time#Instant"/>
        <rdfs:comment>Denotes a time of a quality evaluation.</rdfs:comment>
        <rdfs:label>performedOn</rdfs:label>
    </owl:ObjectProperty>
    


    <!-- http://purl.org/net/EvaluationResult#producedQualityValue -->

    <owl:ObjectProperty rdf:about="http://purl.org/net/EvaluationResult#producedQualityValue">
        <rdfs:domain rdf:resource="http://purl.org/net/EvaluationResult#Evaluation"/>
        <rdfs:range rdf:resource="http://purl.org/net/EvaluationResult#QualityValue"/>
        <rdfs:comment>Denotes a quality value produced in a quality evaluation.</rdfs:comment>
        <rdfs:label>producedQualityValue</rdfs:label>
    </owl:ObjectProperty>
    


    <!-- http://purl.org/net/QualityModel#collaboratesWith -->

    <owl:ObjectProperty rdf:about="http://purl.org/net/QualityModel#collaboratesWith">
        <rdfs:domain rdf:resource="http://purl.org/net/QualityModel#QualityMeasure"/>
        <rdfs:range rdf:resource="http://purl.org/net/QualityModel#QualityMeasure"/>
        <rdfs:comment>Denotes a relationship between two quality measures in which increasing the value of this measure implies increasing the value of another measure.</rdfs:comment>
        <rdfs:label>collaboratesWith</rdfs:label>
    </owl:ObjectProperty>
    


    <!-- http://purl.org/net/QualityModel#damages -->

    <owl:ObjectProperty rdf:about="http://purl.org/net/QualityModel#damages">
        <rdfs:domain rdf:resource="http://purl.org/net/QualityModel#QualityMeasure"/>
        <rdfs:range rdf:resource="http://purl.org/net/QualityModel#QualityMeasure"/>
        <rdfs:comment>Denotes a relationship between two quality measures in which increasing the value of this measure implies decreasing the value of another measure.</rdfs:comment>
        <rdfs:label>damages</rdfs:label>
    </owl:ObjectProperty>
    


    <!-- http://purl.org/net/QualityModel#dependsOn -->

    <owl:ObjectProperty rdf:about="http://purl.org/net/QualityModel#dependsOn">
        <rdfs:domain rdf:resource="http://purl.org/net/QualityModel#QualityMeasure"/>
        <rdfs:range rdf:resource="http://purl.org/net/QualityModel#QualityMeasure"/>
        <rdfs:comment>Denotes a relationship between two quality measures which implies that the values of this measure require that another measure fulfills some conditions.</rdfs:comment>
        <rdfs:label>dependendsOn</rdfs:label>
    </owl:ObjectProperty>
    


    <!-- http://purl.org/net/QualityModel#hasOrdinalScaleItem -->

    <owl:ObjectProperty rdf:about="http://purl.org/net/QualityModel#hasOrdinalScaleItem">
        <rdfs:domain rdf:resource="http://www.wurvoc.org/vocabularies/om-1.8/Ordinal_scale"/>
        <rdfs:range rdf:resource="http://purl.org/net/QualityModel#OrdinalScaleItem"/>
        <rdfs:comment>Denotes an item of an ordinal scale.</rdfs:comment>
        <rdfs:label>hasOrdinalScaleItem</rdfs:label>
    </owl:ObjectProperty>
    


    <!-- http://purl.org/net/QualityModel#hasRankigFunction -->

    <owl:ObjectProperty rdf:about="http://purl.org/net/QualityModel#hasRankigFunction">
        <rdfs:domain rdf:resource="http://www.wurvoc.org/vocabularies/om-1.8/Measurement_scale"/>
        <rdfs:range rdf:resource="http://purl.org/net/QualityModel#RankingFunction"/>
        <rdfs:comment>Denotes a ranking function of a scale.</rdfs:comment>
        <rdfs:label>hasRankingFunction</rdfs:label>
    </owl:ObjectProperty>
    


    <!-- http://purl.org/net/QualityModel#hasScale -->

    <owl:ObjectProperty rdf:about="http://purl.org/net/QualityModel#hasScale">
        <rdfs:domain rdf:resource="http://purl.org/net/QualityModel#QualityMeasure"/>
        <rdfs:range rdf:resource="http://www.wurvoc.org/vocabularies/om-1.8/Measurement_scale"/>
        <rdfs:comment>Denotes a scale a quality measure can be measured on.</rdfs:comment>
        <rdfs:label>hasScale</rdfs:label>
    </owl:ObjectProperty>
    


    <!-- http://purl.org/net/QualityModel#hasSubCharacteristic -->

    <owl:ObjectProperty rdf:about="http://purl.org/net/QualityModel#hasSubCharacteristic">
        <rdfs:domain rdf:resource="http://purl.org/net/QualityModel#QualityCharacteristic"/>
        <rdfs:range rdf:resource="http://purl.org/net/QualityModel#QualityCharacteristic"/>
        <rdfs:comment>Denotes a subcharacteristic of a quality characteristic.</rdfs:comment>
        <rdfs:label>hasSubCharacteristic</rdfs:label>
    </owl:ObjectProperty>
    


    <!-- http://purl.org/net/QualityModel#hasUnitOfMeasurement -->

    <owl:ObjectProperty rdf:about="http://purl.org/net/QualityModel#hasUnitOfMeasurement">
        <rdfs:domain rdf:resource="http://purl.org/net/QualityModel#QualityMeasure"/>
        <rdfs:range rdf:resource="http://www.wurvoc.org/vocabularies/om-1.8/Unit_of_measure"/>
        <rdfs:comment>Denotes a unit of measurement of a quality measure.</rdfs:comment>
        <rdfs:label>hasUnitOfMeasurement</rdfs:label>
    </owl:ObjectProperty>
    


    <!-- http://purl.org/net/QualityModel#isCharacteristicOf -->

    <owl:ObjectProperty rdf:about="http://purl.org/net/QualityModel#isCharacteristicOf">
        <rdfs:domain rdf:resource="http://purl.org/net/QualityModel#QualityCharacteristic"/>
        <rdfs:range rdf:resource="http://purl.org/net/EvaluationResult#SubjectCategory"/>
        <rdfs:comment>Denotes a category of a product, services or actions (e.g., cars, web browsers, investment option) of which this quality characteristic is a characeristic.</rdfs:comment>
        <rdfs:label>isCharacteristicOf</rdfs:label>
    </owl:ObjectProperty>
    


    <!-- http://purl.org/net/QualityModel#isMeasuredWith -->

    <owl:ObjectProperty rdf:about="http://purl.org/net/QualityModel#isMeasuredWith">
        <rdfs:domain rdf:resource="http://purl.org/net/QualityModel#QualityCharacteristic"/>
        <rdfs:range rdf:resource="http://purl.org/net/QualityModel#QualityMeasure"/>
        <rdfs:comment>Denotes a quality measure that is used for measuring a quality characteristic.</rdfs:comment>
        <rdfs:label>isMeasuredWith</rdfs:label>
    </owl:ObjectProperty>
    


    <!-- http://purl.org/net/QualityModel#isUsedToObtain -->

    <owl:ObjectProperty rdf:about="http://purl.org/net/QualityModel#isUsedToObtain">
        <rdfs:domain rdf:resource="http://purl.org/net/QualityModel#QualityMeasure"/>
        <rdfs:range rdf:resource="http://purl.org/net/QualityModel#QualityMeasure"/>
        <rdfs:comment>Denotes a quality measure that is used to obtain (calculate) this quality measure.</rdfs:comment>
        <rdfs:label>isUsedToObtain</rdfs:label>
    </owl:ObjectProperty>
    


    <!-- http://purl.org/net/QualityModel#measuresCharacteristic -->

    <owl:ObjectProperty rdf:about="http://purl.org/net/QualityModel#measuresCharacteristic">
        <rdfs:domain rdf:resource="http://purl.org/net/QualityModel#QualityMeasure"/>
        <rdfs:range rdf:resource="http://purl.org/net/QualityModel#QualityCharacteristic"/>
        <rdfs:comment>Denotes a quality characteristic that is measured with a quality measure.</rdfs:comment>
        <rdfs:label>measuresCharacteristic</rdfs:label>
    </owl:ObjectProperty>
    


    <!-- http://www.w3.org/2002/07/owl#topObjectProperty -->

    <rdf:Description rdf:about="http://www.w3.org/2002/07/owl#topObjectProperty">
        <rdfs:comment>The object property that relates every two individuals.</rdfs:comment>
        <rdfs:isDefinedBy rdf:resource="http://www.w3.org/2002/07/owl#"/>
        <rdfs:label>topObjectProperty</rdfs:label>
    </rdf:Description>
    


    <!-- http://www.w3.org/2006/time#hasTime -->

    <owl:ObjectProperty rdf:about="http://www.w3.org/2006/time#hasTime">
        <rdfs:range rdf:resource="http://www.w3.org/2006/time#Instant"/>
        <rdfs:comment xml:lang="es">Proporciona soporte a la asociación de una entidad temporal (instante o intervalo) a cualquier cosa.</rdfs:comment>
        <rdfs:comment xml:lang="en">Supports the association of a temporal entity (instant or interval) to any thing</rdfs:comment>
        <rdfs:label xml:lang="en">has time</rdfs:label>
        <rdfs:label xml:lang="es">tiene tiempo</rdfs:label>
        <skos:definition xml:lang="es">Proporciona soporte a la asociación de una entidad temporal (instante o intervalo) a cualquier cosa.</skos:definition>
        <skos:definition xml:lang="en">Supports the association of a temporal entity (instant or interval) to any thing</skos:definition>
        <skos:editorialNote xml:lang="es">Característica arriesgada -añadida en la revisión del 2017 que no ha sido todavía utilizada de forma amplia.</skos:editorialNote>
        <skos:editorialNote xml:lang="en">Feature at risk - added in 2017 revision, and not yet widely used. </skos:editorialNote>
    </owl:ObjectProperty>
    


    <!-- https://purl.archive.org/oquo#hasDetectedIssue -->

    <owl:ObjectProperty rdf:about="https://purl.archive.org/oquo#hasDetectedIssue">
        <rdfs:domain rdf:resource="http://purl.org/net/EvaluationResult#Evaluation"/>
        <rdfs:range rdf:resource="http://purl.org/ipo/core#Issue"/>
        <oboInOwl:hasExactSynonym>has detected problem</oboInOwl:hasExactSynonym>
        <rdfs:comment>Links evaluations or observations to the issues that have been detected.</rdfs:comment>
        <rdfs:label>has detected issue</rdfs:label>
    </owl:ObjectProperty>
    


    <!-- https://purl.archive.org/oquo#hasObservation -->

    <owl:ObjectProperty rdf:about="https://purl.archive.org/oquo#hasObservation">
        <rdfs:subPropertyOf rdf:resource="http://www.w3.org/2002/07/owl#topObjectProperty"/>
        <rdfs:range rdf:resource="http://ecoinformatics.org/oboe/oboe.1.2/oboe-core.owl#Observation"/>
        <rdfs:comment>Relates something with an observation</rdfs:comment>
        <rdfs:label>has observation</rdfs:label>
    </owl:ObjectProperty>
    


    <!-- https://purl.archive.org/oquo#lexicalRegularityExhibitedBy -->

    <owl:ObjectProperty rdf:about="https://purl.archive.org/oquo#lexicalRegularityExhibitedBy">
        <rdfs:subPropertyOf rdf:resource="http://www.w3.org/2002/07/owl#topObjectProperty"/>
        <rdfs:comment>Link a lexical regularity with the classes that exhibit it.</rdfs:comment>
        <rdfs:label>lexicalRegularityExhibitedBy</rdfs:label>
    </owl:ObjectProperty>
    


    <!-- https://purl.archive.org/oquo#measuresCharacteristicNegatively -->

    <owl:ObjectProperty rdf:about="https://purl.archive.org/oquo#measuresCharacteristicNegatively">
        <rdfs:subPropertyOf rdf:resource="http://purl.org/net/QualityModel#measuresCharacteristic"/>
        <rdfs:comment>Denotes a quality characteristic that is measured with a quality measure, where high values of the quality measure impact negatively on the quality measure.</rdfs:comment>
        <rdfs:label>measuresCharacteristicNegatively</rdfs:label>
    </owl:ObjectProperty>
    


    <!-- https://purl.archive.org/oquo#measuresCharacteristicPositively -->

    <owl:ObjectProperty rdf:about="https://purl.archive.org/oquo#measuresCharacteristicPositively">
        <rdfs:subPropertyOf rdf:resource="http://purl.org/net/QualityModel#measuresCharacteristic"/>
        <rdfs:comment>Denotes a quality characteristic that is measured with a quality measure, where high values of the quality measure impact positively on the quality measure.</rdfs:comment>
        <rdfs:label>measuresCharacteristicPositively</rdfs:label>
    </owl:ObjectProperty>
    


    <!-- 
    ///////////////////////////////////////////////////////////////////////////////////////
    //
    // Data properties
    //
    ///////////////////////////////////////////////////////////////////////////////////////
     -->

    


    <!-- http://purl.org/dc/elements/1.1/description -->

    <owl:DatatypeProperty rdf:about="http://purl.org/dc/elements/1.1/description"/>
    


    <!-- http://purl.org/dc/elements/1.1/title -->

    <owl:DatatypeProperty rdf:about="http://purl.org/dc/elements/1.1/title"/>
    


    <!-- http://purl.org/net/EvaluationResult#hasLiteralValue -->

    <owl:DatatypeProperty rdf:about="http://purl.org/net/EvaluationResult#hasLiteralValue">
        <rdfs:domain rdf:resource="http://purl.org/net/EvaluationResult#QualityValue"/>
        <rdfs:range rdf:resource="http://www.w3.org/2000/01/rdf-schema#Literal"/>
        <rdfs:comment>Denotes a literal value of a quality value.</rdfs:comment>
        <rdfs:label>hasLiteralValue</rdfs:label>
    </owl:DatatypeProperty>
    


    <!-- http://purl.org/net/QualityModel#hasLabel -->

    <owl:DatatypeProperty rdf:about="http://purl.org/net/QualityModel#hasLabel">
        <rdfs:domain>
            <owl:Class>
                <owl:unionOf rdf:parseType="Collection">
                    <rdf:Description rdf:about="http://purl.org/net/QualityModel#OrdinalScaleItem"/>
                    <rdf:Description rdf:about="http://www.wurvoc.org/vocabularies/om-1.8/Nominal_scale"/>
                </owl:unionOf>
            </owl:Class>
        </rdfs:domain>
        <rdfs:range rdf:resource="http://www.w3.org/2001/XMLSchema#string"/>
        <rdfs:comment>Denotes a label of a nominal scale or of an ordinal scale item.</rdfs:comment>
        <rdfs:label>hasLabel</rdfs:label>
    </owl:DatatypeProperty>
    


    <!-- http://purl.org/net/QualityModel#hasLowerBoundary -->

    <owl:DatatypeProperty rdf:about="http://purl.org/net/QualityModel#hasLowerBoundary">
        <rdfs:domain rdf:resource="http://www.wurvoc.org/vocabularies/om-1.8/Cardinal_scale"/>
        <rdfs:range rdf:resource="http://www.w3.org/2001/XMLSchema#decimal"/>
        <rdfs:comment>Denotes a lower limit of a scale (e.g., -273 on Kelvin scale).</rdfs:comment>
        <rdfs:label>hasLowerBoundary</rdfs:label>
    </owl:DatatypeProperty>
    


    <!-- http://purl.org/net/QualityModel#hasOrder -->

    <owl:DatatypeProperty rdf:about="http://purl.org/net/QualityModel#hasOrder">
        <rdfs:domain rdf:resource="http://purl.org/net/QualityModel#OrdinalScaleItem"/>
        <rdfs:range rdf:resource="http://www.w3.org/2001/XMLSchema#int"/>
        <rdfs:comment>Denotes an order of an ordinal scale item in relation to a set of items of an ordinal scale.</rdfs:comment>
        <rdfs:label>hasOrder</rdfs:label>
    </owl:DatatypeProperty>
    


    <!-- http://purl.org/net/QualityModel#hasUpperBoundary -->

    <owl:DatatypeProperty rdf:about="http://purl.org/net/QualityModel#hasUpperBoundary">
        <rdfs:domain rdf:resource="http://www.wurvoc.org/vocabularies/om-1.8/Cardinal_scale"/>
        <rdfs:range rdf:resource="http://www.w3.org/2001/XMLSchema#decimal"/>
        <rdfs:comment>Denotes an upper limit of a scale.</rdfs:comment>
        <rdfs:label>hasUpperBoundary</rdfs:label>
    </owl:DatatypeProperty>
    


    <!-- http://purl.org/net/QualityModel#symbol -->

    <owl:DatatypeProperty rdf:about="http://purl.org/net/QualityModel#symbol">
        <rdfs:domain rdf:resource="http://www.wurvoc.org/vocabularies/om-1.8/Unit_of_measure"/>
        <rdfs:range rdf:resource="http://www.w3.org/2001/XMLSchema#string"/>
        <rdfs:comment>Denotes a symbol of a unit of measure.</rdfs:comment>
        <rdfs:label>symbol</rdfs:label>
    </owl:DatatypeProperty>
    


    <!-- https://www.omg.org/spec/Commons/TextDatatype/hasTextValue -->

    <owl:DatatypeProperty rdf:about="https://www.omg.org/spec/Commons/TextDatatype/hasTextValue">
        <rdfs:label>has text value</rdfs:label>
        <skos:definition>provides a string value for something, with or without a language tag</skos:definition>
        <skos:note>Note that although the intended range for this property is Text, we have left the range undefined so that it can be used with tools that do not support rdf:langString.</skos:note>
    </owl:DatatypeProperty>
    


    <!-- 
    ///////////////////////////////////////////////////////////////////////////////////////
    //
    // Classes
    //
    ///////////////////////////////////////////////////////////////////////////////////////
     -->

    


    <!-- http://ecoinformatics.org/oboe/oboe.1.2/oboe-core.owl#Characteristic -->

    <owl:Class rdf:about="http://ecoinformatics.org/oboe/oboe.1.2/oboe-core.owl#Characteristic">
        <rdfs:comment>A characteristic represents a property of an entity that can be measured (e.g., height, length, or color).  A characteristic of an entity is observed through a measurement, which further asserts a value of the characteristic for the entity. A characteristic type (e.g., &quot;height&quot;) can be associated with many different entities, whereas an individual characteristic (a particular occurrence of the &quot;height&quot; characteristic) is associated to exactly one entity.</rdfs:comment>
        <rdfs:label xml:lang="en">Characteristic</rdfs:label>
    </owl:Class>
    


    <!-- http://ecoinformatics.org/oboe/oboe.1.2/oboe-core.owl#Entity -->

    <owl:Class rdf:about="http://ecoinformatics.org/oboe/oboe.1.2/oboe-core.owl#Entity">
        <rdfs:comment>An entity is an object (e.g., a tree, a community, an ecological process). Entities constitute the foci of observations, i.e., every observation is of exactly one entity.</rdfs:comment>
        <rdfs:label xml:lang="en">Entity</rdfs:label>
    </owl:Class>
    


    <!-- http://ecoinformatics.org/oboe/oboe.1.2/oboe-core.owl#MeasuredValue -->

    <owl:Class rdf:about="http://ecoinformatics.org/oboe/oboe.1.2/oboe-core.owl#MeasuredValue">
        <rdfs:comment>A measurement value is a quantitative or qualitative result of a measurement. Measurement values can contain a coded representation of the result, e.g., as a number or string.</rdfs:comment>
        <rdfs:label xml:lang="en">Measurement Value</rdfs:label>
    </owl:Class>
    


    <!-- http://ecoinformatics.org/oboe/oboe.1.2/oboe-core.owl#Measurement -->

    <owl:Class rdf:about="http://ecoinformatics.org/oboe/oboe.1.2/oboe-core.owl#Measurement">
        <rdfs:subClassOf>
            <owl:Restriction>
                <owl:onProperty rdf:resource="http://ecoinformatics.org/oboe/oboe.1.2/oboe-core.owl#hasValue"/>
                <owl:someValuesFrom rdf:resource="http://ecoinformatics.org/oboe/oboe.1.2/oboe-core.owl#MeasuredValue"/>
            </owl:Restriction>
        </rdfs:subClassOf>
        <rdfs:subClassOf>
            <owl:Restriction>
                <owl:onProperty rdf:resource="http://ecoinformatics.org/oboe/oboe.1.2/oboe-core.owl#ofCharacteristic"/>
                <owl:someValuesFrom rdf:resource="http://ecoinformatics.org/oboe/oboe.1.2/oboe-core.owl#Characteristic"/>
            </owl:Restriction>
        </rdfs:subClassOf>
        <rdfs:subClassOf>
            <owl:Restriction>
                <owl:onProperty rdf:resource="http://ecoinformatics.org/oboe/oboe.1.2/oboe-core.owl#measurementFor"/>
                <owl:qualifiedCardinality rdf:datatype="http://www.w3.org/2001/XMLSchema#nonNegativeInteger">1</owl:qualifiedCardinality>
                <owl:onClass rdf:resource="http://ecoinformatics.org/oboe/oboe.1.2/oboe-core.owl#Observation"/>
            </owl:Restriction>
        </rdfs:subClassOf>
        <rdfs:comment>A measurement is an assertion that a characteristic of an entity had a particular value with respect to an observation event.  A measurement is comprised of a characteristic, a value, a measurement standard, and a protocol. Measurements can also have precision as well as a description of the methods used. Measurements can encapsulate characteristics that were recorded, but not necessarily measured in a physical sense.  For example, the name of a location and a taxon can be captured through measurements.</rdfs:comment>
        <rdfs:label xml:lang="en">Measurement</rdfs:label>
    </owl:Class>
    


    <!-- http://ecoinformatics.org/oboe/oboe.1.2/oboe-core.owl#Observation -->

    <owl:Class rdf:about="http://ecoinformatics.org/oboe/oboe.1.2/oboe-core.owl#Observation">
        <rdfs:subClassOf>
            <owl:Restriction>
                <owl:onProperty rdf:resource="http://ecoinformatics.org/oboe/oboe.1.2/oboe-core.owl#ofEntity"/>
                <owl:someValuesFrom rdf:resource="http://ecoinformatics.org/oboe/oboe.1.2/oboe-core.owl#Entity"/>
            </owl:Restriction>
        </rdfs:subClassOf>
        <rdfs:comment> An observation is an assertion that an entity (e.g., biological organisms, geographic locations, or environmental features, among others) was observed by an observer. An observation primarily serves to group a set of measurements together into a single &quot;observation event&quot;. Observations are often made within a broader context. The context of an observation is given by other observations, implying that an observed entity (and specifically each corresponding measurement) contextualizes another observed entity (and its corresponding measurements). For example, an observation associated with a location may serve as context for an observation associated with an organism. In this case, the observed characteristic values of the location (such as humidity) are assumed constant for the corresponding measurements of the organism.</rdfs:comment>
        <rdfs:label xml:lang="en">Observation</rdfs:label>
    </owl:Class>
    


    <!-- http://purl.org/ipo/core#Asset -->

    <owl:Class rdf:about="http://purl.org/ipo/core#Asset">
        <owl:equivalentClass>
            <owl:Class>
                <owl:intersectionOf rdf:parseType="Collection">
                    <rdf:Description rdf:about="http://ecoinformatics.org/oboe/oboe.1.2/oboe-core.owl#Entity"/>
                    <owl:Restriction>
                        <owl:onProperty rdf:resource="http://purl.org/ipo/core#hostAssetOf"/>
                        <owl:someValuesFrom rdf:resource="http://purl.org/ipo/core#Issue"/>
                    </owl:Restriction>
                </owl:intersectionOf>
            </owl:Class>
        </owl:equivalentClass>
        <rdfs:subClassOf rdf:resource="http://ecoinformatics.org/oboe/oboe.1.2/oboe-core.owl#Entity"/>
        <rdfs:comment xml:lang="en">Any &quot;thing&quot; that a IssueEntity is related. 
For example, a problem (disease) diagnosed in a patient, can have a virus and the patient as Asset, since the virus is the causative agent of the problem and the patient is the host in which the problem manifests itself.
An Asset can be a person, an object, a report, a document, etc.</rdfs:comment>
        <rdfs:isDefinedBy rdf:resource="http://purl.org/ipo/core"/>
        <rdfs:label xml:lang="en">Asset</rdfs:label>
    </owl:Class>
    


    <!-- http://purl.org/ipo/core#Issue -->

    <owl:Class rdf:about="http://purl.org/ipo/core#Issue">
        <rdfs:subClassOf rdf:resource="http://purl.org/ipo/core#IssueEntity"/>
        <rdfs:subClassOf>
            <owl:Restriction>
                <owl:onProperty rdf:resource="http://purl.org/ipo/core#indicatedBy"/>
                <owl:someValuesFrom rdf:resource="http://purl.org/ipo/core#Symptom"/>
            </owl:Restriction>
        </rdfs:subClassOf>
        <owl:disjointWith rdf:resource="http://purl.org/ipo/core#Symptom"/>
        <rdfs:comment xml:lang="en">A problem or issue to be resolved. For example, something that is not operating normally or a hindrance to performing some task.
A Issue can be cause and/or caused, directly or indirectly, by another Issue, the same that the Issue A can depend on the Issue B, needing that the Issue B be solved before solving Issue A.
The Issue can have a set of Actions (Procedures) that will fix it and also a Issue can be indicated by several Symptoms, where a set of Symptoms can identify a Issue.</rdfs:comment>
        <rdfs:isDefinedBy rdf:resource="http://purl.org/ipo/core"/>
        <rdfs:label xml:lang="en">Issue</rdfs:label>
    </owl:Class>
    


    <!-- http://purl.org/ipo/core#IssueEntity -->

    <owl:Class rdf:about="http://purl.org/ipo/core#IssueEntity">
        <rdfs:comment xml:lang="en">A generic class representing the three main concepts within the domain of ontology: Symptom, Problem and Action.</rdfs:comment>
        <rdfs:isDefinedBy rdf:resource="http://purl.org/ipo/core"/>
        <rdfs:label xml:lang="en">IssueEntity</rdfs:label>
    </owl:Class>
    


    <!-- http://purl.org/ipo/core#Symptom -->

    <owl:Class rdf:about="http://purl.org/ipo/core#Symptom">
        <rdfs:subClassOf rdf:resource="http://ecoinformatics.org/oboe/oboe.1.2/oboe-core.owl#Observation"/>
        <rdfs:subClassOf rdf:resource="http://purl.org/ipo/core#IssueEntity"/>
        <rdfs:subClassOf>
            <owl:Restriction>
                <owl:onProperty rdf:resource="http://purl.org/ipo/core#indicates"/>
                <owl:someValuesFrom rdf:resource="http://purl.org/ipo/core#Issue"/>
            </owl:Restriction>
        </rdfs:subClassOf>
        <rdfs:comment xml:lang="en">Represents a sign or indication of one or more Issues. Something that is perceived when a problem occurs.
</rdfs:comment>
        <rdfs:isDefinedBy rdf:resource="http://purl.org/ipo/core"/>
        <rdfs:label xml:lang="en">Symptom</rdfs:label>
    </owl:Class>
    


    <!-- http://purl.org/net/EvaluationResult#Evaluation -->

    <owl:Class rdf:about="http://purl.org/net/EvaluationResult#Evaluation">
        <rdfs:comment>Evaluation. A process of quality measurement.</rdfs:comment>
        <rdfs:label>Evaluation</rdfs:label>
    </owl:Class>
    


    <!-- http://purl.org/net/EvaluationResult#EvaluationData -->

    <owl:Class rdf:about="http://purl.org/net/EvaluationResult#EvaluationData">
        <rdfs:comment>Evaluation data is any data that is used as an input in an evaluation process.</rdfs:comment>
        <rdfs:label>EvaluationData</rdfs:label>
    </owl:Class>
    


    <!-- http://purl.org/net/EvaluationResult#EvaluationSubject -->

    <owl:Class rdf:about="http://purl.org/net/EvaluationResult#EvaluationSubject">
        <rdfs:subClassOf rdf:resource="http://ecoinformatics.org/oboe/oboe.1.2/oboe-core.owl#Entity"/>
        <rdfs:comment>Evaluation subject is any product, service or action (e.g., Seat Ibiza, Chrome, corn crops) that is evaluated in an evaluation process.</rdfs:comment>
        <rdfs:label>EvaluationSubject</rdfs:label>
    </owl:Class>
    


    <!-- http://purl.org/net/EvaluationResult#QualityValue -->

    <owl:Class rdf:about="http://purl.org/net/EvaluationResult#QualityValue">
        <rdfs:subClassOf rdf:resource="http://ecoinformatics.org/oboe/oboe.1.2/oboe-core.owl#MeasuredValue"/>
        <rdfs:comment>Quality value is a value obtained in a quality evaluation.</rdfs:comment>
        <rdfs:label>QualityValue</rdfs:label>
    </owl:Class>
    


    <!-- http://purl.org/net/EvaluationResult#SubjectCategory -->

    <owl:Class rdf:about="http://purl.org/net/EvaluationResult#SubjectCategory">
        <rdfs:comment>Subject category is a category or type of an evaluation subject (eg., a car, web browser, investment).</rdfs:comment>
        <rdfs:label>SubjectCategory</rdfs:label>
    </owl:Class>
    


    <!-- http://purl.org/net/QualityModel#BaseMeasure -->

    <owl:Class rdf:about="http://purl.org/net/QualityModel#BaseMeasure">
        <rdfs:subClassOf rdf:resource="http://purl.org/net/QualityModel#QualityMeasure"/>
        <rdfs:comment>Base measure is a quality measure for which, in the process of evaluation, the results are obtained in an individual test and are related to direct outputs of the evaluation. </rdfs:comment>
        <rdfs:label>BaseMeasure</rdfs:label>
    </owl:Class>
    


    <!-- http://purl.org/net/QualityModel#DerivedMeasure -->

    <owl:Class rdf:about="http://purl.org/net/QualityModel#DerivedMeasure">
        <rdfs:subClassOf rdf:resource="http://purl.org/net/QualityModel#QualityMeasure"/>
        <rdfs:subClassOf>
            <owl:Restriction>
                <owl:onProperty rdf:resource="http://purl.org/net/QualityModel#hasScale"/>
                <owl:someValuesFrom rdf:resource="https://purl.archive.org/oquo#RawScale"/>
            </owl:Restriction>
        </rdfs:subClassOf>
        <rdfs:comment>Derived measure is a measure that is obtained in an individual evaluation test by combining base measures.</rdfs:comment>
        <rdfs:label>DerivedMeasure</rdfs:label>
    </owl:Class>
    


    <!-- http://purl.org/net/QualityModel#OrdinalScaleItem -->

    <owl:Class rdf:about="http://purl.org/net/QualityModel#OrdinalScaleItem">
        <rdfs:comment>Ordinal scale item is an item that belongs to a particular ordinal scale. Ordinal scale item is described with a label (e.g., &quot;Excellent&quot;/&quot;Good&quot;/...) and an order on the scale (e.g., 1/2/...).</rdfs:comment>
        <rdfs:label>OrdinalScaleItem</rdfs:label>
    </owl:Class>
    


    <!-- http://purl.org/net/QualityModel#QualityCharacteristic -->

    <owl:Class rdf:about="http://purl.org/net/QualityModel#QualityCharacteristic">
        <rdfs:subClassOf rdf:resource="http://ecoinformatics.org/oboe/oboe.1.2/oboe-core.owl#Characteristic"/>
        <rdfs:comment>Quality characteristic is a characteristic of a product, service or action that can be measured in an evaluation using quality measures.</rdfs:comment>
        <rdfs:label>QualityCharacteristic</rdfs:label>
    </owl:Class>
    


    <!-- http://purl.org/net/QualityModel#QualityIndicator -->

    <owl:Class rdf:about="http://purl.org/net/QualityModel#QualityIndicator">
        <rdfs:subClassOf rdf:resource="http://purl.org/net/QualityModel#QualityMeasure"/>
        <rdfs:comment>Quality indicator is a quality measure that is obtained by combining base and/or derived measures. Unlike base and derived measures, quality indicators are related to a set of tests in the evaluation.</rdfs:comment>
        <rdfs:label>QualityIndicator</rdfs:label>
    </owl:Class>
    


    <!-- http://purl.org/net/QualityModel#QualityMeasure -->

    <owl:Class rdf:about="http://purl.org/net/QualityModel#QualityMeasure">
        <rdfs:subClassOf rdf:resource="http://ecoinformatics.org/oboe/oboe.1.2/oboe-core.owl#Measurement"/>
        <rdfs:comment>Quality measure is any measure that captures information about a specific quality characteristic related to a specific product, service or action.</rdfs:comment>
        <rdfs:label>QualityMeasure</rdfs:label>
    </owl:Class>
    


    <!-- http://purl.org/net/QualityModel#RankingFunction -->

    <owl:Class rdf:about="http://purl.org/net/QualityModel#RankingFunction">
        <owl:equivalentClass>
            <owl:Class>
                <owl:oneOf rdf:parseType="Collection">
                    <rdf:Description rdf:about="http://purl.org/net/QualityModel#HigherBest"/>
                    <rdf:Description rdf:about="http://purl.org/net/QualityModel#LowerBest"/>
                </owl:oneOf>
            </owl:Class>
        </owl:equivalentClass>
        <rdfs:comment>Ranking function is a function which denotes how two values of a measurement scale can be ranked, i.e., if higher or lower value is better.</rdfs:comment>
        <rdfs:label>RankingFunction</rdfs:label>
    </owl:Class>
    


    <!-- http://www.w3.org/2002/07/owl#Thing -->

    <owl:Class rdf:about="http://www.w3.org/2002/07/owl#Thing">
        <rdfs:comment>The class of OWL individuals.</rdfs:comment>
        <rdfs:isDefinedBy rdf:resource="http://www.w3.org/2002/07/owl#"/>
        <rdfs:label>Thing</rdfs:label>
    </owl:Class>
    


    <!-- http://www.w3.org/2006/time#Instant -->

    <owl:Class rdf:about="http://www.w3.org/2006/time#Instant">
        <rdfs:comment xml:lang="en">A temporal entity with zero extent or duration</rdfs:comment>
        <rdfs:comment xml:lang="es">Una entidad temporal con una extensión o duración cero.</rdfs:comment>
        <rdfs:label xml:lang="en">Time instant</rdfs:label>
        <rdfs:label xml:lang="es">instante de tiempo.</rdfs:label>
        <skos:definition xml:lang="en">A temporal entity with zero extent or duration</skos:definition>
        <skos:definition xml:lang="es">Una entidad temporal con una extensión o duración cero.</skos:definition>
    </owl:Class>
    


    <!-- http://www.wurvoc.org/vocabularies/om-1.8/Cardinal_scale -->

    <owl:Class rdf:about="http://www.wurvoc.org/vocabularies/om-1.8/Cardinal_scale">
        <rdfs:subClassOf rdf:resource="http://www.wurvoc.org/vocabularies/om-1.8/Measurement_scale"/>
        <rdfs:label xml:lang="en">cardinal scale</rdfs:label>
    </owl:Class>
    


    <!-- http://www.wurvoc.org/vocabularies/om-1.8/Interval_scale -->

    <owl:Class rdf:about="http://www.wurvoc.org/vocabularies/om-1.8/Interval_scale">
        <rdfs:subClassOf rdf:resource="http://www.wurvoc.org/vocabularies/om-1.8/Cardinal_scale"/>
        <owl:disjointWith rdf:resource="http://www.wurvoc.org/vocabularies/om-1.8/Ratio_scale"/>
        <obo:IAO_0000112>Celsius and Fahrenheit are examples of interval scales. Each point on these scales differs from neighboring points by intervals of exactly one degree. The difference between 20 and 21 degrees is identical to the difference between 225 and 226 degrees. However, these scales have arbitrary zero points – zero degrees isn’t the lowest possible temperature.</obo:IAO_0000112>
        <rdfs:comment>Interval data is measured along a numerical scale that has equal distances between adjacent values. These distances are called intervals. There is no true zero on an interval scale, which is what distinguishes it from a ratio scale. On an interval scale, zero is an arbitrary point, not a complete absence of the variable.</rdfs:comment>
        <rdfs:label xml:lang="en">interval scale</rdfs:label>
    </owl:Class>
    <owl:Axiom>
        <owl:annotatedSource rdf:resource="http://www.wurvoc.org/vocabularies/om-1.8/Interval_scale"/>
        <owl:annotatedProperty rdf:resource="http://www.w3.org/2000/01/rdf-schema#comment"/>
        <owl:annotatedTarget>Interval data is measured along a numerical scale that has equal distances between adjacent values. These distances are called intervals. There is no true zero on an interval scale, which is what distinguishes it from a ratio scale. On an interval scale, zero is an arbitrary point, not a complete absence of the variable.</owl:annotatedTarget>
        <rdfs:isDefinedBy>https://www.scribbr.com/statistics/interval-data/</rdfs:isDefinedBy>
    </owl:Axiom>
    


    <!-- http://www.wurvoc.org/vocabularies/om-1.8/Measurement_scale -->

    <owl:Class rdf:about="http://www.wurvoc.org/vocabularies/om-1.8/Measurement_scale">
        <rdfs:comment xml:lang="en">Measurement scales are concepts used for the expression of quantities. Four types of measurement scales are: nominal scales, ordinal scales, interval scales and ratio scales. The latter two scales are also called cardinal scales. An example of a scale is the Celsius scale, a temperature scale.</rdfs:comment>
        <rdfs:label xml:lang="en">measurement scale</rdfs:label>
        <om-1:alternative_label xml:lang="en">scale</om-1:alternative_label>
    </owl:Class>
    


    <!-- http://www.wurvoc.org/vocabularies/om-1.8/Nominal_scale -->

    <owl:Class rdf:about="http://www.wurvoc.org/vocabularies/om-1.8/Nominal_scale">
        <rdfs:subClassOf rdf:resource="http://www.wurvoc.org/vocabularies/om-1.8/Measurement_scale"/>
        <rdfs:label xml:lang="en">nominal scale</rdfs:label>
    </owl:Class>
    


    <!-- http://www.wurvoc.org/vocabularies/om-1.8/Ordinal_scale -->

    <owl:Class rdf:about="http://www.wurvoc.org/vocabularies/om-1.8/Ordinal_scale">
        <rdfs:subClassOf rdf:resource="http://www.wurvoc.org/vocabularies/om-1.8/Measurement_scale"/>
        <rdfs:label xml:lang="en">ordinal scale</rdfs:label>
    </owl:Class>
    


    <!-- http://www.wurvoc.org/vocabularies/om-1.8/Ratio_scale -->

    <owl:Class rdf:about="http://www.wurvoc.org/vocabularies/om-1.8/Ratio_scale">
        <rdfs:subClassOf rdf:resource="http://www.wurvoc.org/vocabularies/om-1.8/Cardinal_scale"/>
        <obo:IAO_0000112>Length, area, and population are examples of ratio scales.</obo:IAO_0000112>
        <rdfs:comment>A ratio scale is a quantitative scale where there is a true zero and equal intervals between neighboring points. Unlike on an interval scale, a zero on a ratio scale means there is a total absence of the variable you are measuring.</rdfs:comment>
        <rdfs:label xml:lang="en">ratio scale</rdfs:label>
    </owl:Class>
    <owl:Axiom>
        <owl:annotatedSource rdf:resource="http://www.wurvoc.org/vocabularies/om-1.8/Ratio_scale"/>
        <owl:annotatedProperty rdf:resource="http://www.w3.org/2000/01/rdf-schema#comment"/>
        <owl:annotatedTarget>A ratio scale is a quantitative scale where there is a true zero and equal intervals between neighboring points. Unlike on an interval scale, a zero on a ratio scale means there is a total absence of the variable you are measuring.</owl:annotatedTarget>
        <rdfs:isDefinedBy>https://www.scribbr.com/statistics/ratio-data/</rdfs:isDefinedBy>
    </owl:Axiom>
    


    <!-- http://www.wurvoc.org/vocabularies/om-1.8/Unit_of_measure -->

    <owl:Class rdf:about="http://www.wurvoc.org/vocabularies/om-1.8/Unit_of_measure">
        <rdfs:comment xml:lang="en">A unit of measure is a definite magnitude of a quantity, defined and adopted by convention and/or by law. It is used as a standard for measurement of the same quantity, where any other value of the quantity can be expressed as a simple multiple of the unit of measure. For example, length is a quantity; the metre is a unit of length that represents a definite predetermined length. When we say 10 metre (or 10 m), we actually mean 10 times the definite predetermined length called &quot;metre&quot;.</rdfs:comment>
        <rdfs:label xml:lang="en">unit of measure</rdfs:label>
        <om-1:alternative_label xml:lang="en">unit</om-1:alternative_label>
        <om-1:alternative_label xml:lang="en">unit of measurement</om-1:alternative_label>
    </owl:Class>
    


    <!-- https://purl.archive.org/oquo#AdaptabilityCharacteristic -->

    <owl:Class rdf:about="https://purl.archive.org/oquo#AdaptabilityCharacteristic">
        <rdfs:subClassOf rdf:resource="http://purl.org/net/QualityModel#QualityCharacteristic"/>
        <obo:IAO_0000115 xml:lang="en">The degree to which The ontology can be adapted for different specified environments (languages, expresivity levels) without applying actions or means other than those provided for this purpose for the Ontology considered.</obo:IAO_0000115>
        <rdfs:label>adaptability characteristic</rdfs:label>
    </owl:Class>
    


    <!-- https://purl.archive.org/oquo#AnalysabilityCharacteristic -->

    <owl:Class rdf:about="https://purl.archive.org/oquo#AnalysabilityCharacteristic">
        <rdfs:subClassOf rdf:resource="http://purl.org/net/QualityModel#QualityCharacteristic"/>
        <obo:IAO_0000115 xml:lang="en">The degree to which The ontology can be diagnosed for deficiencies or causes of failures (inconsistences), or for the parts to be modified to be identified.</obo:IAO_0000115>
        <rdfs:label>analysability characteristic</rdfs:label>
    </owl:Class>
    


    <!-- https://purl.archive.org/oquo#AncestorsPerClassMetric -->

    <owl:Class rdf:about="https://purl.archive.org/oquo#AncestorsPerClassMetric">
        <rdfs:subClassOf rdf:resource="http://purl.org/net/QualityModel#DerivedMeasure"/>
        <rdfs:subClassOf>
            <owl:Restriction>
                <owl:onProperty rdf:resource="http://purl.org/net/QualityModel#hasScale"/>
                <owl:someValuesFrom>
                    <owl:Class>
                        <owl:intersectionOf rdf:parseType="Collection">
                            <rdf:Description rdf:about="https://purl.archive.org/oquo#RawScale"/>
                            <owl:Restriction>
                                <owl:onProperty rdf:resource="http://purl.org/net/QualityModel#hasRankigFunction"/>
                                <owl:hasValue rdf:resource="http://purl.org/net/QualityModel#HigherBest"/>
                            </owl:Restriction>
                        </owl:intersectionOf>
                    </owl:Class>
                </owl:someValuesFrom>
            </owl:Restriction>
        </rdfs:subClassOf>
        <rdfs:subClassOf>
            <owl:Restriction>
                <owl:onProperty rdf:resource="http://purl.org/net/QualityModel#hasScale"/>
                <owl:hasValue rdf:resource="https://purl.archive.org/oquo#AncestorsPerClassMetricScale"/>
            </owl:Restriction>
        </rdfs:subClassOf>
        <obo:IAO_0000115 xml:lang="en">Mean number of direct ancestor per class POnto=∑|SupCi| /∑|Ci| </obo:IAO_0000115>
        <rdf1:acronym>POnto</rdf1:acronym>
        <rdfs:label>ancestors per class metric</rdfs:label>
    </owl:Class>
    


    <!-- https://purl.archive.org/oquo#AnnotationPropertiesWithNoDescriptionMetric -->

    <owl:Class rdf:about="https://purl.archive.org/oquo#AnnotationPropertiesWithNoDescriptionMetric">
        <rdfs:subClassOf rdf:resource="http://purl.org/net/QualityModel#DerivedMeasure"/>
        <rdfs:subClassOf>
            <owl:Restriction>
                <owl:onProperty rdf:resource="http://purl.org/net/QualityModel#hasScale"/>
                <owl:someValuesFrom>
                    <owl:Class>
                        <owl:intersectionOf rdf:parseType="Collection">
                            <rdf:Description rdf:about="https://purl.archive.org/oquo#RawScale"/>
                            <owl:Restriction>
                                <owl:onProperty rdf:resource="http://purl.org/net/QualityModel#hasRankigFunction"/>
                                <owl:hasValue rdf:resource="http://purl.org/net/QualityModel#LowerBest"/>
                            </owl:Restriction>
                        </owl:intersectionOf>
                    </owl:Class>
                </owl:someValuesFrom>
            </owl:Restriction>
        </rdfs:subClassOf>
        <rdfs:subClassOf>
            <owl:Restriction>
                <owl:onProperty rdf:resource="https://purl.archive.org/oquo#measuresCharacteristicNegatively"/>
                <owl:someValuesFrom rdf:resource="https://purl.archive.org/oquo#EaseOfUseCharacteristic"/>
            </owl:Restriction>
        </rdfs:subClassOf>
        <rdfs:subClassOf>
            <owl:Restriction>
                <owl:onProperty rdf:resource="https://purl.archive.org/oquo#measuresCharacteristicNegatively"/>
                <owl:someValuesFrom rdf:resource="https://purl.archive.org/oquo#EfficiencyInUseCharacteristic"/>
            </owl:Restriction>
        </rdfs:subClassOf>
        <rdfs:subClassOf>
            <owl:Restriction>
                <owl:onProperty rdf:resource="https://purl.archive.org/oquo#measuresCharacteristicNegatively"/>
                <owl:someValuesFrom rdf:resource="https://purl.archive.org/oquo#HelpfulnessCharacteristic"/>
            </owl:Restriction>
        </rdfs:subClassOf>
        <rdfs:subClassOf>
            <owl:Restriction>
                <owl:onProperty rdf:resource="https://purl.archive.org/oquo#measuresCharacteristicNegatively"/>
                <owl:someValuesFrom rdf:resource="https://purl.archive.org/oquo#IndexingAndLinkingCharacteristic"/>
            </owl:Restriction>
        </rdfs:subClassOf>
        <rdfs:subClassOf>
            <owl:Restriction>
                <owl:onProperty rdf:resource="https://purl.archive.org/oquo#measuresCharacteristicNegatively"/>
                <owl:someValuesFrom rdf:resource="https://purl.archive.org/oquo#KnowledgeReuseCharacteristic"/>
            </owl:Restriction>
        </rdfs:subClassOf>
        <rdfs:subClassOf>
            <owl:Restriction>
                <owl:onProperty rdf:resource="https://purl.archive.org/oquo#measuresCharacteristicNegatively"/>
                <owl:someValuesFrom rdf:resource="https://purl.archive.org/oquo#LearnabilityCharacteristic"/>
            </owl:Restriction>
        </rdfs:subClassOf>
        <rdfs:subClassOf>
            <owl:Restriction>
                <owl:onProperty rdf:resource="https://purl.archive.org/oquo#measuresCharacteristicNegatively"/>
                <owl:allValuesFrom>
                    <owl:Class>
                        <owl:unionOf rdf:parseType="Collection">
                            <rdf:Description rdf:about="https://purl.archive.org/oquo#EaseOfUseCharacteristic"/>
                            <rdf:Description rdf:about="https://purl.archive.org/oquo#EfficiencyInUseCharacteristic"/>
                            <rdf:Description rdf:about="https://purl.archive.org/oquo#HelpfulnessCharacteristic"/>
                            <rdf:Description rdf:about="https://purl.archive.org/oquo#IndexingAndLinkingCharacteristic"/>
                            <rdf:Description rdf:about="https://purl.archive.org/oquo#KnowledgeReuseCharacteristic"/>
                            <rdf:Description rdf:about="https://purl.archive.org/oquo#LearnabilityCharacteristic"/>
                        </owl:unionOf>
                    </owl:Class>
                </owl:allValuesFrom>
            </owl:Restriction>
        </rdfs:subClassOf>
        <rdfs:subClassOf>
            <owl:Restriction>
                <owl:onProperty rdf:resource="http://purl.org/net/QualityModel#hasScale"/>
                <owl:hasValue rdf:resource="https://purl.archive.org/oquo#AnnotationPropertiesWithNoDescriptionMetricScale"/>
            </owl:Restriction>
        </rdfs:subClassOf>
        <obo:IAO_0000115>The Percentage of annotation properties lacking a description in the ontology.</obo:IAO_0000115>
        <rdf1:acronym>APWND</rdf1:acronym>
        <rdfs:label>annotation properties with no description metric</rdfs:label>
    </owl:Class>
    


    <!-- https://purl.archive.org/oquo#AnnotationPropertiesWithNoNameMetric -->

    <owl:Class rdf:about="https://purl.archive.org/oquo#AnnotationPropertiesWithNoNameMetric">
        <rdfs:subClassOf rdf:resource="http://purl.org/net/QualityModel#DerivedMeasure"/>
        <rdfs:subClassOf>
            <owl:Restriction>
                <owl:onProperty rdf:resource="http://purl.org/net/QualityModel#hasScale"/>
                <owl:someValuesFrom>
                    <owl:Class>
                        <owl:intersectionOf rdf:parseType="Collection">
                            <rdf:Description rdf:about="https://purl.archive.org/oquo#RawScale"/>
                            <owl:Restriction>
                                <owl:onProperty rdf:resource="http://purl.org/net/QualityModel#hasRankigFunction"/>
                                <owl:hasValue rdf:resource="http://purl.org/net/QualityModel#LowerBest"/>
                            </owl:Restriction>
                        </owl:intersectionOf>
                    </owl:Class>
                </owl:someValuesFrom>
            </owl:Restriction>
        </rdfs:subClassOf>
        <rdfs:subClassOf>
            <owl:Restriction>
                <owl:onProperty rdf:resource="https://purl.archive.org/oquo#measuresCharacteristicNegatively"/>
                <owl:someValuesFrom rdf:resource="https://purl.archive.org/oquo#EaseOfUseCharacteristic"/>
            </owl:Restriction>
        </rdfs:subClassOf>
        <rdfs:subClassOf>
            <owl:Restriction>
                <owl:onProperty rdf:resource="https://purl.archive.org/oquo#measuresCharacteristicNegatively"/>
                <owl:someValuesFrom rdf:resource="https://purl.archive.org/oquo#EfficiencyInUseCharacteristic"/>
            </owl:Restriction>
        </rdfs:subClassOf>
        <rdfs:subClassOf>
            <owl:Restriction>
                <owl:onProperty rdf:resource="https://purl.archive.org/oquo#measuresCharacteristicNegatively"/>
                <owl:someValuesFrom rdf:resource="https://purl.archive.org/oquo#IndexingAndLinkingCharacteristic"/>
            </owl:Restriction>
        </rdfs:subClassOf>
        <rdfs:subClassOf>
            <owl:Restriction>
                <owl:onProperty rdf:resource="https://purl.archive.org/oquo#measuresCharacteristicNegatively"/>
                <owl:someValuesFrom rdf:resource="https://purl.archive.org/oquo#KnowledgeReuseCharacteristic"/>
            </owl:Restriction>
        </rdfs:subClassOf>
        <rdfs:subClassOf>
            <owl:Restriction>
                <owl:onProperty rdf:resource="https://purl.archive.org/oquo#measuresCharacteristicNegatively"/>
                <owl:someValuesFrom rdf:resource="https://purl.archive.org/oquo#TextAnalysisCharacteristic"/>
            </owl:Restriction>
        </rdfs:subClassOf>
        <rdfs:subClassOf>
            <owl:Restriction>
                <owl:onProperty rdf:resource="https://purl.archive.org/oquo#measuresCharacteristicNegatively"/>
                <owl:allValuesFrom>
                    <owl:Class>
                        <owl:unionOf rdf:parseType="Collection">
                            <rdf:Description rdf:about="https://purl.archive.org/oquo#EaseOfUseCharacteristic"/>
                            <rdf:Description rdf:about="https://purl.archive.org/oquo#EfficiencyInUseCharacteristic"/>
                            <rdf:Description rdf:about="https://purl.archive.org/oquo#IndexingAndLinkingCharacteristic"/>
                            <rdf:Description rdf:about="https://purl.archive.org/oquo#KnowledgeReuseCharacteristic"/>
                            <rdf:Description rdf:about="https://purl.archive.org/oquo#TextAnalysisCharacteristic"/>
                        </owl:unionOf>
                    </owl:Class>
                </owl:allValuesFrom>
            </owl:Restriction>
        </rdfs:subClassOf>
        <rdfs:subClassOf>
            <owl:Restriction>
                <owl:onProperty rdf:resource="http://purl.org/net/QualityModel#hasScale"/>
                <owl:hasValue rdf:resource="https://purl.archive.org/oquo#AnnotationPropertiesWithNoNameMetricScale"/>
            </owl:Restriction>
        </rdfs:subClassOf>
        <obo:IAO_0000115>The Percentage of annotation properties lacking a name in the ontology.</obo:IAO_0000115>
        <rdf1:acronym>APWNN</rdf1:acronym>
        <rdfs:label>annotation properties with no name metric</rdfs:label>
    </owl:Class>
    


    <!-- https://purl.archive.org/oquo#AnnotationPropertiesWithNoSynonymMetric -->

    <owl:Class rdf:about="https://purl.archive.org/oquo#AnnotationPropertiesWithNoSynonymMetric">
        <rdfs:subClassOf rdf:resource="http://purl.org/net/QualityModel#DerivedMeasure"/>
        <rdfs:subClassOf>
            <owl:Restriction>
                <owl:onProperty rdf:resource="http://purl.org/net/QualityModel#hasScale"/>
                <owl:someValuesFrom>
                    <owl:Class>
                        <owl:intersectionOf rdf:parseType="Collection">
                            <rdf:Description rdf:about="https://purl.archive.org/oquo#RawScale"/>
                            <owl:Restriction>
                                <owl:onProperty rdf:resource="http://purl.org/net/QualityModel#hasRankigFunction"/>
                                <owl:hasValue rdf:resource="http://purl.org/net/QualityModel#LowerBest"/>
                            </owl:Restriction>
                        </owl:intersectionOf>
                    </owl:Class>
                </owl:someValuesFrom>
            </owl:Restriction>
        </rdfs:subClassOf>
        <rdfs:subClassOf>
            <owl:Restriction>
                <owl:onProperty rdf:resource="https://purl.archive.org/oquo#measuresCharacteristicNegatively"/>
                <owl:someValuesFrom rdf:resource="https://purl.archive.org/oquo#EaseOfUseCharacteristic"/>
            </owl:Restriction>
        </rdfs:subClassOf>
        <rdfs:subClassOf>
            <owl:Restriction>
                <owl:onProperty rdf:resource="https://purl.archive.org/oquo#measuresCharacteristicNegatively"/>
                <owl:someValuesFrom rdf:resource="https://purl.archive.org/oquo#EfficiencyInUseCharacteristic"/>
            </owl:Restriction>
        </rdfs:subClassOf>
        <rdfs:subClassOf>
            <owl:Restriction>
                <owl:onProperty rdf:resource="https://purl.archive.org/oquo#measuresCharacteristicNegatively"/>
                <owl:someValuesFrom rdf:resource="https://purl.archive.org/oquo#IndexingAndLinkingCharacteristic"/>
            </owl:Restriction>
        </rdfs:subClassOf>
        <rdfs:subClassOf>
            <owl:Restriction>
                <owl:onProperty rdf:resource="https://purl.archive.org/oquo#measuresCharacteristicNegatively"/>
                <owl:someValuesFrom rdf:resource="https://purl.archive.org/oquo#KnowledgeReuseCharacteristic"/>
            </owl:Restriction>
        </rdfs:subClassOf>
        <rdfs:subClassOf>
            <owl:Restriction>
                <owl:onProperty rdf:resource="https://purl.archive.org/oquo#measuresCharacteristicNegatively"/>
                <owl:someValuesFrom rdf:resource="https://purl.archive.org/oquo#TextAnalysisCharacteristic"/>
            </owl:Restriction>
        </rdfs:subClassOf>
        <rdfs:subClassOf>
            <owl:Restriction>
                <owl:onProperty rdf:resource="https://purl.archive.org/oquo#measuresCharacteristicNegatively"/>
                <owl:allValuesFrom>
                    <owl:Class>
                        <owl:unionOf rdf:parseType="Collection">
                            <rdf:Description rdf:about="https://purl.archive.org/oquo#EaseOfUseCharacteristic"/>
                            <rdf:Description rdf:about="https://purl.archive.org/oquo#EfficiencyInUseCharacteristic"/>
                            <rdf:Description rdf:about="https://purl.archive.org/oquo#IndexingAndLinkingCharacteristic"/>
                            <rdf:Description rdf:about="https://purl.archive.org/oquo#KnowledgeReuseCharacteristic"/>
                            <rdf:Description rdf:about="https://purl.archive.org/oquo#TextAnalysisCharacteristic"/>
                        </owl:unionOf>
                    </owl:Class>
                </owl:allValuesFrom>
            </owl:Restriction>
        </rdfs:subClassOf>
        <rdfs:subClassOf>
            <owl:Restriction>
                <owl:onProperty rdf:resource="http://purl.org/net/QualityModel#hasScale"/>
                <owl:hasValue rdf:resource="https://purl.archive.org/oquo#AnnotationPropertiesWithNoSynonymMetricScale"/>
            </owl:Restriction>
        </rdfs:subClassOf>
        <obo:IAO_0000115>The Percentage of annotation properties lacking a synonym in the ontology.</obo:IAO_0000115>
        <rdf1:acronym>APWNS</rdf1:acronym>
        <rdfs:label>annotation properties with no synonym metric</rdfs:label>
    </owl:Class>
    


    <!-- https://purl.archive.org/oquo#AnnotationRichnessMetric -->

    <owl:Class rdf:about="https://purl.archive.org/oquo#AnnotationRichnessMetric">
        <rdfs:subClassOf rdf:resource="http://purl.org/net/QualityModel#DerivedMeasure"/>
        <rdfs:subClassOf>
            <owl:Restriction>
                <owl:onProperty rdf:resource="http://purl.org/net/QualityModel#hasScale"/>
                <owl:someValuesFrom>
                    <owl:Class>
                        <owl:intersectionOf rdf:parseType="Collection">
                            <rdf:Description rdf:about="https://purl.archive.org/oquo#RawScale"/>
                            <owl:Restriction>
                                <owl:onProperty rdf:resource="http://purl.org/net/QualityModel#hasRankigFunction"/>
                                <owl:hasValue rdf:resource="http://purl.org/net/QualityModel#HigherBest"/>
                            </owl:Restriction>
                        </owl:intersectionOf>
                    </owl:Class>
                </owl:someValuesFrom>
            </owl:Restriction>
        </rdfs:subClassOf>
        <rdfs:subClassOf>
            <owl:Restriction>
                <owl:onProperty rdf:resource="https://purl.archive.org/oquo#measuresCharacteristicPositively"/>
                <owl:someValuesFrom rdf:resource="https://purl.archive.org/oquo#ClusteringCharacteristic"/>
            </owl:Restriction>
        </rdfs:subClassOf>
        <rdfs:subClassOf>
            <owl:Restriction>
                <owl:onProperty rdf:resource="https://purl.archive.org/oquo#measuresCharacteristicPositively"/>
                <owl:someValuesFrom rdf:resource="https://purl.archive.org/oquo#ConsistentSearchAndQueryCharacteristic"/>
            </owl:Restriction>
        </rdfs:subClassOf>
        <rdfs:subClassOf>
            <owl:Restriction>
                <owl:onProperty rdf:resource="https://purl.archive.org/oquo#measuresCharacteristicPositively"/>
                <owl:someValuesFrom rdf:resource="https://purl.archive.org/oquo#ControlledVocabularyCharacteristic"/>
            </owl:Restriction>
        </rdfs:subClassOf>
        <rdfs:subClassOf>
            <owl:Restriction>
                <owl:onProperty rdf:resource="https://purl.archive.org/oquo#measuresCharacteristicPositively"/>
                <owl:someValuesFrom rdf:resource="https://purl.archive.org/oquo#KnowledgeAcquisitionRepresentationCharacteristic"/>
            </owl:Restriction>
        </rdfs:subClassOf>
        <rdfs:subClassOf>
            <owl:Restriction>
                <owl:onProperty rdf:resource="https://purl.archive.org/oquo#measuresCharacteristicPositively"/>
                <owl:someValuesFrom rdf:resource="https://purl.archive.org/oquo#KnowledgeReuseCharacteristic"/>
            </owl:Restriction>
        </rdfs:subClassOf>
        <rdfs:subClassOf>
            <owl:Restriction>
                <owl:onProperty rdf:resource="https://purl.archive.org/oquo#measuresCharacteristicPositively"/>
                <owl:someValuesFrom rdf:resource="https://purl.archive.org/oquo#RedundancyCharacteristic"/>
            </owl:Restriction>
        </rdfs:subClassOf>
        <rdfs:subClassOf>
            <owl:Restriction>
                <owl:onProperty rdf:resource="https://purl.archive.org/oquo#measuresCharacteristicPositively"/>
                <owl:allValuesFrom>
                    <owl:Class>
                        <owl:unionOf rdf:parseType="Collection">
                            <rdf:Description rdf:about="https://purl.archive.org/oquo#ClusteringCharacteristic"/>
                            <rdf:Description rdf:about="https://purl.archive.org/oquo#ConsistentSearchAndQueryCharacteristic"/>
                            <rdf:Description rdf:about="https://purl.archive.org/oquo#ControlledVocabularyCharacteristic"/>
                            <rdf:Description rdf:about="https://purl.archive.org/oquo#KnowledgeAcquisitionRepresentationCharacteristic"/>
                            <rdf:Description rdf:about="https://purl.archive.org/oquo#KnowledgeReuseCharacteristic"/>
                            <rdf:Description rdf:about="https://purl.archive.org/oquo#RedundancyCharacteristic"/>
                        </owl:unionOf>
                    </owl:Class>
                </owl:allValuesFrom>
            </owl:Restriction>
        </rdfs:subClassOf>
        <rdfs:subClassOf>
            <owl:Restriction>
                <owl:onProperty rdf:resource="http://purl.org/net/QualityModel#hasScale"/>
                <owl:hasValue rdf:resource="https://purl.archive.org/oquo#AnnotationRichnessMetricScale"/>
            </owl:Restriction>
        </rdfs:subClassOf>
        <obo:IAO_0000115 xml:lang="en">Mean number of annotation properties per class ANOnto=∑|ACi| /∑|Ci|; where Ci is the i-th class in the ontology </obo:IAO_0000115>
        <rdf1:acronym>ANOnto</rdf1:acronym>
        <rdfs:comment>Mean number of annotation properties per class.</rdfs:comment>
        <rdfs:label>annotation richness metric</rdfs:label>
    </owl:Class>
    


    <!-- https://purl.archive.org/oquo#AppropriatenessRecognisabilityCharacteristic -->

    <owl:Class rdf:about="https://purl.archive.org/oquo#AppropriatenessRecognisabilityCharacteristic">
        <rdfs:subClassOf rdf:resource="http://purl.org/net/QualityModel#QualityCharacteristic"/>
        <obo:IAO_0000115 xml:lang="en">The degree to which the Ontology enables users to recognise whether it is appropriate for their needs.</obo:IAO_0000115>
        <rdfs:label>appropriateness recognisability characteristic</rdfs:label>
    </owl:Class>
    


    <!-- https://purl.archive.org/oquo#AttributeRichnessMetric -->

    <owl:Class rdf:about="https://purl.archive.org/oquo#AttributeRichnessMetric">
        <rdfs:subClassOf rdf:resource="http://purl.org/net/QualityModel#DerivedMeasure"/>
        <rdfs:subClassOf>
            <owl:Restriction>
                <owl:onProperty rdf:resource="http://purl.org/net/QualityModel#hasScale"/>
                <owl:someValuesFrom>
                    <owl:Class>
                        <owl:intersectionOf rdf:parseType="Collection">
                            <rdf:Description rdf:about="https://purl.archive.org/oquo#RawScale"/>
                            <owl:Restriction>
                                <owl:onProperty rdf:resource="http://purl.org/net/QualityModel#hasRankigFunction"/>
                                <owl:hasValue rdf:resource="http://purl.org/net/QualityModel#HigherBest"/>
                            </owl:Restriction>
                        </owl:intersectionOf>
                    </owl:Class>
                </owl:someValuesFrom>
            </owl:Restriction>
        </rdfs:subClassOf>
        <rdfs:subClassOf>
            <owl:Restriction>
                <owl:onProperty rdf:resource="https://purl.archive.org/oquo#measuresCharacteristicPositively"/>
                <owl:someValuesFrom rdf:resource="https://purl.archive.org/oquo#ConsistentSearchAndQueryCharacteristic"/>
            </owl:Restriction>
        </rdfs:subClassOf>
        <rdfs:subClassOf>
            <owl:Restriction>
                <owl:onProperty rdf:resource="https://purl.archive.org/oquo#measuresCharacteristicPositively"/>
                <owl:someValuesFrom rdf:resource="https://purl.archive.org/oquo#DecisionTreesCharacteristic"/>
            </owl:Restriction>
        </rdfs:subClassOf>
        <rdfs:subClassOf>
            <owl:Restriction>
                <owl:onProperty rdf:resource="https://purl.archive.org/oquo#measuresCharacteristicPositively"/>
                <owl:someValuesFrom rdf:resource="https://purl.archive.org/oquo#GuidanceCharacteristic"/>
            </owl:Restriction>
        </rdfs:subClassOf>
        <rdfs:subClassOf>
            <owl:Restriction>
                <owl:onProperty rdf:resource="https://purl.archive.org/oquo#measuresCharacteristicPositively"/>
                <owl:someValuesFrom rdf:resource="https://purl.archive.org/oquo#IndexingAndLinkingCharacteristic"/>
            </owl:Restriction>
        </rdfs:subClassOf>
        <rdfs:subClassOf>
            <owl:Restriction>
                <owl:onProperty rdf:resource="https://purl.archive.org/oquo#measuresCharacteristicPositively"/>
                <owl:someValuesFrom rdf:resource="https://purl.archive.org/oquo#KnowledgeReuseCharacteristic"/>
            </owl:Restriction>
        </rdfs:subClassOf>
        <rdfs:subClassOf>
            <owl:Restriction>
                <owl:onProperty rdf:resource="https://purl.archive.org/oquo#measuresCharacteristicPositively"/>
                <owl:someValuesFrom rdf:resource="https://purl.archive.org/oquo#ResultsRepresentationCharacteristic"/>
            </owl:Restriction>
        </rdfs:subClassOf>
        <rdfs:subClassOf>
            <owl:Restriction>
                <owl:onProperty rdf:resource="https://purl.archive.org/oquo#measuresCharacteristicPositively"/>
                <owl:someValuesFrom rdf:resource="https://purl.archive.org/oquo#SchemaAndValueReconciliationCharacteristic"/>
            </owl:Restriction>
        </rdfs:subClassOf>
        <rdfs:subClassOf>
            <owl:Restriction>
                <owl:onProperty rdf:resource="https://purl.archive.org/oquo#measuresCharacteristicPositively"/>
                <owl:someValuesFrom rdf:resource="https://purl.archive.org/oquo#SimilarityCharacteristic"/>
            </owl:Restriction>
        </rdfs:subClassOf>
        <rdfs:subClassOf>
            <owl:Restriction>
                <owl:onProperty rdf:resource="https://purl.archive.org/oquo#measuresCharacteristicPositively"/>
                <owl:allValuesFrom>
                    <owl:Class>
                        <owl:unionOf rdf:parseType="Collection">
                            <rdf:Description rdf:about="https://purl.archive.org/oquo#ConsistentSearchAndQueryCharacteristic"/>
                            <rdf:Description rdf:about="https://purl.archive.org/oquo#DecisionTreesCharacteristic"/>
                            <rdf:Description rdf:about="https://purl.archive.org/oquo#GuidanceCharacteristic"/>
                            <rdf:Description rdf:about="https://purl.archive.org/oquo#IndexingAndLinkingCharacteristic"/>
                            <rdf:Description rdf:about="https://purl.archive.org/oquo#KnowledgeReuseCharacteristic"/>
                            <rdf:Description rdf:about="https://purl.archive.org/oquo#ResultsRepresentationCharacteristic"/>
                            <rdf:Description rdf:about="https://purl.archive.org/oquo#SchemaAndValueReconciliationCharacteristic"/>
                            <rdf:Description rdf:about="https://purl.archive.org/oquo#SimilarityCharacteristic"/>
                        </owl:unionOf>
                    </owl:Class>
                </owl:allValuesFrom>
            </owl:Restriction>
        </rdfs:subClassOf>
        <rdfs:subClassOf>
            <owl:Restriction>
                <owl:onProperty rdf:resource="http://purl.org/net/QualityModel#hasScale"/>
                <owl:hasValue rdf:resource="https://purl.archive.org/oquo#AttributeRichnessMetricScale"/>
            </owl:Restriction>
        </rdfs:subClassOf>
        <obo:IAO_0000115 xml:lang="en">Number of restrictions of the ontology per classes AROnto=∑|AttCi| / ∑|Ci |; where AttCi, is the set of Attributes of the Ci </obo:IAO_0000115>
        <rdf1:acronym>AROnto</rdf1:acronym>
        <rdfs:comment>Number of restrictions of the ontology per classes.</rdfs:comment>
        <rdfs:label>attribute richness metric</rdfs:label>
    </owl:Class>
    


    <!-- https://purl.archive.org/oquo#AvailabilityCharacteristic -->

    <owl:Class rdf:about="https://purl.archive.org/oquo#AvailabilityCharacteristic">
        <rdfs:subClassOf rdf:resource="http://purl.org/net/QualityModel#QualityCharacteristic"/>
        <obo:IAO_0000115 xml:lang="en">The degree to which an ontology, or part of it, is operational and available when required for use with different applications.</obo:IAO_0000115>
        <rdfs:label xml:lang="en">availability characteristic</rdfs:label>
    </owl:Class>
    


    <!-- https://purl.archive.org/oquo#ChangeabilityCharacteristic -->

    <owl:Class rdf:about="https://purl.archive.org/oquo#ChangeabilityCharacteristic">
        <rdfs:subClassOf rdf:resource="http://purl.org/net/QualityModel#QualityCharacteristic"/>
        <obo:IAO_0000115 xml:lang="en">The degree to which The Ontology enables a specified modification to be implemented. The ease with which a The ontology can be modified.</obo:IAO_0000115>
        <rdfs:label>changeability characteristic</rdfs:label>
    </owl:Class>
    


    <!-- https://purl.archive.org/oquo#ClassRichnessMetric -->

    <owl:Class rdf:about="https://purl.archive.org/oquo#ClassRichnessMetric">
        <rdfs:subClassOf rdf:resource="http://purl.org/net/QualityModel#DerivedMeasure"/>
        <rdfs:subClassOf>
            <owl:Restriction>
                <owl:onProperty rdf:resource="http://purl.org/net/QualityModel#hasScale"/>
                <owl:someValuesFrom>
                    <owl:Class>
                        <owl:intersectionOf rdf:parseType="Collection">
                            <rdf:Description rdf:about="https://purl.archive.org/oquo#RawScale"/>
                            <owl:Restriction>
                                <owl:onProperty rdf:resource="http://purl.org/net/QualityModel#hasRankigFunction"/>
                                <owl:hasValue rdf:resource="http://purl.org/net/QualityModel#HigherBest"/>
                            </owl:Restriction>
                        </owl:intersectionOf>
                    </owl:Class>
                </owl:someValuesFrom>
            </owl:Restriction>
        </rdfs:subClassOf>
        <rdfs:subClassOf>
            <owl:Restriction>
                <owl:onProperty rdf:resource="https://purl.archive.org/oquo#measuresCharacteristicPositively"/>
                <owl:someValuesFrom rdf:resource="https://purl.archive.org/oquo#InferenceCharacteristic"/>
            </owl:Restriction>
        </rdfs:subClassOf>
        <rdfs:subClassOf>
            <owl:Restriction>
                <owl:onProperty rdf:resource="https://purl.archive.org/oquo#measuresCharacteristicPositively"/>
                <owl:someValuesFrom rdf:resource="https://purl.archive.org/oquo#ResultsRepresentationCharacteristic"/>
            </owl:Restriction>
        </rdfs:subClassOf>
        <rdfs:subClassOf>
            <owl:Restriction>
                <owl:onProperty rdf:resource="https://purl.archive.org/oquo#measuresCharacteristicPositively"/>
                <owl:allValuesFrom>
                    <owl:Class>
                        <owl:unionOf rdf:parseType="Collection">
                            <rdf:Description rdf:about="https://purl.archive.org/oquo#InferenceCharacteristic"/>
                            <rdf:Description rdf:about="https://purl.archive.org/oquo#ResultsRepresentationCharacteristic"/>
                        </owl:unionOf>
                    </owl:Class>
                </owl:allValuesFrom>
            </owl:Restriction>
        </rdfs:subClassOf>
        <rdfs:subClassOf>
            <owl:Restriction>
                <owl:onProperty rdf:resource="http://purl.org/net/QualityModel#hasScale"/>
                <owl:hasValue rdf:resource="https://purl.archive.org/oquo#ClassRichnessMetricScale"/>
            </owl:Restriction>
        </rdfs:subClassOf>
        <obo:IAO_0000115 xml:lang="en">Mean number of individuals per class CROnto=∑| ICi| / ∑|Ci |; where ICi, is the set ofindividuals of the Ci </obo:IAO_0000115>
        <rdf1:acronym>CROnto</rdf1:acronym>
        <rdfs:comment>Mean number of individuals per class.</rdfs:comment>
        <rdfs:label>class richness metric</rdfs:label>
    </owl:Class>
    


    <!-- https://purl.archive.org/oquo#ClassesWithNoDescriptionMetric -->

    <owl:Class rdf:about="https://purl.archive.org/oquo#ClassesWithNoDescriptionMetric">
        <rdfs:subClassOf rdf:resource="http://purl.org/net/QualityModel#DerivedMeasure"/>
        <rdfs:subClassOf>
            <owl:Restriction>
                <owl:onProperty rdf:resource="http://purl.org/net/QualityModel#hasScale"/>
                <owl:someValuesFrom>
                    <owl:Class>
                        <owl:intersectionOf rdf:parseType="Collection">
                            <rdf:Description rdf:about="https://purl.archive.org/oquo#RawScale"/>
                            <owl:Restriction>
                                <owl:onProperty rdf:resource="http://purl.org/net/QualityModel#hasRankigFunction"/>
                                <owl:hasValue rdf:resource="http://purl.org/net/QualityModel#LowerBest"/>
                            </owl:Restriction>
                        </owl:intersectionOf>
                    </owl:Class>
                </owl:someValuesFrom>
            </owl:Restriction>
        </rdfs:subClassOf>
        <rdfs:subClassOf>
            <owl:Restriction>
                <owl:onProperty rdf:resource="https://purl.archive.org/oquo#measuresCharacteristicNegatively"/>
                <owl:someValuesFrom rdf:resource="https://purl.archive.org/oquo#EaseOfUseCharacteristic"/>
            </owl:Restriction>
        </rdfs:subClassOf>
        <rdfs:subClassOf>
            <owl:Restriction>
                <owl:onProperty rdf:resource="https://purl.archive.org/oquo#measuresCharacteristicNegatively"/>
                <owl:someValuesFrom rdf:resource="https://purl.archive.org/oquo#EfficiencyInUseCharacteristic"/>
            </owl:Restriction>
        </rdfs:subClassOf>
        <rdfs:subClassOf>
            <owl:Restriction>
                <owl:onProperty rdf:resource="https://purl.archive.org/oquo#measuresCharacteristicNegatively"/>
                <owl:someValuesFrom rdf:resource="https://purl.archive.org/oquo#HelpfulnessCharacteristic"/>
            </owl:Restriction>
        </rdfs:subClassOf>
        <rdfs:subClassOf>
            <owl:Restriction>
                <owl:onProperty rdf:resource="https://purl.archive.org/oquo#measuresCharacteristicNegatively"/>
                <owl:someValuesFrom rdf:resource="https://purl.archive.org/oquo#IndexingAndLinkingCharacteristic"/>
            </owl:Restriction>
        </rdfs:subClassOf>
        <rdfs:subClassOf>
            <owl:Restriction>
                <owl:onProperty rdf:resource="https://purl.archive.org/oquo#measuresCharacteristicNegatively"/>
                <owl:someValuesFrom rdf:resource="https://purl.archive.org/oquo#KnowledgeReuseCharacteristic"/>
            </owl:Restriction>
        </rdfs:subClassOf>
        <rdfs:subClassOf>
            <owl:Restriction>
                <owl:onProperty rdf:resource="https://purl.archive.org/oquo#measuresCharacteristicNegatively"/>
                <owl:someValuesFrom rdf:resource="https://purl.archive.org/oquo#LearnabilityCharacteristic"/>
            </owl:Restriction>
        </rdfs:subClassOf>
        <rdfs:subClassOf>
            <owl:Restriction>
                <owl:onProperty rdf:resource="https://purl.archive.org/oquo#measuresCharacteristicNegatively"/>
                <owl:allValuesFrom>
                    <owl:Class>
                        <owl:unionOf rdf:parseType="Collection">
                            <rdf:Description rdf:about="https://purl.archive.org/oquo#EaseOfUseCharacteristic"/>
                            <rdf:Description rdf:about="https://purl.archive.org/oquo#EfficiencyInUseCharacteristic"/>
                            <rdf:Description rdf:about="https://purl.archive.org/oquo#HelpfulnessCharacteristic"/>
                            <rdf:Description rdf:about="https://purl.archive.org/oquo#IndexingAndLinkingCharacteristic"/>
                            <rdf:Description rdf:about="https://purl.archive.org/oquo#KnowledgeReuseCharacteristic"/>
                            <rdf:Description rdf:about="https://purl.archive.org/oquo#LearnabilityCharacteristic"/>
                        </owl:unionOf>
                    </owl:Class>
                </owl:allValuesFrom>
            </owl:Restriction>
        </rdfs:subClassOf>
        <rdfs:subClassOf>
            <owl:Restriction>
                <owl:onProperty rdf:resource="http://purl.org/net/QualityModel#hasScale"/>
                <owl:hasValue rdf:resource="https://purl.archive.org/oquo#ClassesWithNoDescriptionMetricScale"/>
            </owl:Restriction>
        </rdfs:subClassOf>
        <obo:IAO_0000115>The Percentage of classes lacking a description in the ontology.</obo:IAO_0000115>
        <rdf1:acronym>CWND</rdf1:acronym>
        <rdfs:label>classes with no description metric</rdfs:label>
    </owl:Class>
    


    <!-- https://purl.archive.org/oquo#ClassesWithNoNameMetric -->

    <owl:Class rdf:about="https://purl.archive.org/oquo#ClassesWithNoNameMetric">
        <rdfs:subClassOf rdf:resource="http://purl.org/net/QualityModel#DerivedMeasure"/>
        <rdfs:subClassOf>
            <owl:Restriction>
                <owl:onProperty rdf:resource="http://purl.org/net/QualityModel#hasScale"/>
                <owl:someValuesFrom>
                    <owl:Class>
                        <owl:intersectionOf rdf:parseType="Collection">
                            <rdf:Description rdf:about="https://purl.archive.org/oquo#RawScale"/>
                            <owl:Restriction>
                                <owl:onProperty rdf:resource="http://purl.org/net/QualityModel#hasRankigFunction"/>
                                <owl:hasValue rdf:resource="http://purl.org/net/QualityModel#LowerBest"/>
                            </owl:Restriction>
                        </owl:intersectionOf>
                    </owl:Class>
                </owl:someValuesFrom>
            </owl:Restriction>
        </rdfs:subClassOf>
        <rdfs:subClassOf>
            <owl:Restriction>
                <owl:onProperty rdf:resource="https://purl.archive.org/oquo#measuresCharacteristicNegatively"/>
                <owl:someValuesFrom rdf:resource="https://purl.archive.org/oquo#EaseOfUseCharacteristic"/>
            </owl:Restriction>
        </rdfs:subClassOf>
        <rdfs:subClassOf>
            <owl:Restriction>
                <owl:onProperty rdf:resource="https://purl.archive.org/oquo#measuresCharacteristicNegatively"/>
                <owl:someValuesFrom rdf:resource="https://purl.archive.org/oquo#EfficiencyInUseCharacteristic"/>
            </owl:Restriction>
        </rdfs:subClassOf>
        <rdfs:subClassOf>
            <owl:Restriction>
                <owl:onProperty rdf:resource="https://purl.archive.org/oquo#measuresCharacteristicNegatively"/>
                <owl:someValuesFrom rdf:resource="https://purl.archive.org/oquo#IndexingAndLinkingCharacteristic"/>
            </owl:Restriction>
        </rdfs:subClassOf>
        <rdfs:subClassOf>
            <owl:Restriction>
                <owl:onProperty rdf:resource="https://purl.archive.org/oquo#measuresCharacteristicNegatively"/>
                <owl:someValuesFrom rdf:resource="https://purl.archive.org/oquo#KnowledgeReuseCharacteristic"/>
            </owl:Restriction>
        </rdfs:subClassOf>
        <rdfs:subClassOf>
            <owl:Restriction>
                <owl:onProperty rdf:resource="https://purl.archive.org/oquo#measuresCharacteristicNegatively"/>
                <owl:someValuesFrom rdf:resource="https://purl.archive.org/oquo#TextAnalysisCharacteristic"/>
            </owl:Restriction>
        </rdfs:subClassOf>
        <rdfs:subClassOf>
            <owl:Restriction>
                <owl:onProperty rdf:resource="https://purl.archive.org/oquo#measuresCharacteristicNegatively"/>
                <owl:allValuesFrom>
                    <owl:Class>
                        <owl:unionOf rdf:parseType="Collection">
                            <rdf:Description rdf:about="https://purl.archive.org/oquo#EaseOfUseCharacteristic"/>
                            <rdf:Description rdf:about="https://purl.archive.org/oquo#EfficiencyInUseCharacteristic"/>
                            <rdf:Description rdf:about="https://purl.archive.org/oquo#IndexingAndLinkingCharacteristic"/>
                            <rdf:Description rdf:about="https://purl.archive.org/oquo#KnowledgeReuseCharacteristic"/>
                            <rdf:Description rdf:about="https://purl.archive.org/oquo#TextAnalysisCharacteristic"/>
                        </owl:unionOf>
                    </owl:Class>
                </owl:allValuesFrom>
            </owl:Restriction>
        </rdfs:subClassOf>
        <rdfs:subClassOf>
            <owl:Restriction>
                <owl:onProperty rdf:resource="http://purl.org/net/QualityModel#hasScale"/>
                <owl:hasValue rdf:resource="https://purl.archive.org/oquo#ClassesWithNoNameMetricScale"/>
            </owl:Restriction>
        </rdfs:subClassOf>
        <obo:IAO_0000115>The Percentage of classes lacking a name in the ontology.</obo:IAO_0000115>
        <rdf1:acronym>CWNN</rdf1:acronym>
        <rdfs:label>classes with no name metric</rdfs:label>
    </owl:Class>
    


    <!-- https://purl.archive.org/oquo#ClassesWithNoSynonymMetric -->

    <owl:Class rdf:about="https://purl.archive.org/oquo#ClassesWithNoSynonymMetric">
        <rdfs:subClassOf rdf:resource="http://purl.org/net/QualityModel#DerivedMeasure"/>
        <rdfs:subClassOf>
            <owl:Restriction>
                <owl:onProperty rdf:resource="http://purl.org/net/QualityModel#hasScale"/>
                <owl:someValuesFrom>
                    <owl:Class>
                        <owl:intersectionOf rdf:parseType="Collection">
                            <rdf:Description rdf:about="https://purl.archive.org/oquo#RawScale"/>
                            <owl:Restriction>
                                <owl:onProperty rdf:resource="http://purl.org/net/QualityModel#hasRankigFunction"/>
                                <owl:hasValue rdf:resource="http://purl.org/net/QualityModel#LowerBest"/>
                            </owl:Restriction>
                        </owl:intersectionOf>
                    </owl:Class>
                </owl:someValuesFrom>
            </owl:Restriction>
        </rdfs:subClassOf>
        <rdfs:subClassOf>
            <owl:Restriction>
                <owl:onProperty rdf:resource="https://purl.archive.org/oquo#measuresCharacteristicNegatively"/>
                <owl:someValuesFrom rdf:resource="https://purl.archive.org/oquo#EaseOfUseCharacteristic"/>
            </owl:Restriction>
        </rdfs:subClassOf>
        <rdfs:subClassOf>
            <owl:Restriction>
                <owl:onProperty rdf:resource="https://purl.archive.org/oquo#measuresCharacteristicNegatively"/>
                <owl:someValuesFrom rdf:resource="https://purl.archive.org/oquo#EfficiencyInUseCharacteristic"/>
            </owl:Restriction>
        </rdfs:subClassOf>
        <rdfs:subClassOf>
            <owl:Restriction>
                <owl:onProperty rdf:resource="https://purl.archive.org/oquo#measuresCharacteristicNegatively"/>
                <owl:someValuesFrom rdf:resource="https://purl.archive.org/oquo#IndexingAndLinkingCharacteristic"/>
            </owl:Restriction>
        </rdfs:subClassOf>
        <rdfs:subClassOf>
            <owl:Restriction>
                <owl:onProperty rdf:resource="https://purl.archive.org/oquo#measuresCharacteristicNegatively"/>
                <owl:someValuesFrom rdf:resource="https://purl.archive.org/oquo#KnowledgeReuseCharacteristic"/>
            </owl:Restriction>
        </rdfs:subClassOf>
        <rdfs:subClassOf>
            <owl:Restriction>
                <owl:onProperty rdf:resource="https://purl.archive.org/oquo#measuresCharacteristicNegatively"/>
                <owl:someValuesFrom rdf:resource="https://purl.archive.org/oquo#TextAnalysisCharacteristic"/>
            </owl:Restriction>
        </rdfs:subClassOf>
        <rdfs:subClassOf>
            <owl:Restriction>
                <owl:onProperty rdf:resource="https://purl.archive.org/oquo#measuresCharacteristicNegatively"/>
                <owl:allValuesFrom>
                    <owl:Class>
                        <owl:unionOf rdf:parseType="Collection">
                            <rdf:Description rdf:about="https://purl.archive.org/oquo#EaseOfUseCharacteristic"/>
                            <rdf:Description rdf:about="https://purl.archive.org/oquo#EfficiencyInUseCharacteristic"/>
                            <rdf:Description rdf:about="https://purl.archive.org/oquo#IndexingAndLinkingCharacteristic"/>
                            <rdf:Description rdf:about="https://purl.archive.org/oquo#KnowledgeReuseCharacteristic"/>
                            <rdf:Description rdf:about="https://purl.archive.org/oquo#TextAnalysisCharacteristic"/>
                        </owl:unionOf>
                    </owl:Class>
                </owl:allValuesFrom>
            </owl:Restriction>
        </rdfs:subClassOf>
        <rdfs:subClassOf>
            <owl:Restriction>
                <owl:onProperty rdf:resource="http://purl.org/net/QualityModel#hasScale"/>
                <owl:hasValue rdf:resource="https://purl.archive.org/oquo#ClassesWithNoSynonymMetricScale"/>
            </owl:Restriction>
        </rdfs:subClassOf>
        <obo:IAO_0000115>The Percentage of classes lacking a synonym in the ontology.</obo:IAO_0000115>
        <rdf1:acronym>CWNS</rdf1:acronym>
        <rdfs:label>classes with no synonym metric</rdfs:label>
    </owl:Class>
    


    <!-- https://purl.archive.org/oquo#ClassifyingInstancesCharacteristic -->

    <owl:Class rdf:about="https://purl.archive.org/oquo#ClassifyingInstancesCharacteristic">
        <rdfs:subClassOf rdf:resource="http://purl.org/net/QualityModel#QualityCharacteristic"/>
        <obo:IAO_0000115 xml:lang="en">Degree in which ontology Instances can be recognized as member of a certain class.</obo:IAO_0000115>
        <rdfs:label>classifying instances characteristic</rdfs:label>
    </owl:Class>
    


    <!-- https://purl.archive.org/oquo#ClusteringCharacteristic -->

    <owl:Class rdf:about="https://purl.archive.org/oquo#ClusteringCharacteristic">
        <rdfs:subClassOf rdf:resource="http://purl.org/net/QualityModel#QualityCharacteristic"/>
        <obo:IAO_0000115 xml:lang="en">Degree in which the annotations of data with respect to ontology terms can be used for clustering such data against the aspects of the ontology.</obo:IAO_0000115>
        <rdfs:label>clustering characteristic</rdfs:label>
    </owl:Class>
    


    <!-- https://purl.archive.org/oquo#CognitiveSatisfactionCharacteristic -->

    <owl:Class rdf:about="https://purl.archive.org/oquo#CognitiveSatisfactionCharacteristic">
        <rdfs:subClassOf rdf:resource="http://purl.org/net/QualityModel#QualityCharacteristic"/>
        <obo:IAO_0000115 xml:lang="en">Cognitive satisfaction</obo:IAO_0000115>
        <oboInOwl:hasExactSynonym xml:lang="en">Likability characteristic</oboInOwl:hasExactSynonym>
        <rdfs:label>cognitive satisfaction characteristic</rdfs:label>
    </owl:Class>
    


    <!-- https://purl.archive.org/oquo#CohesionCharacteristic -->

    <owl:Class rdf:about="https://purl.archive.org/oquo#CohesionCharacteristic">
        <rdfs:subClassOf rdf:resource="http://purl.org/net/QualityModel#QualityCharacteristic"/>
        <obo:IAO_0000115 xml:lang="en">An ontology has a high cohesion if the classes are strongly related.</obo:IAO_0000115>
        <rdfs:label>cohesion characteristic</rdfs:label>
    </owl:Class>
    


    <!-- https://purl.archive.org/oquo#CompatibilityCharacteristic -->

    <owl:Class rdf:about="https://purl.archive.org/oquo#CompatibilityCharacteristic">
        <rdfs:subClassOf rdf:resource="http://purl.org/net/QualityModel#QualityCharacteristic"/>
        <rdfs:subClassOf>
            <owl:Restriction>
                <owl:onProperty rdf:resource="http://purl.org/net/QualityModel#hasSubCharacteristic"/>
                <owl:someValuesFrom rdf:resource="https://purl.archive.org/oquo#InteroperabilityCharacteristic"/>
            </owl:Restriction>
        </rdfs:subClassOf>
        <rdfs:subClassOf>
            <owl:Restriction>
                <owl:onProperty rdf:resource="http://purl.org/net/QualityModel#hasSubCharacteristic"/>
                <owl:someValuesFrom rdf:resource="https://purl.archive.org/oquo#ReplaceabilityCharacteristic"/>
            </owl:Restriction>
        </rdfs:subClassOf>
        <rdfs:subClassOf>
            <owl:Restriction>
                <owl:onProperty rdf:resource="http://purl.org/net/QualityModel#hasSubCharacteristic"/>
                <owl:allValuesFrom>
                    <owl:Class>
                        <owl:unionOf rdf:parseType="Collection">
                            <rdf:Description rdf:about="https://purl.archive.org/oquo#InteroperabilityCharacteristic"/>
                            <rdf:Description rdf:about="https://purl.archive.org/oquo#ReplaceabilityCharacteristic"/>
                        </owl:unionOf>
                    </owl:Class>
                </owl:allValuesFrom>
            </owl:Restriction>
        </rdfs:subClassOf>
        <obo:IAO_0000115 xml:lang="en">The ability of two or more software components to exchange information and/or to perform their required functions while sharing the same hardware or software environment.</obo:IAO_0000115>
        <rdfs:label>compatibility characteristic</rdfs:label>
    </owl:Class>
    


    <!-- https://purl.archive.org/oquo#ConsistencyCharacteristic -->

    <owl:Class rdf:about="https://purl.archive.org/oquo#ConsistencyCharacteristic">
        <rdfs:subClassOf rdf:resource="http://purl.org/net/QualityModel#QualityCharacteristic"/>
        <obo:IAO_0000115 xml:lang="en">Degree of the consistency of the ontology.</obo:IAO_0000115>
        <rdfs:label>consistency characteristic</rdfs:label>
    </owl:Class>
    


    <!-- https://purl.archive.org/oquo#ConsistencyMetric -->

    <owl:Class rdf:about="https://purl.archive.org/oquo#ConsistencyMetric">
        <rdfs:subClassOf rdf:resource="http://purl.org/net/QualityModel#DerivedMeasure"/>
        <rdfs:subClassOf>
            <owl:Restriction>
                <owl:onProperty rdf:resource="http://purl.org/net/QualityModel#hasScale"/>
                <owl:someValuesFrom>
                    <owl:Class>
                        <owl:intersectionOf rdf:parseType="Collection">
                            <rdf:Description rdf:about="https://purl.archive.org/oquo#RawScale"/>
                            <owl:Restriction>
                                <owl:onProperty rdf:resource="http://purl.org/net/QualityModel#hasRankigFunction"/>
                                <owl:hasValue rdf:resource="http://purl.org/net/QualityModel#HigherBest"/>
                            </owl:Restriction>
                        </owl:intersectionOf>
                    </owl:Class>
                </owl:someValuesFrom>
            </owl:Restriction>
        </rdfs:subClassOf>
        <rdfs:subClassOf>
            <owl:Restriction>
                <owl:onProperty rdf:resource="https://purl.archive.org/oquo#measuresCharacteristicPositively"/>
                <owl:someValuesFrom rdf:resource="https://purl.archive.org/oquo#ConsistencyCharacteristic"/>
            </owl:Restriction>
        </rdfs:subClassOf>
        <rdfs:subClassOf>
            <owl:Restriction>
                <owl:onProperty rdf:resource="https://purl.archive.org/oquo#measuresCharacteristicPositively"/>
                <owl:allValuesFrom rdf:resource="https://purl.archive.org/oquo#ConsistencyCharacteristic"/>
            </owl:Restriction>
        </rdfs:subClassOf>
        <obo:IAO_0000115>Checks if the ontology is consistent or not.</obo:IAO_0000115>
        <rdfs:label>consistency metric</rdfs:label>
    </owl:Class>
    


    <!-- https://purl.archive.org/oquo#ConsistentSearchAndQueryCharacteristic -->

    <owl:Class rdf:about="https://purl.archive.org/oquo#ConsistentSearchAndQueryCharacteristic">
        <rdfs:subClassOf rdf:resource="http://purl.org/net/QualityModel#QualityCharacteristic"/>
        <obo:IAO_0000115 xml:lang="en">The degree which the formal model and structure of the ontology provide a semantic context to evaluate which are the data wanted by the users, allowing better querying and searching methods.</obo:IAO_0000115>
        <rdfs:label>consistent search and query characteristic</rdfs:label>
    </owl:Class>
    


    <!-- https://purl.archive.org/oquo#ContextConformityInUseCharacteristic -->

    <owl:Class rdf:about="https://purl.archive.org/oquo#ContextConformityInUseCharacteristic">
        <rdfs:subClassOf rdf:resource="http://purl.org/net/QualityModel#QualityCharacteristic"/>
        <obo:IAO_0000115 xml:lang="en">The degree to which usability in use meets requirements in all the intended contexts of use.</obo:IAO_0000115>
        <rdfs:label>context conformity in use characteristic</rdfs:label>
    </owl:Class>
    


    <!-- https://purl.archive.org/oquo#ContextExtendibilityInUseCharacteristic -->

    <owl:Class rdf:about="https://purl.archive.org/oquo#ContextExtendibilityInUseCharacteristic">
        <rdfs:subClassOf rdf:resource="http://purl.org/net/QualityModel#QualityCharacteristic"/>
        <obo:IAO_0000115 xml:lang="en">The degree of usability in use in contexts beyond those initially intended.</obo:IAO_0000115>
        <rdfs:label>context extendibility in use characteristic</rdfs:label>
    </owl:Class>
    


    <!-- https://purl.archive.org/oquo#ControlledVocabularyCharacteristic -->

    <owl:Class rdf:about="https://purl.archive.org/oquo#ControlledVocabularyCharacteristic">
        <rdfs:subClassOf rdf:resource="http://purl.org/net/QualityModel#QualityCharacteristic"/>
        <obo:IAO_0000115 xml:lang="en">Capability of the ontology to avoid heterogeneity of the terms.</obo:IAO_0000115>
        <rdfs:label>controlled vocabulary characteristic</rdfs:label>
    </owl:Class>
    


    <!-- https://purl.archive.org/oquo#CouplingBetweenObjectsMetric -->

    <owl:Class rdf:about="https://purl.archive.org/oquo#CouplingBetweenObjectsMetric">
        <rdfs:subClassOf rdf:resource="http://purl.org/net/QualityModel#DerivedMeasure"/>
        <rdfs:subClassOf>
            <owl:Restriction>
                <owl:onProperty rdf:resource="http://purl.org/net/QualityModel#hasScale"/>
                <owl:someValuesFrom>
                    <owl:Class>
                        <owl:intersectionOf rdf:parseType="Collection">
                            <rdf:Description rdf:about="https://purl.archive.org/oquo#RawScale"/>
                            <owl:Restriction>
                                <owl:onProperty rdf:resource="http://purl.org/net/QualityModel#hasRankigFunction"/>
                                <owl:hasValue rdf:resource="http://purl.org/net/QualityModel#LowerBest"/>
                            </owl:Restriction>
                        </owl:intersectionOf>
                    </owl:Class>
                </owl:someValuesFrom>
            </owl:Restriction>
        </rdfs:subClassOf>
        <rdfs:subClassOf>
            <owl:Restriction>
                <owl:onProperty rdf:resource="https://purl.archive.org/oquo#measuresCharacteristicPositively"/>
                <owl:someValuesFrom rdf:resource="https://purl.archive.org/oquo#AdaptabilityCharacteristic"/>
            </owl:Restriction>
        </rdfs:subClassOf>
        <rdfs:subClassOf>
            <owl:Restriction>
                <owl:onProperty rdf:resource="https://purl.archive.org/oquo#measuresCharacteristicPositively"/>
                <owl:someValuesFrom rdf:resource="https://purl.archive.org/oquo#AnalysabilityCharacteristic"/>
            </owl:Restriction>
        </rdfs:subClassOf>
        <rdfs:subClassOf>
            <owl:Restriction>
                <owl:onProperty rdf:resource="https://purl.archive.org/oquo#measuresCharacteristicPositively"/>
                <owl:someValuesFrom rdf:resource="https://purl.archive.org/oquo#ChangeabilityCharacteristic"/>
            </owl:Restriction>
        </rdfs:subClassOf>
        <rdfs:subClassOf>
            <owl:Restriction>
                <owl:onProperty rdf:resource="https://purl.archive.org/oquo#measuresCharacteristicPositively"/>
                <owl:someValuesFrom rdf:resource="https://purl.archive.org/oquo#LearnabilityCharacteristic"/>
            </owl:Restriction>
        </rdfs:subClassOf>
        <rdfs:subClassOf>
            <owl:Restriction>
                <owl:onProperty rdf:resource="https://purl.archive.org/oquo#measuresCharacteristicPositively"/>
                <owl:someValuesFrom rdf:resource="https://purl.archive.org/oquo#ModificationStabilityCharacteristic"/>
            </owl:Restriction>
        </rdfs:subClassOf>
        <rdfs:subClassOf>
            <owl:Restriction>
                <owl:onProperty rdf:resource="https://purl.archive.org/oquo#measuresCharacteristicPositively"/>
                <owl:someValuesFrom rdf:resource="https://purl.archive.org/oquo#ModularityCharacteristic"/>
            </owl:Restriction>
        </rdfs:subClassOf>
        <rdfs:subClassOf>
            <owl:Restriction>
                <owl:onProperty rdf:resource="https://purl.archive.org/oquo#measuresCharacteristicPositively"/>
                <owl:someValuesFrom rdf:resource="https://purl.archive.org/oquo#ReusabilityCharacteristic"/>
            </owl:Restriction>
        </rdfs:subClassOf>
        <rdfs:subClassOf>
            <owl:Restriction>
                <owl:onProperty rdf:resource="https://purl.archive.org/oquo#measuresCharacteristicPositively"/>
                <owl:someValuesFrom rdf:resource="https://purl.archive.org/oquo#TestabilityCharacteristic"/>
            </owl:Restriction>
        </rdfs:subClassOf>
        <rdfs:subClassOf>
            <owl:Restriction>
                <owl:onProperty rdf:resource="https://purl.archive.org/oquo#measuresCharacteristicPositively"/>
                <owl:allValuesFrom>
                    <owl:Class>
                        <owl:unionOf rdf:parseType="Collection">
                            <rdf:Description rdf:about="https://purl.archive.org/oquo#AdaptabilityCharacteristic"/>
                            <rdf:Description rdf:about="https://purl.archive.org/oquo#AnalysabilityCharacteristic"/>
                            <rdf:Description rdf:about="https://purl.archive.org/oquo#ChangeabilityCharacteristic"/>
                            <rdf:Description rdf:about="https://purl.archive.org/oquo#LearnabilityCharacteristic"/>
                            <rdf:Description rdf:about="https://purl.archive.org/oquo#ModificationStabilityCharacteristic"/>
                            <rdf:Description rdf:about="https://purl.archive.org/oquo#ModularityCharacteristic"/>
                            <rdf:Description rdf:about="https://purl.archive.org/oquo#ReusabilityCharacteristic"/>
                            <rdf:Description rdf:about="https://purl.archive.org/oquo#TestabilityCharacteristic"/>
                        </owl:unionOf>
                    </owl:Class>
                </owl:allValuesFrom>
            </owl:Restriction>
        </rdfs:subClassOf>
        <rdfs:subClassOf>
            <owl:Restriction>
                <owl:onProperty rdf:resource="http://purl.org/net/QualityModel#hasScale"/>
                <owl:hasValue rdf:resource="https://purl.archive.org/oquo#CouplingBetweenObjectsMetricScale"/>
            </owl:Restriction>
        </rdfs:subClassOf>
        <obo:IAO_0000115 xml:lang="en">Number of related classes. Number of direct ancestor of classes divided by the number of classes minus subclasses of Thing CBOOnto=∑|SupCi|/(∑|Ci| -| RThing|) </obo:IAO_0000115>
        <rdf1:acronym>CBOOnto</rdf1:acronym>
        <rdfs:comment>Number of related classes. Number of direct ancestor of classes divided by the number of classes minus subclasses of Thing.</rdfs:comment>
        <rdfs:label>coupling between objects metric</rdfs:label>
    </owl:Class>
    


    <!-- https://purl.archive.org/oquo#CriticalIssue -->

    <owl:Class rdf:about="https://purl.archive.org/oquo#CriticalIssue">
        <rdfs:subClassOf rdf:resource="http://purl.org/ipo/core#Issue"/>
        <rdfs:comment>A critical incident with very high impact</rdfs:comment>
        <rdfs:label>critical issue</rdfs:label>
    </owl:Class>
    


    <!-- https://purl.archive.org/oquo#CyclesCharacteristic -->

    <owl:Class rdf:about="https://purl.archive.org/oquo#CyclesCharacteristic">
        <rdfs:subClassOf rdf:resource="http://purl.org/net/QualityModel#QualityCharacteristic"/>
        <obo:IAO_0000115 xml:lang="en">The existence of cycles through a particular semantic relation is usually a sign of bad design, since they may lead to inconsistencies.</obo:IAO_0000115>
        <rdfs:label>cycles characteristic</rdfs:label>
    </owl:Class>
    


    <!-- https://purl.archive.org/oquo#DataPropertiesWithNoDescriptionMetric -->

    <owl:Class rdf:about="https://purl.archive.org/oquo#DataPropertiesWithNoDescriptionMetric">
        <rdfs:subClassOf rdf:resource="http://purl.org/net/QualityModel#DerivedMeasure"/>
        <rdfs:subClassOf>
            <owl:Restriction>
                <owl:onProperty rdf:resource="http://purl.org/net/QualityModel#hasScale"/>
                <owl:someValuesFrom>
                    <owl:Class>
                        <owl:intersectionOf rdf:parseType="Collection">
                            <rdf:Description rdf:about="https://purl.archive.org/oquo#RawScale"/>
                            <owl:Restriction>
                                <owl:onProperty rdf:resource="http://purl.org/net/QualityModel#hasRankigFunction"/>
                                <owl:hasValue rdf:resource="http://purl.org/net/QualityModel#LowerBest"/>
                            </owl:Restriction>
                        </owl:intersectionOf>
                    </owl:Class>
                </owl:someValuesFrom>
            </owl:Restriction>
        </rdfs:subClassOf>
        <rdfs:subClassOf>
            <owl:Restriction>
                <owl:onProperty rdf:resource="https://purl.archive.org/oquo#measuresCharacteristicNegatively"/>
                <owl:someValuesFrom rdf:resource="https://purl.archive.org/oquo#EaseOfUseCharacteristic"/>
            </owl:Restriction>
        </rdfs:subClassOf>
        <rdfs:subClassOf>
            <owl:Restriction>
                <owl:onProperty rdf:resource="https://purl.archive.org/oquo#measuresCharacteristicNegatively"/>
                <owl:someValuesFrom rdf:resource="https://purl.archive.org/oquo#EfficiencyInUseCharacteristic"/>
            </owl:Restriction>
        </rdfs:subClassOf>
        <rdfs:subClassOf>
            <owl:Restriction>
                <owl:onProperty rdf:resource="https://purl.archive.org/oquo#measuresCharacteristicNegatively"/>
                <owl:someValuesFrom rdf:resource="https://purl.archive.org/oquo#HelpfulnessCharacteristic"/>
            </owl:Restriction>
        </rdfs:subClassOf>
        <rdfs:subClassOf>
            <owl:Restriction>
                <owl:onProperty rdf:resource="https://purl.archive.org/oquo#measuresCharacteristicNegatively"/>
                <owl:someValuesFrom rdf:resource="https://purl.archive.org/oquo#IndexingAndLinkingCharacteristic"/>
            </owl:Restriction>
        </rdfs:subClassOf>
        <rdfs:subClassOf>
            <owl:Restriction>
                <owl:onProperty rdf:resource="https://purl.archive.org/oquo#measuresCharacteristicNegatively"/>
                <owl:someValuesFrom rdf:resource="https://purl.archive.org/oquo#KnowledgeReuseCharacteristic"/>
            </owl:Restriction>
        </rdfs:subClassOf>
        <rdfs:subClassOf>
            <owl:Restriction>
                <owl:onProperty rdf:resource="https://purl.archive.org/oquo#measuresCharacteristicNegatively"/>
                <owl:someValuesFrom rdf:resource="https://purl.archive.org/oquo#LearnabilityCharacteristic"/>
            </owl:Restriction>
        </rdfs:subClassOf>
        <rdfs:subClassOf>
            <owl:Restriction>
                <owl:onProperty rdf:resource="https://purl.archive.org/oquo#measuresCharacteristicNegatively"/>
                <owl:allValuesFrom>
                    <owl:Class>
                        <owl:unionOf rdf:parseType="Collection">
                            <rdf:Description rdf:about="https://purl.archive.org/oquo#EaseOfUseCharacteristic"/>
                            <rdf:Description rdf:about="https://purl.archive.org/oquo#EfficiencyInUseCharacteristic"/>
                            <rdf:Description rdf:about="https://purl.archive.org/oquo#HelpfulnessCharacteristic"/>
                            <rdf:Description rdf:about="https://purl.archive.org/oquo#IndexingAndLinkingCharacteristic"/>
                            <rdf:Description rdf:about="https://purl.archive.org/oquo#KnowledgeReuseCharacteristic"/>
                            <rdf:Description rdf:about="https://purl.archive.org/oquo#LearnabilityCharacteristic"/>
                        </owl:unionOf>
                    </owl:Class>
                </owl:allValuesFrom>
            </owl:Restriction>
        </rdfs:subClassOf>
        <rdfs:subClassOf>
            <owl:Restriction>
                <owl:onProperty rdf:resource="http://purl.org/net/QualityModel#hasScale"/>
                <owl:hasValue rdf:resource="https://purl.archive.org/oquo#DataPropertiesWithNoDescriptionMetricScale"/>
            </owl:Restriction>
        </rdfs:subClassOf>
        <obo:IAO_0000115>The Percentage of data properties lacking a description in the ontology.</obo:IAO_0000115>
        <rdf1:acronym>DPWND</rdf1:acronym>
        <rdfs:label>data properties with no description metric</rdfs:label>
    </owl:Class>
    


    <!-- https://purl.archive.org/oquo#DataPropertiesWithNoNameMetric -->

    <owl:Class rdf:about="https://purl.archive.org/oquo#DataPropertiesWithNoNameMetric">
        <rdfs:subClassOf rdf:resource="http://purl.org/net/QualityModel#DerivedMeasure"/>
        <rdfs:subClassOf>
            <owl:Restriction>
                <owl:onProperty rdf:resource="http://purl.org/net/QualityModel#hasScale"/>
                <owl:someValuesFrom>
                    <owl:Class>
                        <owl:intersectionOf rdf:parseType="Collection">
                            <rdf:Description rdf:about="https://purl.archive.org/oquo#RawScale"/>
                            <owl:Restriction>
                                <owl:onProperty rdf:resource="http://purl.org/net/QualityModel#hasRankigFunction"/>
                                <owl:hasValue rdf:resource="http://purl.org/net/QualityModel#LowerBest"/>
                            </owl:Restriction>
                        </owl:intersectionOf>
                    </owl:Class>
                </owl:someValuesFrom>
            </owl:Restriction>
        </rdfs:subClassOf>
        <rdfs:subClassOf>
            <owl:Restriction>
                <owl:onProperty rdf:resource="https://purl.archive.org/oquo#measuresCharacteristicNegatively"/>
                <owl:someValuesFrom rdf:resource="https://purl.archive.org/oquo#EaseOfUseCharacteristic"/>
            </owl:Restriction>
        </rdfs:subClassOf>
        <rdfs:subClassOf>
            <owl:Restriction>
                <owl:onProperty rdf:resource="https://purl.archive.org/oquo#measuresCharacteristicNegatively"/>
                <owl:someValuesFrom rdf:resource="https://purl.archive.org/oquo#EfficiencyInUseCharacteristic"/>
            </owl:Restriction>
        </rdfs:subClassOf>
        <rdfs:subClassOf>
            <owl:Restriction>
                <owl:onProperty rdf:resource="https://purl.archive.org/oquo#measuresCharacteristicNegatively"/>
                <owl:someValuesFrom rdf:resource="https://purl.archive.org/oquo#IndexingAndLinkingCharacteristic"/>
            </owl:Restriction>
        </rdfs:subClassOf>
        <rdfs:subClassOf>
            <owl:Restriction>
                <owl:onProperty rdf:resource="https://purl.archive.org/oquo#measuresCharacteristicNegatively"/>
                <owl:someValuesFrom rdf:resource="https://purl.archive.org/oquo#KnowledgeReuseCharacteristic"/>
            </owl:Restriction>
        </rdfs:subClassOf>
        <rdfs:subClassOf>
            <owl:Restriction>
                <owl:onProperty rdf:resource="https://purl.archive.org/oquo#measuresCharacteristicNegatively"/>
                <owl:someValuesFrom rdf:resource="https://purl.archive.org/oquo#TextAnalysisCharacteristic"/>
            </owl:Restriction>
        </rdfs:subClassOf>
        <rdfs:subClassOf>
            <owl:Restriction>
                <owl:onProperty rdf:resource="https://purl.archive.org/oquo#measuresCharacteristicNegatively"/>
                <owl:allValuesFrom>
                    <owl:Class>
                        <owl:unionOf rdf:parseType="Collection">
                            <rdf:Description rdf:about="https://purl.archive.org/oquo#EaseOfUseCharacteristic"/>
                            <rdf:Description rdf:about="https://purl.archive.org/oquo#EfficiencyInUseCharacteristic"/>
                            <rdf:Description rdf:about="https://purl.archive.org/oquo#IndexingAndLinkingCharacteristic"/>
                            <rdf:Description rdf:about="https://purl.archive.org/oquo#KnowledgeReuseCharacteristic"/>
                            <rdf:Description rdf:about="https://purl.archive.org/oquo#TextAnalysisCharacteristic"/>
                        </owl:unionOf>
                    </owl:Class>
                </owl:allValuesFrom>
            </owl:Restriction>
        </rdfs:subClassOf>
        <rdfs:subClassOf>
            <owl:Restriction>
                <owl:onProperty rdf:resource="http://purl.org/net/QualityModel#hasScale"/>
                <owl:hasValue rdf:resource="https://purl.archive.org/oquo#DataPropertiesWithNoNameMetricScale"/>
            </owl:Restriction>
        </rdfs:subClassOf>
        <obo:IAO_0000115>The Percentage of data properties lacking a name in the ontology.</obo:IAO_0000115>
        <rdf1:acronym>DPWNN</rdf1:acronym>
        <rdfs:label>data properties with no name metric</rdfs:label>
    </owl:Class>
    


    <!-- https://purl.archive.org/oquo#DataPropertiesWithNoSynonymMetric -->

    <owl:Class rdf:about="https://purl.archive.org/oquo#DataPropertiesWithNoSynonymMetric">
        <rdfs:subClassOf rdf:resource="http://purl.org/net/QualityModel#DerivedMeasure"/>
        <rdfs:subClassOf>
            <owl:Restriction>
                <owl:onProperty rdf:resource="http://purl.org/net/QualityModel#hasScale"/>
                <owl:someValuesFrom>
                    <owl:Class>
                        <owl:intersectionOf rdf:parseType="Collection">
                            <rdf:Description rdf:about="https://purl.archive.org/oquo#RawScale"/>
                            <owl:Restriction>
                                <owl:onProperty rdf:resource="http://purl.org/net/QualityModel#hasRankigFunction"/>
                                <owl:hasValue rdf:resource="http://purl.org/net/QualityModel#LowerBest"/>
                            </owl:Restriction>
                        </owl:intersectionOf>
                    </owl:Class>
                </owl:someValuesFrom>
            </owl:Restriction>
        </rdfs:subClassOf>
        <rdfs:subClassOf>
            <owl:Restriction>
                <owl:onProperty rdf:resource="https://purl.archive.org/oquo#measuresCharacteristicNegatively"/>
                <owl:someValuesFrom rdf:resource="https://purl.archive.org/oquo#EaseOfUseCharacteristic"/>
            </owl:Restriction>
        </rdfs:subClassOf>
        <rdfs:subClassOf>
            <owl:Restriction>
                <owl:onProperty rdf:resource="https://purl.archive.org/oquo#measuresCharacteristicNegatively"/>
                <owl:someValuesFrom rdf:resource="https://purl.archive.org/oquo#EfficiencyInUseCharacteristic"/>
            </owl:Restriction>
        </rdfs:subClassOf>
        <rdfs:subClassOf>
            <owl:Restriction>
                <owl:onProperty rdf:resource="https://purl.archive.org/oquo#measuresCharacteristicNegatively"/>
                <owl:someValuesFrom rdf:resource="https://purl.archive.org/oquo#IndexingAndLinkingCharacteristic"/>
            </owl:Restriction>
        </rdfs:subClassOf>
        <rdfs:subClassOf>
            <owl:Restriction>
                <owl:onProperty rdf:resource="https://purl.archive.org/oquo#measuresCharacteristicNegatively"/>
                <owl:someValuesFrom rdf:resource="https://purl.archive.org/oquo#KnowledgeReuseCharacteristic"/>
            </owl:Restriction>
        </rdfs:subClassOf>
        <rdfs:subClassOf>
            <owl:Restriction>
                <owl:onProperty rdf:resource="https://purl.archive.org/oquo#measuresCharacteristicNegatively"/>
                <owl:someValuesFrom rdf:resource="https://purl.archive.org/oquo#TextAnalysisCharacteristic"/>
            </owl:Restriction>
        </rdfs:subClassOf>
        <rdfs:subClassOf>
            <owl:Restriction>
                <owl:onProperty rdf:resource="https://purl.archive.org/oquo#measuresCharacteristicNegatively"/>
                <owl:allValuesFrom>
                    <owl:Class>
                        <owl:unionOf rdf:parseType="Collection">
                            <rdf:Description rdf:about="https://purl.archive.org/oquo#EaseOfUseCharacteristic"/>
                            <rdf:Description rdf:about="https://purl.archive.org/oquo#EfficiencyInUseCharacteristic"/>
                            <rdf:Description rdf:about="https://purl.archive.org/oquo#IndexingAndLinkingCharacteristic"/>
                            <rdf:Description rdf:about="https://purl.archive.org/oquo#KnowledgeReuseCharacteristic"/>
                            <rdf:Description rdf:about="https://purl.archive.org/oquo#TextAnalysisCharacteristic"/>
                        </owl:unionOf>
                    </owl:Class>
                </owl:allValuesFrom>
            </owl:Restriction>
        </rdfs:subClassOf>
        <rdfs:subClassOf>
            <owl:Restriction>
                <owl:onProperty rdf:resource="http://purl.org/net/QualityModel#hasScale"/>
                <owl:hasValue rdf:resource="https://purl.archive.org/oquo#DataPropertiesWithNoSynonymMetricScale"/>
            </owl:Restriction>
        </rdfs:subClassOf>
        <obo:IAO_0000115>The Percentage of data properties lacking a synonym in the ontology.</obo:IAO_0000115>
        <rdf1:acronym>DPWNS</rdf1:acronym>
        <rdfs:label>data properties with no synonym metric</rdfs:label>
    </owl:Class>
    


    <!-- https://purl.archive.org/oquo#DecisionTreesCharacteristic -->

    <owl:Class rdf:about="https://purl.archive.org/oquo#DecisionTreesCharacteristic">
        <rdfs:subClassOf rdf:resource="http://purl.org/net/QualityModel#QualityCharacteristic"/>
        <obo:IAO_0000115 xml:lang="en">Capability of the ontology to be used building Decision trees.</obo:IAO_0000115>
        <rdfs:label>decision trees characteristic</rdfs:label>
    </owl:Class>
    


    <!-- https://purl.archive.org/oquo#DepthOfSubsumptionHierarchyMetric -->

    <owl:Class rdf:about="https://purl.archive.org/oquo#DepthOfSubsumptionHierarchyMetric">
        <rdfs:subClassOf rdf:resource="http://purl.org/net/QualityModel#DerivedMeasure"/>
        <rdfs:subClassOf>
            <owl:Class>
                <owl:intersectionOf rdf:parseType="Collection">
                    <owl:Restriction>
                        <owl:onProperty rdf:resource="https://purl.archive.org/oquo#measuresCharacteristicNegatively"/>
                        <owl:allValuesFrom rdf:resource="https://purl.archive.org/oquo#RecoverabilityCharacteristic"/>
                    </owl:Restriction>
                    <owl:Restriction>
                        <owl:onProperty rdf:resource="https://purl.archive.org/oquo#measuresCharacteristicPositively"/>
                        <owl:allValuesFrom>
                            <owl:Class>
                                <owl:unionOf rdf:parseType="Collection">
                                    <rdf:Description rdf:about="https://purl.archive.org/oquo#AdaptabilityCharacteristic"/>
                                    <rdf:Description rdf:about="https://purl.archive.org/oquo#AnalysabilityCharacteristic"/>
                                    <rdf:Description rdf:about="https://purl.archive.org/oquo#ChangeabilityCharacteristic"/>
                                    <rdf:Description rdf:about="https://purl.archive.org/oquo#ReplaceabilityCharacteristic"/>
                                    <rdf:Description rdf:about="https://purl.archive.org/oquo#ReusabilityCharacteristic"/>
                                    <rdf:Description rdf:about="https://purl.archive.org/oquo#TestabilityCharacteristic"/>
                                </owl:unionOf>
                            </owl:Class>
                        </owl:allValuesFrom>
                    </owl:Restriction>
                </owl:intersectionOf>
            </owl:Class>
        </rdfs:subClassOf>
        <rdfs:subClassOf>
            <owl:Restriction>
                <owl:onProperty rdf:resource="http://purl.org/net/QualityModel#hasScale"/>
                <owl:someValuesFrom>
                    <owl:Class>
                        <owl:intersectionOf rdf:parseType="Collection">
                            <rdf:Description rdf:about="https://purl.archive.org/oquo#RawScale"/>
                            <owl:Restriction>
                                <owl:onProperty rdf:resource="http://purl.org/net/QualityModel#hasRankigFunction"/>
                                <owl:hasValue rdf:resource="http://purl.org/net/QualityModel#LowerBest"/>
                            </owl:Restriction>
                        </owl:intersectionOf>
                    </owl:Class>
                </owl:someValuesFrom>
            </owl:Restriction>
        </rdfs:subClassOf>
        <rdfs:subClassOf>
            <owl:Restriction>
                <owl:onProperty rdf:resource="https://purl.archive.org/oquo#measuresCharacteristicNegatively"/>
                <owl:someValuesFrom rdf:resource="https://purl.archive.org/oquo#RecoverabilityCharacteristic"/>
            </owl:Restriction>
        </rdfs:subClassOf>
        <rdfs:subClassOf>
            <owl:Restriction>
                <owl:onProperty rdf:resource="https://purl.archive.org/oquo#measuresCharacteristicPositively"/>
                <owl:someValuesFrom rdf:resource="https://purl.archive.org/oquo#AdaptabilityCharacteristic"/>
            </owl:Restriction>
        </rdfs:subClassOf>
        <rdfs:subClassOf>
            <owl:Restriction>
                <owl:onProperty rdf:resource="https://purl.archive.org/oquo#measuresCharacteristicPositively"/>
                <owl:someValuesFrom rdf:resource="https://purl.archive.org/oquo#AnalysabilityCharacteristic"/>
            </owl:Restriction>
        </rdfs:subClassOf>
        <rdfs:subClassOf>
            <owl:Restriction>
                <owl:onProperty rdf:resource="https://purl.archive.org/oquo#measuresCharacteristicPositively"/>
                <owl:someValuesFrom rdf:resource="https://purl.archive.org/oquo#ChangeabilityCharacteristic"/>
            </owl:Restriction>
        </rdfs:subClassOf>
        <rdfs:subClassOf>
            <owl:Restriction>
                <owl:onProperty rdf:resource="https://purl.archive.org/oquo#measuresCharacteristicPositively"/>
                <owl:someValuesFrom rdf:resource="https://purl.archive.org/oquo#ReplaceabilityCharacteristic"/>
            </owl:Restriction>
        </rdfs:subClassOf>
        <rdfs:subClassOf>
            <owl:Restriction>
                <owl:onProperty rdf:resource="https://purl.archive.org/oquo#measuresCharacteristicPositively"/>
                <owl:someValuesFrom rdf:resource="https://purl.archive.org/oquo#ReusabilityCharacteristic"/>
            </owl:Restriction>
        </rdfs:subClassOf>
        <rdfs:subClassOf>
            <owl:Restriction>
                <owl:onProperty rdf:resource="https://purl.archive.org/oquo#measuresCharacteristicPositively"/>
                <owl:someValuesFrom rdf:resource="https://purl.archive.org/oquo#TestabilityCharacteristic"/>
            </owl:Restriction>
        </rdfs:subClassOf>
        <rdfs:subClassOf>
            <owl:Restriction>
                <owl:onProperty rdf:resource="http://purl.org/net/QualityModel#hasScale"/>
                <owl:hasValue rdf:resource="https://purl.archive.org/oquo#DepthOfSubsumptionHierarchyMetricScale"/>
            </owl:Restriction>
        </rdfs:subClassOf>
        <obo:IAO_0000115 xml:lang="en">Length of the largest path from Thing to a leaf class DITOnto=Max (∑D|Ci|), where Ci are the classes and D|Ci| is the length of the path from the i-thleaf class of the ontology to Thing </obo:IAO_0000115>
        <rdf1:acronym>DITOnto</rdf1:acronym>
        <rdfs:comment>Length of the largest path from Thing to a leaf class.</rdfs:comment>
        <rdfs:label>depth of subsumption hierarchy metric</rdfs:label>
    </owl:Class>
    


    <!-- https://purl.archive.org/oquo#DescriptionsPerAnnotationPropertyMetric -->

    <owl:Class rdf:about="https://purl.archive.org/oquo#DescriptionsPerAnnotationPropertyMetric">
        <rdfs:subClassOf rdf:resource="http://purl.org/net/QualityModel#DerivedMeasure"/>
        <rdfs:subClassOf>
            <owl:Restriction>
                <owl:onProperty rdf:resource="http://purl.org/net/QualityModel#hasScale"/>
                <owl:someValuesFrom>
                    <owl:Class>
                        <owl:intersectionOf rdf:parseType="Collection">
                            <rdf:Description rdf:about="https://purl.archive.org/oquo#RawScale"/>
                            <owl:Restriction>
                                <owl:onProperty rdf:resource="http://purl.org/net/QualityModel#hasRankigFunction"/>
                                <owl:hasValue rdf:resource="http://purl.org/net/QualityModel#HigherBest"/>
                            </owl:Restriction>
                        </owl:intersectionOf>
                    </owl:Class>
                </owl:someValuesFrom>
            </owl:Restriction>
        </rdfs:subClassOf>
        <rdfs:subClassOf>
            <owl:Restriction>
                <owl:onProperty rdf:resource="https://purl.archive.org/oquo#measuresCharacteristicPositively"/>
                <owl:someValuesFrom rdf:resource="https://purl.archive.org/oquo#EaseOfUseCharacteristic"/>
            </owl:Restriction>
        </rdfs:subClassOf>
        <rdfs:subClassOf>
            <owl:Restriction>
                <owl:onProperty rdf:resource="https://purl.archive.org/oquo#measuresCharacteristicPositively"/>
                <owl:someValuesFrom rdf:resource="https://purl.archive.org/oquo#EfficiencyInUseCharacteristic"/>
            </owl:Restriction>
        </rdfs:subClassOf>
        <rdfs:subClassOf>
            <owl:Restriction>
                <owl:onProperty rdf:resource="https://purl.archive.org/oquo#measuresCharacteristicPositively"/>
                <owl:someValuesFrom rdf:resource="https://purl.archive.org/oquo#HelpfulnessCharacteristic"/>
            </owl:Restriction>
        </rdfs:subClassOf>
        <rdfs:subClassOf>
            <owl:Restriction>
                <owl:onProperty rdf:resource="https://purl.archive.org/oquo#measuresCharacteristicPositively"/>
                <owl:someValuesFrom rdf:resource="https://purl.archive.org/oquo#IndexingAndLinkingCharacteristic"/>
            </owl:Restriction>
        </rdfs:subClassOf>
        <rdfs:subClassOf>
            <owl:Restriction>
                <owl:onProperty rdf:resource="https://purl.archive.org/oquo#measuresCharacteristicPositively"/>
                <owl:someValuesFrom rdf:resource="https://purl.archive.org/oquo#KnowledgeReuseCharacteristic"/>
            </owl:Restriction>
        </rdfs:subClassOf>
        <rdfs:subClassOf>
            <owl:Restriction>
                <owl:onProperty rdf:resource="https://purl.archive.org/oquo#measuresCharacteristicPositively"/>
                <owl:someValuesFrom rdf:resource="https://purl.archive.org/oquo#LearnabilityCharacteristic"/>
            </owl:Restriction>
        </rdfs:subClassOf>
        <rdfs:subClassOf>
            <owl:Restriction>
                <owl:onProperty rdf:resource="https://purl.archive.org/oquo#measuresCharacteristicPositively"/>
                <owl:allValuesFrom>
                    <owl:Class>
                        <owl:unionOf rdf:parseType="Collection">
                            <rdf:Description rdf:about="https://purl.archive.org/oquo#EaseOfUseCharacteristic"/>
                            <rdf:Description rdf:about="https://purl.archive.org/oquo#EfficiencyInUseCharacteristic"/>
                            <rdf:Description rdf:about="https://purl.archive.org/oquo#HelpfulnessCharacteristic"/>
                            <rdf:Description rdf:about="https://purl.archive.org/oquo#IndexingAndLinkingCharacteristic"/>
                            <rdf:Description rdf:about="https://purl.archive.org/oquo#KnowledgeReuseCharacteristic"/>
                            <rdf:Description rdf:about="https://purl.archive.org/oquo#LearnabilityCharacteristic"/>
                        </owl:unionOf>
                    </owl:Class>
                </owl:allValuesFrom>
            </owl:Restriction>
        </rdfs:subClassOf>
        <rdfs:subClassOf>
            <owl:Restriction>
                <owl:onProperty rdf:resource="http://purl.org/net/QualityModel#hasScale"/>
                <owl:hasValue rdf:resource="https://purl.archive.org/oquo#DescriptionsPerAnnotationPropertyMetricScale"/>
            </owl:Restriction>
        </rdfs:subClassOf>
        <obo:IAO_0000115 xml:lang="en">This metric accounts for the number of descriptions associated with annotation properties, which can also be provided by using different annotation properties used by the community to include descriptions (rdfs:comment, skos:definition, dcterms:description, etc.). This metric is calculated as the total number of descriptions associated with ontology annotation properties divided by the total number of annotation properties in the ontology. The range of the value of this metric is the set of real positive numbers.</obo:IAO_0000115>
        <rdf1:acronym>DxAP</rdf1:acronym>
        <rdfs:comment>The total number of annotation property descriptions over the total number of annotation properties.</rdfs:comment>
        <rdfs:label>descriptions per annotation property metric</rdfs:label>
    </owl:Class>
    


    <!-- https://purl.archive.org/oquo#DescriptionsPerClassMetric -->

    <owl:Class rdf:about="https://purl.archive.org/oquo#DescriptionsPerClassMetric">
        <rdfs:subClassOf rdf:resource="http://purl.org/net/QualityModel#DerivedMeasure"/>
        <rdfs:subClassOf>
            <owl:Restriction>
                <owl:onProperty rdf:resource="http://purl.org/net/QualityModel#hasScale"/>
                <owl:someValuesFrom>
                    <owl:Class>
                        <owl:intersectionOf rdf:parseType="Collection">
                            <rdf:Description rdf:about="https://purl.archive.org/oquo#RawScale"/>
                            <owl:Restriction>
                                <owl:onProperty rdf:resource="http://purl.org/net/QualityModel#hasRankigFunction"/>
                                <owl:hasValue rdf:resource="http://purl.org/net/QualityModel#HigherBest"/>
                            </owl:Restriction>
                        </owl:intersectionOf>
                    </owl:Class>
                </owl:someValuesFrom>
            </owl:Restriction>
        </rdfs:subClassOf>
        <rdfs:subClassOf>
            <owl:Restriction>
                <owl:onProperty rdf:resource="https://purl.archive.org/oquo#measuresCharacteristicPositively"/>
                <owl:someValuesFrom rdf:resource="https://purl.archive.org/oquo#EaseOfUseCharacteristic"/>
            </owl:Restriction>
        </rdfs:subClassOf>
        <rdfs:subClassOf>
            <owl:Restriction>
                <owl:onProperty rdf:resource="https://purl.archive.org/oquo#measuresCharacteristicPositively"/>
                <owl:someValuesFrom rdf:resource="https://purl.archive.org/oquo#EfficiencyInUseCharacteristic"/>
            </owl:Restriction>
        </rdfs:subClassOf>
        <rdfs:subClassOf>
            <owl:Restriction>
                <owl:onProperty rdf:resource="https://purl.archive.org/oquo#measuresCharacteristicPositively"/>
                <owl:someValuesFrom rdf:resource="https://purl.archive.org/oquo#HelpfulnessCharacteristic"/>
            </owl:Restriction>
        </rdfs:subClassOf>
        <rdfs:subClassOf>
            <owl:Restriction>
                <owl:onProperty rdf:resource="https://purl.archive.org/oquo#measuresCharacteristicPositively"/>
                <owl:someValuesFrom rdf:resource="https://purl.archive.org/oquo#IndexingAndLinkingCharacteristic"/>
            </owl:Restriction>
        </rdfs:subClassOf>
        <rdfs:subClassOf>
            <owl:Restriction>
                <owl:onProperty rdf:resource="https://purl.archive.org/oquo#measuresCharacteristicPositively"/>
                <owl:someValuesFrom rdf:resource="https://purl.archive.org/oquo#KnowledgeReuseCharacteristic"/>
            </owl:Restriction>
        </rdfs:subClassOf>
        <rdfs:subClassOf>
            <owl:Restriction>
                <owl:onProperty rdf:resource="https://purl.archive.org/oquo#measuresCharacteristicPositively"/>
                <owl:someValuesFrom rdf:resource="https://purl.archive.org/oquo#LearnabilityCharacteristic"/>
            </owl:Restriction>
        </rdfs:subClassOf>
        <rdfs:subClassOf>
            <owl:Restriction>
                <owl:onProperty rdf:resource="https://purl.archive.org/oquo#measuresCharacteristicPositively"/>
                <owl:allValuesFrom>
                    <owl:Class>
                        <owl:unionOf rdf:parseType="Collection">
                            <rdf:Description rdf:about="https://purl.archive.org/oquo#EaseOfUseCharacteristic"/>
                            <rdf:Description rdf:about="https://purl.archive.org/oquo#EfficiencyInUseCharacteristic"/>
                            <rdf:Description rdf:about="https://purl.archive.org/oquo#HelpfulnessCharacteristic"/>
                            <rdf:Description rdf:about="https://purl.archive.org/oquo#IndexingAndLinkingCharacteristic"/>
                            <rdf:Description rdf:about="https://purl.archive.org/oquo#KnowledgeReuseCharacteristic"/>
                            <rdf:Description rdf:about="https://purl.archive.org/oquo#LearnabilityCharacteristic"/>
                        </owl:unionOf>
                    </owl:Class>
                </owl:allValuesFrom>
            </owl:Restriction>
        </rdfs:subClassOf>
        <rdfs:subClassOf>
            <owl:Restriction>
                <owl:onProperty rdf:resource="http://purl.org/net/QualityModel#hasScale"/>
                <owl:hasValue rdf:resource="https://purl.archive.org/oquo#DescriptionsPerClassMetricScale"/>
            </owl:Restriction>
        </rdfs:subClassOf>
        <obo:IAO_0000115 xml:lang="en">This metric accounts for the number of descriptions associated with classes, which can also be provided by using different annotation properties used by the community to include descriptions (rdfs:comment, skos:definition, dcterms:description, etc.). This metric is calculated as the total number of descriptions associated with ontology classes divided by the total number of classes in the ontology. The range of the value of this metric is the set of real positive numbers.</obo:IAO_0000115>
        <rdf1:acronym>DxC</rdf1:acronym>
        <rdfs:comment>The total number of class descriptions over the total number of classes.</rdfs:comment>
        <rdfs:label>descriptions per class metric</rdfs:label>
    </owl:Class>
    


    <!-- https://purl.archive.org/oquo#DescriptionsPerDataPropertyMetric -->

    <owl:Class rdf:about="https://purl.archive.org/oquo#DescriptionsPerDataPropertyMetric">
        <rdfs:subClassOf rdf:resource="http://purl.org/net/QualityModel#DerivedMeasure"/>
        <rdfs:subClassOf>
            <owl:Restriction>
                <owl:onProperty rdf:resource="http://purl.org/net/QualityModel#hasScale"/>
                <owl:someValuesFrom>
                    <owl:Class>
                        <owl:intersectionOf rdf:parseType="Collection">
                            <rdf:Description rdf:about="https://purl.archive.org/oquo#RawScale"/>
                            <owl:Restriction>
                                <owl:onProperty rdf:resource="http://purl.org/net/QualityModel#hasRankigFunction"/>
                                <owl:hasValue rdf:resource="http://purl.org/net/QualityModel#HigherBest"/>
                            </owl:Restriction>
                        </owl:intersectionOf>
                    </owl:Class>
                </owl:someValuesFrom>
            </owl:Restriction>
        </rdfs:subClassOf>
        <rdfs:subClassOf>
            <owl:Restriction>
                <owl:onProperty rdf:resource="https://purl.archive.org/oquo#measuresCharacteristicPositively"/>
                <owl:someValuesFrom rdf:resource="https://purl.archive.org/oquo#EaseOfUseCharacteristic"/>
            </owl:Restriction>
        </rdfs:subClassOf>
        <rdfs:subClassOf>
            <owl:Restriction>
                <owl:onProperty rdf:resource="https://purl.archive.org/oquo#measuresCharacteristicPositively"/>
                <owl:someValuesFrom rdf:resource="https://purl.archive.org/oquo#EfficiencyInUseCharacteristic"/>
            </owl:Restriction>
        </rdfs:subClassOf>
        <rdfs:subClassOf>
            <owl:Restriction>
                <owl:onProperty rdf:resource="https://purl.archive.org/oquo#measuresCharacteristicPositively"/>
                <owl:someValuesFrom rdf:resource="https://purl.archive.org/oquo#HelpfulnessCharacteristic"/>
            </owl:Restriction>
        </rdfs:subClassOf>
        <rdfs:subClassOf>
            <owl:Restriction>
                <owl:onProperty rdf:resource="https://purl.archive.org/oquo#measuresCharacteristicPositively"/>
                <owl:someValuesFrom rdf:resource="https://purl.archive.org/oquo#IndexingAndLinkingCharacteristic"/>
            </owl:Restriction>
        </rdfs:subClassOf>
        <rdfs:subClassOf>
            <owl:Restriction>
                <owl:onProperty rdf:resource="https://purl.archive.org/oquo#measuresCharacteristicPositively"/>
                <owl:someValuesFrom rdf:resource="https://purl.archive.org/oquo#KnowledgeReuseCharacteristic"/>
            </owl:Restriction>
        </rdfs:subClassOf>
        <rdfs:subClassOf>
            <owl:Restriction>
                <owl:onProperty rdf:resource="https://purl.archive.org/oquo#measuresCharacteristicPositively"/>
                <owl:someValuesFrom rdf:resource="https://purl.archive.org/oquo#LearnabilityCharacteristic"/>
            </owl:Restriction>
        </rdfs:subClassOf>
        <rdfs:subClassOf>
            <owl:Restriction>
                <owl:onProperty rdf:resource="https://purl.archive.org/oquo#measuresCharacteristicPositively"/>
                <owl:allValuesFrom>
                    <owl:Class>
                        <owl:unionOf rdf:parseType="Collection">
                            <rdf:Description rdf:about="https://purl.archive.org/oquo#EaseOfUseCharacteristic"/>
                            <rdf:Description rdf:about="https://purl.archive.org/oquo#EfficiencyInUseCharacteristic"/>
                            <rdf:Description rdf:about="https://purl.archive.org/oquo#HelpfulnessCharacteristic"/>
                            <rdf:Description rdf:about="https://purl.archive.org/oquo#IndexingAndLinkingCharacteristic"/>
                            <rdf:Description rdf:about="https://purl.archive.org/oquo#KnowledgeReuseCharacteristic"/>
                            <rdf:Description rdf:about="https://purl.archive.org/oquo#LearnabilityCharacteristic"/>
                        </owl:unionOf>
                    </owl:Class>
                </owl:allValuesFrom>
            </owl:Restriction>
        </rdfs:subClassOf>
        <rdfs:subClassOf>
            <owl:Restriction>
                <owl:onProperty rdf:resource="http://purl.org/net/QualityModel#hasScale"/>
                <owl:hasValue rdf:resource="https://purl.archive.org/oquo#DescriptionsPerDataPropertyMetricScale"/>
            </owl:Restriction>
        </rdfs:subClassOf>
        <obo:IAO_0000115 xml:lang="en">This metric accounts for the number of descriptions associated with data type properties, which can also be provided by using different annotation properties used by the community to include descriptions (rdfs:comment, skos:definition, dcterms:description, etc.). This metric is calculated as the total number of descriptions associated with ontology data type properties divided by the total number of data type properties in the ontology. The range of the value of this metric is the set of real positive numbers.</obo:IAO_0000115>
        <rdf1:acronym>DxDP</rdf1:acronym>
        <rdfs:comment>The total number of data property descriptions over the total number of data properties.</rdfs:comment>
        <rdfs:label>descriptions per data property metric</rdfs:label>
    </owl:Class>
    


    <!-- https://purl.archive.org/oquo#DescriptionsPerObjectPropertyMetric -->

    <owl:Class rdf:about="https://purl.archive.org/oquo#DescriptionsPerObjectPropertyMetric">
        <rdfs:subClassOf rdf:resource="http://purl.org/net/QualityModel#DerivedMeasure"/>
        <rdfs:subClassOf>
            <owl:Restriction>
                <owl:onProperty rdf:resource="http://purl.org/net/QualityModel#hasScale"/>
                <owl:someValuesFrom>
                    <owl:Class>
                        <owl:intersectionOf rdf:parseType="Collection">
                            <rdf:Description rdf:about="https://purl.archive.org/oquo#RawScale"/>
                            <owl:Restriction>
                                <owl:onProperty rdf:resource="http://purl.org/net/QualityModel#hasRankigFunction"/>
                                <owl:hasValue rdf:resource="http://purl.org/net/QualityModel#HigherBest"/>
                            </owl:Restriction>
                        </owl:intersectionOf>
                    </owl:Class>
                </owl:someValuesFrom>
            </owl:Restriction>
        </rdfs:subClassOf>
        <rdfs:subClassOf>
            <owl:Restriction>
                <owl:onProperty rdf:resource="https://purl.archive.org/oquo#measuresCharacteristicPositively"/>
                <owl:someValuesFrom rdf:resource="https://purl.archive.org/oquo#EaseOfUseCharacteristic"/>
            </owl:Restriction>
        </rdfs:subClassOf>
        <rdfs:subClassOf>
            <owl:Restriction>
                <owl:onProperty rdf:resource="https://purl.archive.org/oquo#measuresCharacteristicPositively"/>
                <owl:someValuesFrom rdf:resource="https://purl.archive.org/oquo#EfficiencyInUseCharacteristic"/>
            </owl:Restriction>
        </rdfs:subClassOf>
        <rdfs:subClassOf>
            <owl:Restriction>
                <owl:onProperty rdf:resource="https://purl.archive.org/oquo#measuresCharacteristicPositively"/>
                <owl:someValuesFrom rdf:resource="https://purl.archive.org/oquo#HelpfulnessCharacteristic"/>
            </owl:Restriction>
        </rdfs:subClassOf>
        <rdfs:subClassOf>
            <owl:Restriction>
                <owl:onProperty rdf:resource="https://purl.archive.org/oquo#measuresCharacteristicPositively"/>
                <owl:someValuesFrom rdf:resource="https://purl.archive.org/oquo#IndexingAndLinkingCharacteristic"/>
            </owl:Restriction>
        </rdfs:subClassOf>
        <rdfs:subClassOf>
            <owl:Restriction>
                <owl:onProperty rdf:resource="https://purl.archive.org/oquo#measuresCharacteristicPositively"/>
                <owl:someValuesFrom rdf:resource="https://purl.archive.org/oquo#KnowledgeReuseCharacteristic"/>
            </owl:Restriction>
        </rdfs:subClassOf>
        <rdfs:subClassOf>
            <owl:Restriction>
                <owl:onProperty rdf:resource="https://purl.archive.org/oquo#measuresCharacteristicPositively"/>
                <owl:someValuesFrom rdf:resource="https://purl.archive.org/oquo#LearnabilityCharacteristic"/>
            </owl:Restriction>
        </rdfs:subClassOf>
        <rdfs:subClassOf>
            <owl:Restriction>
                <owl:onProperty rdf:resource="https://purl.archive.org/oquo#measuresCharacteristicPositively"/>
                <owl:allValuesFrom>
                    <owl:Class>
                        <owl:unionOf rdf:parseType="Collection">
                            <rdf:Description rdf:about="https://purl.archive.org/oquo#EaseOfUseCharacteristic"/>
                            <rdf:Description rdf:about="https://purl.archive.org/oquo#EfficiencyInUseCharacteristic"/>
                            <rdf:Description rdf:about="https://purl.archive.org/oquo#HelpfulnessCharacteristic"/>
                            <rdf:Description rdf:about="https://purl.archive.org/oquo#IndexingAndLinkingCharacteristic"/>
                            <rdf:Description rdf:about="https://purl.archive.org/oquo#KnowledgeReuseCharacteristic"/>
                            <rdf:Description rdf:about="https://purl.archive.org/oquo#LearnabilityCharacteristic"/>
                        </owl:unionOf>
                    </owl:Class>
                </owl:allValuesFrom>
            </owl:Restriction>
        </rdfs:subClassOf>
        <rdfs:subClassOf>
            <owl:Restriction>
                <owl:onProperty rdf:resource="http://purl.org/net/QualityModel#hasScale"/>
                <owl:hasValue rdf:resource="https://purl.archive.org/oquo#DescriptionsPerObjectPropertyMetricScale"/>
            </owl:Restriction>
        </rdfs:subClassOf>
        <obo:IAO_0000115 xml:lang="en">This metric accounts for the number of descriptions associated with object properties, which can also be provided by using different annotation properties used by the community to include descriptions (rdfs:comment, skos:definition, dcterms:description, etc.). This metric is calculated as the total number of descriptions associated with ontology object properties divided by the total number of object properties in the ontology. The range of the value of this metric is the set of real positive numbers.</obo:IAO_0000115>
        <rdf1:acronym>DxOP</rdf1:acronym>
        <rdfs:comment>The total number of object property descriptions over the total number of object properties.</rdfs:comment>
        <rdfs:label>descriptions per object property metric</rdfs:label>
    </owl:Class>
    


    <!-- https://purl.archive.org/oquo#DescriptionsPerPropertyMetric -->

    <owl:Class rdf:about="https://purl.archive.org/oquo#DescriptionsPerPropertyMetric">
        <rdfs:subClassOf rdf:resource="http://purl.org/net/QualityModel#DerivedMeasure"/>
        <rdfs:subClassOf>
            <owl:Restriction>
                <owl:onProperty rdf:resource="http://purl.org/net/QualityModel#hasScale"/>
                <owl:someValuesFrom>
                    <owl:Class>
                        <owl:intersectionOf rdf:parseType="Collection">
                            <rdf:Description rdf:about="https://purl.archive.org/oquo#RawScale"/>
                            <owl:Restriction>
                                <owl:onProperty rdf:resource="http://purl.org/net/QualityModel#hasRankigFunction"/>
                                <owl:hasValue rdf:resource="http://purl.org/net/QualityModel#HigherBest"/>
                            </owl:Restriction>
                        </owl:intersectionOf>
                    </owl:Class>
                </owl:someValuesFrom>
            </owl:Restriction>
        </rdfs:subClassOf>
        <rdfs:subClassOf>
            <owl:Restriction>
                <owl:onProperty rdf:resource="https://purl.archive.org/oquo#measuresCharacteristicPositively"/>
                <owl:someValuesFrom rdf:resource="https://purl.archive.org/oquo#EaseOfUseCharacteristic"/>
            </owl:Restriction>
        </rdfs:subClassOf>
        <rdfs:subClassOf>
            <owl:Restriction>
                <owl:onProperty rdf:resource="https://purl.archive.org/oquo#measuresCharacteristicPositively"/>
                <owl:someValuesFrom rdf:resource="https://purl.archive.org/oquo#EfficiencyInUseCharacteristic"/>
            </owl:Restriction>
        </rdfs:subClassOf>
        <rdfs:subClassOf>
            <owl:Restriction>
                <owl:onProperty rdf:resource="https://purl.archive.org/oquo#measuresCharacteristicPositively"/>
                <owl:someValuesFrom rdf:resource="https://purl.archive.org/oquo#HelpfulnessCharacteristic"/>
            </owl:Restriction>
        </rdfs:subClassOf>
        <rdfs:subClassOf>
            <owl:Restriction>
                <owl:onProperty rdf:resource="https://purl.archive.org/oquo#measuresCharacteristicPositively"/>
                <owl:someValuesFrom rdf:resource="https://purl.archive.org/oquo#IndexingAndLinkingCharacteristic"/>
            </owl:Restriction>
        </rdfs:subClassOf>
        <rdfs:subClassOf>
            <owl:Restriction>
                <owl:onProperty rdf:resource="https://purl.archive.org/oquo#measuresCharacteristicPositively"/>
                <owl:someValuesFrom rdf:resource="https://purl.archive.org/oquo#KnowledgeReuseCharacteristic"/>
            </owl:Restriction>
        </rdfs:subClassOf>
        <rdfs:subClassOf>
            <owl:Restriction>
                <owl:onProperty rdf:resource="https://purl.archive.org/oquo#measuresCharacteristicPositively"/>
                <owl:someValuesFrom rdf:resource="https://purl.archive.org/oquo#LearnabilityCharacteristic"/>
            </owl:Restriction>
        </rdfs:subClassOf>
        <rdfs:subClassOf>
            <owl:Restriction>
                <owl:onProperty rdf:resource="https://purl.archive.org/oquo#measuresCharacteristicPositively"/>
                <owl:allValuesFrom>
                    <owl:Class>
                        <owl:unionOf rdf:parseType="Collection">
                            <rdf:Description rdf:about="https://purl.archive.org/oquo#EaseOfUseCharacteristic"/>
                            <rdf:Description rdf:about="https://purl.archive.org/oquo#EfficiencyInUseCharacteristic"/>
                            <rdf:Description rdf:about="https://purl.archive.org/oquo#HelpfulnessCharacteristic"/>
                            <rdf:Description rdf:about="https://purl.archive.org/oquo#IndexingAndLinkingCharacteristic"/>
                            <rdf:Description rdf:about="https://purl.archive.org/oquo#KnowledgeReuseCharacteristic"/>
                            <rdf:Description rdf:about="https://purl.archive.org/oquo#LearnabilityCharacteristic"/>
                        </owl:unionOf>
                    </owl:Class>
                </owl:allValuesFrom>
            </owl:Restriction>
        </rdfs:subClassOf>
        <rdfs:subClassOf>
            <owl:Restriction>
                <owl:onProperty rdf:resource="http://purl.org/net/QualityModel#hasScale"/>
                <owl:hasValue rdf:resource="https://purl.archive.org/oquo#DescriptionsPerPropertyMetricScale"/>
            </owl:Restriction>
        </rdfs:subClassOf>
        <obo:IAO_0000115 xml:lang="en">This metric accounts for the number of descriptions associated with properties, which can also be provided by using different annotation properties used by the community to include descriptions (rdfs:comment, skos:definition, dcterms:description, etc.). This metric is calculated as the total number of descriptions associated with ontology properties (including annotation, data, and object properties) divided by the total number of properties in the ontology. The range of the value of this metric is the set of real positive numbers.</obo:IAO_0000115>
        <rdf1:acronym>DxP</rdf1:acronym>
        <rdfs:label>descriptions per property metric</rdfs:label>
    </owl:Class>
    


    <!-- https://purl.archive.org/oquo#DomainCoverageCharacteristic -->

    <owl:Class rdf:about="https://purl.archive.org/oquo#DomainCoverageCharacteristic">
        <rdfs:subClassOf rdf:resource="http://purl.org/net/QualityModel#QualityCharacteristic"/>
        <obo:IAO_0000115 xml:lang="en">The degree to which The ontology cover the specified domain</obo:IAO_0000115>
        <rdfs:label>domain coverage characteristic</rdfs:label>
    </owl:Class>
    


    <!-- https://purl.archive.org/oquo#EaseOfUseCharacteristic -->

    <owl:Class rdf:about="https://purl.archive.org/oquo#EaseOfUseCharacteristic">
        <rdfs:subClassOf rdf:resource="http://purl.org/net/QualityModel#QualityCharacteristic"/>
        <obo:IAO_0000115 xml:lang="en">The degree to which the ontology makes it easy for users to operate and control it.</obo:IAO_0000115>
        <rdfs:label>ease of use characteristic</rdfs:label>
    </owl:Class>
    


    <!-- https://purl.archive.org/oquo#EffectivenessInUseCharacteristic -->

    <owl:Class rdf:about="https://purl.archive.org/oquo#EffectivenessInUseCharacteristic">
        <rdfs:subClassOf rdf:resource="http://purl.org/net/QualityModel#QualityCharacteristic"/>
        <obo:IAO_0000115 xml:lang="en">The degree to which specified users can achieve specified goals with accuracy and completeness in a specified context of use.</obo:IAO_0000115>
        <rdfs:label>effectiveness in use characteristic</rdfs:label>
    </owl:Class>
    


    <!-- https://purl.archive.org/oquo#EfficiencyInUseCharacteristic -->

    <owl:Class rdf:about="https://purl.archive.org/oquo#EfficiencyInUseCharacteristic">
        <rdfs:subClassOf rdf:resource="http://purl.org/net/QualityModel#QualityCharacteristic"/>
        <obo:IAO_0000115 xml:lang="en">The degree to which specified users expend appropriate amounts of resources in relation to the effectiveness achieved in a specified context of use.</obo:IAO_0000115>
        <rdfs:label>efficiency in use characteristic</rdfs:label>
    </owl:Class>
    


    <!-- https://purl.archive.org/oquo#EmotionalSatisfactionCharacteristic -->

    <owl:Class rdf:about="https://purl.archive.org/oquo#EmotionalSatisfactionCharacteristic">
        <rdfs:subClassOf rdf:resource="http://purl.org/net/QualityModel#QualityCharacteristic"/>
        <obo:IAO_0000115 xml:lang="en">Emotional satisfaction</obo:IAO_0000115>
        <oboInOwl:hasExactSynonym xml:lang="en">Pleasure characteristic</oboInOwl:hasExactSynonym>
        <rdfs:label>emotional satisfaction characteristic</rdfs:label>
    </owl:Class>
    


    <!-- https://purl.archive.org/oquo#EvaluationConfigurationData -->

    <owl:Class rdf:about="https://purl.archive.org/oquo#EvaluationConfigurationData">
        <rdfs:subClassOf rdf:resource="http://purl.org/net/EvaluationResult#EvaluationData"/>
        <rdfs:subClassOf>
            <owl:Restriction>
                <owl:onProperty rdf:resource="https://www.omg.org/spec/Commons/TextDatatype/hasTextValue"/>
                <owl:someValuesFrom rdf:resource="http://www.w3.org/2001/XMLSchema#string"/>
            </owl:Restriction>
        </rdfs:subClassOf>
        <owl:disjointWith rdf:resource="https://purl.archive.org/oquo#EvaluationInputData"/>
        <rdfs:comment>Class to specify the configuration used for an evaluation. This configuration is stored as plain text through &apos;hasLiteralValue&apos;. The ontology user should decide the format to store its configuration data (xml, json, etc...).</rdfs:comment>
        <rdfs:label>evaluation configuration data</rdfs:label>
    </owl:Class>
    


    <!-- https://purl.archive.org/oquo#EvaluationInputData -->

    <owl:Class rdf:about="https://purl.archive.org/oquo#EvaluationInputData">
        <rdfs:subClassOf rdf:resource="http://purl.org/net/EvaluationResult#EvaluationData"/>
        <obo:IAO_0000115>Input data used for an evaluation (i.e. an ontology, a free text corpus, etc.).</obo:IAO_0000115>
        <rdfs:label>evaluation input data</rdfs:label>
    </owl:Class>
    


    <!-- https://purl.archive.org/oquo#FlexibilityInUseCharacteristic -->

    <owl:Class rdf:about="https://purl.archive.org/oquo#FlexibilityInUseCharacteristic">
        <rdfs:subClassOf rdf:resource="http://purl.org/net/QualityModel#QualityCharacteristic"/>
        <rdfs:subClassOf>
            <owl:Restriction>
                <owl:onProperty rdf:resource="http://purl.org/net/QualityModel#hasSubCharacteristic"/>
                <owl:someValuesFrom rdf:resource="https://purl.archive.org/oquo#ContextConformityInUseCharacteristic"/>
            </owl:Restriction>
        </rdfs:subClassOf>
        <rdfs:subClassOf>
            <owl:Restriction>
                <owl:onProperty rdf:resource="http://purl.org/net/QualityModel#hasSubCharacteristic"/>
                <owl:someValuesFrom rdf:resource="https://purl.archive.org/oquo#ContextExtendibilityInUseCharacteristic"/>
            </owl:Restriction>
        </rdfs:subClassOf>
        <rdfs:subClassOf>
            <owl:Restriction>
                <owl:onProperty rdf:resource="http://purl.org/net/QualityModel#hasSubCharacteristic"/>
                <owl:allValuesFrom>
                    <owl:Class>
                        <owl:unionOf rdf:parseType="Collection">
                            <rdf:Description rdf:about="https://purl.archive.org/oquo#ContextConformityInUseCharacteristic"/>
                            <rdf:Description rdf:about="https://purl.archive.org/oquo#ContextExtendibilityInUseCharacteristic"/>
                        </owl:unionOf>
                    </owl:Class>
                </owl:allValuesFrom>
            </owl:Restriction>
        </rdfs:subClassOf>
        <rdfs:label>flexibility in use characteristic</rdfs:label>
    </owl:Class>
    


    <!-- https://purl.archive.org/oquo#FormalDegreeMetric -->

    <owl:Class rdf:about="https://purl.archive.org/oquo#FormalDegreeMetric">
        <rdfs:subClassOf rdf:resource="http://purl.org/net/QualityModel#DerivedMeasure"/>
        <rdfs:subClassOf>
            <owl:Restriction>
                <owl:onProperty rdf:resource="https://purl.archive.org/oquo#measuresCharacteristicPositively"/>
                <owl:someValuesFrom rdf:resource="https://purl.archive.org/oquo#ConsistentSearchAndQueryCharacteristic"/>
            </owl:Restriction>
        </rdfs:subClassOf>
        <rdfs:subClassOf>
            <owl:Restriction>
                <owl:onProperty rdf:resource="https://purl.archive.org/oquo#measuresCharacteristicPositively"/>
                <owl:someValuesFrom rdf:resource="https://purl.archive.org/oquo#FormalisationCharacteristic"/>
            </owl:Restriction>
        </rdfs:subClassOf>
        <rdfs:subClassOf>
            <owl:Restriction>
                <owl:onProperty rdf:resource="https://purl.archive.org/oquo#measuresCharacteristicPositively"/>
                <owl:someValuesFrom rdf:resource="https://purl.archive.org/oquo#InferenceCharacteristic"/>
            </owl:Restriction>
        </rdfs:subClassOf>
        <rdfs:subClassOf>
            <owl:Restriction>
                <owl:onProperty rdf:resource="https://purl.archive.org/oquo#measuresCharacteristicPositively"/>
                <owl:someValuesFrom rdf:resource="https://purl.archive.org/oquo#KnowledgeReuseCharacteristic"/>
            </owl:Restriction>
        </rdfs:subClassOf>
        <rdfs:subClassOf>
            <owl:Restriction>
                <owl:onProperty rdf:resource="https://purl.archive.org/oquo#measuresCharacteristicPositively"/>
                <owl:someValuesFrom rdf:resource="https://purl.archive.org/oquo#ReferenceOntologyCharacteristic"/>
            </owl:Restriction>
        </rdfs:subClassOf>
        <rdfs:subClassOf>
            <owl:Restriction>
                <owl:onProperty rdf:resource="https://purl.archive.org/oquo#measuresCharacteristicPositively"/>
                <owl:someValuesFrom rdf:resource="https://purl.archive.org/oquo#SchemaAndValueReconciliationCharacteristic"/>
            </owl:Restriction>
        </rdfs:subClassOf>
        <rdfs:subClassOf>
            <owl:Restriction>
                <owl:onProperty rdf:resource="https://purl.archive.org/oquo#measuresCharacteristicPositively"/>
                <owl:someValuesFrom rdf:resource="https://purl.archive.org/oquo#TextAnalysisCharacteristic"/>
            </owl:Restriction>
        </rdfs:subClassOf>
        <rdfs:subClassOf>
            <owl:Restriction>
                <owl:onProperty rdf:resource="https://purl.archive.org/oquo#measuresCharacteristicPositively"/>
                <owl:allValuesFrom>
                    <owl:Class>
                        <owl:unionOf rdf:parseType="Collection">
                            <rdf:Description rdf:about="https://purl.archive.org/oquo#ConsistentSearchAndQueryCharacteristic"/>
                            <rdf:Description rdf:about="https://purl.archive.org/oquo#FormalisationCharacteristic"/>
                            <rdf:Description rdf:about="https://purl.archive.org/oquo#InferenceCharacteristic"/>
                            <rdf:Description rdf:about="https://purl.archive.org/oquo#KnowledgeReuseCharacteristic"/>
                            <rdf:Description rdf:about="https://purl.archive.org/oquo#ReferenceOntologyCharacteristic"/>
                            <rdf:Description rdf:about="https://purl.archive.org/oquo#SchemaAndValueReconciliationCharacteristic"/>
                            <rdf:Description rdf:about="https://purl.archive.org/oquo#TextAnalysisCharacteristic"/>
                        </owl:unionOf>
                    </owl:Class>
                </owl:allValuesFrom>
            </owl:Restriction>
        </rdfs:subClassOf>
        <rdfs:label>formal degree metric</rdfs:label>
    </owl:Class>
    


    <!-- https://purl.archive.org/oquo#FormalRelationSupportCharacteristic -->

    <owl:Class rdf:about="https://purl.archive.org/oquo#FormalRelationSupportCharacteristic">
        <rdfs:subClassOf rdf:resource="http://purl.org/net/QualityModel#QualityCharacteristic"/>
        <obo:IAO_0000115 xml:lang="en">Capability of the ontology to represent relations supported for formal theories different to the formal support for taxonomy.</obo:IAO_0000115>
        <rdfs:label>formal relation support characteristic</rdfs:label>
    </owl:Class>
    


    <!-- https://purl.archive.org/oquo#FormalisationCharacteristic -->

    <owl:Class rdf:about="https://purl.archive.org/oquo#FormalisationCharacteristic">
        <rdfs:subClassOf rdf:resource="http://purl.org/net/QualityModel#QualityCharacteristic"/>
        <obo:IAO_0000115 xml:lang="en">Capability of the ontology to support reasoning</obo:IAO_0000115>
        <rdfs:label>formalisation characteristic</rdfs:label>
    </owl:Class>
    


    <!-- https://purl.archive.org/oquo#FunctionalAdequacyCharacteristic -->

    <owl:Class rdf:about="https://purl.archive.org/oquo#FunctionalAdequacyCharacteristic">
        <rdfs:subClassOf rdf:resource="http://purl.org/net/QualityModel#QualityCharacteristic"/>
        <rdfs:subClassOf>
            <owl:Restriction>
                <owl:onProperty rdf:resource="http://purl.org/net/QualityModel#hasSubCharacteristic"/>
                <owl:someValuesFrom rdf:resource="https://purl.archive.org/oquo#ClassifyingInstancesCharacteristic"/>
            </owl:Restriction>
        </rdfs:subClassOf>
        <rdfs:subClassOf>
            <owl:Restriction>
                <owl:onProperty rdf:resource="http://purl.org/net/QualityModel#hasSubCharacteristic"/>
                <owl:someValuesFrom rdf:resource="https://purl.archive.org/oquo#ClusteringCharacteristic"/>
            </owl:Restriction>
        </rdfs:subClassOf>
        <rdfs:subClassOf>
            <owl:Restriction>
                <owl:onProperty rdf:resource="http://purl.org/net/QualityModel#hasSubCharacteristic"/>
                <owl:someValuesFrom rdf:resource="https://purl.archive.org/oquo#ConsistentSearchAndQueryCharacteristic"/>
            </owl:Restriction>
        </rdfs:subClassOf>
        <rdfs:subClassOf>
            <owl:Restriction>
                <owl:onProperty rdf:resource="http://purl.org/net/QualityModel#hasSubCharacteristic"/>
                <owl:someValuesFrom rdf:resource="https://purl.archive.org/oquo#ControlledVocabularyCharacteristic"/>
            </owl:Restriction>
        </rdfs:subClassOf>
        <rdfs:subClassOf>
            <owl:Restriction>
                <owl:onProperty rdf:resource="http://purl.org/net/QualityModel#hasSubCharacteristic"/>
                <owl:someValuesFrom rdf:resource="https://purl.archive.org/oquo#DecisionTreesCharacteristic"/>
            </owl:Restriction>
        </rdfs:subClassOf>
        <rdfs:subClassOf>
            <owl:Restriction>
                <owl:onProperty rdf:resource="http://purl.org/net/QualityModel#hasSubCharacteristic"/>
                <owl:someValuesFrom rdf:resource="https://purl.archive.org/oquo#GuidanceCharacteristic"/>
            </owl:Restriction>
        </rdfs:subClassOf>
        <rdfs:subClassOf>
            <owl:Restriction>
                <owl:onProperty rdf:resource="http://purl.org/net/QualityModel#hasSubCharacteristic"/>
                <owl:someValuesFrom rdf:resource="https://purl.archive.org/oquo#IndexingAndLinkingCharacteristic"/>
            </owl:Restriction>
        </rdfs:subClassOf>
        <rdfs:subClassOf>
            <owl:Restriction>
                <owl:onProperty rdf:resource="http://purl.org/net/QualityModel#hasSubCharacteristic"/>
                <owl:someValuesFrom rdf:resource="https://purl.archive.org/oquo#InferenceCharacteristic"/>
            </owl:Restriction>
        </rdfs:subClassOf>
        <rdfs:subClassOf>
            <owl:Restriction>
                <owl:onProperty rdf:resource="http://purl.org/net/QualityModel#hasSubCharacteristic"/>
                <owl:someValuesFrom rdf:resource="https://purl.archive.org/oquo#KnowledgeAcquisitionRepresentationCharacteristic"/>
            </owl:Restriction>
        </rdfs:subClassOf>
        <rdfs:subClassOf>
            <owl:Restriction>
                <owl:onProperty rdf:resource="http://purl.org/net/QualityModel#hasSubCharacteristic"/>
                <owl:someValuesFrom rdf:resource="https://purl.archive.org/oquo#KnowledgeReuseCharacteristic"/>
            </owl:Restriction>
        </rdfs:subClassOf>
        <rdfs:subClassOf>
            <owl:Restriction>
                <owl:onProperty rdf:resource="http://purl.org/net/QualityModel#hasSubCharacteristic"/>
                <owl:someValuesFrom rdf:resource="https://purl.archive.org/oquo#PrecisionCharacteristic"/>
            </owl:Restriction>
        </rdfs:subClassOf>
        <rdfs:subClassOf>
            <owl:Restriction>
                <owl:onProperty rdf:resource="http://purl.org/net/QualityModel#hasSubCharacteristic"/>
                <owl:someValuesFrom rdf:resource="https://purl.archive.org/oquo#ReferenceOntologyCharacteristic"/>
            </owl:Restriction>
        </rdfs:subClassOf>
        <rdfs:subClassOf>
            <owl:Restriction>
                <owl:onProperty rdf:resource="http://purl.org/net/QualityModel#hasSubCharacteristic"/>
                <owl:someValuesFrom rdf:resource="https://purl.archive.org/oquo#ResultsRepresentationCharacteristic"/>
            </owl:Restriction>
        </rdfs:subClassOf>
        <rdfs:subClassOf>
            <owl:Restriction>
                <owl:onProperty rdf:resource="http://purl.org/net/QualityModel#hasSubCharacteristic"/>
                <owl:someValuesFrom rdf:resource="https://purl.archive.org/oquo#SchemaAndValueReconciliationCharacteristic"/>
            </owl:Restriction>
        </rdfs:subClassOf>
        <rdfs:subClassOf>
            <owl:Restriction>
                <owl:onProperty rdf:resource="http://purl.org/net/QualityModel#hasSubCharacteristic"/>
                <owl:someValuesFrom rdf:resource="https://purl.archive.org/oquo#SimilarityCharacteristic"/>
            </owl:Restriction>
        </rdfs:subClassOf>
        <rdfs:subClassOf>
            <owl:Restriction>
                <owl:onProperty rdf:resource="http://purl.org/net/QualityModel#hasSubCharacteristic"/>
                <owl:someValuesFrom rdf:resource="https://purl.archive.org/oquo#TextAnalysisCharacteristic"/>
            </owl:Restriction>
        </rdfs:subClassOf>
        <rdfs:subClassOf>
            <owl:Restriction>
                <owl:onProperty rdf:resource="http://purl.org/net/QualityModel#hasSubCharacteristic"/>
                <owl:allValuesFrom>
                    <owl:Class>
                        <owl:unionOf rdf:parseType="Collection">
                            <rdf:Description rdf:about="https://purl.archive.org/oquo#ClassifyingInstancesCharacteristic"/>
                            <rdf:Description rdf:about="https://purl.archive.org/oquo#ClusteringCharacteristic"/>
                            <rdf:Description rdf:about="https://purl.archive.org/oquo#ConsistentSearchAndQueryCharacteristic"/>
                            <rdf:Description rdf:about="https://purl.archive.org/oquo#ControlledVocabularyCharacteristic"/>
                            <rdf:Description rdf:about="https://purl.archive.org/oquo#DecisionTreesCharacteristic"/>
                            <rdf:Description rdf:about="https://purl.archive.org/oquo#GuidanceCharacteristic"/>
                            <rdf:Description rdf:about="https://purl.archive.org/oquo#IndexingAndLinkingCharacteristic"/>
                            <rdf:Description rdf:about="https://purl.archive.org/oquo#InferenceCharacteristic"/>
                            <rdf:Description rdf:about="https://purl.archive.org/oquo#KnowledgeAcquisitionRepresentationCharacteristic"/>
                            <rdf:Description rdf:about="https://purl.archive.org/oquo#KnowledgeReuseCharacteristic"/>
                            <rdf:Description rdf:about="https://purl.archive.org/oquo#PrecisionCharacteristic"/>
                            <rdf:Description rdf:about="https://purl.archive.org/oquo#ReferenceOntologyCharacteristic"/>
                            <rdf:Description rdf:about="https://purl.archive.org/oquo#ResultsRepresentationCharacteristic"/>
                            <rdf:Description rdf:about="https://purl.archive.org/oquo#SchemaAndValueReconciliationCharacteristic"/>
                            <rdf:Description rdf:about="https://purl.archive.org/oquo#SimilarityCharacteristic"/>
                            <rdf:Description rdf:about="https://purl.archive.org/oquo#TextAnalysisCharacteristic"/>
                        </owl:unionOf>
                    </owl:Class>
                </owl:allValuesFrom>
            </owl:Restriction>
        </rdfs:subClassOf>
        <obo:IAO_0000115 xml:lang="en">The capability of the ontologies to provide concrete functions.</obo:IAO_0000115>
        <rdfs:label>functional adequacy characteristic</rdfs:label>
    </owl:Class>
    


    <!-- https://purl.archive.org/oquo#GuidanceCharacteristic -->

    <owl:Class rdf:about="https://purl.archive.org/oquo#GuidanceCharacteristic">
        <rdfs:subClassOf rdf:resource="http://purl.org/net/QualityModel#QualityCharacteristic"/>
        <obo:IAO_0000115 xml:lang="en">Capability of the ontology to guide the specification of domain theories.</obo:IAO_0000115>
        <rdfs:label>guidance characteristic</rdfs:label>
    </owl:Class>
    


    <!-- https://purl.archive.org/oquo#HelpfulnessCharacteristic -->

    <owl:Class rdf:about="https://purl.archive.org/oquo#HelpfulnessCharacteristic">
        <rdfs:subClassOf rdf:resource="http://purl.org/net/QualityModel#QualityCharacteristic"/>
        <obo:IAO_0000115 xml:lang="en">The degree to which the Ontology provides help when users need assistance.</obo:IAO_0000115>
        <rdfs:label>helpfulness characteristic</rdfs:label>
    </owl:Class>
    


    <!-- https://purl.archive.org/oquo#IndexingAndLinkingCharacteristic -->

    <owl:Class rdf:about="https://purl.archive.org/oquo#IndexingAndLinkingCharacteristic">
        <rdfs:subClassOf rdf:resource="http://purl.org/net/QualityModel#QualityCharacteristic"/>
        <obo:IAO_0000115 xml:lang="en">Degree in which the classes defined in the ontology can act as indexes for quick information retrieval.</obo:IAO_0000115>
        <rdfs:label>indexing and linking characteristic</rdfs:label>
    </owl:Class>
    


    <!-- https://purl.archive.org/oquo#InferenceCharacteristic -->

    <owl:Class rdf:about="https://purl.archive.org/oquo#InferenceCharacteristic">
        <rdfs:subClassOf rdf:resource="http://purl.org/net/QualityModel#QualityCharacteristic"/>
        <obo:IAO_0000115 xml:lang="en">The degree to which The formal model of the ontology can be used by reasoners to make implicit knowledge explicit.</obo:IAO_0000115>
        <rdfs:label>inference characteristic</rdfs:label>
    </owl:Class>
    


    <!-- https://purl.archive.org/oquo#InteroperabilityCharacteristic -->

    <owl:Class rdf:about="https://purl.archive.org/oquo#InteroperabilityCharacteristic">
        <rdfs:subClassOf rdf:resource="http://purl.org/net/QualityModel#QualityCharacteristic"/>
        <obo:IAO_0000115 xml:lang="en">The degree to which the ontology can be cooperatively operable combining its knowledge with one or more other ontologies.</obo:IAO_0000115>
        <rdfs:label>interoperability characteristic</rdfs:label>
    </owl:Class>
    


    <!-- https://purl.archive.org/oquo#KnowledgeAcquisitionRepresentationCharacteristic -->

    <owl:Class rdf:about="https://purl.archive.org/oquo#KnowledgeAcquisitionRepresentationCharacteristic">
        <rdfs:subClassOf rdf:resource="http://purl.org/net/QualityModel#QualityCharacteristic"/>
        <obo:IAO_0000115 xml:lang="en">Capability of the Ontology to represent the knowledge acquired.</obo:IAO_0000115>
        <rdfs:label>knowledge acquisition representation characteristic</rdfs:label>
    </owl:Class>
    


    <!-- https://purl.archive.org/oquo#KnowledgeReuseCharacteristic -->

    <owl:Class rdf:about="https://purl.archive.org/oquo#KnowledgeReuseCharacteristic">
        <rdfs:subClassOf rdf:resource="http://purl.org/net/QualityModel#QualityCharacteristic"/>
        <obo:IAO_0000115 xml:lang="en">The degree to which The ontology knowledge can be used to build other ontologies.</obo:IAO_0000115>
        <rdfs:label>knowledge reuse characteristic</rdfs:label>
    </owl:Class>
    


    <!-- https://purl.archive.org/oquo#LackOfCohesionInMethodsMetric -->

    <owl:Class rdf:about="https://purl.archive.org/oquo#LackOfCohesionInMethodsMetric">
        <rdfs:subClassOf rdf:resource="http://purl.org/net/QualityModel#DerivedMeasure"/>
        <rdfs:subClassOf>
            <owl:Class>
                <owl:intersectionOf rdf:parseType="Collection">
                    <owl:Restriction>
                        <owl:onProperty rdf:resource="https://purl.archive.org/oquo#measuresCharacteristicNegatively"/>
                        <owl:allValuesFrom rdf:resource="https://purl.archive.org/oquo#RecoverabilityCharacteristic"/>
                    </owl:Restriction>
                    <owl:Restriction>
                        <owl:onProperty rdf:resource="https://purl.archive.org/oquo#measuresCharacteristicPositively"/>
                        <owl:allValuesFrom>
                            <owl:Class>
                                <owl:unionOf rdf:parseType="Collection">
                                    <rdf:Description rdf:about="https://purl.archive.org/oquo#AnalysabilityCharacteristic"/>
                                    <rdf:Description rdf:about="https://purl.archive.org/oquo#AvailabilityCharacteristic"/>
                                    <rdf:Description rdf:about="https://purl.archive.org/oquo#ChangeabilityCharacteristic"/>
                                    <rdf:Description rdf:about="https://purl.archive.org/oquo#CohesionCharacteristic"/>
                                    <rdf:Description rdf:about="https://purl.archive.org/oquo#KnowledgeReuseCharacteristic"/>
                                    <rdf:Description rdf:about="https://purl.archive.org/oquo#LearnabilityCharacteristic"/>
                                </owl:unionOf>
                            </owl:Class>
                        </owl:allValuesFrom>
                    </owl:Restriction>
                </owl:intersectionOf>
            </owl:Class>
        </rdfs:subClassOf>
        <rdfs:subClassOf>
            <owl:Restriction>
                <owl:onProperty rdf:resource="http://purl.org/net/QualityModel#hasScale"/>
                <owl:someValuesFrom>
                    <owl:Class>
                        <owl:intersectionOf rdf:parseType="Collection">
                            <rdf:Description rdf:about="https://purl.archive.org/oquo#RawScale"/>
                            <owl:Restriction>
                                <owl:onProperty rdf:resource="http://purl.org/net/QualityModel#hasRankigFunction"/>
                                <owl:hasValue rdf:resource="http://purl.org/net/QualityModel#LowerBest"/>
                            </owl:Restriction>
                        </owl:intersectionOf>
                    </owl:Class>
                </owl:someValuesFrom>
            </owl:Restriction>
        </rdfs:subClassOf>
        <rdfs:subClassOf>
            <owl:Restriction>
                <owl:onProperty rdf:resource="https://purl.archive.org/oquo#measuresCharacteristicNegatively"/>
                <owl:someValuesFrom rdf:resource="https://purl.archive.org/oquo#RecoverabilityCharacteristic"/>
            </owl:Restriction>
        </rdfs:subClassOf>
        <rdfs:subClassOf>
            <owl:Restriction>
                <owl:onProperty rdf:resource="https://purl.archive.org/oquo#measuresCharacteristicPositively"/>
                <owl:someValuesFrom rdf:resource="https://purl.archive.org/oquo#AnalysabilityCharacteristic"/>
            </owl:Restriction>
        </rdfs:subClassOf>
        <rdfs:subClassOf>
            <owl:Restriction>
                <owl:onProperty rdf:resource="https://purl.archive.org/oquo#measuresCharacteristicPositively"/>
                <owl:someValuesFrom rdf:resource="https://purl.archive.org/oquo#AvailabilityCharacteristic"/>
            </owl:Restriction>
        </rdfs:subClassOf>
        <rdfs:subClassOf>
            <owl:Restriction>
                <owl:onProperty rdf:resource="https://purl.archive.org/oquo#measuresCharacteristicPositively"/>
                <owl:someValuesFrom rdf:resource="https://purl.archive.org/oquo#ChangeabilityCharacteristic"/>
            </owl:Restriction>
        </rdfs:subClassOf>
        <rdfs:subClassOf>
            <owl:Restriction>
                <owl:onProperty rdf:resource="https://purl.archive.org/oquo#measuresCharacteristicPositively"/>
                <owl:someValuesFrom rdf:resource="https://purl.archive.org/oquo#CohesionCharacteristic"/>
            </owl:Restriction>
        </rdfs:subClassOf>
        <rdfs:subClassOf>
            <owl:Restriction>
                <owl:onProperty rdf:resource="https://purl.archive.org/oquo#measuresCharacteristicPositively"/>
                <owl:someValuesFrom rdf:resource="https://purl.archive.org/oquo#KnowledgeReuseCharacteristic"/>
            </owl:Restriction>
        </rdfs:subClassOf>
        <rdfs:subClassOf>
            <owl:Restriction>
                <owl:onProperty rdf:resource="https://purl.archive.org/oquo#measuresCharacteristicPositively"/>
                <owl:someValuesFrom rdf:resource="https://purl.archive.org/oquo#LearnabilityCharacteristic"/>
            </owl:Restriction>
        </rdfs:subClassOf>
        <rdfs:subClassOf>
            <owl:Restriction>
                <owl:onProperty rdf:resource="http://purl.org/net/QualityModel#hasScale"/>
                <owl:hasValue rdf:resource="https://purl.archive.org/oquo#LackOfCohesionInMethodsMetricScale"/>
            </owl:Restriction>
        </rdfs:subClassOf>
        <obo:IAO_0000115 xml:lang="en">Semantic and conceptual relatedness of classes. It can be used to measure the separation of responsibilities and independence of components of ontologies LCOMOnto=∑Lenght(path(|C(leaf)i|))/m , where Lenght(path|C(leaf)i|) is the length of the path from the leaf class i to Thing, and m is the total number of paths in the ontology </obo:IAO_0000115>
        <rdf1:acronym>LCOMOnto</rdf1:acronym>
        <rdfs:comment>Semantic and conceptual relatedness of classes.</rdfs:comment>
        <rdfs:label>lack of cohesion in methods metric</rdfs:label>
    </owl:Class>
    


    <!-- https://purl.archive.org/oquo#LearnabilityCharacteristic -->

    <owl:Class rdf:about="https://purl.archive.org/oquo#LearnabilityCharacteristic">
        <rdfs:subClassOf rdf:resource="http://purl.org/net/QualityModel#QualityCharacteristic"/>
        <obo:IAO_0000115 xml:lang="en">The degree to which the ontology enables users to learn its application.</obo:IAO_0000115>
        <rdfs:label>learnability characteristic</rdfs:label>
    </owl:Class>
    


    <!-- https://purl.archive.org/oquo#LexicalRegularitiesPerClassMetric -->

    <owl:Class rdf:about="https://purl.archive.org/oquo#LexicalRegularitiesPerClassMetric">
        <rdfs:subClassOf rdf:resource="http://purl.org/net/QualityModel#DerivedMeasure"/>
        <rdfs:subClassOf>
            <owl:Restriction>
                <owl:onProperty rdf:resource="http://purl.org/net/QualityModel#hasScale"/>
                <owl:someValuesFrom>
                    <owl:Class>
                        <owl:intersectionOf rdf:parseType="Collection">
                            <rdf:Description rdf:about="https://purl.archive.org/oquo#RawScale"/>
                            <owl:Restriction>
                                <owl:onProperty rdf:resource="http://purl.org/net/QualityModel#hasRankigFunction"/>
                                <owl:hasValue rdf:resource="http://purl.org/net/QualityModel#HigherBest"/>
                            </owl:Restriction>
                        </owl:intersectionOf>
                    </owl:Class>
                </owl:someValuesFrom>
            </owl:Restriction>
        </rdfs:subClassOf>
        <rdfs:subClassOf>
            <owl:Restriction>
                <owl:onProperty rdf:resource="https://purl.archive.org/oquo#measuresCharacteristicPositively"/>
                <owl:someValuesFrom rdf:resource="https://purl.archive.org/oquo#StructuralAccuracyCharacteristic"/>
            </owl:Restriction>
        </rdfs:subClassOf>
        <rdfs:subClassOf>
            <owl:Restriction>
                <owl:onProperty rdf:resource="https://purl.archive.org/oquo#measuresCharacteristicPositively"/>
                <owl:someValuesFrom rdf:resource="https://purl.archive.org/oquo#TextAnalysisCharacteristic"/>
            </owl:Restriction>
        </rdfs:subClassOf>
        <rdfs:subClassOf>
            <owl:Restriction>
                <owl:onProperty rdf:resource="https://purl.archive.org/oquo#measuresCharacteristicPositively"/>
                <owl:allValuesFrom>
                    <owl:Class>
                        <owl:unionOf rdf:parseType="Collection">
                            <rdf:Description rdf:about="https://purl.archive.org/oquo#StructuralAccuracyCharacteristic"/>
                            <rdf:Description rdf:about="https://purl.archive.org/oquo#TextAnalysisCharacteristic"/>
                        </owl:unionOf>
                    </owl:Class>
                </owl:allValuesFrom>
            </owl:Restriction>
        </rdfs:subClassOf>
        <rdfs:subClassOf>
            <owl:Restriction>
                <owl:onProperty rdf:resource="http://purl.org/net/QualityModel#hasScale"/>
                <owl:hasValue rdf:resource="https://purl.archive.org/oquo#LexicalRegularitiesPerClassMetricScale"/>
            </owl:Restriction>
        </rdfs:subClassOf>
        <obo:IAO_0000115 xml:lang="en">This metric measures the proportion between the total number of lexical regularities appearing in the ontology and the total number of classes. This metric can measure whether the ontology is using genus-differentia naming style.</obo:IAO_0000115>
        <rdf1:acronym>LRsxC</rdf1:acronym>
        <rdfs:comment>The number of lexical regularities appearing in the ontology over the number of classes.</rdfs:comment>
        <rdfs:label>lexical regularities per class metric</rdfs:label>
    </owl:Class>
    


    <!-- https://purl.archive.org/oquo#LexicalRegularity -->

    <owl:Class rdf:about="https://purl.archive.org/oquo#LexicalRegularity">
        <rdfs:subClassOf rdf:resource="http://purl.org/net/EvaluationResult#EvaluationSubject"/>
        <rdfs:comment>A group of tokens that are exhibited in more than one classes.</rdfs:comment>
        <rdfs:label>LexicalRegularity</rdfs:label>
    </owl:Class>
    


    <!-- https://purl.archive.org/oquo#LexicalRegularityClassPercentageMetric -->

    <owl:Class rdf:about="https://purl.archive.org/oquo#LexicalRegularityClassPercentageMetric">
        <rdfs:subClassOf rdf:resource="http://purl.org/net/QualityModel#DerivedMeasure"/>
        <rdfs:subClassOf>
            <owl:Restriction>
                <owl:onProperty rdf:resource="http://purl.org/net/QualityModel#hasScale"/>
                <owl:someValuesFrom>
                    <owl:Class>
                        <owl:intersectionOf rdf:parseType="Collection">
                            <rdf:Description rdf:about="https://purl.archive.org/oquo#RawScale"/>
                            <owl:Restriction>
                                <owl:onProperty rdf:resource="http://purl.org/net/QualityModel#hasRankigFunction"/>
                                <owl:hasValue rdf:resource="http://purl.org/net/QualityModel#HigherBest"/>
                            </owl:Restriction>
                        </owl:intersectionOf>
                    </owl:Class>
                </owl:someValuesFrom>
            </owl:Restriction>
        </rdfs:subClassOf>
        <rdfs:subClassOf>
            <owl:Restriction>
                <owl:onProperty rdf:resource="https://purl.archive.org/oquo#measuresCharacteristicPositively"/>
                <owl:someValuesFrom rdf:resource="https://purl.archive.org/oquo#StructuralAccuracyCharacteristic"/>
            </owl:Restriction>
        </rdfs:subClassOf>
        <rdfs:subClassOf>
            <owl:Restriction>
                <owl:onProperty rdf:resource="https://purl.archive.org/oquo#measuresCharacteristicPositively"/>
                <owl:someValuesFrom rdf:resource="https://purl.archive.org/oquo#TextAnalysisCharacteristic"/>
            </owl:Restriction>
        </rdfs:subClassOf>
        <rdfs:subClassOf>
            <owl:Restriction>
                <owl:onProperty rdf:resource="https://purl.archive.org/oquo#measuresCharacteristicPositively"/>
                <owl:allValuesFrom>
                    <owl:Class>
                        <owl:unionOf rdf:parseType="Collection">
                            <rdf:Description rdf:about="https://purl.archive.org/oquo#StructuralAccuracyCharacteristic"/>
                            <rdf:Description rdf:about="https://purl.archive.org/oquo#TextAnalysisCharacteristic"/>
                        </owl:unionOf>
                    </owl:Class>
                </owl:allValuesFrom>
            </owl:Restriction>
        </rdfs:subClassOf>
        <rdfs:subClassOf>
            <owl:Restriction>
                <owl:onProperty rdf:resource="http://purl.org/net/QualityModel#hasScale"/>
                <owl:hasValue rdf:resource="https://purl.archive.org/oquo#LexicalRegularityClassPercentageMetricScale"/>
            </owl:Restriction>
        </rdfs:subClassOf>
        <obo:IAO_0000115 xml:lang="en">The percentage of classes in the ontology that are LR classes. In other words, the percentage of classes whose complete name is a lexical regularity.</obo:IAO_0000115>
        <rdf1:acronym>LRClassPCT</rdf1:acronym>
        <rdfs:comment>The percentage of classes in the ontology that are LR classes.</rdfs:comment>
        <rdfs:label>lexical regularity class percentage metric</rdfs:label>
    </owl:Class>
    


    <!-- https://purl.archive.org/oquo#LexicallySuggestLogicallyDefineMetric -->

    <owl:Class rdf:about="https://purl.archive.org/oquo#LexicallySuggestLogicallyDefineMetric">
        <rdfs:subClassOf rdf:resource="http://purl.org/net/QualityModel#DerivedMeasure"/>
        <rdfs:subClassOf>
            <owl:Restriction>
                <owl:onProperty rdf:resource="http://purl.org/net/QualityModel#hasScale"/>
                <owl:someValuesFrom>
                    <owl:Class>
                        <owl:intersectionOf rdf:parseType="Collection">
                            <rdf:Description rdf:about="https://purl.archive.org/oquo#RawScale"/>
                            <owl:Restriction>
                                <owl:onProperty rdf:resource="http://purl.org/net/QualityModel#hasRankigFunction"/>
                                <owl:hasValue rdf:resource="http://purl.org/net/QualityModel#HigherBest"/>
                            </owl:Restriction>
                        </owl:intersectionOf>
                    </owl:Class>
                </owl:someValuesFrom>
            </owl:Restriction>
        </rdfs:subClassOf>
        <rdfs:subClassOf>
            <owl:Restriction>
                <owl:onProperty rdf:resource="https://purl.archive.org/oquo#measuresCharacteristicPositively"/>
                <owl:someValuesFrom rdf:resource="https://purl.archive.org/oquo#StructuralAccuracyCharacteristic"/>
            </owl:Restriction>
        </rdfs:subClassOf>
        <rdfs:subClassOf>
            <owl:Restriction>
                <owl:onProperty rdf:resource="https://purl.archive.org/oquo#measuresCharacteristicPositively"/>
                <owl:someValuesFrom rdf:resource="https://purl.archive.org/oquo#TextAnalysisCharacteristic"/>
            </owl:Restriction>
        </rdfs:subClassOf>
        <rdfs:subClassOf>
            <owl:Restriction>
                <owl:onProperty rdf:resource="https://purl.archive.org/oquo#measuresCharacteristicPositively"/>
                <owl:allValuesFrom>
                    <owl:Class>
                        <owl:unionOf rdf:parseType="Collection">
                            <rdf:Description rdf:about="https://purl.archive.org/oquo#StructuralAccuracyCharacteristic"/>
                            <rdf:Description rdf:about="https://purl.archive.org/oquo#TextAnalysisCharacteristic"/>
                        </owl:unionOf>
                    </owl:Class>
                </owl:allValuesFrom>
            </owl:Restriction>
        </rdfs:subClassOf>
        <rdfs:subClassOf>
            <owl:Restriction>
                <owl:onProperty rdf:resource="http://purl.org/net/QualityModel#hasScale"/>
                <owl:hasValue rdf:resource="https://purl.archive.org/oquo#LexicallySuggestLogicallyDefineMetricScale"/>
            </owl:Restriction>
        </rdfs:subClassOf>
        <obo:IAO_0000115 xml:lang="en">This metric is related to the design principle of the same name, which we interpret as follows: what is expressed in natural language for humans should be expressed as logical axioms for the machine. It is calculated as the ratio in which an LR class is semantically related to other classes exhibiting its lexical regularity. Here, two classes are semantically related if there exist a path of an arbitrary length between them through the axioms in the ontology (i.e. subclass of, equivalency, or domain/range property). For computational reasons, we limited the length of the path between classes up to 5 steps; thus, classes semantically related between them through longer paths will be considered as not semantically related. In this case, positive cases are classes exhibiting a lexical regularity and that are semantically linked with the corresponding LR class. Negative cases are classes exhibiting a lexical regularity and that are not semantically linked with the corresponding LR class. The value of the metric is calculated by dividing the positive cases by the total number of cases. This metric is calculated for each LR class. The final value of the metric for an ontology is calculated as the sum of all the positive cases divided by the sum of all the positive and negative cases obtained by each LR class in the ontology. The value is in the range [0, 1], the highest values representing the best values for the metric.</obo:IAO_0000115>
        <rdf1:acronym>LSLD</rdf1:acronym>
        <rdfs:comment>The degree in which LR classes are semantically linked to the classes exhibiting the corresponding lexical regularity.</rdfs:comment>
        <rdfs:label>lexically suggest logically define metric</rdfs:label>
    </owl:Class>
    


    <!-- https://purl.archive.org/oquo#MaintainabilityCharacteristic -->

    <owl:Class rdf:about="https://purl.archive.org/oquo#MaintainabilityCharacteristic">
        <rdfs:subClassOf rdf:resource="http://purl.org/net/QualityModel#QualityCharacteristic"/>
        <rdfs:subClassOf>
            <owl:Restriction>
                <owl:onProperty rdf:resource="http://purl.org/net/QualityModel#hasSubCharacteristic"/>
                <owl:someValuesFrom rdf:resource="https://purl.archive.org/oquo#AnalysabilityCharacteristic"/>
            </owl:Restriction>
        </rdfs:subClassOf>
        <rdfs:subClassOf>
            <owl:Restriction>
                <owl:onProperty rdf:resource="http://purl.org/net/QualityModel#hasSubCharacteristic"/>
                <owl:someValuesFrom rdf:resource="https://purl.archive.org/oquo#ChangeabilityCharacteristic"/>
            </owl:Restriction>
        </rdfs:subClassOf>
        <rdfs:subClassOf>
            <owl:Restriction>
                <owl:onProperty rdf:resource="http://purl.org/net/QualityModel#hasSubCharacteristic"/>
                <owl:someValuesFrom rdf:resource="https://purl.archive.org/oquo#ModificationStabilityCharacteristic"/>
            </owl:Restriction>
        </rdfs:subClassOf>
        <rdfs:subClassOf>
            <owl:Restriction>
                <owl:onProperty rdf:resource="http://purl.org/net/QualityModel#hasSubCharacteristic"/>
                <owl:someValuesFrom rdf:resource="https://purl.archive.org/oquo#ModularityCharacteristic"/>
            </owl:Restriction>
        </rdfs:subClassOf>
        <rdfs:subClassOf>
            <owl:Restriction>
                <owl:onProperty rdf:resource="http://purl.org/net/QualityModel#hasSubCharacteristic"/>
                <owl:someValuesFrom rdf:resource="https://purl.archive.org/oquo#ReusabilityCharacteristic"/>
            </owl:Restriction>
        </rdfs:subClassOf>
        <rdfs:subClassOf>
            <owl:Restriction>
                <owl:onProperty rdf:resource="http://purl.org/net/QualityModel#hasSubCharacteristic"/>
                <owl:someValuesFrom rdf:resource="https://purl.archive.org/oquo#TestabilityCharacteristic"/>
            </owl:Restriction>
        </rdfs:subClassOf>
        <rdfs:subClassOf>
            <owl:Restriction>
                <owl:onProperty rdf:resource="http://purl.org/net/QualityModel#hasSubCharacteristic"/>
                <owl:allValuesFrom>
                    <owl:Class>
                        <owl:unionOf rdf:parseType="Collection">
                            <rdf:Description rdf:about="https://purl.archive.org/oquo#AnalysabilityCharacteristic"/>
                            <rdf:Description rdf:about="https://purl.archive.org/oquo#ChangeabilityCharacteristic"/>
                            <rdf:Description rdf:about="https://purl.archive.org/oquo#ModificationStabilityCharacteristic"/>
                            <rdf:Description rdf:about="https://purl.archive.org/oquo#ModularityCharacteristic"/>
                            <rdf:Description rdf:about="https://purl.archive.org/oquo#ReusabilityCharacteristic"/>
                            <rdf:Description rdf:about="https://purl.archive.org/oquo#TestabilityCharacteristic"/>
                        </owl:unionOf>
                    </owl:Class>
                </owl:allValuesFrom>
            </owl:Restriction>
        </rdfs:subClassOf>
        <obo:IAO_0000115 xml:lang="en">The capability of ontologies to be modified for changes in environments, in requirements or in functional specifications.</obo:IAO_0000115>
        <rdfs:label>maintainability characteristic</rdfs:label>
    </owl:Class>
    


    <!-- https://purl.archive.org/oquo#MajorIssue -->

    <owl:Class rdf:about="https://purl.archive.org/oquo#MajorIssue">
        <rdfs:subClassOf rdf:resource="http://purl.org/ipo/core#Issue"/>
        <rdfs:comment>A major incident with significant impact</rdfs:comment>
        <rdfs:label>major issue</rdfs:label>
    </owl:Class>
    


    <!-- https://purl.archive.org/oquo#MinorIssue -->

    <owl:Class rdf:about="https://purl.archive.org/oquo#MinorIssue">
        <rdfs:subClassOf rdf:resource="http://purl.org/ipo/core#Issue"/>
        <rdfs:comment>A minor incident with low impact</rdfs:comment>
        <rdfs:label>minor issue</rdfs:label>
    </owl:Class>
    


    <!-- https://purl.archive.org/oquo#ModificationStabilityCharacteristic -->

    <owl:Class rdf:about="https://purl.archive.org/oquo#ModificationStabilityCharacteristic">
        <rdfs:subClassOf rdf:resource="http://purl.org/net/QualityModel#QualityCharacteristic"/>
        <obo:IAO_0000115 xml:lang="en">The degree to which The ontology can avoid unexpected effects from modifications of the software or knowledge.</obo:IAO_0000115>
        <rdfs:label>modification stability characteristic</rdfs:label>
    </owl:Class>
    


    <!-- https://purl.archive.org/oquo#ModularityCharacteristic -->

    <owl:Class rdf:about="https://purl.archive.org/oquo#ModularityCharacteristic">
        <rdfs:subClassOf rdf:resource="http://purl.org/net/QualityModel#QualityCharacteristic"/>
        <obo:IAO_0000115 xml:lang="en">The degree to which the ontology is composed of discrete components such that a change to one component has minimal impact on other components.</obo:IAO_0000115>
        <rdfs:label>modularity characteristic</rdfs:label>
    </owl:Class>
    


    <!-- https://purl.archive.org/oquo#NamesPerAnnotationPropertyMetric -->

    <owl:Class rdf:about="https://purl.archive.org/oquo#NamesPerAnnotationPropertyMetric">
        <rdfs:subClassOf rdf:resource="http://purl.org/net/QualityModel#DerivedMeasure"/>
        <rdfs:subClassOf>
            <owl:Restriction>
                <owl:onProperty rdf:resource="http://purl.org/net/QualityModel#hasScale"/>
                <owl:someValuesFrom>
                    <owl:Class>
                        <owl:intersectionOf rdf:parseType="Collection">
                            <rdf:Description rdf:about="https://purl.archive.org/oquo#RawScale"/>
                            <owl:Restriction>
                                <owl:onProperty rdf:resource="http://purl.org/net/QualityModel#hasRankigFunction"/>
                                <owl:hasValue rdf:resource="http://purl.org/net/QualityModel#HigherBest"/>
                            </owl:Restriction>
                        </owl:intersectionOf>
                    </owl:Class>
                </owl:someValuesFrom>
            </owl:Restriction>
        </rdfs:subClassOf>
        <rdfs:subClassOf>
            <owl:Restriction>
                <owl:onProperty rdf:resource="https://purl.archive.org/oquo#measuresCharacteristicPositively"/>
                <owl:someValuesFrom rdf:resource="https://purl.archive.org/oquo#EaseOfUseCharacteristic"/>
            </owl:Restriction>
        </rdfs:subClassOf>
        <rdfs:subClassOf>
            <owl:Restriction>
                <owl:onProperty rdf:resource="https://purl.archive.org/oquo#measuresCharacteristicPositively"/>
                <owl:someValuesFrom rdf:resource="https://purl.archive.org/oquo#EfficiencyInUseCharacteristic"/>
            </owl:Restriction>
        </rdfs:subClassOf>
        <rdfs:subClassOf>
            <owl:Restriction>
                <owl:onProperty rdf:resource="https://purl.archive.org/oquo#measuresCharacteristicPositively"/>
                <owl:someValuesFrom rdf:resource="https://purl.archive.org/oquo#IndexingAndLinkingCharacteristic"/>
            </owl:Restriction>
        </rdfs:subClassOf>
        <rdfs:subClassOf>
            <owl:Restriction>
                <owl:onProperty rdf:resource="https://purl.archive.org/oquo#measuresCharacteristicPositively"/>
                <owl:someValuesFrom rdf:resource="https://purl.archive.org/oquo#KnowledgeReuseCharacteristic"/>
            </owl:Restriction>
        </rdfs:subClassOf>
        <rdfs:subClassOf>
            <owl:Restriction>
                <owl:onProperty rdf:resource="https://purl.archive.org/oquo#measuresCharacteristicPositively"/>
                <owl:someValuesFrom rdf:resource="https://purl.archive.org/oquo#TextAnalysisCharacteristic"/>
            </owl:Restriction>
        </rdfs:subClassOf>
        <rdfs:subClassOf>
            <owl:Restriction>
                <owl:onProperty rdf:resource="https://purl.archive.org/oquo#measuresCharacteristicPositively"/>
                <owl:allValuesFrom>
                    <owl:Class>
                        <owl:unionOf rdf:parseType="Collection">
                            <rdf:Description rdf:about="https://purl.archive.org/oquo#EaseOfUseCharacteristic"/>
                            <rdf:Description rdf:about="https://purl.archive.org/oquo#EfficiencyInUseCharacteristic"/>
                            <rdf:Description rdf:about="https://purl.archive.org/oquo#IndexingAndLinkingCharacteristic"/>
                            <rdf:Description rdf:about="https://purl.archive.org/oquo#KnowledgeReuseCharacteristic"/>
                            <rdf:Description rdf:about="https://purl.archive.org/oquo#TextAnalysisCharacteristic"/>
                        </owl:unionOf>
                    </owl:Class>
                </owl:allValuesFrom>
            </owl:Restriction>
        </rdfs:subClassOf>
        <rdfs:subClassOf>
            <owl:Restriction>
                <owl:onProperty rdf:resource="http://purl.org/net/QualityModel#hasScale"/>
                <owl:hasValue rdf:resource="https://purl.archive.org/oquo#NamesPerAnnotationPropertyMetricScale"/>
            </owl:Restriction>
        </rdfs:subClassOf>
        <obo:IAO_0000115 xml:lang="en">This metric accounts for the number of names associated with annotation properties, and uses the list of annotation properties used by the community for names (rdfs:label, skos:prefLabel, foaf:name, etc.). Then, this metric is calculated as the number of names associated with ontology annotation properties divided by the total number of annotation properties in the ontology. The range of the value of this metric is the set of real positive numbers. Values lower than one mean that there are annotation properties without any name in the ontology. Contrariwise, a value greater than 1 indicates that there are annotation properties with multiple names; possibly caused by the inclusion of multilingual names or by some design decision.</obo:IAO_0000115>
        <rdf1:acronym>NxAP</rdf1:acronym>
        <rdfs:comment>The total number of annotation property names over the total number of annotation properties.</rdfs:comment>
        <rdfs:label>names per annotation property metric</rdfs:label>
    </owl:Class>
    


    <!-- https://purl.archive.org/oquo#NamesPerClassMetric -->

    <owl:Class rdf:about="https://purl.archive.org/oquo#NamesPerClassMetric">
        <rdfs:subClassOf rdf:resource="http://purl.org/net/QualityModel#DerivedMeasure"/>
        <rdfs:subClassOf>
            <owl:Restriction>
                <owl:onProperty rdf:resource="http://purl.org/net/QualityModel#hasScale"/>
                <owl:someValuesFrom>
                    <owl:Class>
                        <owl:intersectionOf rdf:parseType="Collection">
                            <rdf:Description rdf:about="https://purl.archive.org/oquo#RawScale"/>
                            <owl:Restriction>
                                <owl:onProperty rdf:resource="http://purl.org/net/QualityModel#hasRankigFunction"/>
                                <owl:hasValue rdf:resource="http://purl.org/net/QualityModel#HigherBest"/>
                            </owl:Restriction>
                        </owl:intersectionOf>
                    </owl:Class>
                </owl:someValuesFrom>
            </owl:Restriction>
        </rdfs:subClassOf>
        <rdfs:subClassOf>
            <owl:Restriction>
                <owl:onProperty rdf:resource="https://purl.archive.org/oquo#measuresCharacteristicPositively"/>
                <owl:someValuesFrom rdf:resource="https://purl.archive.org/oquo#EaseOfUseCharacteristic"/>
            </owl:Restriction>
        </rdfs:subClassOf>
        <rdfs:subClassOf>
            <owl:Restriction>
                <owl:onProperty rdf:resource="https://purl.archive.org/oquo#measuresCharacteristicPositively"/>
                <owl:someValuesFrom rdf:resource="https://purl.archive.org/oquo#EfficiencyInUseCharacteristic"/>
            </owl:Restriction>
        </rdfs:subClassOf>
        <rdfs:subClassOf>
            <owl:Restriction>
                <owl:onProperty rdf:resource="https://purl.archive.org/oquo#measuresCharacteristicPositively"/>
                <owl:someValuesFrom rdf:resource="https://purl.archive.org/oquo#IndexingAndLinkingCharacteristic"/>
            </owl:Restriction>
        </rdfs:subClassOf>
        <rdfs:subClassOf>
            <owl:Restriction>
                <owl:onProperty rdf:resource="https://purl.archive.org/oquo#measuresCharacteristicPositively"/>
                <owl:someValuesFrom rdf:resource="https://purl.archive.org/oquo#KnowledgeReuseCharacteristic"/>
            </owl:Restriction>
        </rdfs:subClassOf>
        <rdfs:subClassOf>
            <owl:Restriction>
                <owl:onProperty rdf:resource="https://purl.archive.org/oquo#measuresCharacteristicPositively"/>
                <owl:someValuesFrom rdf:resource="https://purl.archive.org/oquo#TextAnalysisCharacteristic"/>
            </owl:Restriction>
        </rdfs:subClassOf>
        <rdfs:subClassOf>
            <owl:Restriction>
                <owl:onProperty rdf:resource="https://purl.archive.org/oquo#measuresCharacteristicPositively"/>
                <owl:allValuesFrom>
                    <owl:Class>
                        <owl:unionOf rdf:parseType="Collection">
                            <rdf:Description rdf:about="https://purl.archive.org/oquo#EaseOfUseCharacteristic"/>
                            <rdf:Description rdf:about="https://purl.archive.org/oquo#EfficiencyInUseCharacteristic"/>
                            <rdf:Description rdf:about="https://purl.archive.org/oquo#IndexingAndLinkingCharacteristic"/>
                            <rdf:Description rdf:about="https://purl.archive.org/oquo#KnowledgeReuseCharacteristic"/>
                            <rdf:Description rdf:about="https://purl.archive.org/oquo#TextAnalysisCharacteristic"/>
                        </owl:unionOf>
                    </owl:Class>
                </owl:allValuesFrom>
            </owl:Restriction>
        </rdfs:subClassOf>
        <rdfs:subClassOf>
            <owl:Restriction>
                <owl:onProperty rdf:resource="http://purl.org/net/QualityModel#hasScale"/>
                <owl:hasValue rdf:resource="https://purl.archive.org/oquo#NamesPerClassMetricScale"/>
            </owl:Restriction>
        </rdfs:subClassOf>
        <obo:IAO_0000115 xml:lang="en">This metric accounts for the number of names associated with classes, and uses the list of annotation properties used by the community for names (rdfs:label, skos:prefLabel, foaf:name, etc.). Then, this metric is calculated as the number of names associated with ontology classes divided by the total number of classes in the ontology. The range of the value of this metric is the set of real positive numbers. Values lower than one mean that there are classes without any name in the ontology. Contrariwise, a value greater than 1 indicates that there are classes with multiple names; possibly caused by the inclusion of multilingual names or by some design decision.</obo:IAO_0000115>
        <rdf1:acronym>NxC</rdf1:acronym>
        <rdfs:comment>The total number of class names over the total number of classes.</rdfs:comment>
        <rdfs:label>names per class metric</rdfs:label>
    </owl:Class>
    


    <!-- https://purl.archive.org/oquo#NamesPerDataPropertyMetric -->

    <owl:Class rdf:about="https://purl.archive.org/oquo#NamesPerDataPropertyMetric">
        <rdfs:subClassOf rdf:resource="http://purl.org/net/QualityModel#DerivedMeasure"/>
        <rdfs:subClassOf>
            <owl:Restriction>
                <owl:onProperty rdf:resource="http://purl.org/net/QualityModel#hasScale"/>
                <owl:someValuesFrom>
                    <owl:Class>
                        <owl:intersectionOf rdf:parseType="Collection">
                            <rdf:Description rdf:about="https://purl.archive.org/oquo#RawScale"/>
                            <owl:Restriction>
                                <owl:onProperty rdf:resource="http://purl.org/net/QualityModel#hasRankigFunction"/>
                                <owl:hasValue rdf:resource="http://purl.org/net/QualityModel#HigherBest"/>
                            </owl:Restriction>
                        </owl:intersectionOf>
                    </owl:Class>
                </owl:someValuesFrom>
            </owl:Restriction>
        </rdfs:subClassOf>
        <rdfs:subClassOf>
            <owl:Restriction>
                <owl:onProperty rdf:resource="https://purl.archive.org/oquo#measuresCharacteristicPositively"/>
                <owl:someValuesFrom rdf:resource="https://purl.archive.org/oquo#EaseOfUseCharacteristic"/>
            </owl:Restriction>
        </rdfs:subClassOf>
        <rdfs:subClassOf>
            <owl:Restriction>
                <owl:onProperty rdf:resource="https://purl.archive.org/oquo#measuresCharacteristicPositively"/>
                <owl:someValuesFrom rdf:resource="https://purl.archive.org/oquo#EfficiencyInUseCharacteristic"/>
            </owl:Restriction>
        </rdfs:subClassOf>
        <rdfs:subClassOf>
            <owl:Restriction>
                <owl:onProperty rdf:resource="https://purl.archive.org/oquo#measuresCharacteristicPositively"/>
                <owl:someValuesFrom rdf:resource="https://purl.archive.org/oquo#IndexingAndLinkingCharacteristic"/>
            </owl:Restriction>
        </rdfs:subClassOf>
        <rdfs:subClassOf>
            <owl:Restriction>
                <owl:onProperty rdf:resource="https://purl.archive.org/oquo#measuresCharacteristicPositively"/>
                <owl:someValuesFrom rdf:resource="https://purl.archive.org/oquo#KnowledgeReuseCharacteristic"/>
            </owl:Restriction>
        </rdfs:subClassOf>
        <rdfs:subClassOf>
            <owl:Restriction>
                <owl:onProperty rdf:resource="https://purl.archive.org/oquo#measuresCharacteristicPositively"/>
                <owl:someValuesFrom rdf:resource="https://purl.archive.org/oquo#TextAnalysisCharacteristic"/>
            </owl:Restriction>
        </rdfs:subClassOf>
        <rdfs:subClassOf>
            <owl:Restriction>
                <owl:onProperty rdf:resource="https://purl.archive.org/oquo#measuresCharacteristicPositively"/>
                <owl:allValuesFrom>
                    <owl:Class>
                        <owl:unionOf rdf:parseType="Collection">
                            <rdf:Description rdf:about="https://purl.archive.org/oquo#EaseOfUseCharacteristic"/>
                            <rdf:Description rdf:about="https://purl.archive.org/oquo#EfficiencyInUseCharacteristic"/>
                            <rdf:Description rdf:about="https://purl.archive.org/oquo#IndexingAndLinkingCharacteristic"/>
                            <rdf:Description rdf:about="https://purl.archive.org/oquo#KnowledgeReuseCharacteristic"/>
                            <rdf:Description rdf:about="https://purl.archive.org/oquo#TextAnalysisCharacteristic"/>
                        </owl:unionOf>
                    </owl:Class>
                </owl:allValuesFrom>
            </owl:Restriction>
        </rdfs:subClassOf>
        <rdfs:subClassOf>
            <owl:Restriction>
                <owl:onProperty rdf:resource="http://purl.org/net/QualityModel#hasScale"/>
                <owl:hasValue rdf:resource="https://purl.archive.org/oquo#NamesPerDataPropertyMetricScale"/>
            </owl:Restriction>
        </rdfs:subClassOf>
        <obo:IAO_0000115 xml:lang="en">This metric accounts for the number of names associated with data type properties, and uses the list of annotation properties used by the community for names (rdfs:label, skos:prefLabel, foaf:name, etc.). Then, this metric is calculated as the number of names associated with ontology data type properties divided by the total number of data type properties in the ontology. The range of the value of this metric is the set of real positive numbers. Values lower than one mean that there are data type properties without any name in the ontology. Contrariwise, a value greater than 1 indicates that there are data type properties with multiple names; possibly caused by the inclusion of multilingual names or by some design decision.</obo:IAO_0000115>
        <rdf1:acronym>NxDP</rdf1:acronym>
        <rdfs:comment>The total number of data property names over the total number of data properties.</rdfs:comment>
        <rdfs:label>names per data property metric</rdfs:label>
    </owl:Class>
    


    <!-- https://purl.archive.org/oquo#NamesPerObjectPropertyMetric -->

    <owl:Class rdf:about="https://purl.archive.org/oquo#NamesPerObjectPropertyMetric">
        <rdfs:subClassOf rdf:resource="http://purl.org/net/QualityModel#DerivedMeasure"/>
        <rdfs:subClassOf>
            <owl:Restriction>
                <owl:onProperty rdf:resource="http://purl.org/net/QualityModel#hasScale"/>
                <owl:someValuesFrom>
                    <owl:Class>
                        <owl:intersectionOf rdf:parseType="Collection">
                            <rdf:Description rdf:about="https://purl.archive.org/oquo#RawScale"/>
                            <owl:Restriction>
                                <owl:onProperty rdf:resource="http://purl.org/net/QualityModel#hasRankigFunction"/>
                                <owl:hasValue rdf:resource="http://purl.org/net/QualityModel#HigherBest"/>
                            </owl:Restriction>
                        </owl:intersectionOf>
                    </owl:Class>
                </owl:someValuesFrom>
            </owl:Restriction>
        </rdfs:subClassOf>
        <rdfs:subClassOf>
            <owl:Restriction>
                <owl:onProperty rdf:resource="https://purl.archive.org/oquo#measuresCharacteristicPositively"/>
                <owl:someValuesFrom rdf:resource="https://purl.archive.org/oquo#EaseOfUseCharacteristic"/>
            </owl:Restriction>
        </rdfs:subClassOf>
        <rdfs:subClassOf>
            <owl:Restriction>
                <owl:onProperty rdf:resource="https://purl.archive.org/oquo#measuresCharacteristicPositively"/>
                <owl:someValuesFrom rdf:resource="https://purl.archive.org/oquo#EfficiencyInUseCharacteristic"/>
            </owl:Restriction>
        </rdfs:subClassOf>
        <rdfs:subClassOf>
            <owl:Restriction>
                <owl:onProperty rdf:resource="https://purl.archive.org/oquo#measuresCharacteristicPositively"/>
                <owl:someValuesFrom rdf:resource="https://purl.archive.org/oquo#IndexingAndLinkingCharacteristic"/>
            </owl:Restriction>
        </rdfs:subClassOf>
        <rdfs:subClassOf>
            <owl:Restriction>
                <owl:onProperty rdf:resource="https://purl.archive.org/oquo#measuresCharacteristicPositively"/>
                <owl:someValuesFrom rdf:resource="https://purl.archive.org/oquo#KnowledgeReuseCharacteristic"/>
            </owl:Restriction>
        </rdfs:subClassOf>
        <rdfs:subClassOf>
            <owl:Restriction>
                <owl:onProperty rdf:resource="https://purl.archive.org/oquo#measuresCharacteristicPositively"/>
                <owl:someValuesFrom rdf:resource="https://purl.archive.org/oquo#TextAnalysisCharacteristic"/>
            </owl:Restriction>
        </rdfs:subClassOf>
        <rdfs:subClassOf>
            <owl:Restriction>
                <owl:onProperty rdf:resource="https://purl.archive.org/oquo#measuresCharacteristicPositively"/>
                <owl:allValuesFrom>
                    <owl:Class>
                        <owl:unionOf rdf:parseType="Collection">
                            <rdf:Description rdf:about="https://purl.archive.org/oquo#EaseOfUseCharacteristic"/>
                            <rdf:Description rdf:about="https://purl.archive.org/oquo#EfficiencyInUseCharacteristic"/>
                            <rdf:Description rdf:about="https://purl.archive.org/oquo#IndexingAndLinkingCharacteristic"/>
                            <rdf:Description rdf:about="https://purl.archive.org/oquo#KnowledgeReuseCharacteristic"/>
                            <rdf:Description rdf:about="https://purl.archive.org/oquo#TextAnalysisCharacteristic"/>
                        </owl:unionOf>
                    </owl:Class>
                </owl:allValuesFrom>
            </owl:Restriction>
        </rdfs:subClassOf>
        <rdfs:subClassOf>
            <owl:Restriction>
                <owl:onProperty rdf:resource="http://purl.org/net/QualityModel#hasScale"/>
                <owl:hasValue rdf:resource="https://purl.archive.org/oquo#NamesPerObjectPropertyMetricScale"/>
            </owl:Restriction>
        </rdfs:subClassOf>
        <obo:IAO_0000115 xml:lang="en">This metric accounts for the number of names associated with object properties, and uses the list of annotation properties used by the community for names (rdfs:label, skos:prefLabel, foaf:name, etc.). Then, this metric is calculated as the number of names associated with ontology object properties divided by the total number of object properties in the ontology. The range of the value of this metric is the set of real positive numbers. Values lower than one mean that there are object properties without any name in the ontology. Contrariwise, a value greater than 1 indicates that there are object properties with multiple names; possibly caused by the inclusion of multilingual names or by some design decision.</obo:IAO_0000115>
        <rdf1:acronym>NxOP</rdf1:acronym>
        <rdfs:comment>The total number of object property names over the total number of object properties.</rdfs:comment>
        <rdfs:label>names per object property metric</rdfs:label>
    </owl:Class>
    


    <!-- https://purl.archive.org/oquo#NamesPerPropertyMetric -->

    <owl:Class rdf:about="https://purl.archive.org/oquo#NamesPerPropertyMetric">
        <rdfs:subClassOf rdf:resource="http://purl.org/net/QualityModel#DerivedMeasure"/>
        <rdfs:subClassOf>
            <owl:Restriction>
                <owl:onProperty rdf:resource="http://purl.org/net/QualityModel#hasScale"/>
                <owl:someValuesFrom>
                    <owl:Class>
                        <owl:intersectionOf rdf:parseType="Collection">
                            <rdf:Description rdf:about="https://purl.archive.org/oquo#RawScale"/>
                            <owl:Restriction>
                                <owl:onProperty rdf:resource="http://purl.org/net/QualityModel#hasRankigFunction"/>
                                <owl:hasValue rdf:resource="http://purl.org/net/QualityModel#HigherBest"/>
                            </owl:Restriction>
                        </owl:intersectionOf>
                    </owl:Class>
                </owl:someValuesFrom>
            </owl:Restriction>
        </rdfs:subClassOf>
        <rdfs:subClassOf>
            <owl:Restriction>
                <owl:onProperty rdf:resource="https://purl.archive.org/oquo#measuresCharacteristicPositively"/>
                <owl:someValuesFrom rdf:resource="https://purl.archive.org/oquo#EaseOfUseCharacteristic"/>
            </owl:Restriction>
        </rdfs:subClassOf>
        <rdfs:subClassOf>
            <owl:Restriction>
                <owl:onProperty rdf:resource="https://purl.archive.org/oquo#measuresCharacteristicPositively"/>
                <owl:someValuesFrom rdf:resource="https://purl.archive.org/oquo#EfficiencyInUseCharacteristic"/>
            </owl:Restriction>
        </rdfs:subClassOf>
        <rdfs:subClassOf>
            <owl:Restriction>
                <owl:onProperty rdf:resource="https://purl.archive.org/oquo#measuresCharacteristicPositively"/>
                <owl:someValuesFrom rdf:resource="https://purl.archive.org/oquo#HelpfulnessCharacteristic"/>
            </owl:Restriction>
        </rdfs:subClassOf>
        <rdfs:subClassOf>
            <owl:Restriction>
                <owl:onProperty rdf:resource="https://purl.archive.org/oquo#measuresCharacteristicPositively"/>
                <owl:someValuesFrom rdf:resource="https://purl.archive.org/oquo#IndexingAndLinkingCharacteristic"/>
            </owl:Restriction>
        </rdfs:subClassOf>
        <rdfs:subClassOf>
            <owl:Restriction>
                <owl:onProperty rdf:resource="https://purl.archive.org/oquo#measuresCharacteristicPositively"/>
                <owl:someValuesFrom rdf:resource="https://purl.archive.org/oquo#KnowledgeReuseCharacteristic"/>
            </owl:Restriction>
        </rdfs:subClassOf>
        <rdfs:subClassOf>
            <owl:Restriction>
                <owl:onProperty rdf:resource="https://purl.archive.org/oquo#measuresCharacteristicPositively"/>
                <owl:someValuesFrom rdf:resource="https://purl.archive.org/oquo#LearnabilityCharacteristic"/>
            </owl:Restriction>
        </rdfs:subClassOf>
        <rdfs:subClassOf>
            <owl:Restriction>
                <owl:onProperty rdf:resource="https://purl.archive.org/oquo#measuresCharacteristicPositively"/>
                <owl:allValuesFrom>
                    <owl:Class>
                        <owl:unionOf rdf:parseType="Collection">
                            <rdf:Description rdf:about="https://purl.archive.org/oquo#EaseOfUseCharacteristic"/>
                            <rdf:Description rdf:about="https://purl.archive.org/oquo#EfficiencyInUseCharacteristic"/>
                            <rdf:Description rdf:about="https://purl.archive.org/oquo#HelpfulnessCharacteristic"/>
                            <rdf:Description rdf:about="https://purl.archive.org/oquo#IndexingAndLinkingCharacteristic"/>
                            <rdf:Description rdf:about="https://purl.archive.org/oquo#KnowledgeReuseCharacteristic"/>
                            <rdf:Description rdf:about="https://purl.archive.org/oquo#LearnabilityCharacteristic"/>
                        </owl:unionOf>
                    </owl:Class>
                </owl:allValuesFrom>
            </owl:Restriction>
        </rdfs:subClassOf>
        <rdfs:subClassOf>
            <owl:Restriction>
                <owl:onProperty rdf:resource="http://purl.org/net/QualityModel#hasScale"/>
                <owl:hasValue rdf:resource="https://purl.archive.org/oquo#NamesPerPropertyMetricScale"/>
            </owl:Restriction>
        </rdfs:subClassOf>
        <obo:IAO_0000115 xml:lang="en">This metric accounts for the number of names associated with properties, which can also be provided by using different annotation properties used by the community to include names (rdfs:label, skos:prefLabel, foaf:name, etc.). This metric is calculated as the total number of names associated with ontology properties (including annotation, data, and object properties) divided by the total number of properties in the ontology. The range of the value of this metric is the set of real positive numbers.</obo:IAO_0000115>
        <rdf1:acronym>DxP</rdf1:acronym>
        <rdfs:label>names per property metric</rdfs:label>
    </owl:Class>
    


    <!-- https://purl.archive.org/oquo#NumberOfAncestorClassesMetric -->

    <owl:Class rdf:about="https://purl.archive.org/oquo#NumberOfAncestorClassesMetric">
        <rdfs:subClassOf rdf:resource="http://purl.org/net/QualityModel#DerivedMeasure"/>
        <rdfs:subClassOf>
            <owl:Restriction>
                <owl:onProperty rdf:resource="http://purl.org/net/QualityModel#hasScale"/>
                <owl:someValuesFrom>
                    <owl:Class>
                        <owl:intersectionOf rdf:parseType="Collection">
                            <rdf:Description rdf:about="https://purl.archive.org/oquo#RawScale"/>
                            <owl:Restriction>
                                <owl:onProperty rdf:resource="http://purl.org/net/QualityModel#hasRankigFunction"/>
                                <owl:hasValue rdf:resource="http://purl.org/net/QualityModel#LowerBest"/>
                            </owl:Restriction>
                        </owl:intersectionOf>
                    </owl:Class>
                </owl:someValuesFrom>
            </owl:Restriction>
        </rdfs:subClassOf>
        <rdfs:subClassOf>
            <owl:Restriction>
                <owl:onProperty rdf:resource="https://purl.archive.org/oquo#measuresCharacteristicPositively"/>
                <owl:someValuesFrom rdf:resource="https://purl.archive.org/oquo#KnowledgeReuseCharacteristic"/>
            </owl:Restriction>
        </rdfs:subClassOf>
        <rdfs:subClassOf>
            <owl:Restriction>
                <owl:onProperty rdf:resource="https://purl.archive.org/oquo#measuresCharacteristicPositively"/>
                <owl:allValuesFrom>
                    <owl:Class>
                        <owl:unionOf rdf:parseType="Collection">
                            <rdf:Description rdf:about="https://purl.archive.org/oquo#KnowledgeReuseCharacteristic"/>
                        </owl:unionOf>
                    </owl:Class>
                </owl:allValuesFrom>
            </owl:Restriction>
        </rdfs:subClassOf>
        <rdfs:subClassOf>
            <owl:Restriction>
                <owl:onProperty rdf:resource="http://purl.org/net/QualityModel#hasScale"/>
                <owl:hasValue rdf:resource="https://purl.archive.org/oquo#NumberOfAncestorClassesMetricScale"/>
            </owl:Restriction>
        </rdfs:subClassOf>
        <obo:IAO_0000115 xml:lang="en">Mean number of ancestor classes per leaf class. It is the number of direct superclasses per leaf class NACOnto=∑|SupC(Leaf)i|/∑|C(leaf)i)| </obo:IAO_0000115>
        <rdf1:acronym>NACOnto</rdf1:acronym>
        <rdfs:comment>Mean number of ancestor classes per leaf class.</rdfs:comment>
        <rdfs:label>number of ancestor classes metric</rdfs:label>
    </owl:Class>
    


    <!-- https://purl.archive.org/oquo#NumberOfChildrenClassesMetric -->

    <owl:Class rdf:about="https://purl.archive.org/oquo#NumberOfChildrenClassesMetric">
        <rdfs:subClassOf rdf:resource="http://purl.org/net/QualityModel#DerivedMeasure"/>
        <rdfs:subClassOf>
            <owl:Class>
                <owl:intersectionOf rdf:parseType="Collection">
                    <owl:Restriction>
                        <owl:onProperty rdf:resource="https://purl.archive.org/oquo#measuresCharacteristicNegatively"/>
                        <owl:allValuesFrom>
                            <owl:Class>
                                <owl:unionOf rdf:parseType="Collection">
                                    <rdf:Description rdf:about="https://purl.archive.org/oquo#LearnabilityCharacteristic"/>
                                    <rdf:Description rdf:about="https://purl.archive.org/oquo#ReusabilityCharacteristic"/>
                                </owl:unionOf>
                            </owl:Class>
                        </owl:allValuesFrom>
                    </owl:Restriction>
                    <owl:Restriction>
                        <owl:onProperty rdf:resource="https://purl.archive.org/oquo#measuresCharacteristicPositively"/>
                        <owl:allValuesFrom>
                            <owl:Class>
                                <owl:unionOf rdf:parseType="Collection">
                                    <rdf:Description rdf:about="https://purl.archive.org/oquo#ChangeabilityCharacteristic"/>
                                    <rdf:Description rdf:about="https://purl.archive.org/oquo#ModificationStabilityCharacteristic"/>
                                    <rdf:Description rdf:about="https://purl.archive.org/oquo#ReplaceabilityCharacteristic"/>
                                </owl:unionOf>
                            </owl:Class>
                        </owl:allValuesFrom>
                    </owl:Restriction>
                </owl:intersectionOf>
            </owl:Class>
        </rdfs:subClassOf>
        <rdfs:subClassOf>
            <owl:Restriction>
                <owl:onProperty rdf:resource="http://purl.org/net/QualityModel#hasScale"/>
                <owl:someValuesFrom>
                    <owl:Class>
                        <owl:intersectionOf rdf:parseType="Collection">
                            <rdf:Description rdf:about="https://purl.archive.org/oquo#RawScale"/>
                            <owl:Restriction>
                                <owl:onProperty rdf:resource="http://purl.org/net/QualityModel#hasRankigFunction"/>
                                <owl:hasValue rdf:resource="http://purl.org/net/QualityModel#HigherBest"/>
                            </owl:Restriction>
                        </owl:intersectionOf>
                    </owl:Class>
                </owl:someValuesFrom>
            </owl:Restriction>
        </rdfs:subClassOf>
        <rdfs:subClassOf>
            <owl:Restriction>
                <owl:onProperty rdf:resource="https://purl.archive.org/oquo#measuresCharacteristicNegatively"/>
                <owl:someValuesFrom rdf:resource="https://purl.archive.org/oquo#LearnabilityCharacteristic"/>
            </owl:Restriction>
        </rdfs:subClassOf>
        <rdfs:subClassOf>
            <owl:Restriction>
                <owl:onProperty rdf:resource="https://purl.archive.org/oquo#measuresCharacteristicNegatively"/>
                <owl:someValuesFrom rdf:resource="https://purl.archive.org/oquo#ReusabilityCharacteristic"/>
            </owl:Restriction>
        </rdfs:subClassOf>
        <rdfs:subClassOf>
            <owl:Restriction>
                <owl:onProperty rdf:resource="https://purl.archive.org/oquo#measuresCharacteristicPositively"/>
                <owl:someValuesFrom rdf:resource="https://purl.archive.org/oquo#ChangeabilityCharacteristic"/>
            </owl:Restriction>
        </rdfs:subClassOf>
        <rdfs:subClassOf>
            <owl:Restriction>
                <owl:onProperty rdf:resource="https://purl.archive.org/oquo#measuresCharacteristicPositively"/>
                <owl:someValuesFrom rdf:resource="https://purl.archive.org/oquo#ModificationStabilityCharacteristic"/>
            </owl:Restriction>
        </rdfs:subClassOf>
        <rdfs:subClassOf>
            <owl:Restriction>
                <owl:onProperty rdf:resource="https://purl.archive.org/oquo#measuresCharacteristicPositively"/>
                <owl:someValuesFrom rdf:resource="https://purl.archive.org/oquo#ReplaceabilityCharacteristic"/>
            </owl:Restriction>
        </rdfs:subClassOf>
        <rdfs:subClassOf>
            <owl:Restriction>
                <owl:onProperty rdf:resource="http://purl.org/net/QualityModel#hasScale"/>
                <owl:hasValue rdf:resource="https://purl.archive.org/oquo#NumberOfChildrenClassesMetricScale"/>
            </owl:Restriction>
        </rdfs:subClassOf>
        <obo:IAO_0000115 xml:lang="en">Number of the direct subclasses divided by the number of classes minus the number of leaf classes NOCOnto=∑|RCi|/(∑|Ci| - ∑|C(leaf)i)|) </obo:IAO_0000115>
        <rdf1:acronym>NOCOnto</rdf1:acronym>
        <rdfs:comment>Number of the direct subclasses divided by the number of classes minus the number of leaf classes</rdfs:comment>
        <rdfs:label>number of children classes metric</rdfs:label>
    </owl:Class>
    


    <!-- https://purl.archive.org/oquo#NumberOfClassesMetric -->

    <owl:Class rdf:about="https://purl.archive.org/oquo#NumberOfClassesMetric">
        <rdfs:subClassOf rdf:resource="http://purl.org/net/QualityModel#BaseMeasure"/>
        <obo:IAO_0000115>This metric calculates the number of classes asserted in the ontology.</obo:IAO_0000115>
        <rdf1:acronym>NCLASSES</rdf1:acronym>
        <rdfs:label>number of classes metric</rdfs:label>
    </owl:Class>
    


    <!-- https://purl.archive.org/oquo#NumberOfLexicalRegularitiesMetric -->

    <owl:Class rdf:about="https://purl.archive.org/oquo#NumberOfLexicalRegularitiesMetric">
        <rdfs:subClassOf rdf:resource="http://purl.org/net/QualityModel#DerivedMeasure"/>
        <rdfs:subClassOf>
            <owl:Restriction>
                <owl:onProperty rdf:resource="http://purl.org/net/QualityModel#hasScale"/>
                <owl:someValuesFrom>
                    <owl:Class>
                        <owl:intersectionOf rdf:parseType="Collection">
                            <rdf:Description rdf:about="https://purl.archive.org/oquo#RawScale"/>
                            <owl:Restriction>
                                <owl:onProperty rdf:resource="http://purl.org/net/QualityModel#hasRankigFunction"/>
                                <owl:hasValue rdf:resource="http://purl.org/net/QualityModel#HigherBest"/>
                            </owl:Restriction>
                        </owl:intersectionOf>
                    </owl:Class>
                </owl:someValuesFrom>
            </owl:Restriction>
        </rdfs:subClassOf>
        <rdfs:subClassOf>
            <owl:Restriction>
                <owl:onProperty rdf:resource="https://purl.archive.org/oquo#measuresCharacteristicPositively"/>
                <owl:someValuesFrom rdf:resource="https://purl.archive.org/oquo#ControlledVocabularyCharacteristic"/>
            </owl:Restriction>
        </rdfs:subClassOf>
        <rdfs:subClassOf>
            <owl:Restriction>
                <owl:onProperty rdf:resource="https://purl.archive.org/oquo#measuresCharacteristicPositively"/>
                <owl:allValuesFrom>
                    <owl:Class>
                        <owl:unionOf rdf:parseType="Collection">
                            <rdf:Description rdf:about="https://purl.archive.org/oquo#ControlledVocabularyCharacteristic"/>
                        </owl:unionOf>
                    </owl:Class>
                </owl:allValuesFrom>
            </owl:Restriction>
        </rdfs:subClassOf>
        <rdfs:subClassOf>
            <owl:Restriction>
                <owl:onProperty rdf:resource="http://purl.org/net/QualityModel#hasScale"/>
                <owl:hasValue rdf:resource="https://purl.archive.org/oquo#NumberOfLexicalRegularitiesMetricScale"/>
            </owl:Restriction>
        </rdfs:subClassOf>
        <obo:IAO_0000115 xml:lang="en">This metric examines the names of the ontology classes, stabished by using &apos;rdfs:label&apos;, and identifies the number of lexical regularities appearing in the ontology.</obo:IAO_0000115>
        <rdf1:acronym>NLR</rdf1:acronym>
        <rdfs:comment>The number of lexical regularities found in the ontology.</rdfs:comment>
        <rdfs:label>number of lexical regularities metric</rdfs:label>
    </owl:Class>
    


    <!-- https://purl.archive.org/oquo#NumberOfLexicalRegularityClassesMetric -->

    <owl:Class rdf:about="https://purl.archive.org/oquo#NumberOfLexicalRegularityClassesMetric">
        <rdfs:subClassOf rdf:resource="http://purl.org/net/QualityModel#DerivedMeasure"/>
        <rdfs:subClassOf>
            <owl:Restriction>
                <owl:onProperty rdf:resource="http://purl.org/net/QualityModel#hasScale"/>
                <owl:someValuesFrom>
                    <owl:Class>
                        <owl:intersectionOf rdf:parseType="Collection">
                            <rdf:Description rdf:about="https://purl.archive.org/oquo#RawScale"/>
                            <owl:Restriction>
                                <owl:onProperty rdf:resource="http://purl.org/net/QualityModel#hasRankigFunction"/>
                                <owl:hasValue rdf:resource="http://purl.org/net/QualityModel#HigherBest"/>
                            </owl:Restriction>
                        </owl:intersectionOf>
                    </owl:Class>
                </owl:someValuesFrom>
            </owl:Restriction>
        </rdfs:subClassOf>
        <rdfs:subClassOf>
            <owl:Restriction>
                <owl:onProperty rdf:resource="https://purl.archive.org/oquo#measuresCharacteristicPositively"/>
                <owl:someValuesFrom rdf:resource="https://purl.archive.org/oquo#ControlledVocabularyCharacteristic"/>
            </owl:Restriction>
        </rdfs:subClassOf>
        <rdfs:subClassOf>
            <owl:Restriction>
                <owl:onProperty rdf:resource="https://purl.archive.org/oquo#measuresCharacteristicPositively"/>
                <owl:allValuesFrom>
                    <owl:Class>
                        <owl:unionOf rdf:parseType="Collection">
                            <rdf:Description rdf:about="https://purl.archive.org/oquo#ControlledVocabularyCharacteristic"/>
                        </owl:unionOf>
                    </owl:Class>
                </owl:allValuesFrom>
            </owl:Restriction>
        </rdfs:subClassOf>
        <rdfs:subClassOf>
            <owl:Restriction>
                <owl:onProperty rdf:resource="http://purl.org/net/QualityModel#hasScale"/>
                <owl:hasValue rdf:resource="https://purl.archive.org/oquo#NumberOfLexicalRegularityClassesMetricScale"/>
            </owl:Restriction>
        </rdfs:subClassOf>
        <obo:IAO_0000115 xml:lang="en">This metric returns the number of ontology classes whose complete name, set by using &apos;rdfs:label&apos;, is a lexical regularity.</obo:IAO_0000115>
        <rdf1:acronym>NLRC</rdf1:acronym>
        <rdfs:comment>The number of ontology classes whose name is a lexical regularity.</rdfs:comment>
        <rdfs:label>number of lexical regularity classes metric</rdfs:label>
    </owl:Class>
    


    <!-- https://purl.archive.org/oquo#NumberOfPropertiesMetric -->

    <owl:Class rdf:about="https://purl.archive.org/oquo#NumberOfPropertiesMetric">
        <rdfs:subClassOf rdf:resource="http://purl.org/net/QualityModel#DerivedMeasure"/>
        <rdfs:subClassOf>
            <owl:Class>
                <owl:intersectionOf rdf:parseType="Collection">
                    <owl:Restriction>
                        <owl:onProperty rdf:resource="https://purl.archive.org/oquo#measuresCharacteristicNegatively"/>
                        <owl:allValuesFrom rdf:resource="https://purl.archive.org/oquo#RecoverabilityCharacteristic"/>
                    </owl:Restriction>
                    <owl:Restriction>
                        <owl:onProperty rdf:resource="https://purl.archive.org/oquo#measuresCharacteristicPositively"/>
                        <owl:allValuesFrom>
                            <owl:Class>
                                <owl:unionOf rdf:parseType="Collection">
                                    <rdf:Description rdf:about="https://purl.archive.org/oquo#AnalysabilityCharacteristic"/>
                                    <rdf:Description rdf:about="https://purl.archive.org/oquo#ChangeabilityCharacteristic"/>
                                    <rdf:Description rdf:about="https://purl.archive.org/oquo#KnowledgeAcquisitionRepresentationCharacteristic"/>
                                    <rdf:Description rdf:about="https://purl.archive.org/oquo#KnowledgeReuseCharacteristic"/>
                                    <rdf:Description rdf:about="https://purl.archive.org/oquo#LearnabilityCharacteristic"/>
                                    <rdf:Description rdf:about="https://purl.archive.org/oquo#ModificationStabilityCharacteristic"/>
                                    <rdf:Description rdf:about="https://purl.archive.org/oquo#ReplaceabilityCharacteristic"/>
                                    <rdf:Description rdf:about="https://purl.archive.org/oquo#ReusabilityCharacteristic"/>
                                    <rdf:Description rdf:about="https://purl.archive.org/oquo#TestabilityCharacteristic"/>
                                </owl:unionOf>
                            </owl:Class>
                        </owl:allValuesFrom>
                    </owl:Restriction>
                </owl:intersectionOf>
            </owl:Class>
        </rdfs:subClassOf>
        <rdfs:subClassOf>
            <owl:Restriction>
                <owl:onProperty rdf:resource="http://purl.org/net/QualityModel#hasScale"/>
                <owl:someValuesFrom>
                    <owl:Class>
                        <owl:intersectionOf rdf:parseType="Collection">
                            <rdf:Description rdf:about="https://purl.archive.org/oquo#RawScale"/>
                            <owl:Restriction>
                                <owl:onProperty rdf:resource="http://purl.org/net/QualityModel#hasRankigFunction"/>
                                <owl:hasValue rdf:resource="http://purl.org/net/QualityModel#LowerBest"/>
                            </owl:Restriction>
                        </owl:intersectionOf>
                    </owl:Class>
                </owl:someValuesFrom>
            </owl:Restriction>
        </rdfs:subClassOf>
        <rdfs:subClassOf>
            <owl:Restriction>
                <owl:onProperty rdf:resource="https://purl.archive.org/oquo#measuresCharacteristicNegatively"/>
                <owl:someValuesFrom rdf:resource="https://purl.archive.org/oquo#RecoverabilityCharacteristic"/>
            </owl:Restriction>
        </rdfs:subClassOf>
        <rdfs:subClassOf>
            <owl:Restriction>
                <owl:onProperty rdf:resource="https://purl.archive.org/oquo#measuresCharacteristicPositively"/>
                <owl:someValuesFrom rdf:resource="https://purl.archive.org/oquo#AnalysabilityCharacteristic"/>
            </owl:Restriction>
        </rdfs:subClassOf>
        <rdfs:subClassOf>
            <owl:Restriction>
                <owl:onProperty rdf:resource="https://purl.archive.org/oquo#measuresCharacteristicPositively"/>
                <owl:someValuesFrom rdf:resource="https://purl.archive.org/oquo#ChangeabilityCharacteristic"/>
            </owl:Restriction>
        </rdfs:subClassOf>
        <rdfs:subClassOf>
            <owl:Restriction>
                <owl:onProperty rdf:resource="https://purl.archive.org/oquo#measuresCharacteristicPositively"/>
                <owl:someValuesFrom rdf:resource="https://purl.archive.org/oquo#KnowledgeAcquisitionRepresentationCharacteristic"/>
            </owl:Restriction>
        </rdfs:subClassOf>
        <rdfs:subClassOf>
            <owl:Restriction>
                <owl:onProperty rdf:resource="https://purl.archive.org/oquo#measuresCharacteristicPositively"/>
                <owl:someValuesFrom rdf:resource="https://purl.archive.org/oquo#KnowledgeReuseCharacteristic"/>
            </owl:Restriction>
        </rdfs:subClassOf>
        <rdfs:subClassOf>
            <owl:Restriction>
                <owl:onProperty rdf:resource="https://purl.archive.org/oquo#measuresCharacteristicPositively"/>
                <owl:someValuesFrom rdf:resource="https://purl.archive.org/oquo#LearnabilityCharacteristic"/>
            </owl:Restriction>
        </rdfs:subClassOf>
        <rdfs:subClassOf>
            <owl:Restriction>
                <owl:onProperty rdf:resource="https://purl.archive.org/oquo#measuresCharacteristicPositively"/>
                <owl:someValuesFrom rdf:resource="https://purl.archive.org/oquo#ModificationStabilityCharacteristic"/>
            </owl:Restriction>
        </rdfs:subClassOf>
        <rdfs:subClassOf>
            <owl:Restriction>
                <owl:onProperty rdf:resource="https://purl.archive.org/oquo#measuresCharacteristicPositively"/>
                <owl:someValuesFrom rdf:resource="https://purl.archive.org/oquo#ReplaceabilityCharacteristic"/>
            </owl:Restriction>
        </rdfs:subClassOf>
        <rdfs:subClassOf>
            <owl:Restriction>
                <owl:onProperty rdf:resource="https://purl.archive.org/oquo#measuresCharacteristicPositively"/>
                <owl:someValuesFrom rdf:resource="https://purl.archive.org/oquo#ReusabilityCharacteristic"/>
            </owl:Restriction>
        </rdfs:subClassOf>
        <rdfs:subClassOf>
            <owl:Restriction>
                <owl:onProperty rdf:resource="https://purl.archive.org/oquo#measuresCharacteristicPositively"/>
                <owl:someValuesFrom rdf:resource="https://purl.archive.org/oquo#TestabilityCharacteristic"/>
            </owl:Restriction>
        </rdfs:subClassOf>
        <rdfs:subClassOf>
            <owl:Restriction>
                <owl:onProperty rdf:resource="http://purl.org/net/QualityModel#hasScale"/>
                <owl:hasValue rdf:resource="https://purl.archive.org/oquo#NumberOfPropertiesMetricScale"/>
            </owl:Restriction>
        </rdfs:subClassOf>
        <obo:IAO_0000115 xml:lang="en">Number of properties per class. Mean number of object and data property usages per class NOMOnto=∑| PCi|∕∑|Ci| </obo:IAO_0000115>
        <rdf1:acronym>NOMOnto</rdf1:acronym>
        <rdfs:comment>Number of properties per class. Mean number of object and data property usages per class.</rdfs:comment>
        <rdfs:label>number of properties metric</rdfs:label>
    </owl:Class>
    


    <!-- https://purl.archive.org/oquo#ObjectPropertiesWithNoDescriptionMetric -->

    <owl:Class rdf:about="https://purl.archive.org/oquo#ObjectPropertiesWithNoDescriptionMetric">
        <rdfs:subClassOf rdf:resource="http://purl.org/net/QualityModel#DerivedMeasure"/>
        <rdfs:subClassOf>
            <owl:Restriction>
                <owl:onProperty rdf:resource="http://purl.org/net/QualityModel#hasScale"/>
                <owl:someValuesFrom>
                    <owl:Class>
                        <owl:intersectionOf rdf:parseType="Collection">
                            <rdf:Description rdf:about="https://purl.archive.org/oquo#RawScale"/>
                            <owl:Restriction>
                                <owl:onProperty rdf:resource="http://purl.org/net/QualityModel#hasRankigFunction"/>
                                <owl:hasValue rdf:resource="http://purl.org/net/QualityModel#LowerBest"/>
                            </owl:Restriction>
                        </owl:intersectionOf>
                    </owl:Class>
                </owl:someValuesFrom>
            </owl:Restriction>
        </rdfs:subClassOf>
        <rdfs:subClassOf>
            <owl:Restriction>
                <owl:onProperty rdf:resource="https://purl.archive.org/oquo#measuresCharacteristicNegatively"/>
                <owl:someValuesFrom rdf:resource="https://purl.archive.org/oquo#EaseOfUseCharacteristic"/>
            </owl:Restriction>
        </rdfs:subClassOf>
        <rdfs:subClassOf>
            <owl:Restriction>
                <owl:onProperty rdf:resource="https://purl.archive.org/oquo#measuresCharacteristicNegatively"/>
                <owl:someValuesFrom rdf:resource="https://purl.archive.org/oquo#EfficiencyInUseCharacteristic"/>
            </owl:Restriction>
        </rdfs:subClassOf>
        <rdfs:subClassOf>
            <owl:Restriction>
                <owl:onProperty rdf:resource="https://purl.archive.org/oquo#measuresCharacteristicNegatively"/>
                <owl:someValuesFrom rdf:resource="https://purl.archive.org/oquo#HelpfulnessCharacteristic"/>
            </owl:Restriction>
        </rdfs:subClassOf>
        <rdfs:subClassOf>
            <owl:Restriction>
                <owl:onProperty rdf:resource="https://purl.archive.org/oquo#measuresCharacteristicNegatively"/>
                <owl:someValuesFrom rdf:resource="https://purl.archive.org/oquo#IndexingAndLinkingCharacteristic"/>
            </owl:Restriction>
        </rdfs:subClassOf>
        <rdfs:subClassOf>
            <owl:Restriction>
                <owl:onProperty rdf:resource="https://purl.archive.org/oquo#measuresCharacteristicNegatively"/>
                <owl:someValuesFrom rdf:resource="https://purl.archive.org/oquo#KnowledgeReuseCharacteristic"/>
            </owl:Restriction>
        </rdfs:subClassOf>
        <rdfs:subClassOf>
            <owl:Restriction>
                <owl:onProperty rdf:resource="https://purl.archive.org/oquo#measuresCharacteristicNegatively"/>
                <owl:someValuesFrom rdf:resource="https://purl.archive.org/oquo#LearnabilityCharacteristic"/>
            </owl:Restriction>
        </rdfs:subClassOf>
        <rdfs:subClassOf>
            <owl:Restriction>
                <owl:onProperty rdf:resource="https://purl.archive.org/oquo#measuresCharacteristicNegatively"/>
                <owl:allValuesFrom>
                    <owl:Class>
                        <owl:unionOf rdf:parseType="Collection">
                            <rdf:Description rdf:about="https://purl.archive.org/oquo#EaseOfUseCharacteristic"/>
                            <rdf:Description rdf:about="https://purl.archive.org/oquo#EfficiencyInUseCharacteristic"/>
                            <rdf:Description rdf:about="https://purl.archive.org/oquo#HelpfulnessCharacteristic"/>
                            <rdf:Description rdf:about="https://purl.archive.org/oquo#IndexingAndLinkingCharacteristic"/>
                            <rdf:Description rdf:about="https://purl.archive.org/oquo#KnowledgeReuseCharacteristic"/>
                            <rdf:Description rdf:about="https://purl.archive.org/oquo#LearnabilityCharacteristic"/>
                        </owl:unionOf>
                    </owl:Class>
                </owl:allValuesFrom>
            </owl:Restriction>
        </rdfs:subClassOf>
        <rdfs:subClassOf>
            <owl:Restriction>
                <owl:onProperty rdf:resource="http://purl.org/net/QualityModel#hasScale"/>
                <owl:hasValue rdf:resource="https://purl.archive.org/oquo#ObjectPropertiesWithNoDescriptionMetricScale"/>
            </owl:Restriction>
        </rdfs:subClassOf>
        <obo:IAO_0000115>The Percentage of object properties lacking a description in the ontology.</obo:IAO_0000115>
        <rdf1:acronym>OPWND</rdf1:acronym>
        <rdfs:label>object properties with no description metric</rdfs:label>
    </owl:Class>
    


    <!-- https://purl.archive.org/oquo#ObjectPropertiesWithNoNameMetric -->

    <owl:Class rdf:about="https://purl.archive.org/oquo#ObjectPropertiesWithNoNameMetric">
        <rdfs:subClassOf rdf:resource="http://purl.org/net/QualityModel#DerivedMeasure"/>
        <rdfs:subClassOf>
            <owl:Restriction>
                <owl:onProperty rdf:resource="http://purl.org/net/QualityModel#hasScale"/>
                <owl:someValuesFrom>
                    <owl:Class>
                        <owl:intersectionOf rdf:parseType="Collection">
                            <rdf:Description rdf:about="https://purl.archive.org/oquo#RawScale"/>
                            <owl:Restriction>
                                <owl:onProperty rdf:resource="http://purl.org/net/QualityModel#hasRankigFunction"/>
                                <owl:hasValue rdf:resource="http://purl.org/net/QualityModel#LowerBest"/>
                            </owl:Restriction>
                        </owl:intersectionOf>
                    </owl:Class>
                </owl:someValuesFrom>
            </owl:Restriction>
        </rdfs:subClassOf>
        <rdfs:subClassOf>
            <owl:Restriction>
                <owl:onProperty rdf:resource="https://purl.archive.org/oquo#measuresCharacteristicNegatively"/>
                <owl:someValuesFrom rdf:resource="https://purl.archive.org/oquo#EaseOfUseCharacteristic"/>
            </owl:Restriction>
        </rdfs:subClassOf>
        <rdfs:subClassOf>
            <owl:Restriction>
                <owl:onProperty rdf:resource="https://purl.archive.org/oquo#measuresCharacteristicNegatively"/>
                <owl:someValuesFrom rdf:resource="https://purl.archive.org/oquo#EfficiencyInUseCharacteristic"/>
            </owl:Restriction>
        </rdfs:subClassOf>
        <rdfs:subClassOf>
            <owl:Restriction>
                <owl:onProperty rdf:resource="https://purl.archive.org/oquo#measuresCharacteristicNegatively"/>
                <owl:someValuesFrom rdf:resource="https://purl.archive.org/oquo#IndexingAndLinkingCharacteristic"/>
            </owl:Restriction>
        </rdfs:subClassOf>
        <rdfs:subClassOf>
            <owl:Restriction>
                <owl:onProperty rdf:resource="https://purl.archive.org/oquo#measuresCharacteristicNegatively"/>
                <owl:someValuesFrom rdf:resource="https://purl.archive.org/oquo#KnowledgeReuseCharacteristic"/>
            </owl:Restriction>
        </rdfs:subClassOf>
        <rdfs:subClassOf>
            <owl:Restriction>
                <owl:onProperty rdf:resource="https://purl.archive.org/oquo#measuresCharacteristicNegatively"/>
                <owl:someValuesFrom rdf:resource="https://purl.archive.org/oquo#TextAnalysisCharacteristic"/>
            </owl:Restriction>
        </rdfs:subClassOf>
        <rdfs:subClassOf>
            <owl:Restriction>
                <owl:onProperty rdf:resource="https://purl.archive.org/oquo#measuresCharacteristicNegatively"/>
                <owl:allValuesFrom>
                    <owl:Class>
                        <owl:unionOf rdf:parseType="Collection">
                            <rdf:Description rdf:about="https://purl.archive.org/oquo#EaseOfUseCharacteristic"/>
                            <rdf:Description rdf:about="https://purl.archive.org/oquo#EfficiencyInUseCharacteristic"/>
                            <rdf:Description rdf:about="https://purl.archive.org/oquo#IndexingAndLinkingCharacteristic"/>
                            <rdf:Description rdf:about="https://purl.archive.org/oquo#KnowledgeReuseCharacteristic"/>
                            <rdf:Description rdf:about="https://purl.archive.org/oquo#TextAnalysisCharacteristic"/>
                        </owl:unionOf>
                    </owl:Class>
                </owl:allValuesFrom>
            </owl:Restriction>
        </rdfs:subClassOf>
        <rdfs:subClassOf>
            <owl:Restriction>
                <owl:onProperty rdf:resource="http://purl.org/net/QualityModel#hasScale"/>
                <owl:hasValue rdf:resource="https://purl.archive.org/oquo#ObjectPropertiesWithNoNameMetricScale"/>
            </owl:Restriction>
        </rdfs:subClassOf>
        <obo:IAO_0000115>The Percentage of object properties lacking a name in the ontology.</obo:IAO_0000115>
        <rdf1:acronym>OPWNN</rdf1:acronym>
        <rdfs:label>object properties with no name metric</rdfs:label>
    </owl:Class>
    


    <!-- https://purl.archive.org/oquo#ObjectPropertiesWithNoSynonymMetric -->

    <owl:Class rdf:about="https://purl.archive.org/oquo#ObjectPropertiesWithNoSynonymMetric">
        <rdfs:subClassOf rdf:resource="http://purl.org/net/QualityModel#DerivedMeasure"/>
        <rdfs:subClassOf>
            <owl:Restriction>
                <owl:onProperty rdf:resource="http://purl.org/net/QualityModel#hasScale"/>
                <owl:someValuesFrom>
                    <owl:Class>
                        <owl:intersectionOf rdf:parseType="Collection">
                            <rdf:Description rdf:about="https://purl.archive.org/oquo#RawScale"/>
                            <owl:Restriction>
                                <owl:onProperty rdf:resource="http://purl.org/net/QualityModel#hasRankigFunction"/>
                                <owl:hasValue rdf:resource="http://purl.org/net/QualityModel#LowerBest"/>
                            </owl:Restriction>
                        </owl:intersectionOf>
                    </owl:Class>
                </owl:someValuesFrom>
            </owl:Restriction>
        </rdfs:subClassOf>
        <rdfs:subClassOf>
            <owl:Restriction>
                <owl:onProperty rdf:resource="https://purl.archive.org/oquo#measuresCharacteristicNegatively"/>
                <owl:someValuesFrom rdf:resource="https://purl.archive.org/oquo#EaseOfUseCharacteristic"/>
            </owl:Restriction>
        </rdfs:subClassOf>
        <rdfs:subClassOf>
            <owl:Restriction>
                <owl:onProperty rdf:resource="https://purl.archive.org/oquo#measuresCharacteristicNegatively"/>
                <owl:someValuesFrom rdf:resource="https://purl.archive.org/oquo#EfficiencyInUseCharacteristic"/>
            </owl:Restriction>
        </rdfs:subClassOf>
        <rdfs:subClassOf>
            <owl:Restriction>
                <owl:onProperty rdf:resource="https://purl.archive.org/oquo#measuresCharacteristicNegatively"/>
                <owl:someValuesFrom rdf:resource="https://purl.archive.org/oquo#IndexingAndLinkingCharacteristic"/>
            </owl:Restriction>
        </rdfs:subClassOf>
        <rdfs:subClassOf>
            <owl:Restriction>
                <owl:onProperty rdf:resource="https://purl.archive.org/oquo#measuresCharacteristicNegatively"/>
                <owl:someValuesFrom rdf:resource="https://purl.archive.org/oquo#KnowledgeReuseCharacteristic"/>
            </owl:Restriction>
        </rdfs:subClassOf>
        <rdfs:subClassOf>
            <owl:Restriction>
                <owl:onProperty rdf:resource="https://purl.archive.org/oquo#measuresCharacteristicNegatively"/>
                <owl:someValuesFrom rdf:resource="https://purl.archive.org/oquo#TextAnalysisCharacteristic"/>
            </owl:Restriction>
        </rdfs:subClassOf>
        <rdfs:subClassOf>
            <owl:Restriction>
                <owl:onProperty rdf:resource="https://purl.archive.org/oquo#measuresCharacteristicNegatively"/>
                <owl:allValuesFrom>
                    <owl:Class>
                        <owl:unionOf rdf:parseType="Collection">
                            <rdf:Description rdf:about="https://purl.archive.org/oquo#EaseOfUseCharacteristic"/>
                            <rdf:Description rdf:about="https://purl.archive.org/oquo#EfficiencyInUseCharacteristic"/>
                            <rdf:Description rdf:about="https://purl.archive.org/oquo#IndexingAndLinkingCharacteristic"/>
                            <rdf:Description rdf:about="https://purl.archive.org/oquo#KnowledgeReuseCharacteristic"/>
                            <rdf:Description rdf:about="https://purl.archive.org/oquo#TextAnalysisCharacteristic"/>
                        </owl:unionOf>
                    </owl:Class>
                </owl:allValuesFrom>
            </owl:Restriction>
        </rdfs:subClassOf>
        <rdfs:subClassOf>
            <owl:Restriction>
                <owl:onProperty rdf:resource="http://purl.org/net/QualityModel#hasScale"/>
                <owl:hasValue rdf:resource="https://purl.archive.org/oquo#ObjectPropertiesWithNoSynonymMetricScale"/>
            </owl:Restriction>
        </rdfs:subClassOf>
        <obo:IAO_0000115>The Percentage of object properties lacking a synonym in the ontology.</obo:IAO_0000115>
        <rdf1:acronym>OPWNS</rdf1:acronym>
        <rdfs:label>object properties with no synonym metric</rdfs:label>
    </owl:Class>
    


    <!-- https://purl.archive.org/oquo#OperabilityCharacteristic -->

    <owl:Class rdf:about="https://purl.archive.org/oquo#OperabilityCharacteristic">
        <rdfs:subClassOf rdf:resource="http://purl.org/net/QualityModel#QualityCharacteristic"/>
        <rdfs:subClassOf>
            <owl:Restriction>
                <owl:onProperty rdf:resource="http://purl.org/net/QualityModel#hasSubCharacteristic"/>
                <owl:someValuesFrom rdf:resource="https://purl.archive.org/oquo#AppropriatenessRecognisabilityCharacteristic"/>
            </owl:Restriction>
        </rdfs:subClassOf>
        <rdfs:subClassOf>
            <owl:Restriction>
                <owl:onProperty rdf:resource="http://purl.org/net/QualityModel#hasSubCharacteristic"/>
                <owl:someValuesFrom rdf:resource="https://purl.archive.org/oquo#EaseOfUseCharacteristic"/>
            </owl:Restriction>
        </rdfs:subClassOf>
        <rdfs:subClassOf>
            <owl:Restriction>
                <owl:onProperty rdf:resource="http://purl.org/net/QualityModel#hasSubCharacteristic"/>
                <owl:someValuesFrom rdf:resource="https://purl.archive.org/oquo#HelpfulnessCharacteristic"/>
            </owl:Restriction>
        </rdfs:subClassOf>
        <rdfs:subClassOf>
            <owl:Restriction>
                <owl:onProperty rdf:resource="http://purl.org/net/QualityModel#hasSubCharacteristic"/>
                <owl:someValuesFrom rdf:resource="https://purl.archive.org/oquo#LearnabilityCharacteristic"/>
            </owl:Restriction>
        </rdfs:subClassOf>
        <rdfs:subClassOf>
            <owl:Restriction>
                <owl:onProperty rdf:resource="http://purl.org/net/QualityModel#hasSubCharacteristic"/>
                <owl:allValuesFrom>
                    <owl:Class>
                        <owl:unionOf rdf:parseType="Collection">
                            <rdf:Description rdf:about="https://purl.archive.org/oquo#AppropriatenessRecognisabilityCharacteristic"/>
                            <rdf:Description rdf:about="https://purl.archive.org/oquo#EaseOfUseCharacteristic"/>
                            <rdf:Description rdf:about="https://purl.archive.org/oquo#HelpfulnessCharacteristic"/>
                            <rdf:Description rdf:about="https://purl.archive.org/oquo#LearnabilityCharacteristic"/>
                        </owl:unionOf>
                    </owl:Class>
                </owl:allValuesFrom>
            </owl:Restriction>
        </rdfs:subClassOf>
        <obo:IAO_0000115 xml:lang="en">Effort needed for use, and on the individual assessment of such use, by a stated or implied set of users.</obo:IAO_0000115>
        <rdfs:label>operability characteristic</rdfs:label>
    </owl:Class>
    


    <!-- https://purl.archive.org/oquo#PhysicalSatisfactionCharacteristic -->

    <owl:Class rdf:about="https://purl.archive.org/oquo#PhysicalSatisfactionCharacteristic">
        <rdfs:subClassOf rdf:resource="http://purl.org/net/QualityModel#QualityCharacteristic"/>
        <obo:IAO_0000115 xml:lang="en">Physical satisfaction</obo:IAO_0000115>
        <oboInOwl:hasExactSynonym xml:lang="en">Comfort characteristic</oboInOwl:hasExactSynonym>
        <rdfs:label>physical satisfaction characteristic</rdfs:label>
    </owl:Class>
    


    <!-- https://purl.archive.org/oquo#PortabilityCharacteristic -->

    <owl:Class rdf:about="https://purl.archive.org/oquo#PortabilityCharacteristic">
        <rdfs:subClassOf rdf:resource="http://purl.org/net/QualityModel#QualityCharacteristic"/>
        <obo:IAO_0000115 xml:lang="en">The degree in which an Ontology or one part of the ontology can be transferred from one hardware or software environment to another.</obo:IAO_0000115>
        <rdfs:label>portability characteristic</rdfs:label>
    </owl:Class>
    


    <!-- https://purl.archive.org/oquo#PrecisionCharacteristic -->

    <owl:Class rdf:about="https://purl.archive.org/oquo#PrecisionCharacteristic">
        <rdfs:subClassOf rdf:resource="http://purl.org/net/QualityModel#QualityCharacteristic"/>
        <obo:IAO_0000115 xml:lang="en">The degree to which The ontology provides the right or specified results with the needed degree of accuracy.</obo:IAO_0000115>
        <rdfs:label>precision characteristic</rdfs:label>
    </owl:Class>
    


    <!-- https://purl.archive.org/oquo#PropertiesRichnessMetric -->

    <owl:Class rdf:about="https://purl.archive.org/oquo#PropertiesRichnessMetric">
        <rdfs:subClassOf rdf:resource="http://purl.org/net/QualityModel#DerivedMeasure"/>
        <rdfs:subClassOf>
            <owl:Restriction>
                <owl:onProperty rdf:resource="http://purl.org/net/QualityModel#hasScale"/>
                <owl:someValuesFrom>
                    <owl:Class>
                        <owl:intersectionOf rdf:parseType="Collection">
                            <rdf:Description rdf:about="https://purl.archive.org/oquo#RawScale"/>
                            <owl:Restriction>
                                <owl:onProperty rdf:resource="http://purl.org/net/QualityModel#hasRankigFunction"/>
                                <owl:hasValue rdf:resource="http://purl.org/net/QualityModel#HigherBest"/>
                            </owl:Restriction>
                        </owl:intersectionOf>
                    </owl:Class>
                </owl:someValuesFrom>
            </owl:Restriction>
        </rdfs:subClassOf>
        <rdfs:subClassOf>
            <owl:Restriction>
                <owl:onProperty rdf:resource="http://purl.org/net/QualityModel#hasScale"/>
                <owl:hasValue rdf:resource="https://purl.archive.org/oquo#PropertiesRichnessMetricScale"/>
            </owl:Restriction>
        </rdfs:subClassOf>
        <obo:IAO_0000115 xml:lang="en">Number of usages of object and data properties divided by the number of subclassof relations and properties PROnto=∑|PCi| ∕∑(|RCi| + ∑|PCi|) </obo:IAO_0000115>
        <rdf1:acronym>PROnto</rdf1:acronym>
        <rdfs:comment>Number of usages of object and data properties divided by the number of subclassof relations and properties</rdfs:comment>
        <rdfs:label>properties richness metric</rdfs:label>
    </owl:Class>
    


    <!-- https://purl.archive.org/oquo#QualityInUseCharacteristic -->

    <owl:Class rdf:about="https://purl.archive.org/oquo#QualityInUseCharacteristic">
        <rdfs:subClassOf rdf:resource="http://purl.org/net/QualityModel#QualityCharacteristic"/>
        <rdfs:subClassOf>
            <owl:Restriction>
                <owl:onProperty rdf:resource="http://purl.org/net/QualityModel#hasSubCharacteristic"/>
                <owl:someValuesFrom rdf:resource="https://purl.archive.org/oquo#FlexibilityInUseCharacteristic"/>
            </owl:Restriction>
        </rdfs:subClassOf>
        <rdfs:subClassOf>
            <owl:Restriction>
                <owl:onProperty rdf:resource="http://purl.org/net/QualityModel#hasSubCharacteristic"/>
                <owl:someValuesFrom rdf:resource="https://purl.archive.org/oquo#UsabilityInUseCharacteristic"/>
            </owl:Restriction>
        </rdfs:subClassOf>
        <rdfs:subClassOf>
            <owl:Restriction>
                <owl:onProperty rdf:resource="http://purl.org/net/QualityModel#hasSubCharacteristic"/>
                <owl:allValuesFrom>
                    <owl:Class>
                        <owl:unionOf rdf:parseType="Collection">
                            <rdf:Description rdf:about="https://purl.archive.org/oquo#FlexibilityInUseCharacteristic"/>
                            <rdf:Description rdf:about="https://purl.archive.org/oquo#UsabilityInUseCharacteristic"/>
                        </owl:unionOf>
                    </owl:Class>
                </owl:allValuesFrom>
            </owl:Restriction>
        </rdfs:subClassOf>
        <obo:IAO_0000115 xml:lang="en">Quality in a particular context of use. Quality in use is the degree to which a product used by specific users meets their needs to achieve specific goals.</obo:IAO_0000115>
        <rdfs:label>quality in use characteristic</rdfs:label>
    </owl:Class>
    


    <!-- https://purl.archive.org/oquo#RawScale -->

    <owl:Class rdf:about="https://purl.archive.org/oquo#RawScale">
        <rdfs:subClassOf rdf:resource="http://www.wurvoc.org/vocabularies/om-1.8/Measurement_scale"/>
        <obo:IAO_0000115 xml:lang="en">The raw scale provided by a metric directly without applying any scale.</obo:IAO_0000115>
        <rdfs:label>raw scale</rdfs:label>
    </owl:Class>
    


    <!-- https://purl.archive.org/oquo#RecoverabilityCharacteristic -->

    <owl:Class rdf:about="https://purl.archive.org/oquo#RecoverabilityCharacteristic">
        <rdfs:subClassOf rdf:resource="http://purl.org/net/QualityModel#QualityCharacteristic"/>
        <obo:IAO_0000115 xml:lang="en">The degree to which the ontology can reestablish a specified level of performance and recover the data directly affected in the case of a failure.</obo:IAO_0000115>
        <rdfs:label xml:lang="en">recoverability characteristic</rdfs:label>
    </owl:Class>
    


    <!-- https://purl.archive.org/oquo#RedundancyCharacteristic -->

    <owl:Class rdf:about="https://purl.archive.org/oquo#RedundancyCharacteristic">
        <rdfs:subClassOf rdf:resource="http://purl.org/net/QualityModel#QualityCharacteristic"/>
        <obo:IAO_0000115 xml:lang="en">Capability of the ontology to be informative</obo:IAO_0000115>
        <rdfs:label>redundancy characteristic</rdfs:label>
    </owl:Class>
    


    <!-- https://purl.archive.org/oquo#ReferenceOntologyCharacteristic -->

    <owl:Class rdf:about="https://purl.archive.org/oquo#ReferenceOntologyCharacteristic">
        <rdfs:subClassOf rdf:resource="http://purl.org/net/QualityModel#QualityCharacteristic"/>
        <obo:IAO_0000115 xml:lang="en">Degree in which the ontology can be used as a reference resource for the particular domain the ontology is built for.</obo:IAO_0000115>
        <rdfs:label>reference ontology characteristic</rdfs:label>
    </owl:Class>
    


    <!-- https://purl.archive.org/oquo#RelationshipRichnessMetric -->

    <owl:Class rdf:about="https://purl.archive.org/oquo#RelationshipRichnessMetric">
        <rdfs:subClassOf rdf:resource="http://purl.org/net/QualityModel#DerivedMeasure"/>
        <rdfs:subClassOf>
            <owl:Restriction>
                <owl:onProperty rdf:resource="http://purl.org/net/QualityModel#hasScale"/>
                <owl:someValuesFrom>
                    <owl:Class>
                        <owl:intersectionOf rdf:parseType="Collection">
                            <rdf:Description rdf:about="https://purl.archive.org/oquo#RawScale"/>
                            <owl:Restriction>
                                <owl:onProperty rdf:resource="http://purl.org/net/QualityModel#hasRankigFunction"/>
                                <owl:hasValue rdf:resource="http://purl.org/net/QualityModel#HigherBest"/>
                            </owl:Restriction>
                        </owl:intersectionOf>
                    </owl:Class>
                </owl:someValuesFrom>
            </owl:Restriction>
        </rdfs:subClassOf>
        <rdfs:subClassOf>
            <owl:Restriction>
                <owl:onProperty rdf:resource="https://purl.archive.org/oquo#measuresCharacteristicPositively"/>
                <owl:someValuesFrom rdf:resource="https://purl.archive.org/oquo#ConsistentSearchAndQueryCharacteristic"/>
            </owl:Restriction>
        </rdfs:subClassOf>
        <rdfs:subClassOf>
            <owl:Restriction>
                <owl:onProperty rdf:resource="https://purl.archive.org/oquo#measuresCharacteristicPositively"/>
                <owl:someValuesFrom rdf:resource="https://purl.archive.org/oquo#FormalRelationSupportCharacteristic"/>
            </owl:Restriction>
        </rdfs:subClassOf>
        <rdfs:subClassOf>
            <owl:Restriction>
                <owl:onProperty rdf:resource="https://purl.archive.org/oquo#measuresCharacteristicPositively"/>
                <owl:someValuesFrom rdf:resource="https://purl.archive.org/oquo#IndexingAndLinkingCharacteristic"/>
            </owl:Restriction>
        </rdfs:subClassOf>
        <rdfs:subClassOf>
            <owl:Restriction>
                <owl:onProperty rdf:resource="https://purl.archive.org/oquo#measuresCharacteristicPositively"/>
                <owl:someValuesFrom rdf:resource="https://purl.archive.org/oquo#InferenceCharacteristic"/>
            </owl:Restriction>
        </rdfs:subClassOf>
        <rdfs:subClassOf>
            <owl:Restriction>
                <owl:onProperty rdf:resource="https://purl.archive.org/oquo#measuresCharacteristicPositively"/>
                <owl:someValuesFrom rdf:resource="https://purl.archive.org/oquo#KnowledgeAcquisitionRepresentationCharacteristic"/>
            </owl:Restriction>
        </rdfs:subClassOf>
        <rdfs:subClassOf>
            <owl:Restriction>
                <owl:onProperty rdf:resource="https://purl.archive.org/oquo#measuresCharacteristicPositively"/>
                <owl:someValuesFrom rdf:resource="https://purl.archive.org/oquo#ReferenceOntologyCharacteristic"/>
            </owl:Restriction>
        </rdfs:subClassOf>
        <rdfs:subClassOf>
            <owl:Restriction>
                <owl:onProperty rdf:resource="https://purl.archive.org/oquo#measuresCharacteristicPositively"/>
                <owl:someValuesFrom rdf:resource="https://purl.archive.org/oquo#SchemaAndValueReconciliationCharacteristic"/>
            </owl:Restriction>
        </rdfs:subClassOf>
        <rdfs:subClassOf>
            <owl:Restriction>
                <owl:onProperty rdf:resource="https://purl.archive.org/oquo#measuresCharacteristicPositively"/>
                <owl:someValuesFrom rdf:resource="https://purl.archive.org/oquo#SimilarityCharacteristic"/>
            </owl:Restriction>
        </rdfs:subClassOf>
        <rdfs:subClassOf>
            <owl:Restriction>
                <owl:onProperty rdf:resource="https://purl.archive.org/oquo#measuresCharacteristicPositively"/>
                <owl:allValuesFrom>
                    <owl:Class>
                        <owl:unionOf rdf:parseType="Collection">
                            <rdf:Description rdf:about="https://purl.archive.org/oquo#ConsistentSearchAndQueryCharacteristic"/>
                            <rdf:Description rdf:about="https://purl.archive.org/oquo#FormalRelationSupportCharacteristic"/>
                            <rdf:Description rdf:about="https://purl.archive.org/oquo#IndexingAndLinkingCharacteristic"/>
                            <rdf:Description rdf:about="https://purl.archive.org/oquo#InferenceCharacteristic"/>
                            <rdf:Description rdf:about="https://purl.archive.org/oquo#KnowledgeAcquisitionRepresentationCharacteristic"/>
                            <rdf:Description rdf:about="https://purl.archive.org/oquo#ReferenceOntologyCharacteristic"/>
                            <rdf:Description rdf:about="https://purl.archive.org/oquo#SchemaAndValueReconciliationCharacteristic"/>
                            <rdf:Description rdf:about="https://purl.archive.org/oquo#SimilarityCharacteristic"/>
                        </owl:unionOf>
                    </owl:Class>
                </owl:allValuesFrom>
            </owl:Restriction>
        </rdfs:subClassOf>
        <rdfs:subClassOf>
            <owl:Restriction>
                <owl:onProperty rdf:resource="http://purl.org/net/QualityModel#hasScale"/>
                <owl:hasValue rdf:resource="https://purl.archive.org/oquo#RelationshipRichnessMetricScale"/>
            </owl:Restriction>
        </rdfs:subClassOf>
        <obo:IAO_0000115 xml:lang="en">Number of subclassof relationships divided by the number of subclassof relationships and properties RROnto=∑|RCi| ∕∑(|RCi| + ∑|PCi|) </obo:IAO_0000115>
        <rdf1:acronym>RROnto</rdf1:acronym>
        <rdfs:comment>Number of subclassof relationships divided by the number of subclassof relationships and properties.</rdfs:comment>
        <rdfs:label>relationship richness metric</rdfs:label>
    </owl:Class>
    


    <!-- https://purl.archive.org/oquo#RelationshipsPerClassMetric -->

    <owl:Class rdf:about="https://purl.archive.org/oquo#RelationshipsPerClassMetric">
        <rdfs:subClassOf rdf:resource="http://purl.org/net/QualityModel#DerivedMeasure"/>
        <rdfs:subClassOf>
            <owl:Restriction>
                <owl:onProperty rdf:resource="http://purl.org/net/QualityModel#hasScale"/>
                <owl:someValuesFrom>
                    <owl:Class>
                        <owl:intersectionOf rdf:parseType="Collection">
                            <rdf:Description rdf:about="https://purl.archive.org/oquo#RawScale"/>
                            <owl:Restriction>
                                <owl:onProperty rdf:resource="http://purl.org/net/QualityModel#hasRankigFunction"/>
                                <owl:hasValue rdf:resource="http://purl.org/net/QualityModel#HigherBest"/>
                            </owl:Restriction>
                        </owl:intersectionOf>
                    </owl:Class>
                </owl:someValuesFrom>
            </owl:Restriction>
        </rdfs:subClassOf>
        <rdfs:subClassOf>
            <owl:Restriction>
                <owl:onProperty rdf:resource="https://purl.archive.org/oquo#measuresCharacteristicPositively"/>
                <owl:someValuesFrom rdf:resource="https://purl.archive.org/oquo#ConsistentSearchAndQueryCharacteristic"/>
            </owl:Restriction>
        </rdfs:subClassOf>
        <rdfs:subClassOf>
            <owl:Restriction>
                <owl:onProperty rdf:resource="https://purl.archive.org/oquo#measuresCharacteristicPositively"/>
                <owl:someValuesFrom rdf:resource="https://purl.archive.org/oquo#DecisionTreesCharacteristic"/>
            </owl:Restriction>
        </rdfs:subClassOf>
        <rdfs:subClassOf>
            <owl:Restriction>
                <owl:onProperty rdf:resource="https://purl.archive.org/oquo#measuresCharacteristicPositively"/>
                <owl:someValuesFrom rdf:resource="https://purl.archive.org/oquo#GuidanceCharacteristic"/>
            </owl:Restriction>
        </rdfs:subClassOf>
        <rdfs:subClassOf>
            <owl:Restriction>
                <owl:onProperty rdf:resource="https://purl.archive.org/oquo#measuresCharacteristicPositively"/>
                <owl:someValuesFrom rdf:resource="https://purl.archive.org/oquo#IndexingAndLinkingCharacteristic"/>
            </owl:Restriction>
        </rdfs:subClassOf>
        <rdfs:subClassOf>
            <owl:Restriction>
                <owl:onProperty rdf:resource="https://purl.archive.org/oquo#measuresCharacteristicPositively"/>
                <owl:someValuesFrom rdf:resource="https://purl.archive.org/oquo#KnowledgeReuseCharacteristic"/>
            </owl:Restriction>
        </rdfs:subClassOf>
        <rdfs:subClassOf>
            <owl:Restriction>
                <owl:onProperty rdf:resource="https://purl.archive.org/oquo#measuresCharacteristicPositively"/>
                <owl:allValuesFrom>
                    <owl:Class>
                        <owl:unionOf rdf:parseType="Collection">
                            <rdf:Description rdf:about="https://purl.archive.org/oquo#ConsistentSearchAndQueryCharacteristic"/>
                            <rdf:Description rdf:about="https://purl.archive.org/oquo#DecisionTreesCharacteristic"/>
                            <rdf:Description rdf:about="https://purl.archive.org/oquo#GuidanceCharacteristic"/>
                            <rdf:Description rdf:about="https://purl.archive.org/oquo#IndexingAndLinkingCharacteristic"/>
                            <rdf:Description rdf:about="https://purl.archive.org/oquo#KnowledgeReuseCharacteristic"/>
                        </owl:unionOf>
                    </owl:Class>
                </owl:allValuesFrom>
            </owl:Restriction>
        </rdfs:subClassOf>
        <rdfs:subClassOf>
            <owl:Restriction>
                <owl:onProperty rdf:resource="http://purl.org/net/QualityModel#hasScale"/>
                <owl:hasValue rdf:resource="https://purl.archive.org/oquo#RelationshipsPerClassMetricScale"/>
            </owl:Restriction>
        </rdfs:subClassOf>
        <obo:IAO_0000115 xml:lang="en">Mean number of subclasses per class INROnto=∑| RCi| /∑|Ci| </obo:IAO_0000115>
        <rdf1:acronym>INROnto</rdf1:acronym>
        <rdfs:comment>Mean number of subclasses per class</rdfs:comment>
        <rdfs:label>relationships per class metric</rdfs:label>
    </owl:Class>
    


    <!-- https://purl.archive.org/oquo#ReliabilityCharacteristic -->

    <owl:Class rdf:about="https://purl.archive.org/oquo#ReliabilityCharacteristic">
        <rdfs:subClassOf rdf:resource="http://purl.org/net/QualityModel#QualityCharacteristic"/>
        <rdfs:subClassOf>
            <owl:Restriction>
                <owl:onProperty rdf:resource="http://purl.org/net/QualityModel#hasSubCharacteristic"/>
                <owl:someValuesFrom rdf:resource="https://purl.archive.org/oquo#AvailabilityCharacteristic"/>
            </owl:Restriction>
        </rdfs:subClassOf>
        <rdfs:subClassOf>
            <owl:Restriction>
                <owl:onProperty rdf:resource="http://purl.org/net/QualityModel#hasSubCharacteristic"/>
                <owl:someValuesFrom rdf:resource="https://purl.archive.org/oquo#RecoverabilityCharacteristic"/>
            </owl:Restriction>
        </rdfs:subClassOf>
        <obo:IAO_0000115 xml:lang="en">Capability of an ontology to maintain its level of performance under stated conditions for a given period of time.</obo:IAO_0000115>
        <rdfs:label>reliability characteristic</rdfs:label>
    </owl:Class>
    


    <!-- https://purl.archive.org/oquo#ReplaceabilityCharacteristic -->

    <owl:Class rdf:about="https://purl.archive.org/oquo#ReplaceabilityCharacteristic">
        <rdfs:subClassOf rdf:resource="http://purl.org/net/QualityModel#QualityCharacteristic"/>
        <obo:IAO_0000115 xml:lang="en">The degree to which The ontology can be used in place of another specified Ontology for the same purpose in the same environment.</obo:IAO_0000115>
        <rdfs:label>replaceability characteristic</rdfs:label>
    </owl:Class>
    


    <!-- https://purl.archive.org/oquo#ResponseForAClassMetric -->

    <owl:Class rdf:about="https://purl.archive.org/oquo#ResponseForAClassMetric">
        <rdfs:subClassOf rdf:resource="http://purl.org/net/QualityModel#DerivedMeasure"/>
        <rdfs:subClassOf>
            <owl:Restriction>
                <owl:onProperty rdf:resource="http://purl.org/net/QualityModel#hasScale"/>
                <owl:someValuesFrom>
                    <owl:Class>
                        <owl:intersectionOf rdf:parseType="Collection">
                            <rdf:Description rdf:about="https://purl.archive.org/oquo#RawScale"/>
                            <owl:Restriction>
                                <owl:onProperty rdf:resource="http://purl.org/net/QualityModel#hasRankigFunction"/>
                                <owl:hasValue rdf:resource="http://purl.org/net/QualityModel#LowerBest"/>
                            </owl:Restriction>
                        </owl:intersectionOf>
                    </owl:Class>
                </owl:someValuesFrom>
            </owl:Restriction>
        </rdfs:subClassOf>
        <rdfs:subClassOf>
            <owl:Restriction>
                <owl:onProperty rdf:resource="https://purl.archive.org/oquo#measuresCharacteristicPositively"/>
                <owl:someValuesFrom rdf:resource="https://purl.archive.org/oquo#AdaptabilityCharacteristic"/>
            </owl:Restriction>
        </rdfs:subClassOf>
        <rdfs:subClassOf>
            <owl:Restriction>
                <owl:onProperty rdf:resource="https://purl.archive.org/oquo#measuresCharacteristicPositively"/>
                <owl:someValuesFrom rdf:resource="https://purl.archive.org/oquo#AnalysabilityCharacteristic"/>
            </owl:Restriction>
        </rdfs:subClassOf>
        <rdfs:subClassOf>
            <owl:Restriction>
                <owl:onProperty rdf:resource="https://purl.archive.org/oquo#measuresCharacteristicPositively"/>
                <owl:someValuesFrom rdf:resource="https://purl.archive.org/oquo#ChangeabilityCharacteristic"/>
            </owl:Restriction>
        </rdfs:subClassOf>
        <rdfs:subClassOf>
            <owl:Restriction>
                <owl:onProperty rdf:resource="https://purl.archive.org/oquo#measuresCharacteristicPositively"/>
                <owl:someValuesFrom rdf:resource="https://purl.archive.org/oquo#LearnabilityCharacteristic"/>
            </owl:Restriction>
        </rdfs:subClassOf>
        <rdfs:subClassOf>
            <owl:Restriction>
                <owl:onProperty rdf:resource="https://purl.archive.org/oquo#measuresCharacteristicPositively"/>
                <owl:someValuesFrom rdf:resource="https://purl.archive.org/oquo#ModificationStabilityCharacteristic"/>
            </owl:Restriction>
        </rdfs:subClassOf>
        <rdfs:subClassOf>
            <owl:Restriction>
                <owl:onProperty rdf:resource="https://purl.archive.org/oquo#measuresCharacteristicPositively"/>
                <owl:someValuesFrom rdf:resource="https://purl.archive.org/oquo#ReusabilityCharacteristic"/>
            </owl:Restriction>
        </rdfs:subClassOf>
        <rdfs:subClassOf>
            <owl:Restriction>
                <owl:onProperty rdf:resource="https://purl.archive.org/oquo#measuresCharacteristicPositively"/>
                <owl:someValuesFrom rdf:resource="https://purl.archive.org/oquo#TestabilityCharacteristic"/>
            </owl:Restriction>
        </rdfs:subClassOf>
        <rdfs:subClassOf>
            <owl:Restriction>
                <owl:onProperty rdf:resource="https://purl.archive.org/oquo#measuresCharacteristicPositively"/>
                <owl:allValuesFrom>
                    <owl:Class>
                        <owl:unionOf rdf:parseType="Collection">
                            <rdf:Description rdf:about="https://purl.archive.org/oquo#AdaptabilityCharacteristic"/>
                            <rdf:Description rdf:about="https://purl.archive.org/oquo#AnalysabilityCharacteristic"/>
                            <rdf:Description rdf:about="https://purl.archive.org/oquo#ChangeabilityCharacteristic"/>
                            <rdf:Description rdf:about="https://purl.archive.org/oquo#LearnabilityCharacteristic"/>
                            <rdf:Description rdf:about="https://purl.archive.org/oquo#ModificationStabilityCharacteristic"/>
                            <rdf:Description rdf:about="https://purl.archive.org/oquo#ReusabilityCharacteristic"/>
                            <rdf:Description rdf:about="https://purl.archive.org/oquo#TestabilityCharacteristic"/>
                        </owl:unionOf>
                    </owl:Class>
                </owl:allValuesFrom>
            </owl:Restriction>
        </rdfs:subClassOf>
        <rdfs:subClassOf>
            <owl:Restriction>
                <owl:onProperty rdf:resource="http://purl.org/net/QualityModel#hasScale"/>
                <owl:hasValue rdf:resource="https://purl.archive.org/oquo#ResponseForAClassMetricScale"/>
            </owl:Restriction>
        </rdfs:subClassOf>
        <obo:IAO_0000115 xml:lang="en">Number of properties that can be directly accessed from the class. number of usages of object and data properties and superclasses divided by the number of classes RFCOnto=(∑|PCi|+∑|SupCi|/(∑|Ci| </obo:IAO_0000115>
        <rdf1:acronym>RFCOnto</rdf1:acronym>
        <rdfs:comment>Number of properties that can be directly accessed from the class.</rdfs:comment>
        <rdfs:label>response for a class metric</rdfs:label>
    </owl:Class>
    


    <!-- https://purl.archive.org/oquo#ResultsRepresentationCharacteristic -->

    <owl:Class rdf:about="https://purl.archive.org/oquo#ResultsRepresentationCharacteristic">
        <rdfs:subClassOf rdf:resource="http://purl.org/net/QualityModel#QualityCharacteristic"/>
        <obo:IAO_0000115 xml:lang="en">Capability of the ontology to analize complex results such as microarrays experiments.</obo:IAO_0000115>
        <rdfs:label>results representation characteristic</rdfs:label>
    </owl:Class>
    


    <!-- https://purl.archive.org/oquo#ReusabilityCharacteristic -->

    <owl:Class rdf:about="https://purl.archive.org/oquo#ReusabilityCharacteristic">
        <rdfs:subClassOf rdf:resource="http://purl.org/net/QualityModel#QualityCharacteristic"/>
        <obo:IAO_0000115 xml:lang="en">The degree to which an asset (part of) the ontology can be used in more than one ontology, or in building other assets.</obo:IAO_0000115>
        <rdfs:label>reusability characteristic</rdfs:label>
    </owl:Class>
    


    <!-- https://purl.archive.org/oquo#SatisfactionInUseCharacteristic -->

    <owl:Class rdf:about="https://purl.archive.org/oquo#SatisfactionInUseCharacteristic">
        <rdfs:subClassOf rdf:resource="http://purl.org/net/QualityModel#QualityCharacteristic"/>
        <rdfs:subClassOf>
            <owl:Restriction>
                <owl:onProperty rdf:resource="http://purl.org/net/QualityModel#hasSubCharacteristic"/>
                <owl:someValuesFrom rdf:resource="https://purl.archive.org/oquo#CognitiveSatisfactionCharacteristic"/>
            </owl:Restriction>
        </rdfs:subClassOf>
        <rdfs:subClassOf>
            <owl:Restriction>
                <owl:onProperty rdf:resource="http://purl.org/net/QualityModel#hasSubCharacteristic"/>
                <owl:someValuesFrom rdf:resource="https://purl.archive.org/oquo#EmotionalSatisfactionCharacteristic"/>
            </owl:Restriction>
        </rdfs:subClassOf>
        <rdfs:subClassOf>
            <owl:Restriction>
                <owl:onProperty rdf:resource="http://purl.org/net/QualityModel#hasSubCharacteristic"/>
                <owl:someValuesFrom rdf:resource="https://purl.archive.org/oquo#PhysicalSatisfactionCharacteristic"/>
            </owl:Restriction>
        </rdfs:subClassOf>
        <rdfs:subClassOf>
            <owl:Restriction>
                <owl:onProperty rdf:resource="http://purl.org/net/QualityModel#hasSubCharacteristic"/>
                <owl:allValuesFrom>
                    <owl:Class>
                        <owl:unionOf rdf:parseType="Collection">
                            <rdf:Description rdf:about="https://purl.archive.org/oquo#CognitiveSatisfactionCharacteristic"/>
                            <rdf:Description rdf:about="https://purl.archive.org/oquo#EmotionalSatisfactionCharacteristic"/>
                            <rdf:Description rdf:about="https://purl.archive.org/oquo#PhysicalSatisfactionCharacteristic"/>
                        </owl:unionOf>
                    </owl:Class>
                </owl:allValuesFrom>
            </owl:Restriction>
        </rdfs:subClassOf>
        <obo:IAO_0000115 xml:lang="en">The degree to which users are satisfied in a especified context of use.</obo:IAO_0000115>
        <rdfs:label>satisfaction in use characteristic</rdfs:label>
    </owl:Class>
    


    <!-- https://purl.archive.org/oquo#SchemaAndValueReconciliationCharacteristic -->

    <owl:Class rdf:about="https://purl.archive.org/oquo#SchemaAndValueReconciliationCharacteristic">
        <rdfs:subClassOf rdf:resource="http://purl.org/net/QualityModel#QualityCharacteristic"/>
        <obo:IAO_0000115 xml:lang="en">Degree in which ontology provide a common data model that can be applied to reconciliation and integration.</obo:IAO_0000115>
        <rdfs:label>schema and value reconciliation characteristic</rdfs:label>
    </owl:Class>
    


    <!-- https://purl.archive.org/oquo#SimilarityCharacteristic -->

    <owl:Class rdf:about="https://purl.archive.org/oquo#SimilarityCharacteristic">
        <rdfs:subClassOf rdf:resource="http://purl.org/net/QualityModel#QualityCharacteristic"/>
        <obo:IAO_0000115 xml:lang="en">Capability of the component of the ontology to be compared for similarity.</obo:IAO_0000115>
        <rdfs:label>similarity characteristic</rdfs:label>
    </owl:Class>
    


    <!-- https://purl.archive.org/oquo#StructuralAccuracyCharacteristic -->

    <owl:Class rdf:about="https://purl.archive.org/oquo#StructuralAccuracyCharacteristic">
        <rdfs:subClassOf rdf:resource="http://purl.org/net/QualityModel#QualityCharacteristic"/>
        <obo:IAO_0000115 xml:lang="en">Degree of the correctness of the terms used in the ontology.</obo:IAO_0000115>
        <rdfs:label>structural accuracy characteristic</rdfs:label>
    </owl:Class>
    


    <!-- https://purl.archive.org/oquo#StructuralCharacteristic -->

    <owl:Class rdf:about="https://purl.archive.org/oquo#StructuralCharacteristic">
        <rdfs:subClassOf rdf:resource="http://purl.org/net/QualityModel#QualityCharacteristic"/>
        <rdfs:subClassOf>
            <owl:Restriction>
                <owl:onProperty rdf:resource="http://purl.org/net/QualityModel#hasSubCharacteristic"/>
                <owl:someValuesFrom rdf:resource="https://purl.archive.org/oquo#CohesionCharacteristic"/>
            </owl:Restriction>
        </rdfs:subClassOf>
        <rdfs:subClassOf>
            <owl:Restriction>
                <owl:onProperty rdf:resource="http://purl.org/net/QualityModel#hasSubCharacteristic"/>
                <owl:someValuesFrom rdf:resource="https://purl.archive.org/oquo#ConsistencyCharacteristic"/>
            </owl:Restriction>
        </rdfs:subClassOf>
        <rdfs:subClassOf>
            <owl:Restriction>
                <owl:onProperty rdf:resource="http://purl.org/net/QualityModel#hasSubCharacteristic"/>
                <owl:someValuesFrom rdf:resource="https://purl.archive.org/oquo#CyclesCharacteristic"/>
            </owl:Restriction>
        </rdfs:subClassOf>
        <rdfs:subClassOf>
            <owl:Restriction>
                <owl:onProperty rdf:resource="http://purl.org/net/QualityModel#hasSubCharacteristic"/>
                <owl:someValuesFrom rdf:resource="https://purl.archive.org/oquo#DomainCoverageCharacteristic"/>
            </owl:Restriction>
        </rdfs:subClassOf>
        <rdfs:subClassOf>
            <owl:Restriction>
                <owl:onProperty rdf:resource="http://purl.org/net/QualityModel#hasSubCharacteristic"/>
                <owl:someValuesFrom rdf:resource="https://purl.archive.org/oquo#FormalRelationSupportCharacteristic"/>
            </owl:Restriction>
        </rdfs:subClassOf>
        <rdfs:subClassOf>
            <owl:Restriction>
                <owl:onProperty rdf:resource="http://purl.org/net/QualityModel#hasSubCharacteristic"/>
                <owl:someValuesFrom rdf:resource="https://purl.archive.org/oquo#FormalisationCharacteristic"/>
            </owl:Restriction>
        </rdfs:subClassOf>
        <rdfs:subClassOf>
            <owl:Restriction>
                <owl:onProperty rdf:resource="http://purl.org/net/QualityModel#hasSubCharacteristic"/>
                <owl:someValuesFrom rdf:resource="https://purl.archive.org/oquo#RedundancyCharacteristic"/>
            </owl:Restriction>
        </rdfs:subClassOf>
        <rdfs:subClassOf>
            <owl:Restriction>
                <owl:onProperty rdf:resource="http://purl.org/net/QualityModel#hasSubCharacteristic"/>
                <owl:someValuesFrom rdf:resource="https://purl.archive.org/oquo#StructuralAccuracyCharacteristic"/>
            </owl:Restriction>
        </rdfs:subClassOf>
        <rdfs:subClassOf>
            <owl:Restriction>
                <owl:onProperty rdf:resource="http://purl.org/net/QualityModel#hasSubCharacteristic"/>
                <owl:someValuesFrom rdf:resource="https://purl.archive.org/oquo#TanglednessCharacteristic"/>
            </owl:Restriction>
        </rdfs:subClassOf>
        <rdfs:subClassOf>
            <owl:Restriction>
                <owl:onProperty rdf:resource="http://purl.org/net/QualityModel#hasSubCharacteristic"/>
                <owl:allValuesFrom>
                    <owl:Class>
                        <owl:unionOf rdf:parseType="Collection">
                            <rdf:Description rdf:about="https://purl.archive.org/oquo#CohesionCharacteristic"/>
                            <rdf:Description rdf:about="https://purl.archive.org/oquo#ConsistencyCharacteristic"/>
                            <rdf:Description rdf:about="https://purl.archive.org/oquo#CyclesCharacteristic"/>
                            <rdf:Description rdf:about="https://purl.archive.org/oquo#DomainCoverageCharacteristic"/>
                            <rdf:Description rdf:about="https://purl.archive.org/oquo#FormalRelationSupportCharacteristic"/>
                            <rdf:Description rdf:about="https://purl.archive.org/oquo#FormalisationCharacteristic"/>
                            <rdf:Description rdf:about="https://purl.archive.org/oquo#RedundancyCharacteristic"/>
                            <rdf:Description rdf:about="https://purl.archive.org/oquo#StructuralAccuracyCharacteristic"/>
                            <rdf:Description rdf:about="https://purl.archive.org/oquo#TanglednessCharacteristic"/>
                        </owl:unionOf>
                    </owl:Class>
                </owl:allValuesFrom>
            </owl:Restriction>
        </rdfs:subClassOf>
        <obo:IAO_0000115 xml:lang="en">The structural characteristic accounts for ontology quality factors such as consistency, formalisation, redundancy or tangledness.</obo:IAO_0000115>
        <rdfs:label>structural characteristic</rdfs:label>
    </owl:Class>
    


    <!-- https://purl.archive.org/oquo#SynonymsPerAnnotationPropertyMetric -->

    <owl:Class rdf:about="https://purl.archive.org/oquo#SynonymsPerAnnotationPropertyMetric">
        <rdfs:subClassOf rdf:resource="http://purl.org/net/QualityModel#DerivedMeasure"/>
        <rdfs:subClassOf>
            <owl:Restriction>
                <owl:onProperty rdf:resource="http://purl.org/net/QualityModel#hasScale"/>
                <owl:someValuesFrom>
                    <owl:Class>
                        <owl:intersectionOf rdf:parseType="Collection">
                            <rdf:Description rdf:about="https://purl.archive.org/oquo#RawScale"/>
                            <owl:Restriction>
                                <owl:onProperty rdf:resource="http://purl.org/net/QualityModel#hasRankigFunction"/>
                                <owl:hasValue rdf:resource="http://purl.org/net/QualityModel#HigherBest"/>
                            </owl:Restriction>
                        </owl:intersectionOf>
                    </owl:Class>
                </owl:someValuesFrom>
            </owl:Restriction>
        </rdfs:subClassOf>
        <rdfs:subClassOf>
            <owl:Restriction>
                <owl:onProperty rdf:resource="https://purl.archive.org/oquo#measuresCharacteristicPositively"/>
                <owl:someValuesFrom rdf:resource="https://purl.archive.org/oquo#EaseOfUseCharacteristic"/>
            </owl:Restriction>
        </rdfs:subClassOf>
        <rdfs:subClassOf>
            <owl:Restriction>
                <owl:onProperty rdf:resource="https://purl.archive.org/oquo#measuresCharacteristicPositively"/>
                <owl:someValuesFrom rdf:resource="https://purl.archive.org/oquo#EfficiencyInUseCharacteristic"/>
            </owl:Restriction>
        </rdfs:subClassOf>
        <rdfs:subClassOf>
            <owl:Restriction>
                <owl:onProperty rdf:resource="https://purl.archive.org/oquo#measuresCharacteristicPositively"/>
                <owl:someValuesFrom rdf:resource="https://purl.archive.org/oquo#IndexingAndLinkingCharacteristic"/>
            </owl:Restriction>
        </rdfs:subClassOf>
        <rdfs:subClassOf>
            <owl:Restriction>
                <owl:onProperty rdf:resource="https://purl.archive.org/oquo#measuresCharacteristicPositively"/>
                <owl:someValuesFrom rdf:resource="https://purl.archive.org/oquo#KnowledgeReuseCharacteristic"/>
            </owl:Restriction>
        </rdfs:subClassOf>
        <rdfs:subClassOf>
            <owl:Restriction>
                <owl:onProperty rdf:resource="https://purl.archive.org/oquo#measuresCharacteristicPositively"/>
                <owl:someValuesFrom rdf:resource="https://purl.archive.org/oquo#TextAnalysisCharacteristic"/>
            </owl:Restriction>
        </rdfs:subClassOf>
        <rdfs:subClassOf>
            <owl:Restriction>
                <owl:onProperty rdf:resource="https://purl.archive.org/oquo#measuresCharacteristicPositively"/>
                <owl:allValuesFrom>
                    <owl:Class>
                        <owl:unionOf rdf:parseType="Collection">
                            <rdf:Description rdf:about="https://purl.archive.org/oquo#EaseOfUseCharacteristic"/>
                            <rdf:Description rdf:about="https://purl.archive.org/oquo#EfficiencyInUseCharacteristic"/>
                            <rdf:Description rdf:about="https://purl.archive.org/oquo#IndexingAndLinkingCharacteristic"/>
                            <rdf:Description rdf:about="https://purl.archive.org/oquo#KnowledgeReuseCharacteristic"/>
                            <rdf:Description rdf:about="https://purl.archive.org/oquo#TextAnalysisCharacteristic"/>
                        </owl:unionOf>
                    </owl:Class>
                </owl:allValuesFrom>
            </owl:Restriction>
        </rdfs:subClassOf>
        <rdfs:subClassOf>
            <owl:Restriction>
                <owl:onProperty rdf:resource="http://purl.org/net/QualityModel#hasScale"/>
                <owl:hasValue rdf:resource="https://purl.archive.org/oquo#SynonymsPerAnnotationPropertyMetricScale"/>
            </owl:Restriction>
        </rdfs:subClassOf>
        <obo:IAO_0000115 xml:lang="en">This metric accounts for the number of synonyms associated with annotation properties, which can also be provided by using different annotation properties used by the community to include synonyms (oboInOwl:hasExactSynonym, skos:altLabel, iao:0000118, etc.). This metric is calculated as the number of synonyms associated with annotation properties divided by the total number of annotation properties in the ontology. The range of the value of this metric is the set of real positive numbers.</obo:IAO_0000115>
        <rdf1:acronym>SxAP</rdf1:acronym>
        <rdfs:comment>The total number of annotation property synonyms over the total number of annotation properties.</rdfs:comment>
        <rdfs:label>synonyms per annotation property metric</rdfs:label>
    </owl:Class>
    


    <!-- https://purl.archive.org/oquo#SynonymsPerClassMetric -->

    <owl:Class rdf:about="https://purl.archive.org/oquo#SynonymsPerClassMetric">
        <rdfs:subClassOf rdf:resource="http://purl.org/net/QualityModel#DerivedMeasure"/>
        <rdfs:subClassOf>
            <owl:Restriction>
                <owl:onProperty rdf:resource="http://purl.org/net/QualityModel#hasScale"/>
                <owl:someValuesFrom>
                    <owl:Class>
                        <owl:intersectionOf rdf:parseType="Collection">
                            <rdf:Description rdf:about="https://purl.archive.org/oquo#RawScale"/>
                            <owl:Restriction>
                                <owl:onProperty rdf:resource="http://purl.org/net/QualityModel#hasRankigFunction"/>
                                <owl:hasValue rdf:resource="http://purl.org/net/QualityModel#HigherBest"/>
                            </owl:Restriction>
                        </owl:intersectionOf>
                    </owl:Class>
                </owl:someValuesFrom>
            </owl:Restriction>
        </rdfs:subClassOf>
        <rdfs:subClassOf>
            <owl:Restriction>
                <owl:onProperty rdf:resource="https://purl.archive.org/oquo#measuresCharacteristicPositively"/>
                <owl:someValuesFrom rdf:resource="https://purl.archive.org/oquo#EaseOfUseCharacteristic"/>
            </owl:Restriction>
        </rdfs:subClassOf>
        <rdfs:subClassOf>
            <owl:Restriction>
                <owl:onProperty rdf:resource="https://purl.archive.org/oquo#measuresCharacteristicPositively"/>
                <owl:someValuesFrom rdf:resource="https://purl.archive.org/oquo#EfficiencyInUseCharacteristic"/>
            </owl:Restriction>
        </rdfs:subClassOf>
        <rdfs:subClassOf>
            <owl:Restriction>
                <owl:onProperty rdf:resource="https://purl.archive.org/oquo#measuresCharacteristicPositively"/>
                <owl:someValuesFrom rdf:resource="https://purl.archive.org/oquo#IndexingAndLinkingCharacteristic"/>
            </owl:Restriction>
        </rdfs:subClassOf>
        <rdfs:subClassOf>
            <owl:Restriction>
                <owl:onProperty rdf:resource="https://purl.archive.org/oquo#measuresCharacteristicPositively"/>
                <owl:someValuesFrom rdf:resource="https://purl.archive.org/oquo#KnowledgeReuseCharacteristic"/>
            </owl:Restriction>
        </rdfs:subClassOf>
        <rdfs:subClassOf>
            <owl:Restriction>
                <owl:onProperty rdf:resource="https://purl.archive.org/oquo#measuresCharacteristicPositively"/>
                <owl:someValuesFrom rdf:resource="https://purl.archive.org/oquo#TextAnalysisCharacteristic"/>
            </owl:Restriction>
        </rdfs:subClassOf>
        <rdfs:subClassOf>
            <owl:Restriction>
                <owl:onProperty rdf:resource="https://purl.archive.org/oquo#measuresCharacteristicPositively"/>
                <owl:allValuesFrom>
                    <owl:Class>
                        <owl:unionOf rdf:parseType="Collection">
                            <rdf:Description rdf:about="https://purl.archive.org/oquo#EaseOfUseCharacteristic"/>
                            <rdf:Description rdf:about="https://purl.archive.org/oquo#EfficiencyInUseCharacteristic"/>
                            <rdf:Description rdf:about="https://purl.archive.org/oquo#IndexingAndLinkingCharacteristic"/>
                            <rdf:Description rdf:about="https://purl.archive.org/oquo#KnowledgeReuseCharacteristic"/>
                            <rdf:Description rdf:about="https://purl.archive.org/oquo#TextAnalysisCharacteristic"/>
                        </owl:unionOf>
                    </owl:Class>
                </owl:allValuesFrom>
            </owl:Restriction>
        </rdfs:subClassOf>
        <rdfs:subClassOf>
            <owl:Restriction>
                <owl:onProperty rdf:resource="http://purl.org/net/QualityModel#hasScale"/>
                <owl:hasValue rdf:resource="https://purl.archive.org/oquo#SynonymsPerClassMetricScale"/>
            </owl:Restriction>
        </rdfs:subClassOf>
        <obo:IAO_0000115 xml:lang="en">This metric accounts for the number of synonyms associated with classes, which can also be provided by using different annotation properties used by the community to include synonyms (oboInOwl:hasExactSynonym, skos:altLabel, iao:0000118, etc.). This metric is calculated as the number of synonyms associated with classes divided by the total number of classes in the ontology. The range of the value of this metric is the set of real positive numbers.</obo:IAO_0000115>
        <rdf1:acronym>SxC</rdf1:acronym>
        <rdfs:comment>The total number of class synonyms over the total number of classes.</rdfs:comment>
        <rdfs:label>synonyms per class metric</rdfs:label>
    </owl:Class>
    


    <!-- https://purl.archive.org/oquo#SynonymsPerDataPropertyMetric -->

    <owl:Class rdf:about="https://purl.archive.org/oquo#SynonymsPerDataPropertyMetric">
        <rdfs:subClassOf rdf:resource="http://purl.org/net/QualityModel#DerivedMeasure"/>
        <rdfs:subClassOf>
            <owl:Restriction>
                <owl:onProperty rdf:resource="http://purl.org/net/QualityModel#hasScale"/>
                <owl:someValuesFrom>
                    <owl:Class>
                        <owl:intersectionOf rdf:parseType="Collection">
                            <rdf:Description rdf:about="https://purl.archive.org/oquo#RawScale"/>
                            <owl:Restriction>
                                <owl:onProperty rdf:resource="http://purl.org/net/QualityModel#hasRankigFunction"/>
                                <owl:hasValue rdf:resource="http://purl.org/net/QualityModel#HigherBest"/>
                            </owl:Restriction>
                        </owl:intersectionOf>
                    </owl:Class>
                </owl:someValuesFrom>
            </owl:Restriction>
        </rdfs:subClassOf>
        <rdfs:subClassOf>
            <owl:Restriction>
                <owl:onProperty rdf:resource="https://purl.archive.org/oquo#measuresCharacteristicPositively"/>
                <owl:someValuesFrom rdf:resource="https://purl.archive.org/oquo#EaseOfUseCharacteristic"/>
            </owl:Restriction>
        </rdfs:subClassOf>
        <rdfs:subClassOf>
            <owl:Restriction>
                <owl:onProperty rdf:resource="https://purl.archive.org/oquo#measuresCharacteristicPositively"/>
                <owl:someValuesFrom rdf:resource="https://purl.archive.org/oquo#EfficiencyInUseCharacteristic"/>
            </owl:Restriction>
        </rdfs:subClassOf>
        <rdfs:subClassOf>
            <owl:Restriction>
                <owl:onProperty rdf:resource="https://purl.archive.org/oquo#measuresCharacteristicPositively"/>
                <owl:someValuesFrom rdf:resource="https://purl.archive.org/oquo#IndexingAndLinkingCharacteristic"/>
            </owl:Restriction>
        </rdfs:subClassOf>
        <rdfs:subClassOf>
            <owl:Restriction>
                <owl:onProperty rdf:resource="https://purl.archive.org/oquo#measuresCharacteristicPositively"/>
                <owl:someValuesFrom rdf:resource="https://purl.archive.org/oquo#KnowledgeReuseCharacteristic"/>
            </owl:Restriction>
        </rdfs:subClassOf>
        <rdfs:subClassOf>
            <owl:Restriction>
                <owl:onProperty rdf:resource="https://purl.archive.org/oquo#measuresCharacteristicPositively"/>
                <owl:someValuesFrom rdf:resource="https://purl.archive.org/oquo#TextAnalysisCharacteristic"/>
            </owl:Restriction>
        </rdfs:subClassOf>
        <rdfs:subClassOf>
            <owl:Restriction>
                <owl:onProperty rdf:resource="https://purl.archive.org/oquo#measuresCharacteristicPositively"/>
                <owl:allValuesFrom>
                    <owl:Class>
                        <owl:unionOf rdf:parseType="Collection">
                            <rdf:Description rdf:about="https://purl.archive.org/oquo#EaseOfUseCharacteristic"/>
                            <rdf:Description rdf:about="https://purl.archive.org/oquo#EfficiencyInUseCharacteristic"/>
                            <rdf:Description rdf:about="https://purl.archive.org/oquo#IndexingAndLinkingCharacteristic"/>
                            <rdf:Description rdf:about="https://purl.archive.org/oquo#KnowledgeReuseCharacteristic"/>
                            <rdf:Description rdf:about="https://purl.archive.org/oquo#TextAnalysisCharacteristic"/>
                        </owl:unionOf>
                    </owl:Class>
                </owl:allValuesFrom>
            </owl:Restriction>
        </rdfs:subClassOf>
        <rdfs:subClassOf>
            <owl:Restriction>
                <owl:onProperty rdf:resource="http://purl.org/net/QualityModel#hasScale"/>
                <owl:hasValue rdf:resource="https://purl.archive.org/oquo#SynonymsPerDataPropertyMetricScale"/>
            </owl:Restriction>
        </rdfs:subClassOf>
        <obo:IAO_0000115 xml:lang="en">This metric accounts for the number of synonyms associated with data type properties, which can also be provided by using different annotation properties used by the community to include synonyms (oboInOwl:hasExactSynonym, skos:altLabel, iao:0000118, etc.). This metric is calculated as the number of synonyms associated with data type properties divided by the total number of data type properties in the ontology. The range of the value of this metric is the set of real positive numbers.</obo:IAO_0000115>
        <rdf1:acronym>SxDP</rdf1:acronym>
        <rdfs:comment>The total number of data property synonyms over the total number of data properties.</rdfs:comment>
        <rdfs:label>synonyms per data property metric</rdfs:label>
    </owl:Class>
    


    <!-- https://purl.archive.org/oquo#SynonymsPerObjectPropertyMetric -->

    <owl:Class rdf:about="https://purl.archive.org/oquo#SynonymsPerObjectPropertyMetric">
        <rdfs:subClassOf rdf:resource="http://purl.org/net/QualityModel#DerivedMeasure"/>
        <rdfs:subClassOf>
            <owl:Restriction>
                <owl:onProperty rdf:resource="http://purl.org/net/QualityModel#hasScale"/>
                <owl:someValuesFrom>
                    <owl:Class>
                        <owl:intersectionOf rdf:parseType="Collection">
                            <rdf:Description rdf:about="https://purl.archive.org/oquo#RawScale"/>
                            <owl:Restriction>
                                <owl:onProperty rdf:resource="http://purl.org/net/QualityModel#hasRankigFunction"/>
                                <owl:hasValue rdf:resource="http://purl.org/net/QualityModel#HigherBest"/>
                            </owl:Restriction>
                        </owl:intersectionOf>
                    </owl:Class>
                </owl:someValuesFrom>
            </owl:Restriction>
        </rdfs:subClassOf>
        <rdfs:subClassOf>
            <owl:Restriction>
                <owl:onProperty rdf:resource="https://purl.archive.org/oquo#measuresCharacteristicPositively"/>
                <owl:someValuesFrom rdf:resource="https://purl.archive.org/oquo#EaseOfUseCharacteristic"/>
            </owl:Restriction>
        </rdfs:subClassOf>
        <rdfs:subClassOf>
            <owl:Restriction>
                <owl:onProperty rdf:resource="https://purl.archive.org/oquo#measuresCharacteristicPositively"/>
                <owl:someValuesFrom rdf:resource="https://purl.archive.org/oquo#EfficiencyInUseCharacteristic"/>
            </owl:Restriction>
        </rdfs:subClassOf>
        <rdfs:subClassOf>
            <owl:Restriction>
                <owl:onProperty rdf:resource="https://purl.archive.org/oquo#measuresCharacteristicPositively"/>
                <owl:someValuesFrom rdf:resource="https://purl.archive.org/oquo#IndexingAndLinkingCharacteristic"/>
            </owl:Restriction>
        </rdfs:subClassOf>
        <rdfs:subClassOf>
            <owl:Restriction>
                <owl:onProperty rdf:resource="https://purl.archive.org/oquo#measuresCharacteristicPositively"/>
                <owl:someValuesFrom rdf:resource="https://purl.archive.org/oquo#KnowledgeReuseCharacteristic"/>
            </owl:Restriction>
        </rdfs:subClassOf>
        <rdfs:subClassOf>
            <owl:Restriction>
                <owl:onProperty rdf:resource="https://purl.archive.org/oquo#measuresCharacteristicPositively"/>
                <owl:someValuesFrom rdf:resource="https://purl.archive.org/oquo#TextAnalysisCharacteristic"/>
            </owl:Restriction>
        </rdfs:subClassOf>
        <rdfs:subClassOf>
            <owl:Restriction>
                <owl:onProperty rdf:resource="https://purl.archive.org/oquo#measuresCharacteristicPositively"/>
                <owl:allValuesFrom>
                    <owl:Class>
                        <owl:unionOf rdf:parseType="Collection">
                            <rdf:Description rdf:about="https://purl.archive.org/oquo#EaseOfUseCharacteristic"/>
                            <rdf:Description rdf:about="https://purl.archive.org/oquo#EfficiencyInUseCharacteristic"/>
                            <rdf:Description rdf:about="https://purl.archive.org/oquo#IndexingAndLinkingCharacteristic"/>
                            <rdf:Description rdf:about="https://purl.archive.org/oquo#KnowledgeReuseCharacteristic"/>
                            <rdf:Description rdf:about="https://purl.archive.org/oquo#TextAnalysisCharacteristic"/>
                        </owl:unionOf>
                    </owl:Class>
                </owl:allValuesFrom>
            </owl:Restriction>
        </rdfs:subClassOf>
        <rdfs:subClassOf>
            <owl:Restriction>
                <owl:onProperty rdf:resource="http://purl.org/net/QualityModel#hasScale"/>
                <owl:hasValue rdf:resource="https://purl.archive.org/oquo#SynonymsPerObjectPropertyMetricScale"/>
            </owl:Restriction>
        </rdfs:subClassOf>
        <obo:IAO_0000115 xml:lang="en">This metric accounts for the number of synonyms associated with object properties, which can also be provided by using different annotation properties used by the community to include synonyms (oboInOwl:hasExactSynonym, skos:altLabel, iao:0000118, etc.). This metric is calculated as the number of synonyms associated with object properties divided by the total number of object properties in the ontology. The range of the value of this metric is the set of real positive numbers.</obo:IAO_0000115>
        <rdf1:acronym>SxOP</rdf1:acronym>
        <rdfs:comment>The total number of object property synonyms over the total number of object properties.</rdfs:comment>
        <rdfs:label>synonyms per object property metric</rdfs:label>
    </owl:Class>
    


    <!-- https://purl.archive.org/oquo#SynonymsPerPropertyMetric -->

    <owl:Class rdf:about="https://purl.archive.org/oquo#SynonymsPerPropertyMetric">
        <rdfs:subClassOf rdf:resource="http://purl.org/net/QualityModel#DerivedMeasure"/>
        <rdfs:subClassOf>
            <owl:Restriction>
                <owl:onProperty rdf:resource="http://purl.org/net/QualityModel#hasScale"/>
                <owl:someValuesFrom>
                    <owl:Class>
                        <owl:intersectionOf rdf:parseType="Collection">
                            <rdf:Description rdf:about="https://purl.archive.org/oquo#RawScale"/>
                            <owl:Restriction>
                                <owl:onProperty rdf:resource="http://purl.org/net/QualityModel#hasRankigFunction"/>
                                <owl:hasValue rdf:resource="http://purl.org/net/QualityModel#HigherBest"/>
                            </owl:Restriction>
                        </owl:intersectionOf>
                    </owl:Class>
                </owl:someValuesFrom>
            </owl:Restriction>
        </rdfs:subClassOf>
        <rdfs:subClassOf>
            <owl:Restriction>
                <owl:onProperty rdf:resource="https://purl.archive.org/oquo#measuresCharacteristicPositively"/>
                <owl:someValuesFrom rdf:resource="https://purl.archive.org/oquo#EaseOfUseCharacteristic"/>
            </owl:Restriction>
        </rdfs:subClassOf>
        <rdfs:subClassOf>
            <owl:Restriction>
                <owl:onProperty rdf:resource="https://purl.archive.org/oquo#measuresCharacteristicPositively"/>
                <owl:someValuesFrom rdf:resource="https://purl.archive.org/oquo#EfficiencyInUseCharacteristic"/>
            </owl:Restriction>
        </rdfs:subClassOf>
        <rdfs:subClassOf>
            <owl:Restriction>
                <owl:onProperty rdf:resource="https://purl.archive.org/oquo#measuresCharacteristicPositively"/>
                <owl:someValuesFrom rdf:resource="https://purl.archive.org/oquo#IndexingAndLinkingCharacteristic"/>
            </owl:Restriction>
        </rdfs:subClassOf>
        <rdfs:subClassOf>
            <owl:Restriction>
                <owl:onProperty rdf:resource="https://purl.archive.org/oquo#measuresCharacteristicPositively"/>
                <owl:someValuesFrom rdf:resource="https://purl.archive.org/oquo#KnowledgeReuseCharacteristic"/>
            </owl:Restriction>
        </rdfs:subClassOf>
        <rdfs:subClassOf>
            <owl:Restriction>
                <owl:onProperty rdf:resource="https://purl.archive.org/oquo#measuresCharacteristicPositively"/>
                <owl:someValuesFrom rdf:resource="https://purl.archive.org/oquo#TextAnalysisCharacteristic"/>
            </owl:Restriction>
        </rdfs:subClassOf>
        <rdfs:subClassOf>
            <owl:Restriction>
                <owl:onProperty rdf:resource="https://purl.archive.org/oquo#measuresCharacteristicPositively"/>
                <owl:allValuesFrom>
                    <owl:Class>
                        <owl:unionOf rdf:parseType="Collection">
                            <rdf:Description rdf:about="https://purl.archive.org/oquo#EaseOfUseCharacteristic"/>
                            <rdf:Description rdf:about="https://purl.archive.org/oquo#EfficiencyInUseCharacteristic"/>
                            <rdf:Description rdf:about="https://purl.archive.org/oquo#IndexingAndLinkingCharacteristic"/>
                            <rdf:Description rdf:about="https://purl.archive.org/oquo#KnowledgeReuseCharacteristic"/>
                            <rdf:Description rdf:about="https://purl.archive.org/oquo#TextAnalysisCharacteristic"/>
                        </owl:unionOf>
                    </owl:Class>
                </owl:allValuesFrom>
            </owl:Restriction>
        </rdfs:subClassOf>
        <rdfs:subClassOf>
            <owl:Restriction>
                <owl:onProperty rdf:resource="http://purl.org/net/QualityModel#hasScale"/>
                <owl:hasValue rdf:resource="https://purl.archive.org/oquo#SynonymsPerPropertyMetricScale"/>
            </owl:Restriction>
        </rdfs:subClassOf>
        <obo:IAO_0000115 xml:lang="en">This metric accounts for the number of synonyms associated with properties, which can also be provided by using different annotation properties used by the community to include synonyms (oboInOwl:hasExactSynonym, skos:altLabel, iao:0000118, etc.). This metric is calculated as the number of synonyms associated with properties (including annotation, data, and object properties) divided by the total number of properties in the ontology. The range of the value of this metric is the set of real positive numbers.</obo:IAO_0000115>
        <rdf1:acronym>SxC</rdf1:acronym>
        <rdfs:comment>The total number of property synonyms over the total number of properties, including data, object and annotation properties.</rdfs:comment>
        <rdfs:label>synonyms per property metric</rdfs:label>
    </owl:Class>
    


    <!-- https://purl.archive.org/oquo#SystematicNamingMetric -->

    <owl:Class rdf:about="https://purl.archive.org/oquo#SystematicNamingMetric">
        <rdfs:subClassOf rdf:resource="http://purl.org/net/QualityModel#DerivedMeasure"/>
        <rdfs:subClassOf>
            <owl:Restriction>
                <owl:onProperty rdf:resource="http://purl.org/net/QualityModel#hasScale"/>
                <owl:someValuesFrom>
                    <owl:Class>
                        <owl:intersectionOf rdf:parseType="Collection">
                            <rdf:Description rdf:about="https://purl.archive.org/oquo#RawScale"/>
                            <owl:Restriction>
                                <owl:onProperty rdf:resource="http://purl.org/net/QualityModel#hasRankigFunction"/>
                                <owl:hasValue rdf:resource="http://purl.org/net/QualityModel#HigherBest"/>
                            </owl:Restriction>
                        </owl:intersectionOf>
                    </owl:Class>
                </owl:someValuesFrom>
            </owl:Restriction>
        </rdfs:subClassOf>
        <rdfs:subClassOf>
            <owl:Restriction>
                <owl:onProperty rdf:resource="https://purl.archive.org/oquo#measuresCharacteristicPositively"/>
                <owl:someValuesFrom rdf:resource="https://purl.archive.org/oquo#StructuralAccuracyCharacteristic"/>
            </owl:Restriction>
        </rdfs:subClassOf>
        <rdfs:subClassOf>
            <owl:Restriction>
                <owl:onProperty rdf:resource="https://purl.archive.org/oquo#measuresCharacteristicPositively"/>
                <owl:someValuesFrom rdf:resource="https://purl.archive.org/oquo#TextAnalysisCharacteristic"/>
            </owl:Restriction>
        </rdfs:subClassOf>
        <rdfs:subClassOf>
            <owl:Restriction>
                <owl:onProperty rdf:resource="https://purl.archive.org/oquo#measuresCharacteristicPositively"/>
                <owl:allValuesFrom>
                    <owl:Class>
                        <owl:unionOf rdf:parseType="Collection">
                            <rdf:Description rdf:about="https://purl.archive.org/oquo#StructuralAccuracyCharacteristic"/>
                            <rdf:Description rdf:about="https://purl.archive.org/oquo#TextAnalysisCharacteristic"/>
                        </owl:unionOf>
                    </owl:Class>
                </owl:allValuesFrom>
            </owl:Restriction>
        </rdfs:subClassOf>
        <rdfs:subClassOf>
            <owl:Restriction>
                <owl:onProperty rdf:resource="http://purl.org/net/QualityModel#hasScale"/>
                <owl:hasValue rdf:resource="https://purl.archive.org/oquo#SystematicNamingMetricScale"/>
            </owl:Restriction>
        </rdfs:subClassOf>
        <obo:IAO_0000115 xml:lang="en">This metric is related to the ontology design principle that states that classes in the same taxonomy should share part of their name, since subclasses are specializations of the parent class. In other words, class names should follow a genus-differentia style. This metric is calculated as the ratio of subclasses of an LR class that exhibit the lexical regularity of the parent class. This requires to calculate how many subclasses of a given LR class exhibit the lexical regularity in their name (positive cases) and how many do not (negative cases). The value of the metric is calculated by dividing the positive cases by the total number of cases. It is calculated for each LR class. The final value of the metric for an ontology is calculated as the sum of all the positive cases divided by the sum of all the positive and negative cases obtained by each LR class in the ontology. The value is in the range [0, 1], the highest values representing the best values for the metric.</obo:IAO_0000115>
        <rdf1:acronym>SYSNAM</rdf1:acronym>
        <rdfs:comment>The degree in which hierarchies under LR classes exhibit the lexical regularity of the parent class.</rdfs:comment>
        <rdfs:label>systematic naming metric</rdfs:label>
    </owl:Class>
    


    <!-- https://purl.archive.org/oquo#Tangledness2Metric -->

    <owl:Class rdf:about="https://purl.archive.org/oquo#Tangledness2Metric">
        <rdfs:subClassOf rdf:resource="http://purl.org/net/QualityModel#DerivedMeasure"/>
        <rdfs:subClassOf>
            <owl:Restriction>
                <owl:onProperty rdf:resource="http://purl.org/net/QualityModel#hasScale"/>
                <owl:someValuesFrom>
                    <owl:Class>
                        <owl:intersectionOf rdf:parseType="Collection">
                            <rdf:Description rdf:about="https://purl.archive.org/oquo#RawScale"/>
                            <owl:Restriction>
                                <owl:onProperty rdf:resource="http://purl.org/net/QualityModel#hasRankigFunction"/>
                                <owl:hasValue rdf:resource="http://purl.org/net/QualityModel#LowerBest"/>
                            </owl:Restriction>
                        </owl:intersectionOf>
                    </owl:Class>
                </owl:someValuesFrom>
            </owl:Restriction>
        </rdfs:subClassOf>
        <rdfs:subClassOf>
            <owl:Restriction>
                <owl:onProperty rdf:resource="https://purl.archive.org/oquo#measuresCharacteristicPositively"/>
                <owl:someValuesFrom rdf:resource="https://purl.archive.org/oquo#DecisionTreesCharacteristic"/>
            </owl:Restriction>
        </rdfs:subClassOf>
        <rdfs:subClassOf>
            <owl:Restriction>
                <owl:onProperty rdf:resource="https://purl.archive.org/oquo#measuresCharacteristicPositively"/>
                <owl:someValuesFrom rdf:resource="https://purl.archive.org/oquo#TanglednessCharacteristic"/>
            </owl:Restriction>
        </rdfs:subClassOf>
        <rdfs:subClassOf>
            <owl:Restriction>
                <owl:onProperty rdf:resource="https://purl.archive.org/oquo#measuresCharacteristicPositively"/>
                <owl:allValuesFrom>
                    <owl:Class>
                        <owl:unionOf rdf:parseType="Collection">
                            <rdf:Description rdf:about="https://purl.archive.org/oquo#DecisionTreesCharacteristic"/>
                            <rdf:Description rdf:about="https://purl.archive.org/oquo#TanglednessCharacteristic"/>
                        </owl:unionOf>
                    </owl:Class>
                </owl:allValuesFrom>
            </owl:Restriction>
        </rdfs:subClassOf>
        <rdfs:subClassOf>
            <owl:Restriction>
                <owl:onProperty rdf:resource="http://purl.org/net/QualityModel#hasScale"/>
                <owl:hasValue rdf:resource="https://purl.archive.org/oquo#Tangledness2MetricScale"/>
            </owl:Restriction>
        </rdfs:subClassOf>
        <obo:IAO_0000115 xml:lang="en">Mean number of direct ancestor of classes with more than 1 direct ancestor. TMOnto2=∑|SUP(CDP)i|/∑|CDPi|; where Ci is the i-th class in the ontology and SUP(CDP)i is the supperclass of the thei-th class in the ontology with more than one direct parent </obo:IAO_0000115>
        <rdf1:acronym>TMOnto2</rdf1:acronym>
        <rdfs:comment>Mean number of direct ancestor of classes with more than 1 direct ancestor.</rdfs:comment>
        <rdfs:label>tangledness 2 metric</rdfs:label>
    </owl:Class>
    


    <!-- https://purl.archive.org/oquo#TanglednessCharacteristic -->

    <owl:Class rdf:about="https://purl.archive.org/oquo#TanglednessCharacteristic">
        <rdfs:subClassOf rdf:resource="http://purl.org/net/QualityModel#QualityCharacteristic"/>
        <obo:IAO_0000115 xml:lang="en">This measures the distribution of multiple parent categories, so that it is related to the existence of multiple inheritance.</obo:IAO_0000115>
        <rdfs:label>tangledness characteristic</rdfs:label>
    </owl:Class>
    


    <!-- https://purl.archive.org/oquo#TanglednessMetric -->

    <owl:Class rdf:about="https://purl.archive.org/oquo#TanglednessMetric">
        <rdfs:subClassOf rdf:resource="http://purl.org/net/QualityModel#DerivedMeasure"/>
        <rdfs:subClassOf>
            <owl:Restriction>
                <owl:onProperty rdf:resource="http://purl.org/net/QualityModel#hasScale"/>
                <owl:someValuesFrom>
                    <owl:Class>
                        <owl:intersectionOf rdf:parseType="Collection">
                            <rdf:Description rdf:about="https://purl.archive.org/oquo#RawScale"/>
                            <owl:Restriction>
                                <owl:onProperty rdf:resource="http://purl.org/net/QualityModel#hasRankigFunction"/>
                                <owl:hasValue rdf:resource="http://purl.org/net/QualityModel#LowerBest"/>
                            </owl:Restriction>
                        </owl:intersectionOf>
                    </owl:Class>
                </owl:someValuesFrom>
            </owl:Restriction>
        </rdfs:subClassOf>
        <rdfs:subClassOf>
            <owl:Restriction>
                <owl:onProperty rdf:resource="https://purl.archive.org/oquo#measuresCharacteristicPositively"/>
                <owl:someValuesFrom rdf:resource="https://purl.archive.org/oquo#DecisionTreesCharacteristic"/>
            </owl:Restriction>
        </rdfs:subClassOf>
        <rdfs:subClassOf>
            <owl:Restriction>
                <owl:onProperty rdf:resource="https://purl.archive.org/oquo#measuresCharacteristicPositively"/>
                <owl:someValuesFrom rdf:resource="https://purl.archive.org/oquo#TanglednessCharacteristic"/>
            </owl:Restriction>
        </rdfs:subClassOf>
        <rdfs:subClassOf>
            <owl:Restriction>
                <owl:onProperty rdf:resource="https://purl.archive.org/oquo#measuresCharacteristicPositively"/>
                <owl:allValuesFrom>
                    <owl:Class>
                        <owl:unionOf rdf:parseType="Collection">
                            <rdf:Description rdf:about="https://purl.archive.org/oquo#DecisionTreesCharacteristic"/>
                            <rdf:Description rdf:about="https://purl.archive.org/oquo#TanglednessCharacteristic"/>
                        </owl:unionOf>
                    </owl:Class>
                </owl:allValuesFrom>
            </owl:Restriction>
        </rdfs:subClassOf>
        <rdfs:subClassOf>
            <owl:Restriction>
                <owl:onProperty rdf:resource="http://purl.org/net/QualityModel#hasScale"/>
                <owl:hasValue rdf:resource="https://purl.archive.org/oquo#TanglednessMetricScale"/>
            </owl:Restriction>
        </rdfs:subClassOf>
        <obo:IAO_0000115 xml:lang="en">Mean number of classes with more than 1 direct ancestor TMOnto=∑|C(DP)i|/∑|Ci|-1; where Ci is the i-th class in the ontology and C(DP)i is thei-th class in the ontology with more than one direct parent </obo:IAO_0000115>
        <rdf1:acronym>TMOnto</rdf1:acronym>
        <rdfs:comment>Mean number of classes with more than 1 direct ancestor</rdfs:comment>
        <rdfs:label>tangledness metric</rdfs:label>
    </owl:Class>
    


    <!-- https://purl.archive.org/oquo#TestabilityCharacteristic -->

    <owl:Class rdf:about="https://purl.archive.org/oquo#TestabilityCharacteristic">
        <rdfs:subClassOf rdf:resource="http://purl.org/net/QualityModel#QualityCharacteristic"/>
        <obo:IAO_0000115 xml:lang="en">The degree to which the ontology modified can be validated.</obo:IAO_0000115>
        <rdfs:label>testability characteristic</rdfs:label>
    </owl:Class>
    


    <!-- https://purl.archive.org/oquo#TextAnalysisCharacteristic -->

    <owl:Class rdf:about="https://purl.archive.org/oquo#TextAnalysisCharacteristic">
        <rdfs:subClassOf rdf:resource="http://purl.org/net/QualityModel#QualityCharacteristic"/>
        <obo:IAO_0000115 xml:lang="en">Capability of the structure of the ontology to helps detecting associations between words or concepts and classifying word types.</obo:IAO_0000115>
        <rdfs:label>text analysis characteristic</rdfs:label>
    </owl:Class>
    


    <!-- https://purl.archive.org/oquo#TransferabilityCharacteristic -->

    <owl:Class rdf:about="https://purl.archive.org/oquo#TransferabilityCharacteristic">
        <rdfs:subClassOf rdf:resource="http://purl.org/net/QualityModel#QualityCharacteristic"/>
        <rdfs:subClassOf>
            <owl:Restriction>
                <owl:onProperty rdf:resource="http://purl.org/net/QualityModel#hasSubCharacteristic"/>
                <owl:someValuesFrom rdf:resource="https://purl.archive.org/oquo#AdaptabilityCharacteristic"/>
            </owl:Restriction>
        </rdfs:subClassOf>
        <rdfs:subClassOf>
            <owl:Restriction>
                <owl:onProperty rdf:resource="http://purl.org/net/QualityModel#hasSubCharacteristic"/>
                <owl:someValuesFrom rdf:resource="https://purl.archive.org/oquo#PortabilityCharacteristic"/>
            </owl:Restriction>
        </rdfs:subClassOf>
        <rdfs:subClassOf>
            <owl:Restriction>
                <owl:onProperty rdf:resource="http://purl.org/net/QualityModel#hasSubCharacteristic"/>
                <owl:allValuesFrom>
                    <owl:Class>
                        <owl:unionOf rdf:parseType="Collection">
                            <rdf:Description rdf:about="https://purl.archive.org/oquo#AdaptabilityCharacteristic"/>
                            <rdf:Description rdf:about="https://purl.archive.org/oquo#PortabilityCharacteristic"/>
                        </owl:unionOf>
                    </owl:Class>
                </owl:allValuesFrom>
            </owl:Restriction>
        </rdfs:subClassOf>
        <obo:IAO_0000115 xml:lang="en">The degree to which the software product can be transferred from one environment to another.</obo:IAO_0000115>
        <rdfs:label>transferability characteristic</rdfs:label>
    </owl:Class>
    


    <!-- https://purl.archive.org/oquo#TrivialIssue -->

    <owl:Class rdf:about="https://purl.archive.org/oquo#TrivialIssue">
        <rdfs:subClassOf rdf:resource="http://purl.org/ipo/core#Issue"/>
        <rdfs:comment>The defect does not affect functionality or data. It does not even need a workaround. It does not impact productivity or efficiency. It is merely an inconvenience.</rdfs:comment>
        <rdfs:label>trivial issue</rdfs:label>
    </owl:Class>
    


    <!-- https://purl.archive.org/oquo#UsabilityInUseCharacteristic -->

    <owl:Class rdf:about="https://purl.archive.org/oquo#UsabilityInUseCharacteristic">
        <rdfs:subClassOf rdf:resource="http://purl.org/net/QualityModel#QualityCharacteristic"/>
        <rdfs:subClassOf>
            <owl:Restriction>
                <owl:onProperty rdf:resource="http://purl.org/net/QualityModel#hasSubCharacteristic"/>
                <owl:someValuesFrom rdf:resource="https://purl.archive.org/oquo#EffectivenessInUseCharacteristic"/>
            </owl:Restriction>
        </rdfs:subClassOf>
        <rdfs:subClassOf>
            <owl:Restriction>
                <owl:onProperty rdf:resource="http://purl.org/net/QualityModel#hasSubCharacteristic"/>
                <owl:someValuesFrom rdf:resource="https://purl.archive.org/oquo#EfficiencyInUseCharacteristic"/>
            </owl:Restriction>
        </rdfs:subClassOf>
        <rdfs:subClassOf>
            <owl:Restriction>
                <owl:onProperty rdf:resource="http://purl.org/net/QualityModel#hasSubCharacteristic"/>
                <owl:someValuesFrom rdf:resource="https://purl.archive.org/oquo#SatisfactionInUseCharacteristic"/>
            </owl:Restriction>
        </rdfs:subClassOf>
        <rdfs:subClassOf>
            <owl:Restriction>
                <owl:onProperty rdf:resource="http://purl.org/net/QualityModel#hasSubCharacteristic"/>
                <owl:allValuesFrom>
                    <owl:Class>
                        <owl:unionOf rdf:parseType="Collection">
                            <rdf:Description rdf:about="https://purl.archive.org/oquo#EffectivenessInUseCharacteristic"/>
                            <rdf:Description rdf:about="https://purl.archive.org/oquo#EfficiencyInUseCharacteristic"/>
                            <rdf:Description rdf:about="https://purl.archive.org/oquo#SatisfactionInUseCharacteristic"/>
                        </owl:unionOf>
                    </owl:Class>
                </owl:allValuesFrom>
            </owl:Restriction>
        </rdfs:subClassOf>
        <rdfs:label>usability in use characteristic</rdfs:label>
    </owl:Class>
    


    <!-- https://purl.archive.org/oquo#WeigthMethodPerClass2Metric -->

    <owl:Class rdf:about="https://purl.archive.org/oquo#WeigthMethodPerClass2Metric">
        <rdfs:subClassOf rdf:resource="http://purl.org/net/QualityModel#DerivedMeasure"/>
        <rdfs:subClassOf>
            <owl:Restriction>
                <owl:onProperty rdf:resource="http://purl.org/net/QualityModel#hasScale"/>
                <owl:someValuesFrom>
                    <owl:Class>
                        <owl:intersectionOf rdf:parseType="Collection">
                            <rdf:Description rdf:about="https://purl.archive.org/oquo#RawScale"/>
                            <owl:Restriction>
                                <owl:onProperty rdf:resource="http://purl.org/net/QualityModel#hasRankigFunction"/>
                                <owl:hasValue rdf:resource="http://purl.org/net/QualityModel#LowerBest"/>
                            </owl:Restriction>
                        </owl:intersectionOf>
                    </owl:Class>
                </owl:someValuesFrom>
            </owl:Restriction>
        </rdfs:subClassOf>
        <rdfs:subClassOf>
            <owl:Restriction>
                <owl:onProperty rdf:resource="http://purl.org/net/QualityModel#hasScale"/>
                <owl:hasValue rdf:resource="https://purl.archive.org/oquo#WeigthMethodPerClass2MetricScale"/>
            </owl:Restriction>
        </rdfs:subClassOf>
        <obo:IAO_0000115 xml:lang="en">Mean number of path from Thing to a leaf class per leaf class WMCOnto2=∑path(|C(leaf)i|)/∑|C(leaf)i| , where path|C(leaf)i| is the number of the path from the leaf class i to Thing </obo:IAO_0000115>
        <rdf1:acronym>WMCOnto2</rdf1:acronym>
        <rdfs:comment>Mean number of path from Thing to a leaf class per leaf class.</rdfs:comment>
        <rdfs:label>weigth method per class 2 metric</rdfs:label>
    </owl:Class>
    


    <!-- https://purl.archive.org/oquo#WeigthMethodPerClassMetric -->

    <owl:Class rdf:about="https://purl.archive.org/oquo#WeigthMethodPerClassMetric">
        <rdfs:subClassOf rdf:resource="http://purl.org/net/QualityModel#DerivedMeasure"/>
        <rdfs:subClassOf>
            <owl:Class>
                <owl:intersectionOf rdf:parseType="Collection">
                    <owl:Restriction>
                        <owl:onProperty rdf:resource="https://purl.archive.org/oquo#measuresCharacteristicNegatively"/>
                        <owl:allValuesFrom rdf:resource="https://purl.archive.org/oquo#RecoverabilityCharacteristic"/>
                    </owl:Restriction>
                    <owl:Restriction>
                        <owl:onProperty rdf:resource="https://purl.archive.org/oquo#measuresCharacteristicPositively"/>
                        <owl:allValuesFrom>
                            <owl:Class>
                                <owl:unionOf rdf:parseType="Collection">
                                    <rdf:Description rdf:about="https://purl.archive.org/oquo#AdaptabilityCharacteristic"/>
                                    <rdf:Description rdf:about="https://purl.archive.org/oquo#AnalysabilityCharacteristic"/>
                                    <rdf:Description rdf:about="https://purl.archive.org/oquo#ChangeabilityCharacteristic"/>
                                    <rdf:Description rdf:about="https://purl.archive.org/oquo#LearnabilityCharacteristic"/>
                                    <rdf:Description rdf:about="https://purl.archive.org/oquo#ModificationStabilityCharacteristic"/>
                                    <rdf:Description rdf:about="https://purl.archive.org/oquo#ModularityCharacteristic"/>
                                    <rdf:Description rdf:about="https://purl.archive.org/oquo#ReplaceabilityCharacteristic"/>
                                    <rdf:Description rdf:about="https://purl.archive.org/oquo#ReusabilityCharacteristic"/>
                                    <rdf:Description rdf:about="https://purl.archive.org/oquo#TestabilityCharacteristic"/>
                                </owl:unionOf>
                            </owl:Class>
                        </owl:allValuesFrom>
                    </owl:Restriction>
                </owl:intersectionOf>
            </owl:Class>
        </rdfs:subClassOf>
        <rdfs:subClassOf>
            <owl:Restriction>
                <owl:onProperty rdf:resource="http://purl.org/net/QualityModel#hasScale"/>
                <owl:someValuesFrom>
                    <owl:Class>
                        <owl:intersectionOf rdf:parseType="Collection">
                            <rdf:Description rdf:about="https://purl.archive.org/oquo#RawScale"/>
                            <owl:Restriction>
                                <owl:onProperty rdf:resource="http://purl.org/net/QualityModel#hasRankigFunction"/>
                                <owl:hasValue rdf:resource="http://purl.org/net/QualityModel#LowerBest"/>
                            </owl:Restriction>
                        </owl:intersectionOf>
                    </owl:Class>
                </owl:someValuesFrom>
            </owl:Restriction>
        </rdfs:subClassOf>
        <rdfs:subClassOf>
            <owl:Restriction>
                <owl:onProperty rdf:resource="https://purl.archive.org/oquo#measuresCharacteristicNegatively"/>
                <owl:someValuesFrom rdf:resource="https://purl.archive.org/oquo#RecoverabilityCharacteristic"/>
            </owl:Restriction>
        </rdfs:subClassOf>
        <rdfs:subClassOf>
            <owl:Restriction>
                <owl:onProperty rdf:resource="https://purl.archive.org/oquo#measuresCharacteristicPositively"/>
                <owl:someValuesFrom rdf:resource="https://purl.archive.org/oquo#AdaptabilityCharacteristic"/>
            </owl:Restriction>
        </rdfs:subClassOf>
        <rdfs:subClassOf>
            <owl:Restriction>
                <owl:onProperty rdf:resource="https://purl.archive.org/oquo#measuresCharacteristicPositively"/>
                <owl:someValuesFrom rdf:resource="https://purl.archive.org/oquo#AnalysabilityCharacteristic"/>
            </owl:Restriction>
        </rdfs:subClassOf>
        <rdfs:subClassOf>
            <owl:Restriction>
                <owl:onProperty rdf:resource="https://purl.archive.org/oquo#measuresCharacteristicPositively"/>
                <owl:someValuesFrom rdf:resource="https://purl.archive.org/oquo#ChangeabilityCharacteristic"/>
            </owl:Restriction>
        </rdfs:subClassOf>
        <rdfs:subClassOf>
            <owl:Restriction>
                <owl:onProperty rdf:resource="https://purl.archive.org/oquo#measuresCharacteristicPositively"/>
                <owl:someValuesFrom rdf:resource="https://purl.archive.org/oquo#LearnabilityCharacteristic"/>
            </owl:Restriction>
        </rdfs:subClassOf>
        <rdfs:subClassOf>
            <owl:Restriction>
                <owl:onProperty rdf:resource="https://purl.archive.org/oquo#measuresCharacteristicPositively"/>
                <owl:someValuesFrom rdf:resource="https://purl.archive.org/oquo#ModificationStabilityCharacteristic"/>
            </owl:Restriction>
        </rdfs:subClassOf>
        <rdfs:subClassOf>
            <owl:Restriction>
                <owl:onProperty rdf:resource="https://purl.archive.org/oquo#measuresCharacteristicPositively"/>
                <owl:someValuesFrom rdf:resource="https://purl.archive.org/oquo#ModularityCharacteristic"/>
            </owl:Restriction>
        </rdfs:subClassOf>
        <rdfs:subClassOf>
            <owl:Restriction>
                <owl:onProperty rdf:resource="https://purl.archive.org/oquo#measuresCharacteristicPositively"/>
                <owl:someValuesFrom rdf:resource="https://purl.archive.org/oquo#ReplaceabilityCharacteristic"/>
            </owl:Restriction>
        </rdfs:subClassOf>
        <rdfs:subClassOf>
            <owl:Restriction>
                <owl:onProperty rdf:resource="https://purl.archive.org/oquo#measuresCharacteristicPositively"/>
                <owl:someValuesFrom rdf:resource="https://purl.archive.org/oquo#ReusabilityCharacteristic"/>
            </owl:Restriction>
        </rdfs:subClassOf>
        <rdfs:subClassOf>
            <owl:Restriction>
                <owl:onProperty rdf:resource="https://purl.archive.org/oquo#measuresCharacteristicPositively"/>
                <owl:someValuesFrom rdf:resource="https://purl.archive.org/oquo#TestabilityCharacteristic"/>
            </owl:Restriction>
        </rdfs:subClassOf>
        <rdfs:subClassOf>
            <owl:Restriction>
                <owl:onProperty rdf:resource="http://purl.org/net/QualityModel#hasScale"/>
                <owl:hasValue rdf:resource="https://purl.archive.org/oquo#WeigthMethodPerClassMetricScale"/>
            </owl:Restriction>
        </rdfs:subClassOf>
        <obo:IAO_0000115 xml:lang="en">Mean length of the path from Thing to a leaf class WMCOnto=∑Lenght(path(|C(leaf)i|))/∑|C(leaf)i|, where Lenght(path|C(leaf)i|) is the length of the path from the leaf class i to Thing </obo:IAO_0000115>
        <rdf1:acronym>WMCOnto</rdf1:acronym>
        <rdfs:comment>Mean length of the path from Thing to a leaf class.</rdfs:comment>
        <rdfs:label>weigth method per class metric</rdfs:label>
    </owl:Class>
    


    <!-- 
    ///////////////////////////////////////////////////////////////////////////////////////
    //
    // Individuals
    //
    ///////////////////////////////////////////////////////////////////////////////////////
     -->

    


    <!-- http://purl.org/net/QualityModel#HigherBest -->

    <owl:Thing rdf:about="http://purl.org/net/QualityModel#HigherBest">
        <rdf:type rdf:resource="http://www.w3.org/2002/07/owl#NamedIndividual"/>
        <rdf:type rdf:resource="http://purl.org/net/QualityModel#RankingFunction"/>
        <rdfs:comment>A ranking function that denotes that a higher value is better.</rdfs:comment>
        <rdfs:label>HigherBest</rdfs:label>
    </owl:Thing>
    


    <!-- http://purl.org/net/QualityModel#LowerBest -->

    <owl:Thing rdf:about="http://purl.org/net/QualityModel#LowerBest">
        <rdf:type rdf:resource="http://www.w3.org/2002/07/owl#NamedIndividual"/>
        <rdf:type rdf:resource="http://purl.org/net/QualityModel#RankingFunction"/>
        <rdfs:comment>A ranking function that denotes that a lower value is better.</rdfs:comment>
        <rdfs:label>LowerBest</rdfs:label>
    </owl:Thing>
    


    <!-- https://purl.archive.org/oquo#AncestorsPerClassMetricScale -->

    <owl:NamedIndividual rdf:about="https://purl.archive.org/oquo#AncestorsPerClassMetricScale">
        <rdf:type rdf:resource="http://www.wurvoc.org/vocabularies/om-1.8/Ratio_scale"/>
        <rdf:type rdf:resource="https://purl.archive.org/oquo#RawScale"/>
        <QualityModel:hasRankigFunction rdf:resource="http://purl.org/net/QualityModel#HigherBest"/>
        <obo:IAO_0000115>Mean number of direct ancestor per class</obo:IAO_0000115>
        <rdfs:label>ancestors per class metric scale</rdfs:label>
    </owl:NamedIndividual>
    


    <!-- https://purl.archive.org/oquo#AnnotationPropertiesWithNoDescriptionMetricScale -->

    <owl:NamedIndividual rdf:about="https://purl.archive.org/oquo#AnnotationPropertiesWithNoDescriptionMetricScale">
        <rdf:type rdf:resource="http://www.wurvoc.org/vocabularies/om-1.8/Ratio_scale"/>
        <rdf:type rdf:resource="https://purl.archive.org/oquo#RawScale"/>
        <QualityModel:hasRankigFunction rdf:resource="http://purl.org/net/QualityModel#LowerBest"/>
        <obo:IAO_0000115>The number of annotation properties lacking a description over the number of the annotation properties considered.</obo:IAO_0000115>
        <rdfs:label>annotation properties with no description metric scale</rdfs:label>
    </owl:NamedIndividual>
    


    <!-- https://purl.archive.org/oquo#AnnotationPropertiesWithNoNameMetricScale -->

    <owl:NamedIndividual rdf:about="https://purl.archive.org/oquo#AnnotationPropertiesWithNoNameMetricScale">
        <rdf:type rdf:resource="http://www.wurvoc.org/vocabularies/om-1.8/Ratio_scale"/>
        <rdf:type rdf:resource="https://purl.archive.org/oquo#RawScale"/>
        <QualityModel:hasRankigFunction rdf:resource="http://purl.org/net/QualityModel#LowerBest"/>
        <obo:IAO_0000115>The numberof annotation properties lacking a name over the number of annotation properties considered.</obo:IAO_0000115>
        <rdfs:label>annotation properties with no name metric scale</rdfs:label>
    </owl:NamedIndividual>
    


    <!-- https://purl.archive.org/oquo#AnnotationPropertiesWithNoSynonymMetricScale -->

    <owl:NamedIndividual rdf:about="https://purl.archive.org/oquo#AnnotationPropertiesWithNoSynonymMetricScale">
        <rdf:type rdf:resource="http://www.wurvoc.org/vocabularies/om-1.8/Ratio_scale"/>
        <rdf:type rdf:resource="https://purl.archive.org/oquo#RawScale"/>
        <QualityModel:hasRankigFunction rdf:resource="http://purl.org/net/QualityModel#LowerBest"/>
        <obo:IAO_0000115>The number of annotation properties lacking synonyms over the annotation properties considered.</obo:IAO_0000115>
        <rdfs:label>annotation properties with no synonym metric scale</rdfs:label>
    </owl:NamedIndividual>
    


    <!-- https://purl.archive.org/oquo#AnnotationRichnessMetricScale -->

    <owl:NamedIndividual rdf:about="https://purl.archive.org/oquo#AnnotationRichnessMetricScale">
        <rdf:type rdf:resource="http://www.wurvoc.org/vocabularies/om-1.8/Ratio_scale"/>
        <rdf:type rdf:resource="https://purl.archive.org/oquo#RawScale"/>
        <QualityModel:hasRankigFunction rdf:resource="http://purl.org/net/QualityModel#HigherBest"/>
        <obo:IAO_0000115>Mean number of annotation properties per class.</obo:IAO_0000115>
        <rdfs:label>annotation richness metric scale</rdfs:label>
    </owl:NamedIndividual>
    


    <!-- https://purl.archive.org/oquo#AttributeRichnessMetricScale -->

    <owl:NamedIndividual rdf:about="https://purl.archive.org/oquo#AttributeRichnessMetricScale">
        <rdf:type rdf:resource="http://www.wurvoc.org/vocabularies/om-1.8/Ratio_scale"/>
        <rdf:type rdf:resource="https://purl.archive.org/oquo#RawScale"/>
        <QualityModel:hasRankigFunction rdf:resource="http://purl.org/net/QualityModel#HigherBest"/>
        <obo:IAO_0000115>Number of restrictions of the ontology per classes.</obo:IAO_0000115>
        <rdfs:label>attribute richness metric scale</rdfs:label>
    </owl:NamedIndividual>
    


    <!-- https://purl.archive.org/oquo#ClassRichnessMetricScale -->

    <owl:NamedIndividual rdf:about="https://purl.archive.org/oquo#ClassRichnessMetricScale">
        <rdf:type rdf:resource="http://www.wurvoc.org/vocabularies/om-1.8/Ratio_scale"/>
        <rdf:type rdf:resource="https://purl.archive.org/oquo#RawScale"/>
        <QualityModel:hasRankigFunction rdf:resource="http://purl.org/net/QualityModel#HigherBest"/>
        <obo:IAO_0000115>Mean number of individuals per class.</obo:IAO_0000115>
        <rdfs:label>class richness metric scale</rdfs:label>
    </owl:NamedIndividual>
    


    <!-- https://purl.archive.org/oquo#ClassesWithNoDescriptionMetricScale -->

    <owl:NamedIndividual rdf:about="https://purl.archive.org/oquo#ClassesWithNoDescriptionMetricScale">
        <rdf:type rdf:resource="http://www.wurvoc.org/vocabularies/om-1.8/Ratio_scale"/>
        <rdf:type rdf:resource="https://purl.archive.org/oquo#RawScale"/>
        <QualityModel:hasRankigFunction rdf:resource="http://purl.org/net/QualityModel#LowerBest"/>
        <obo:IAO_0000115>The number of classes lacking a description over the number of classes considered.</obo:IAO_0000115>
        <rdfs:label>classes with no description metric scale</rdfs:label>
    </owl:NamedIndividual>
    


    <!-- https://purl.archive.org/oquo#ClassesWithNoNameMetricScale -->

    <owl:NamedIndividual rdf:about="https://purl.archive.org/oquo#ClassesWithNoNameMetricScale">
        <rdf:type rdf:resource="http://www.wurvoc.org/vocabularies/om-1.8/Ratio_scale"/>
        <rdf:type rdf:resource="https://purl.archive.org/oquo#RawScale"/>
        <QualityModel:hasRankigFunction rdf:resource="http://purl.org/net/QualityModel#LowerBest"/>
        <obo:IAO_0000115>The number of classes lacking a name over the number of classes considered.</obo:IAO_0000115>
        <rdfs:label>classes with no name metric scale</rdfs:label>
    </owl:NamedIndividual>
    


    <!-- https://purl.archive.org/oquo#ClassesWithNoSynonymMetricScale -->

    <owl:NamedIndividual rdf:about="https://purl.archive.org/oquo#ClassesWithNoSynonymMetricScale">
        <rdf:type rdf:resource="http://www.wurvoc.org/vocabularies/om-1.8/Ratio_scale"/>
        <rdf:type rdf:resource="https://purl.archive.org/oquo#RawScale"/>
        <QualityModel:hasRankigFunction rdf:resource="http://purl.org/net/QualityModel#LowerBest"/>
        <obo:IAO_0000115>The number of classes lacking synonyms over the number of classes considered.</obo:IAO_0000115>
        <rdfs:label>classes with no synonym metric scale</rdfs:label>
    </owl:NamedIndividual>
    


    <!-- https://purl.archive.org/oquo#CouplingBetweenObjectsMetricScale -->

    <owl:NamedIndividual rdf:about="https://purl.archive.org/oquo#CouplingBetweenObjectsMetricScale">
        <rdf:type rdf:resource="http://www.wurvoc.org/vocabularies/om-1.8/Ratio_scale"/>
        <rdf:type rdf:resource="https://purl.archive.org/oquo#RawScale"/>
        <QualityModel:hasRankigFunction rdf:resource="http://purl.org/net/QualityModel#LowerBest"/>
        <obo:IAO_0000115>Number of related classes. Number of direct ancestor of classes divided by the number of classes minus subclasses of Thing.</obo:IAO_0000115>
        <rdfs:label>coupling between objects metric scale</rdfs:label>
    </owl:NamedIndividual>
    


    <!-- https://purl.archive.org/oquo#DataPropertiesWithNoDescriptionMetricScale -->

    <owl:NamedIndividual rdf:about="https://purl.archive.org/oquo#DataPropertiesWithNoDescriptionMetricScale">
        <rdf:type rdf:resource="http://www.wurvoc.org/vocabularies/om-1.8/Ratio_scale"/>
        <rdf:type rdf:resource="https://purl.archive.org/oquo#RawScale"/>
        <QualityModel:hasRankigFunction rdf:resource="http://purl.org/net/QualityModel#LowerBest"/>
        <obo:IAO_0000115>The number of data properties lacking a description over the number of data properties considered.</obo:IAO_0000115>
        <rdfs:label>data properties with no description metric scale</rdfs:label>
    </owl:NamedIndividual>
    


    <!-- https://purl.archive.org/oquo#DataPropertiesWithNoNameMetricScale -->

    <owl:NamedIndividual rdf:about="https://purl.archive.org/oquo#DataPropertiesWithNoNameMetricScale">
        <rdf:type rdf:resource="http://www.wurvoc.org/vocabularies/om-1.8/Ratio_scale"/>
        <rdf:type rdf:resource="https://purl.archive.org/oquo#RawScale"/>
        <QualityModel:hasRankigFunction rdf:resource="http://purl.org/net/QualityModel#LowerBest"/>
        <obo:IAO_0000115>The number of data properties lacking a name over the number of data properties considered.</obo:IAO_0000115>
        <rdfs:label>data properties with no name metric scale</rdfs:label>
    </owl:NamedIndividual>
    


    <!-- https://purl.archive.org/oquo#DataPropertiesWithNoSynonymMetricScale -->

    <owl:NamedIndividual rdf:about="https://purl.archive.org/oquo#DataPropertiesWithNoSynonymMetricScale">
        <rdf:type rdf:resource="http://www.wurvoc.org/vocabularies/om-1.8/Ratio_scale"/>
        <rdf:type rdf:resource="https://purl.archive.org/oquo#RawScale"/>
        <QualityModel:hasRankigFunction rdf:resource="http://purl.org/net/QualityModel#LowerBest"/>
        <obo:IAO_0000115>The number of data properties lacking synonyms over the number of data properties considered.</obo:IAO_0000115>
        <rdfs:label>data properties with no synonym metric scale</rdfs:label>
    </owl:NamedIndividual>
    


    <!-- https://purl.archive.org/oquo#DepthOfSubsumptionHierarchyMetricScale -->

    <owl:NamedIndividual rdf:about="https://purl.archive.org/oquo#DepthOfSubsumptionHierarchyMetricScale">
        <rdf:type rdf:resource="http://www.wurvoc.org/vocabularies/om-1.8/Ratio_scale"/>
        <rdf:type rdf:resource="https://purl.archive.org/oquo#RawScale"/>
        <QualityModel:hasRankigFunction rdf:resource="http://purl.org/net/QualityModel#LowerBest"/>
        <obo:IAO_0000115>Length of the largest path from Thing to a leaf class.</obo:IAO_0000115>
        <rdfs:label>depth of subsumption hierarchy metric scale</rdfs:label>
    </owl:NamedIndividual>
    


    <!-- https://purl.archive.org/oquo#DescriptionsPerAnnotationPropertyMetricScale -->

    <owl:NamedIndividual rdf:about="https://purl.archive.org/oquo#DescriptionsPerAnnotationPropertyMetricScale">
        <rdf:type rdf:resource="http://www.wurvoc.org/vocabularies/om-1.8/Ratio_scale"/>
        <rdf:type rdf:resource="https://purl.archive.org/oquo#RawScale"/>
        <QualityModel:hasRankigFunction rdf:resource="http://purl.org/net/QualityModel#HigherBest"/>
        <obo:IAO_0000115>The total number of annotation property descriptions over the total number of annotation properties.</obo:IAO_0000115>
        <rdfs:label>descriptions per annotation property metric scale</rdfs:label>
    </owl:NamedIndividual>
    


    <!-- https://purl.archive.org/oquo#DescriptionsPerClassMetricScale -->

    <owl:NamedIndividual rdf:about="https://purl.archive.org/oquo#DescriptionsPerClassMetricScale">
        <rdf:type rdf:resource="http://www.wurvoc.org/vocabularies/om-1.8/Ratio_scale"/>
        <rdf:type rdf:resource="https://purl.archive.org/oquo#RawScale"/>
        <QualityModel:hasRankigFunction rdf:resource="http://purl.org/net/QualityModel#HigherBest"/>
        <obo:IAO_0000115>The total number of class descriptions over the total number of classes.</obo:IAO_0000115>
        <rdfs:label>descriptions per class metric scale</rdfs:label>
    </owl:NamedIndividual>
    


    <!-- https://purl.archive.org/oquo#DescriptionsPerDataPropertyMetricScale -->

    <owl:NamedIndividual rdf:about="https://purl.archive.org/oquo#DescriptionsPerDataPropertyMetricScale">
        <rdf:type rdf:resource="http://www.wurvoc.org/vocabularies/om-1.8/Ratio_scale"/>
        <rdf:type rdf:resource="https://purl.archive.org/oquo#RawScale"/>
        <QualityModel:hasRankigFunction rdf:resource="http://purl.org/net/QualityModel#HigherBest"/>
        <obo:IAO_0000115>The total number of data property descriptions over the total number of data properties.</obo:IAO_0000115>
        <rdfs:label>descriptions per data property metric scale</rdfs:label>
    </owl:NamedIndividual>
    


    <!-- https://purl.archive.org/oquo#DescriptionsPerObjectPropertyMetricScale -->

    <owl:NamedIndividual rdf:about="https://purl.archive.org/oquo#DescriptionsPerObjectPropertyMetricScale">
        <rdf:type rdf:resource="http://www.wurvoc.org/vocabularies/om-1.8/Ratio_scale"/>
        <rdf:type rdf:resource="https://purl.archive.org/oquo#RawScale"/>
        <QualityModel:hasRankigFunction rdf:resource="http://purl.org/net/QualityModel#HigherBest"/>
        <obo:IAO_0000115>The total number of object property descriptions over the total number of object properties.</obo:IAO_0000115>
        <rdfs:label>descriptions per object property metric scale</rdfs:label>
    </owl:NamedIndividual>
    


    <!-- https://purl.archive.org/oquo#DescriptionsPerPropertyMetricScale -->

    <owl:NamedIndividual rdf:about="https://purl.archive.org/oquo#DescriptionsPerPropertyMetricScale">
        <rdf:type rdf:resource="http://www.wurvoc.org/vocabularies/om-1.8/Ratio_scale"/>
        <rdf:type rdf:resource="https://purl.archive.org/oquo#RawScale"/>
        <QualityModel:hasRankigFunction rdf:resource="http://purl.org/net/QualityModel#HigherBest"/>
        <obo:IAO_0000115>The total property descriptions over the total number of properties.</obo:IAO_0000115>
        <rdfs:label>descriptions per property metric scale</rdfs:label>
    </owl:NamedIndividual>
    


    <!-- https://purl.archive.org/oquo#LackOfCohesionInMethodsMetricScale -->

    <owl:NamedIndividual rdf:about="https://purl.archive.org/oquo#LackOfCohesionInMethodsMetricScale">
        <rdf:type rdf:resource="http://www.wurvoc.org/vocabularies/om-1.8/Ratio_scale"/>
        <rdf:type rdf:resource="https://purl.archive.org/oquo#RawScale"/>
        <QualityModel:hasRankigFunction rdf:resource="http://purl.org/net/QualityModel#LowerBest"/>
        <obo:IAO_0000115>Semantic and conceptual relatedness of classes.</obo:IAO_0000115>
        <rdfs:label>lack of cohesion in methods metric scale</rdfs:label>
    </owl:NamedIndividual>
    


    <!-- https://purl.archive.org/oquo#LexicalRegularitiesPerClassMetricScale -->

    <owl:NamedIndividual rdf:about="https://purl.archive.org/oquo#LexicalRegularitiesPerClassMetricScale">
        <rdf:type rdf:resource="http://www.wurvoc.org/vocabularies/om-1.8/Ratio_scale"/>
        <rdf:type rdf:resource="https://purl.archive.org/oquo#RawScale"/>
        <QualityModel:hasRankigFunction rdf:resource="http://purl.org/net/QualityModel#HigherBest"/>
        <obo:IAO_0000115>The number of lexical regularities appearing in the ontology over the number of classes.</obo:IAO_0000115>
        <rdfs:label>lexical regularities per class metric scale</rdfs:label>
    </owl:NamedIndividual>
    


    <!-- https://purl.archive.org/oquo#LexicalRegularityClassPercentageMetricScale -->

    <owl:NamedIndividual rdf:about="https://purl.archive.org/oquo#LexicalRegularityClassPercentageMetricScale">
        <rdf:type rdf:resource="http://www.wurvoc.org/vocabularies/om-1.8/Ratio_scale"/>
        <rdf:type rdf:resource="https://purl.archive.org/oquo#RawScale"/>
        <QualityModel:hasRankigFunction rdf:resource="http://purl.org/net/QualityModel#HigherBest"/>
        <obo:IAO_0000115>The percentage of classes in the ontology that are LR classes.</obo:IAO_0000115>
        <rdfs:label>lexical resularity class percentage metric scale</rdfs:label>
    </owl:NamedIndividual>
    


    <!-- https://purl.archive.org/oquo#LexicallySuggestLogicallyDefineMetricScale -->

    <owl:NamedIndividual rdf:about="https://purl.archive.org/oquo#LexicallySuggestLogicallyDefineMetricScale">
        <rdf:type rdf:resource="http://www.wurvoc.org/vocabularies/om-1.8/Ratio_scale"/>
        <rdf:type rdf:resource="https://purl.archive.org/oquo#RawScale"/>
        <QualityModel:hasRankigFunction rdf:resource="http://purl.org/net/QualityModel#HigherBest"/>
        <obo:IAO_0000115>The degree in which LR classes are semantically linked to the classes exhibiting the corresponding lexical regularity.</obo:IAO_0000115>
        <rdfs:label>lexically suggest logically define metric scale</rdfs:label>
    </owl:NamedIndividual>
    


    <!-- https://purl.archive.org/oquo#NamesPerAnnotationPropertyMetricScale -->

    <owl:NamedIndividual rdf:about="https://purl.archive.org/oquo#NamesPerAnnotationPropertyMetricScale">
        <rdf:type rdf:resource="http://www.wurvoc.org/vocabularies/om-1.8/Ratio_scale"/>
        <rdf:type rdf:resource="https://purl.archive.org/oquo#RawScale"/>
        <QualityModel:hasRankigFunction rdf:resource="http://purl.org/net/QualityModel#HigherBest"/>
        <obo:IAO_0000115>The total number of annotation property names over the total number of annotation properties.</obo:IAO_0000115>
        <rdfs:label>names per annotation property metrics scale</rdfs:label>
    </owl:NamedIndividual>
    


    <!-- https://purl.archive.org/oquo#NamesPerClassMetricScale -->

    <owl:NamedIndividual rdf:about="https://purl.archive.org/oquo#NamesPerClassMetricScale">
        <rdf:type rdf:resource="http://www.wurvoc.org/vocabularies/om-1.8/Ratio_scale"/>
        <rdf:type rdf:resource="https://purl.archive.org/oquo#RawScale"/>
        <QualityModel:hasRankigFunction rdf:resource="http://purl.org/net/QualityModel#HigherBest"/>
        <obo:IAO_0000115>The total number of class names over the total number of classes.</obo:IAO_0000115>
        <rdfs:label>names per class metric scale</rdfs:label>
    </owl:NamedIndividual>
    


    <!-- https://purl.archive.org/oquo#NamesPerDataPropertyMetricScale -->

    <owl:NamedIndividual rdf:about="https://purl.archive.org/oquo#NamesPerDataPropertyMetricScale">
        <rdf:type rdf:resource="http://www.wurvoc.org/vocabularies/om-1.8/Ratio_scale"/>
        <rdf:type rdf:resource="https://purl.archive.org/oquo#RawScale"/>
        <QualityModel:hasRankigFunction rdf:resource="http://purl.org/net/QualityModel#HigherBest"/>
        <obo:IAO_0000115>The total number of data property names over the total number of data properties.</obo:IAO_0000115>
        <rdfs:label>names per data property metric scale</rdfs:label>
    </owl:NamedIndividual>
    


    <!-- https://purl.archive.org/oquo#NamesPerObjectPropertyMetricScale -->

    <owl:NamedIndividual rdf:about="https://purl.archive.org/oquo#NamesPerObjectPropertyMetricScale">
        <rdf:type rdf:resource="http://www.wurvoc.org/vocabularies/om-1.8/Ratio_scale"/>
        <rdf:type rdf:resource="https://purl.archive.org/oquo#RawScale"/>
        <QualityModel:hasRankigFunction rdf:resource="http://purl.org/net/QualityModel#HigherBest"/>
        <obo:IAO_0000115>The total number of object property names over the total number of object properties.</obo:IAO_0000115>
        <rdfs:label>names per object property metric scale</rdfs:label>
    </owl:NamedIndividual>
    


    <!-- https://purl.archive.org/oquo#NamesPerPropertyMetricScale -->

    <owl:NamedIndividual rdf:about="https://purl.archive.org/oquo#NamesPerPropertyMetricScale">
        <rdf:type rdf:resource="http://www.wurvoc.org/vocabularies/om-1.8/Ratio_scale"/>
        <rdf:type rdf:resource="https://purl.archive.org/oquo#RawScale"/>
        <QualityModel:hasRankigFunction rdf:resource="http://purl.org/net/QualityModel#HigherBest"/>
        <obo:IAO_0000115>The total number of property names over the total number of properties.</obo:IAO_0000115>
        <rdfs:label>names per property metric scale</rdfs:label>
    </owl:NamedIndividual>
    


    <!-- https://purl.archive.org/oquo#NumberOfAncestorClassesMetricScale -->

    <owl:NamedIndividual rdf:about="https://purl.archive.org/oquo#NumberOfAncestorClassesMetricScale">
        <rdf:type rdf:resource="http://www.wurvoc.org/vocabularies/om-1.8/Ratio_scale"/>
        <rdf:type rdf:resource="https://purl.archive.org/oquo#RawScale"/>
        <QualityModel:hasRankigFunction rdf:resource="http://purl.org/net/QualityModel#LowerBest"/>
        <obo:IAO_0000115>Mean number of ancestor classes per leaf class.</obo:IAO_0000115>
        <rdfs:label>number of ancestor classes metric scale</rdfs:label>
    </owl:NamedIndividual>
    


    <!-- https://purl.archive.org/oquo#NumberOfChildrenClassesMetricScale -->

    <owl:NamedIndividual rdf:about="https://purl.archive.org/oquo#NumberOfChildrenClassesMetricScale">
        <rdf:type rdf:resource="http://www.wurvoc.org/vocabularies/om-1.8/Ratio_scale"/>
        <rdf:type rdf:resource="https://purl.archive.org/oquo#RawScale"/>
        <QualityModel:hasRankigFunction rdf:resource="http://purl.org/net/QualityModel#HigherBest"/>
        <obo:IAO_0000115>Number of the direct subclasses divided by the number of classes minus the number of leaf classes</obo:IAO_0000115>
        <rdfs:label>number of children classes metric scale</rdfs:label>
    </owl:NamedIndividual>
    


    <!-- https://purl.archive.org/oquo#NumberOfLexicalRegularitiesMetricScale -->

    <owl:NamedIndividual rdf:about="https://purl.archive.org/oquo#NumberOfLexicalRegularitiesMetricScale">
        <rdf:type rdf:resource="http://www.wurvoc.org/vocabularies/om-1.8/Ratio_scale"/>
        <rdf:type rdf:resource="https://purl.archive.org/oquo#RawScale"/>
        <QualityModel:hasRankigFunction rdf:resource="http://purl.org/net/QualityModel#HigherBest"/>
        <obo:IAO_0000115>The number of lexical regularities found in the ontology.</obo:IAO_0000115>
        <rdfs:label>number of lexical regularities metric scale</rdfs:label>
    </owl:NamedIndividual>
    


    <!-- https://purl.archive.org/oquo#NumberOfLexicalRegularityClassesMetricScale -->

    <owl:NamedIndividual rdf:about="https://purl.archive.org/oquo#NumberOfLexicalRegularityClassesMetricScale">
        <rdf:type rdf:resource="http://www.wurvoc.org/vocabularies/om-1.8/Ratio_scale"/>
        <rdf:type rdf:resource="https://purl.archive.org/oquo#RawScale"/>
        <QualityModel:hasRankigFunction rdf:resource="http://purl.org/net/QualityModel#HigherBest"/>
        <obo:IAO_0000115>The number of ontology classes whose name is a lexical regularity.</obo:IAO_0000115>
        <rdfs:label>number of lexical regularity classes metric scale</rdfs:label>
    </owl:NamedIndividual>
    


    <!-- https://purl.archive.org/oquo#NumberOfPropertiesMetricScale -->

    <owl:NamedIndividual rdf:about="https://purl.archive.org/oquo#NumberOfPropertiesMetricScale">
        <rdf:type rdf:resource="http://www.wurvoc.org/vocabularies/om-1.8/Ratio_scale"/>
        <rdf:type rdf:resource="https://purl.archive.org/oquo#RawScale"/>
        <QualityModel:hasRankigFunction rdf:resource="http://purl.org/net/QualityModel#LowerBest"/>
        <obo:IAO_0000115>Number of properties per class. Mean number of object and data property usages per class.</obo:IAO_0000115>
        <rdfs:label>number of properties metric scale</rdfs:label>
    </owl:NamedIndividual>
    


    <!-- https://purl.archive.org/oquo#ObjectPropertiesWithNoDescriptionMetricScale -->

    <owl:NamedIndividual rdf:about="https://purl.archive.org/oquo#ObjectPropertiesWithNoDescriptionMetricScale">
        <rdf:type rdf:resource="http://www.wurvoc.org/vocabularies/om-1.8/Ratio_scale"/>
        <rdf:type rdf:resource="https://purl.archive.org/oquo#RawScale"/>
        <QualityModel:hasRankigFunction rdf:resource="http://purl.org/net/QualityModel#LowerBest"/>
        <obo:IAO_0000115>The number  of object properties lacking a description over the number of object properties considered.</obo:IAO_0000115>
        <rdfs:label>object properties with no description metric scale</rdfs:label>
    </owl:NamedIndividual>
    


    <!-- https://purl.archive.org/oquo#ObjectPropertiesWithNoNameMetricScale -->

    <owl:NamedIndividual rdf:about="https://purl.archive.org/oquo#ObjectPropertiesWithNoNameMetricScale">
        <rdf:type rdf:resource="http://www.wurvoc.org/vocabularies/om-1.8/Ratio_scale"/>
        <rdf:type rdf:resource="https://purl.archive.org/oquo#RawScale"/>
        <QualityModel:hasRankigFunction rdf:resource="http://purl.org/net/QualityModel#LowerBest"/>
        <obo:IAO_0000115>The number of object properties lacking a name over the number of object properties considered.</obo:IAO_0000115>
        <rdfs:label>object properties with no name metric scale</rdfs:label>
    </owl:NamedIndividual>
    


    <!-- https://purl.archive.org/oquo#ObjectPropertiesWithNoSynonymMetricScale -->

    <owl:NamedIndividual rdf:about="https://purl.archive.org/oquo#ObjectPropertiesWithNoSynonymMetricScale">
        <rdf:type rdf:resource="http://www.wurvoc.org/vocabularies/om-1.8/Ratio_scale"/>
        <rdf:type rdf:resource="https://purl.archive.org/oquo#RawScale"/>
        <QualityModel:hasRankigFunction rdf:resource="http://purl.org/net/QualityModel#LowerBest"/>
        <obo:IAO_0000115>The number of object properties lacking a synonym over the number of object properties considered.</obo:IAO_0000115>
        <rdfs:label>object properties with no synonym metric scale</rdfs:label>
    </owl:NamedIndividual>
    


    <!-- https://purl.archive.org/oquo#PropertiesRichnessMetricScale -->

    <owl:NamedIndividual rdf:about="https://purl.archive.org/oquo#PropertiesRichnessMetricScale">
        <rdf:type rdf:resource="http://www.wurvoc.org/vocabularies/om-1.8/Ratio_scale"/>
        <rdf:type rdf:resource="https://purl.archive.org/oquo#RawScale"/>
        <QualityModel:hasRankigFunction rdf:resource="http://purl.org/net/QualityModel#HigherBest"/>
        <obo:IAO_0000115>Number of usages of object and data properties divided by the number of subclassof relations and properties</obo:IAO_0000115>
        <rdfs:label>properties richness metric scale</rdfs:label>
    </owl:NamedIndividual>
    


    <!-- https://purl.archive.org/oquo#RelationshipRichnessMetricScale -->

    <owl:NamedIndividual rdf:about="https://purl.archive.org/oquo#RelationshipRichnessMetricScale">
        <rdf:type rdf:resource="http://www.wurvoc.org/vocabularies/om-1.8/Ratio_scale"/>
        <rdf:type rdf:resource="https://purl.archive.org/oquo#RawScale"/>
        <QualityModel:hasRankigFunction rdf:resource="http://purl.org/net/QualityModel#HigherBest"/>
        <obo:IAO_0000115>Number of subclassof relationships divided by the number of subclassof relationships and properties.</obo:IAO_0000115>
        <rdfs:label>relationship richness metric scale</rdfs:label>
    </owl:NamedIndividual>
    


    <!-- https://purl.archive.org/oquo#RelationshipsPerClassMetricScale -->

    <owl:NamedIndividual rdf:about="https://purl.archive.org/oquo#RelationshipsPerClassMetricScale">
        <rdf:type rdf:resource="http://www.wurvoc.org/vocabularies/om-1.8/Ratio_scale"/>
        <rdf:type rdf:resource="https://purl.archive.org/oquo#RawScale"/>
        <QualityModel:hasRankigFunction rdf:resource="http://purl.org/net/QualityModel#HigherBest"/>
        <obo:IAO_0000115>Mean number of subclasses per class</obo:IAO_0000115>
        <rdfs:label>relationsships per class metric scale</rdfs:label>
    </owl:NamedIndividual>
    


    <!-- https://purl.archive.org/oquo#ResponseForAClassMetricScale -->

    <owl:NamedIndividual rdf:about="https://purl.archive.org/oquo#ResponseForAClassMetricScale">
        <rdf:type rdf:resource="http://www.wurvoc.org/vocabularies/om-1.8/Ratio_scale"/>
        <rdf:type rdf:resource="https://purl.archive.org/oquo#RawScale"/>
        <QualityModel:hasRankigFunction rdf:resource="http://purl.org/net/QualityModel#LowerBest"/>
        <obo:IAO_0000115>Number of properties that can be directly accessed from the class.</obo:IAO_0000115>
        <rdfs:label>response for a class metric scale</rdfs:label>
    </owl:NamedIndividual>
    


    <!-- https://purl.archive.org/oquo#SynonymsPerAnnotationPropertyMetricScale -->

    <owl:NamedIndividual rdf:about="https://purl.archive.org/oquo#SynonymsPerAnnotationPropertyMetricScale">
        <rdf:type rdf:resource="http://www.wurvoc.org/vocabularies/om-1.8/Ratio_scale"/>
        <rdf:type rdf:resource="https://purl.archive.org/oquo#RawScale"/>
        <QualityModel:hasRankigFunction rdf:resource="http://purl.org/net/QualityModel#HigherBest"/>
        <obo:IAO_0000115>The total number of annotation property synonyms over the total number of annotation properties.</obo:IAO_0000115>
        <rdfs:label>synonyms per annotation property metric scale</rdfs:label>
    </owl:NamedIndividual>
    


    <!-- https://purl.archive.org/oquo#SynonymsPerClassMetricScale -->

    <owl:NamedIndividual rdf:about="https://purl.archive.org/oquo#SynonymsPerClassMetricScale">
        <rdf:type rdf:resource="http://www.wurvoc.org/vocabularies/om-1.8/Ratio_scale"/>
        <rdf:type rdf:resource="https://purl.archive.org/oquo#RawScale"/>
        <QualityModel:hasRankigFunction rdf:resource="http://purl.org/net/QualityModel#HigherBest"/>
        <obo:IAO_0000115>The total number of class synonyms over the total number of classes.</obo:IAO_0000115>
        <rdfs:label>synonyms per class metric scale</rdfs:label>
    </owl:NamedIndividual>
    


    <!-- https://purl.archive.org/oquo#SynonymsPerDataPropertyMetricScale -->

    <owl:NamedIndividual rdf:about="https://purl.archive.org/oquo#SynonymsPerDataPropertyMetricScale">
        <rdf:type rdf:resource="http://www.wurvoc.org/vocabularies/om-1.8/Ratio_scale"/>
        <rdf:type rdf:resource="https://purl.archive.org/oquo#RawScale"/>
        <QualityModel:hasRankigFunction rdf:resource="http://purl.org/net/QualityModel#HigherBest"/>
        <obo:IAO_0000115>The total number of data property synonyms over the total number of data properties.</obo:IAO_0000115>
        <rdfs:label>synonyms per data property metric scale</rdfs:label>
    </owl:NamedIndividual>
    


    <!-- https://purl.archive.org/oquo#SynonymsPerObjectPropertyMetricScale -->

    <owl:NamedIndividual rdf:about="https://purl.archive.org/oquo#SynonymsPerObjectPropertyMetricScale">
        <rdf:type rdf:resource="http://www.wurvoc.org/vocabularies/om-1.8/Ratio_scale"/>
        <rdf:type rdf:resource="https://purl.archive.org/oquo#RawScale"/>
        <QualityModel:hasRankigFunction rdf:resource="http://purl.org/net/QualityModel#HigherBest"/>
        <obo:IAO_0000115>The total number of object property synonyms over the total number of object properties.</obo:IAO_0000115>
        <rdfs:label>synonyms per object property metric scale</rdfs:label>
    </owl:NamedIndividual>
    


    <!-- https://purl.archive.org/oquo#SynonymsPerPropertyMetricScale -->

    <owl:NamedIndividual rdf:about="https://purl.archive.org/oquo#SynonymsPerPropertyMetricScale">
        <rdf:type rdf:resource="http://www.wurvoc.org/vocabularies/om-1.8/Ratio_scale"/>
        <rdf:type rdf:resource="https://purl.archive.org/oquo#RawScale"/>
        <QualityModel:hasRankigFunction rdf:resource="http://purl.org/net/QualityModel#HigherBest"/>
        <obo:IAO_0000115>The total number of property synonyms over the total number of properties, including data, object and annotation properties.</obo:IAO_0000115>
        <rdfs:label>synonyms per property metric scale</rdfs:label>
    </owl:NamedIndividual>
    


    <!-- https://purl.archive.org/oquo#SystematicNamingMetricScale -->

    <owl:NamedIndividual rdf:about="https://purl.archive.org/oquo#SystematicNamingMetricScale">
        <rdf:type rdf:resource="http://www.wurvoc.org/vocabularies/om-1.8/Ratio_scale"/>
        <rdf:type rdf:resource="https://purl.archive.org/oquo#RawScale"/>
        <QualityModel:hasRankigFunction rdf:resource="http://purl.org/net/QualityModel#HigherBest"/>
        <obo:IAO_0000115>The degree in which hierarchies under LR classes exhibit the lexical regularity of the parent class.</obo:IAO_0000115>
        <rdfs:label>systematic naming metric scale</rdfs:label>
    </owl:NamedIndividual>
    


    <!-- https://purl.archive.org/oquo#Tangledness2MetricScale -->

    <owl:NamedIndividual rdf:about="https://purl.archive.org/oquo#Tangledness2MetricScale">
        <rdf:type rdf:resource="http://www.wurvoc.org/vocabularies/om-1.8/Ratio_scale"/>
        <rdf:type rdf:resource="https://purl.archive.org/oquo#RawScale"/>
        <QualityModel:hasRankigFunction rdf:resource="http://purl.org/net/QualityModel#LowerBest"/>
        <obo:IAO_0000115>Mean number of direct ancestor of classes with more than 1 direct ancestor.</obo:IAO_0000115>
        <rdfs:label>tangledness2 metric scale</rdfs:label>
    </owl:NamedIndividual>
    


    <!-- https://purl.archive.org/oquo#TanglednessMetricScale -->

    <owl:NamedIndividual rdf:about="https://purl.archive.org/oquo#TanglednessMetricScale">
        <rdf:type rdf:resource="http://www.wurvoc.org/vocabularies/om-1.8/Ratio_scale"/>
        <rdf:type rdf:resource="https://purl.archive.org/oquo#RawScale"/>
        <QualityModel:hasRankigFunction rdf:resource="http://purl.org/net/QualityModel#LowerBest"/>
        <obo:IAO_0000115>Mean number of classes with more than 1 direct ancestor</obo:IAO_0000115>
        <rdfs:label>tangledness metric scale</rdfs:label>
    </owl:NamedIndividual>
    


    <!-- https://purl.archive.org/oquo#WeigthMethodPerClass2MetricScale -->

    <owl:NamedIndividual rdf:about="https://purl.archive.org/oquo#WeigthMethodPerClass2MetricScale">
        <rdf:type rdf:resource="http://www.wurvoc.org/vocabularies/om-1.8/Ratio_scale"/>
        <rdf:type rdf:resource="https://purl.archive.org/oquo#RawScale"/>
        <QualityModel:hasRankigFunction rdf:resource="http://purl.org/net/QualityModel#LowerBest"/>
        <obo:IAO_0000115>Mean number of path from Thing to a leaf class per leaf class.</obo:IAO_0000115>
        <rdfs:label>weigth method per class 2 metric scale</rdfs:label>
    </owl:NamedIndividual>
    


    <!-- https://purl.archive.org/oquo#WeigthMethodPerClassMetricScale -->

    <owl:NamedIndividual rdf:about="https://purl.archive.org/oquo#WeigthMethodPerClassMetricScale">
        <rdf:type rdf:resource="http://www.wurvoc.org/vocabularies/om-1.8/Ratio_scale"/>
        <rdf:type rdf:resource="https://purl.archive.org/oquo#RawScale"/>
        <QualityModel:hasRankigFunction rdf:resource="http://purl.org/net/QualityModel#LowerBest"/>
        <obo:IAO_0000115>Mean length of the path from Thing to a leaf class.</obo:IAO_0000115>
        <rdfs:label>weigth method per class metric scale</rdfs:label>
    </owl:NamedIndividual>
    


    <!-- 
    ///////////////////////////////////////////////////////////////////////////////////////
    //
    // Annotations
    //
    ///////////////////////////////////////////////////////////////////////////////////////
     -->

    <rdf:Description rdf:about="http://www.w3.org/2000/01/rdf-schema#seeAlso">
        <rdfs:label>seeAlso</rdfs:label>
        <rdfs:isDefinedBy rdf:resource="http://www.w3.org/2000/01/rdf-schema#"/>
        <rdfs:comment>Further information about the subject resource.</rdfs:comment>
    </rdf:Description>
    <rdf:Description rdf:about="http://www.w3.org/2002/07/owl#backwardCompatibleWith">
        <rdfs:comment>The annotation property that indicates that a given ontology is backward compatible with another ontology.</rdfs:comment>
        <rdfs:label>backwardCompatibleWith</rdfs:label>
        <rdfs:isDefinedBy rdf:resource="http://www.w3.org/2002/07/owl#"/>
    </rdf:Description>
    <rdf:Description rdf:about="http://www.w3.org/2002/07/owl#deprecated">
        <rdfs:comment>The annotation property that indicates that a given entity has been deprecated.</rdfs:comment>
        <rdfs:label>deprecated</rdfs:label>
        <rdfs:isDefinedBy rdf:resource="http://www.w3.org/2002/07/owl#"/>
    </rdf:Description>
    <rdf:Description rdf:about="http://www.w3.org/2002/07/owl#incompatibleWith">
        <rdfs:comment>The annotation property that indicates that a given ontology is incompatible with another ontology.</rdfs:comment>
        <rdfs:isDefinedBy rdf:resource="http://www.w3.org/2002/07/owl#"/>
        <rdfs:label>incompatibleWith</rdfs:label>
    </rdf:Description>
    <rdf:Description rdf:about="http://www.w3.org/2002/07/owl#priorVersion">
        <rdfs:isDefinedBy rdf:resource="http://www.w3.org/2002/07/owl#"/>
        <rdfs:comment>The annotation property that indicates the predecessor ontology of a given ontology.</rdfs:comment>
        <rdfs:label>priorVersion</rdfs:label>
    </rdf:Description>
    <rdf:Description rdf:about="http://www.w3.org/2002/07/owl#versionInfo">
        <rdfs:isDefinedBy rdf:resource="http://www.w3.org/2002/07/owl#"/>
        <rdfs:comment>The annotation property that provides version information for an ontology or another OWL construct.</rdfs:comment>
        <rdfs:label>versionInfo</rdfs:label>
    </rdf:Description>
    


    <!-- 
    ///////////////////////////////////////////////////////////////////////////////////////
    //
    // General axioms
    //
    ///////////////////////////////////////////////////////////////////////////////////////
     -->

    <rdf:Description>
        <rdf:type rdf:resource="http://www.w3.org/2002/07/owl#AllDisjointClasses"/>
        <owl:members rdf:parseType="Collection">
            <rdf:Description rdf:about="http://ecoinformatics.org/oboe/oboe.1.2/oboe-core.owl#Characteristic"/>
            <rdf:Description rdf:about="http://ecoinformatics.org/oboe/oboe.1.2/oboe-core.owl#Entity"/>
            <rdf:Description rdf:about="http://ecoinformatics.org/oboe/oboe.1.2/oboe-core.owl#MeasuredValue"/>
            <rdf:Description rdf:about="http://ecoinformatics.org/oboe/oboe.1.2/oboe-core.owl#Measurement"/>
            <rdf:Description rdf:about="http://ecoinformatics.org/oboe/oboe.1.2/oboe-core.owl#Observation"/>
            <rdf:Description rdf:about="http://purl.org/net/EvaluationResult#Evaluation"/>
            <rdf:Description rdf:about="http://purl.org/net/EvaluationResult#EvaluationData"/>
            <rdf:Description rdf:about="http://purl.org/net/EvaluationResult#SubjectCategory"/>
            <rdf:Description rdf:about="http://purl.org/net/QualityModel#OrdinalScaleItem"/>
            <rdf:Description rdf:about="http://purl.org/net/QualityModel#RankingFunction"/>
            <rdf:Description rdf:about="http://www.w3.org/2006/time#Instant"/>
            <rdf:Description rdf:about="http://www.wurvoc.org/vocabularies/om-1.8/Measurement_scale"/>
            <rdf:Description rdf:about="http://www.wurvoc.org/vocabularies/om-1.8/Unit_of_measure"/>
        </owl:members>
    </rdf:Description>
    <rdf:Description>
        <rdf:type rdf:resource="http://www.w3.org/2002/07/owl#AllDisjointClasses"/>
        <owl:members rdf:parseType="Collection">
            <rdf:Description rdf:about="http://ecoinformatics.org/oboe/oboe.1.2/oboe-core.owl#Characteristic"/>
            <rdf:Description rdf:about="http://ecoinformatics.org/oboe/oboe.1.2/oboe-core.owl#Entity"/>
            <rdf:Description rdf:about="http://ecoinformatics.org/oboe/oboe.1.2/oboe-core.owl#MeasuredValue"/>
            <rdf:Description rdf:about="http://ecoinformatics.org/oboe/oboe.1.2/oboe-core.owl#Measurement"/>
            <rdf:Description rdf:about="http://purl.org/ipo/core#IssueEntity"/>
            <rdf:Description rdf:about="http://purl.org/net/EvaluationResult#Evaluation"/>
            <rdf:Description rdf:about="http://purl.org/net/EvaluationResult#EvaluationData"/>
            <rdf:Description rdf:about="http://purl.org/net/EvaluationResult#SubjectCategory"/>
            <rdf:Description rdf:about="http://purl.org/net/QualityModel#OrdinalScaleItem"/>
            <rdf:Description rdf:about="http://purl.org/net/QualityModel#RankingFunction"/>
            <rdf:Description rdf:about="http://www.w3.org/2006/time#Instant"/>
            <rdf:Description rdf:about="http://www.wurvoc.org/vocabularies/om-1.8/Measurement_scale"/>
            <rdf:Description rdf:about="http://www.wurvoc.org/vocabularies/om-1.8/Unit_of_measure"/>
        </owl:members>
    </rdf:Description>
    <rdf:Description>
        <rdf:type rdf:resource="http://www.w3.org/2002/07/owl#AllDisjointClasses"/>
        <owl:members rdf:parseType="Collection">
            <rdf:Description rdf:about="http://purl.org/net/QualityModel#BaseMeasure"/>
            <rdf:Description rdf:about="http://purl.org/net/QualityModel#DerivedMeasure"/>
            <rdf:Description rdf:about="http://purl.org/net/QualityModel#QualityIndicator"/>
        </owl:members>
    </rdf:Description>
    <rdf:Description>
        <rdf:type rdf:resource="http://www.w3.org/2002/07/owl#AllDisjointClasses"/>
        <owl:members rdf:parseType="Collection">
            <rdf:Description rdf:about="http://www.wurvoc.org/vocabularies/om-1.8/Cardinal_scale"/>
            <rdf:Description rdf:about="http://www.wurvoc.org/vocabularies/om-1.8/Nominal_scale"/>
            <rdf:Description rdf:about="http://www.wurvoc.org/vocabularies/om-1.8/Ordinal_scale"/>
        </owl:members>
    </rdf:Description>
    <rdf:Description>
        <rdf:type rdf:resource="http://www.w3.org/2002/07/owl#AllDisjointClasses"/>
        <owl:members rdf:parseType="Collection">
            <rdf:Description rdf:about="https://purl.archive.org/oquo#AdaptabilityCharacteristic"/>
            <rdf:Description rdf:about="https://purl.archive.org/oquo#AnalysabilityCharacteristic"/>
            <rdf:Description rdf:about="https://purl.archive.org/oquo#AppropriatenessRecognisabilityCharacteristic"/>
            <rdf:Description rdf:about="https://purl.archive.org/oquo#AvailabilityCharacteristic"/>
            <rdf:Description rdf:about="https://purl.archive.org/oquo#ChangeabilityCharacteristic"/>
            <rdf:Description rdf:about="https://purl.archive.org/oquo#ClassifyingInstancesCharacteristic"/>
            <rdf:Description rdf:about="https://purl.archive.org/oquo#ClusteringCharacteristic"/>
            <rdf:Description rdf:about="https://purl.archive.org/oquo#CognitiveSatisfactionCharacteristic"/>
            <rdf:Description rdf:about="https://purl.archive.org/oquo#CohesionCharacteristic"/>
            <rdf:Description rdf:about="https://purl.archive.org/oquo#CompatibilityCharacteristic"/>
            <rdf:Description rdf:about="https://purl.archive.org/oquo#ConsistencyCharacteristic"/>
            <rdf:Description rdf:about="https://purl.archive.org/oquo#ConsistentSearchAndQueryCharacteristic"/>
            <rdf:Description rdf:about="https://purl.archive.org/oquo#ContextConformityInUseCharacteristic"/>
            <rdf:Description rdf:about="https://purl.archive.org/oquo#ContextExtendibilityInUseCharacteristic"/>
            <rdf:Description rdf:about="https://purl.archive.org/oquo#ControlledVocabularyCharacteristic"/>
            <rdf:Description rdf:about="https://purl.archive.org/oquo#CyclesCharacteristic"/>
            <rdf:Description rdf:about="https://purl.archive.org/oquo#DecisionTreesCharacteristic"/>
            <rdf:Description rdf:about="https://purl.archive.org/oquo#DomainCoverageCharacteristic"/>
            <rdf:Description rdf:about="https://purl.archive.org/oquo#EaseOfUseCharacteristic"/>
            <rdf:Description rdf:about="https://purl.archive.org/oquo#EffectivenessInUseCharacteristic"/>
            <rdf:Description rdf:about="https://purl.archive.org/oquo#EfficiencyInUseCharacteristic"/>
            <rdf:Description rdf:about="https://purl.archive.org/oquo#EmotionalSatisfactionCharacteristic"/>
            <rdf:Description rdf:about="https://purl.archive.org/oquo#FlexibilityInUseCharacteristic"/>
            <rdf:Description rdf:about="https://purl.archive.org/oquo#FormalRelationSupportCharacteristic"/>
            <rdf:Description rdf:about="https://purl.archive.org/oquo#FormalisationCharacteristic"/>
            <rdf:Description rdf:about="https://purl.archive.org/oquo#FunctionalAdequacyCharacteristic"/>
            <rdf:Description rdf:about="https://purl.archive.org/oquo#GuidanceCharacteristic"/>
            <rdf:Description rdf:about="https://purl.archive.org/oquo#HelpfulnessCharacteristic"/>
            <rdf:Description rdf:about="https://purl.archive.org/oquo#IndexingAndLinkingCharacteristic"/>
            <rdf:Description rdf:about="https://purl.archive.org/oquo#InferenceCharacteristic"/>
            <rdf:Description rdf:about="https://purl.archive.org/oquo#InteroperabilityCharacteristic"/>
            <rdf:Description rdf:about="https://purl.archive.org/oquo#KnowledgeAcquisitionRepresentationCharacteristic"/>
            <rdf:Description rdf:about="https://purl.archive.org/oquo#KnowledgeReuseCharacteristic"/>
            <rdf:Description rdf:about="https://purl.archive.org/oquo#LearnabilityCharacteristic"/>
            <rdf:Description rdf:about="https://purl.archive.org/oquo#MaintainabilityCharacteristic"/>
            <rdf:Description rdf:about="https://purl.archive.org/oquo#ModificationStabilityCharacteristic"/>
            <rdf:Description rdf:about="https://purl.archive.org/oquo#ModularityCharacteristic"/>
            <rdf:Description rdf:about="https://purl.archive.org/oquo#OperabilityCharacteristic"/>
            <rdf:Description rdf:about="https://purl.archive.org/oquo#PhysicalSatisfactionCharacteristic"/>
            <rdf:Description rdf:about="https://purl.archive.org/oquo#PortabilityCharacteristic"/>
            <rdf:Description rdf:about="https://purl.archive.org/oquo#PrecisionCharacteristic"/>
            <rdf:Description rdf:about="https://purl.archive.org/oquo#QualityInUseCharacteristic"/>
            <rdf:Description rdf:about="https://purl.archive.org/oquo#RecoverabilityCharacteristic"/>
            <rdf:Description rdf:about="https://purl.archive.org/oquo#RedundancyCharacteristic"/>
            <rdf:Description rdf:about="https://purl.archive.org/oquo#ReferenceOntologyCharacteristic"/>
            <rdf:Description rdf:about="https://purl.archive.org/oquo#ReliabilityCharacteristic"/>
            <rdf:Description rdf:about="https://purl.archive.org/oquo#ReplaceabilityCharacteristic"/>
            <rdf:Description rdf:about="https://purl.archive.org/oquo#ResultsRepresentationCharacteristic"/>
            <rdf:Description rdf:about="https://purl.archive.org/oquo#ReusabilityCharacteristic"/>
            <rdf:Description rdf:about="https://purl.archive.org/oquo#SatisfactionInUseCharacteristic"/>
            <rdf:Description rdf:about="https://purl.archive.org/oquo#SchemaAndValueReconciliationCharacteristic"/>
            <rdf:Description rdf:about="https://purl.archive.org/oquo#SimilarityCharacteristic"/>
            <rdf:Description rdf:about="https://purl.archive.org/oquo#StructuralAccuracyCharacteristic"/>
            <rdf:Description rdf:about="https://purl.archive.org/oquo#StructuralCharacteristic"/>
            <rdf:Description rdf:about="https://purl.archive.org/oquo#TanglednessCharacteristic"/>
            <rdf:Description rdf:about="https://purl.archive.org/oquo#TestabilityCharacteristic"/>
            <rdf:Description rdf:about="https://purl.archive.org/oquo#TextAnalysisCharacteristic"/>
            <rdf:Description rdf:about="https://purl.archive.org/oquo#TransferabilityCharacteristic"/>
            <rdf:Description rdf:about="https://purl.archive.org/oquo#UsabilityInUseCharacteristic"/>
        </owl:members>
    </rdf:Description>
    <rdf:Description>
        <rdf:type rdf:resource="http://www.w3.org/2002/07/owl#AllDisjointClasses"/>
        <owl:members rdf:parseType="Collection">
            <rdf:Description rdf:about="https://purl.archive.org/oquo#AncestorsPerClassMetric"/>
            <rdf:Description rdf:about="https://purl.archive.org/oquo#AnnotationPropertiesWithNoDescriptionMetric"/>
            <rdf:Description rdf:about="https://purl.archive.org/oquo#AnnotationPropertiesWithNoNameMetric"/>
            <rdf:Description rdf:about="https://purl.archive.org/oquo#AnnotationPropertiesWithNoSynonymMetric"/>
            <rdf:Description rdf:about="https://purl.archive.org/oquo#AnnotationRichnessMetric"/>
            <rdf:Description rdf:about="https://purl.archive.org/oquo#AttributeRichnessMetric"/>
            <rdf:Description rdf:about="https://purl.archive.org/oquo#ClassRichnessMetric"/>
            <rdf:Description rdf:about="https://purl.archive.org/oquo#ClassesWithNoDescriptionMetric"/>
            <rdf:Description rdf:about="https://purl.archive.org/oquo#ClassesWithNoNameMetric"/>
            <rdf:Description rdf:about="https://purl.archive.org/oquo#ClassesWithNoSynonymMetric"/>
            <rdf:Description rdf:about="https://purl.archive.org/oquo#ConsistencyMetric"/>
            <rdf:Description rdf:about="https://purl.archive.org/oquo#CouplingBetweenObjectsMetric"/>
            <rdf:Description rdf:about="https://purl.archive.org/oquo#DataPropertiesWithNoDescriptionMetric"/>
            <rdf:Description rdf:about="https://purl.archive.org/oquo#DataPropertiesWithNoNameMetric"/>
            <rdf:Description rdf:about="https://purl.archive.org/oquo#DataPropertiesWithNoSynonymMetric"/>
            <rdf:Description rdf:about="https://purl.archive.org/oquo#DepthOfSubsumptionHierarchyMetric"/>
            <rdf:Description rdf:about="https://purl.archive.org/oquo#DescriptionsPerAnnotationPropertyMetric"/>
            <rdf:Description rdf:about="https://purl.archive.org/oquo#DescriptionsPerClassMetric"/>
            <rdf:Description rdf:about="https://purl.archive.org/oquo#DescriptionsPerDataPropertyMetric"/>
            <rdf:Description rdf:about="https://purl.archive.org/oquo#DescriptionsPerObjectPropertyMetric"/>
            <rdf:Description rdf:about="https://purl.archive.org/oquo#DescriptionsPerPropertyMetric"/>
            <rdf:Description rdf:about="https://purl.archive.org/oquo#FormalDegreeMetric"/>
            <rdf:Description rdf:about="https://purl.archive.org/oquo#LackOfCohesionInMethodsMetric"/>
            <rdf:Description rdf:about="https://purl.archive.org/oquo#LexicalRegularitiesPerClassMetric"/>
            <rdf:Description rdf:about="https://purl.archive.org/oquo#LexicalRegularityClassPercentageMetric"/>
            <rdf:Description rdf:about="https://purl.archive.org/oquo#LexicallySuggestLogicallyDefineMetric"/>
            <rdf:Description rdf:about="https://purl.archive.org/oquo#NamesPerAnnotationPropertyMetric"/>
            <rdf:Description rdf:about="https://purl.archive.org/oquo#NamesPerClassMetric"/>
            <rdf:Description rdf:about="https://purl.archive.org/oquo#NamesPerDataPropertyMetric"/>
            <rdf:Description rdf:about="https://purl.archive.org/oquo#NamesPerObjectPropertyMetric"/>
            <rdf:Description rdf:about="https://purl.archive.org/oquo#NamesPerPropertyMetric"/>
            <rdf:Description rdf:about="https://purl.archive.org/oquo#NumberOfAncestorClassesMetric"/>
            <rdf:Description rdf:about="https://purl.archive.org/oquo#NumberOfChildrenClassesMetric"/>
            <rdf:Description rdf:about="https://purl.archive.org/oquo#NumberOfLexicalRegularitiesMetric"/>
            <rdf:Description rdf:about="https://purl.archive.org/oquo#NumberOfLexicalRegularityClassesMetric"/>
            <rdf:Description rdf:about="https://purl.archive.org/oquo#NumberOfPropertiesMetric"/>
            <rdf:Description rdf:about="https://purl.archive.org/oquo#ObjectPropertiesWithNoDescriptionMetric"/>
            <rdf:Description rdf:about="https://purl.archive.org/oquo#ObjectPropertiesWithNoNameMetric"/>
            <rdf:Description rdf:about="https://purl.archive.org/oquo#ObjectPropertiesWithNoSynonymMetric"/>
            <rdf:Description rdf:about="https://purl.archive.org/oquo#PropertiesRichnessMetric"/>
            <rdf:Description rdf:about="https://purl.archive.org/oquo#RelationshipRichnessMetric"/>
            <rdf:Description rdf:about="https://purl.archive.org/oquo#RelationshipsPerClassMetric"/>
            <rdf:Description rdf:about="https://purl.archive.org/oquo#ResponseForAClassMetric"/>
            <rdf:Description rdf:about="https://purl.archive.org/oquo#SynonymsPerAnnotationPropertyMetric"/>
            <rdf:Description rdf:about="https://purl.archive.org/oquo#SynonymsPerClassMetric"/>
            <rdf:Description rdf:about="https://purl.archive.org/oquo#SynonymsPerDataPropertyMetric"/>
            <rdf:Description rdf:about="https://purl.archive.org/oquo#SynonymsPerObjectPropertyMetric"/>
            <rdf:Description rdf:about="https://purl.archive.org/oquo#SynonymsPerPropertyMetric"/>
            <rdf:Description rdf:about="https://purl.archive.org/oquo#SystematicNamingMetric"/>
            <rdf:Description rdf:about="https://purl.archive.org/oquo#Tangledness2Metric"/>
            <rdf:Description rdf:about="https://purl.archive.org/oquo#TanglednessMetric"/>
            <rdf:Description rdf:about="https://purl.archive.org/oquo#WeigthMethodPerClass2Metric"/>
            <rdf:Description rdf:about="https://purl.archive.org/oquo#WeigthMethodPerClassMetric"/>
        </owl:members>
    </rdf:Description>
    <rdf:Description>
        <rdf:type rdf:resource="http://www.w3.org/2002/07/owl#AllDisjointClasses"/>
        <owl:members rdf:parseType="Collection">
            <rdf:Description rdf:about="https://purl.archive.org/oquo#CriticalIssue"/>
            <rdf:Description rdf:about="https://purl.archive.org/oquo#MajorIssue"/>
            <rdf:Description rdf:about="https://purl.archive.org/oquo#MinorIssue"/>
            <rdf:Description rdf:about="https://purl.archive.org/oquo#TrivialIssue"/>
        </owl:members>
    </rdf:Description>
</rdf:RDF>



<!-- Generated by the OWL API (version 4.5.9.2019-02-01T07:24:44Z) https://github.com/owlcs/owlapi -->

