<?xml version="1.0"?>
<rdf:RDF xmlns="https://purl.archive.org/oquo#"
     xml:base="https://purl.archive.org/oquo"
     xmlns:dc="http://purl.org/dc/elements/1.1/"
     xmlns:obo="http://purl.obolibrary.org/obo/"
     xmlns:owl="http://www.w3.org/2002/07/owl#"
     xmlns:rdf="http://www.w3.org/1999/02/22-rdf-syntax-ns#"
     xmlns:xml="http://www.w3.org/XML/1998/namespace"
     xmlns:xsd="http://www.w3.org/2001/XMLSchema#"
     xmlns:om-1="http://www.wurvoc.org/vocabularies/om-1.8/"
     xmlns:rdf1="http://www.cropontology.org/rdf/"
     xmlns:rdfs="http://www.w3.org/2000/01/rdf-schema#"
     xmlns:skos="http://www.w3.org/2004/02/skos/core#"
     xmlns:vann="http://purl.org/vocab/vann/"
     xmlns:terms="http://purl.org/dc/terms/"
     xmlns:oboInOwl="http://www.geneontology.org/formats/oboInOwl#"
     xmlns:QualityModel="http://purl.org/net/QualityModel#">
    <owl:Ontology rdf:about="https://purl.archive.org/oquo-huron">
    	<owl:imports rdf:resource="https://purl.archive.org/oquo-core"/>
    </owl:Ontology>
    


  

    <!-- 
    ///////////////////////////////////////////////////////////////////////////////////////
    //
    // Classes
    //
    ///////////////////////////////////////////////////////////////////////////////////////
     -->


    <!-- https://purl.archive.org/oquo#AnnotationPropertiesWithNoDescriptionMetric -->

    <owl:Class rdf:about="https://purl.archive.org/oquo#AnnotationPropertiesWithNoDescriptionMetric">
        <rdfs:subClassOf rdf:resource="http://purl.org/net/QualityModel#DerivedMeasure"/>
        <rdfs:subClassOf>
            <owl:Restriction>
                <owl:onProperty rdf:resource="http://purl.org/net/QualityModel#hasScale"/>
                <owl:someValuesFrom>
                    <owl:Class>
                        <owl:intersectionOf rdf:parseType="Collection">
                            <rdf:Description rdf:about="https://purl.archive.org/oquo#RawScale"/>
                            <owl:Restriction>
                                <owl:onProperty rdf:resource="http://purl.org/net/QualityModel#hasRankigFunction"/>
                                <owl:hasValue rdf:resource="http://purl.org/net/QualityModel#LowerBest"/>
                            </owl:Restriction>
                        </owl:intersectionOf>
                    </owl:Class>
                </owl:someValuesFrom>
            </owl:Restriction>
        </rdfs:subClassOf>
        <rdfs:subClassOf>
            <owl:Restriction>
                <owl:onProperty rdf:resource="https://purl.archive.org/oquo#measuresCharacteristicNegatively"/>
                <owl:someValuesFrom rdf:resource="https://purl.archive.org/oquo#EaseOfUseCharacteristic"/>
            </owl:Restriction>
        </rdfs:subClassOf>
        <rdfs:subClassOf>
            <owl:Restriction>
                <owl:onProperty rdf:resource="https://purl.archive.org/oquo#measuresCharacteristicNegatively"/>
                <owl:someValuesFrom rdf:resource="https://purl.archive.org/oquo#EfficiencyInUseCharacteristic"/>
            </owl:Restriction>
        </rdfs:subClassOf>
        <rdfs:subClassOf>
            <owl:Restriction>
                <owl:onProperty rdf:resource="https://purl.archive.org/oquo#measuresCharacteristicNegatively"/>
                <owl:someValuesFrom rdf:resource="https://purl.archive.org/oquo#HelpfulnessCharacteristic"/>
            </owl:Restriction>
        </rdfs:subClassOf>
        <rdfs:subClassOf>
            <owl:Restriction>
                <owl:onProperty rdf:resource="https://purl.archive.org/oquo#measuresCharacteristicNegatively"/>
                <owl:someValuesFrom rdf:resource="https://purl.archive.org/oquo#IndexingAndLinkingCharacteristic"/>
            </owl:Restriction>
        </rdfs:subClassOf>
        <rdfs:subClassOf>
            <owl:Restriction>
                <owl:onProperty rdf:resource="https://purl.archive.org/oquo#measuresCharacteristicNegatively"/>
                <owl:someValuesFrom rdf:resource="https://purl.archive.org/oquo#KnowledgeReuseCharacteristic"/>
            </owl:Restriction>
        </rdfs:subClassOf>
        <rdfs:subClassOf>
            <owl:Restriction>
                <owl:onProperty rdf:resource="https://purl.archive.org/oquo#measuresCharacteristicNegatively"/>
                <owl:someValuesFrom rdf:resource="https://purl.archive.org/oquo#LearnabilityCharacteristic"/>
            </owl:Restriction>
        </rdfs:subClassOf>
        <rdfs:subClassOf>
            <owl:Restriction>
                <owl:onProperty rdf:resource="https://purl.archive.org/oquo#measuresCharacteristicNegatively"/>
                <owl:allValuesFrom>
                    <owl:Class>
                        <owl:unionOf rdf:parseType="Collection">
                            <rdf:Description rdf:about="https://purl.archive.org/oquo#EaseOfUseCharacteristic"/>
                            <rdf:Description rdf:about="https://purl.archive.org/oquo#EfficiencyInUseCharacteristic"/>
                            <rdf:Description rdf:about="https://purl.archive.org/oquo#HelpfulnessCharacteristic"/>
                            <rdf:Description rdf:about="https://purl.archive.org/oquo#IndexingAndLinkingCharacteristic"/>
                            <rdf:Description rdf:about="https://purl.archive.org/oquo#KnowledgeReuseCharacteristic"/>
                            <rdf:Description rdf:about="https://purl.archive.org/oquo#LearnabilityCharacteristic"/>
                        </owl:unionOf>
                    </owl:Class>
                </owl:allValuesFrom>
            </owl:Restriction>
        </rdfs:subClassOf>
        <rdfs:subClassOf>
            <owl:Restriction>
                <owl:onProperty rdf:resource="http://purl.org/net/QualityModel#hasScale"/>
                <owl:hasValue rdf:resource="https://purl.archive.org/oquo#AnnotationPropertiesWithNoDescriptionMetricScale"/>
            </owl:Restriction>
        </rdfs:subClassOf>
        <obo:IAO_0000115>The Percentage of annotation properties lacking a description in the ontology.</obo:IAO_0000115>
        <rdf1:acronym>APWND</rdf1:acronym>
        <rdfs:label>annotation properties with no description metric</rdfs:label>
    </owl:Class>
    


    <!-- https://purl.archive.org/oquo#AnnotationPropertiesWithNoNameMetric -->

    <owl:Class rdf:about="https://purl.archive.org/oquo#AnnotationPropertiesWithNoNameMetric">
        <rdfs:subClassOf rdf:resource="http://purl.org/net/QualityModel#DerivedMeasure"/>
        <rdfs:subClassOf>
            <owl:Restriction>
                <owl:onProperty rdf:resource="http://purl.org/net/QualityModel#hasScale"/>
                <owl:someValuesFrom>
                    <owl:Class>
                        <owl:intersectionOf rdf:parseType="Collection">
                            <rdf:Description rdf:about="https://purl.archive.org/oquo#RawScale"/>
                            <owl:Restriction>
                                <owl:onProperty rdf:resource="http://purl.org/net/QualityModel#hasRankigFunction"/>
                                <owl:hasValue rdf:resource="http://purl.org/net/QualityModel#LowerBest"/>
                            </owl:Restriction>
                        </owl:intersectionOf>
                    </owl:Class>
                </owl:someValuesFrom>
            </owl:Restriction>
        </rdfs:subClassOf>
        <rdfs:subClassOf>
            <owl:Restriction>
                <owl:onProperty rdf:resource="https://purl.archive.org/oquo#measuresCharacteristicNegatively"/>
                <owl:someValuesFrom rdf:resource="https://purl.archive.org/oquo#EaseOfUseCharacteristic"/>
            </owl:Restriction>
        </rdfs:subClassOf>
        <rdfs:subClassOf>
            <owl:Restriction>
                <owl:onProperty rdf:resource="https://purl.archive.org/oquo#measuresCharacteristicNegatively"/>
                <owl:someValuesFrom rdf:resource="https://purl.archive.org/oquo#EfficiencyInUseCharacteristic"/>
            </owl:Restriction>
        </rdfs:subClassOf>
        <rdfs:subClassOf>
            <owl:Restriction>
                <owl:onProperty rdf:resource="https://purl.archive.org/oquo#measuresCharacteristicNegatively"/>
                <owl:someValuesFrom rdf:resource="https://purl.archive.org/oquo#IndexingAndLinkingCharacteristic"/>
            </owl:Restriction>
        </rdfs:subClassOf>
        <rdfs:subClassOf>
            <owl:Restriction>
                <owl:onProperty rdf:resource="https://purl.archive.org/oquo#measuresCharacteristicNegatively"/>
                <owl:someValuesFrom rdf:resource="https://purl.archive.org/oquo#KnowledgeReuseCharacteristic"/>
            </owl:Restriction>
        </rdfs:subClassOf>
        <rdfs:subClassOf>
            <owl:Restriction>
                <owl:onProperty rdf:resource="https://purl.archive.org/oquo#measuresCharacteristicNegatively"/>
                <owl:someValuesFrom rdf:resource="https://purl.archive.org/oquo#TextAnalysisCharacteristic"/>
            </owl:Restriction>
        </rdfs:subClassOf>
        <rdfs:subClassOf>
            <owl:Restriction>
                <owl:onProperty rdf:resource="https://purl.archive.org/oquo#measuresCharacteristicNegatively"/>
                <owl:allValuesFrom>
                    <owl:Class>
                        <owl:unionOf rdf:parseType="Collection">
                            <rdf:Description rdf:about="https://purl.archive.org/oquo#EaseOfUseCharacteristic"/>
                            <rdf:Description rdf:about="https://purl.archive.org/oquo#EfficiencyInUseCharacteristic"/>
                            <rdf:Description rdf:about="https://purl.archive.org/oquo#IndexingAndLinkingCharacteristic"/>
                            <rdf:Description rdf:about="https://purl.archive.org/oquo#KnowledgeReuseCharacteristic"/>
                            <rdf:Description rdf:about="https://purl.archive.org/oquo#TextAnalysisCharacteristic"/>
                        </owl:unionOf>
                    </owl:Class>
                </owl:allValuesFrom>
            </owl:Restriction>
        </rdfs:subClassOf>
        <rdfs:subClassOf>
            <owl:Restriction>
                <owl:onProperty rdf:resource="http://purl.org/net/QualityModel#hasScale"/>
                <owl:hasValue rdf:resource="https://purl.archive.org/oquo#AnnotationPropertiesWithNoNameMetricScale"/>
            </owl:Restriction>
        </rdfs:subClassOf>
        <obo:IAO_0000115>The Percentage of annotation properties lacking a name in the ontology.</obo:IAO_0000115>
        <rdf1:acronym>APWNN</rdf1:acronym>
        <rdfs:label>annotation properties with no name metric</rdfs:label>
    </owl:Class>
    


    <!-- https://purl.archive.org/oquo#AnnotationPropertiesWithNoSynonymMetric -->

    <owl:Class rdf:about="https://purl.archive.org/oquo#AnnotationPropertiesWithNoSynonymMetric">
        <rdfs:subClassOf rdf:resource="http://purl.org/net/QualityModel#DerivedMeasure"/>
        <rdfs:subClassOf>
            <owl:Restriction>
                <owl:onProperty rdf:resource="http://purl.org/net/QualityModel#hasScale"/>
                <owl:someValuesFrom>
                    <owl:Class>
                        <owl:intersectionOf rdf:parseType="Collection">
                            <rdf:Description rdf:about="https://purl.archive.org/oquo#RawScale"/>
                            <owl:Restriction>
                                <owl:onProperty rdf:resource="http://purl.org/net/QualityModel#hasRankigFunction"/>
                                <owl:hasValue rdf:resource="http://purl.org/net/QualityModel#LowerBest"/>
                            </owl:Restriction>
                        </owl:intersectionOf>
                    </owl:Class>
                </owl:someValuesFrom>
            </owl:Restriction>
        </rdfs:subClassOf>
        <rdfs:subClassOf>
            <owl:Restriction>
                <owl:onProperty rdf:resource="https://purl.archive.org/oquo#measuresCharacteristicNegatively"/>
                <owl:someValuesFrom rdf:resource="https://purl.archive.org/oquo#EaseOfUseCharacteristic"/>
            </owl:Restriction>
        </rdfs:subClassOf>
        <rdfs:subClassOf>
            <owl:Restriction>
                <owl:onProperty rdf:resource="https://purl.archive.org/oquo#measuresCharacteristicNegatively"/>
                <owl:someValuesFrom rdf:resource="https://purl.archive.org/oquo#EfficiencyInUseCharacteristic"/>
            </owl:Restriction>
        </rdfs:subClassOf>
        <rdfs:subClassOf>
            <owl:Restriction>
                <owl:onProperty rdf:resource="https://purl.archive.org/oquo#measuresCharacteristicNegatively"/>
                <owl:someValuesFrom rdf:resource="https://purl.archive.org/oquo#IndexingAndLinkingCharacteristic"/>
            </owl:Restriction>
        </rdfs:subClassOf>
        <rdfs:subClassOf>
            <owl:Restriction>
                <owl:onProperty rdf:resource="https://purl.archive.org/oquo#measuresCharacteristicNegatively"/>
                <owl:someValuesFrom rdf:resource="https://purl.archive.org/oquo#KnowledgeReuseCharacteristic"/>
            </owl:Restriction>
        </rdfs:subClassOf>
        <rdfs:subClassOf>
            <owl:Restriction>
                <owl:onProperty rdf:resource="https://purl.archive.org/oquo#measuresCharacteristicNegatively"/>
                <owl:someValuesFrom rdf:resource="https://purl.archive.org/oquo#TextAnalysisCharacteristic"/>
            </owl:Restriction>
        </rdfs:subClassOf>
        <rdfs:subClassOf>
            <owl:Restriction>
                <owl:onProperty rdf:resource="https://purl.archive.org/oquo#measuresCharacteristicNegatively"/>
                <owl:allValuesFrom>
                    <owl:Class>
                        <owl:unionOf rdf:parseType="Collection">
                            <rdf:Description rdf:about="https://purl.archive.org/oquo#EaseOfUseCharacteristic"/>
                            <rdf:Description rdf:about="https://purl.archive.org/oquo#EfficiencyInUseCharacteristic"/>
                            <rdf:Description rdf:about="https://purl.archive.org/oquo#IndexingAndLinkingCharacteristic"/>
                            <rdf:Description rdf:about="https://purl.archive.org/oquo#KnowledgeReuseCharacteristic"/>
                            <rdf:Description rdf:about="https://purl.archive.org/oquo#TextAnalysisCharacteristic"/>
                        </owl:unionOf>
                    </owl:Class>
                </owl:allValuesFrom>
            </owl:Restriction>
        </rdfs:subClassOf>
        <rdfs:subClassOf>
            <owl:Restriction>
                <owl:onProperty rdf:resource="http://purl.org/net/QualityModel#hasScale"/>
                <owl:hasValue rdf:resource="https://purl.archive.org/oquo#AnnotationPropertiesWithNoSynonymMetricScale"/>
            </owl:Restriction>
        </rdfs:subClassOf>
        <obo:IAO_0000115>The Percentage of annotation properties lacking a synonym in the ontology.</obo:IAO_0000115>
        <rdf1:acronym>APWNS</rdf1:acronym>
        <rdfs:label>annotation properties with no synonym metric</rdfs:label>
    </owl:Class>
    


    <!-- https://purl.archive.org/oquo#ClassesWithNoDescriptionMetric -->

    <owl:Class rdf:about="https://purl.archive.org/oquo#ClassesWithNoDescriptionMetric">
        <rdfs:subClassOf rdf:resource="http://purl.org/net/QualityModel#DerivedMeasure"/>
        <rdfs:subClassOf>
            <owl:Restriction>
                <owl:onProperty rdf:resource="http://purl.org/net/QualityModel#hasScale"/>
                <owl:someValuesFrom>
                    <owl:Class>
                        <owl:intersectionOf rdf:parseType="Collection">
                            <rdf:Description rdf:about="https://purl.archive.org/oquo#RawScale"/>
                            <owl:Restriction>
                                <owl:onProperty rdf:resource="http://purl.org/net/QualityModel#hasRankigFunction"/>
                                <owl:hasValue rdf:resource="http://purl.org/net/QualityModel#LowerBest"/>
                            </owl:Restriction>
                        </owl:intersectionOf>
                    </owl:Class>
                </owl:someValuesFrom>
            </owl:Restriction>
        </rdfs:subClassOf>
        <rdfs:subClassOf>
            <owl:Restriction>
                <owl:onProperty rdf:resource="https://purl.archive.org/oquo#measuresCharacteristicNegatively"/>
                <owl:someValuesFrom rdf:resource="https://purl.archive.org/oquo#EaseOfUseCharacteristic"/>
            </owl:Restriction>
        </rdfs:subClassOf>
        <rdfs:subClassOf>
            <owl:Restriction>
                <owl:onProperty rdf:resource="https://purl.archive.org/oquo#measuresCharacteristicNegatively"/>
                <owl:someValuesFrom rdf:resource="https://purl.archive.org/oquo#EfficiencyInUseCharacteristic"/>
            </owl:Restriction>
        </rdfs:subClassOf>
        <rdfs:subClassOf>
            <owl:Restriction>
                <owl:onProperty rdf:resource="https://purl.archive.org/oquo#measuresCharacteristicNegatively"/>
                <owl:someValuesFrom rdf:resource="https://purl.archive.org/oquo#HelpfulnessCharacteristic"/>
            </owl:Restriction>
        </rdfs:subClassOf>
        <rdfs:subClassOf>
            <owl:Restriction>
                <owl:onProperty rdf:resource="https://purl.archive.org/oquo#measuresCharacteristicNegatively"/>
                <owl:someValuesFrom rdf:resource="https://purl.archive.org/oquo#IndexingAndLinkingCharacteristic"/>
            </owl:Restriction>
        </rdfs:subClassOf>
        <rdfs:subClassOf>
            <owl:Restriction>
                <owl:onProperty rdf:resource="https://purl.archive.org/oquo#measuresCharacteristicNegatively"/>
                <owl:someValuesFrom rdf:resource="https://purl.archive.org/oquo#KnowledgeReuseCharacteristic"/>
            </owl:Restriction>
        </rdfs:subClassOf>
        <rdfs:subClassOf>
            <owl:Restriction>
                <owl:onProperty rdf:resource="https://purl.archive.org/oquo#measuresCharacteristicNegatively"/>
                <owl:someValuesFrom rdf:resource="https://purl.archive.org/oquo#LearnabilityCharacteristic"/>
            </owl:Restriction>
        </rdfs:subClassOf>
        <rdfs:subClassOf>
            <owl:Restriction>
                <owl:onProperty rdf:resource="https://purl.archive.org/oquo#measuresCharacteristicNegatively"/>
                <owl:allValuesFrom>
                    <owl:Class>
                        <owl:unionOf rdf:parseType="Collection">
                            <rdf:Description rdf:about="https://purl.archive.org/oquo#EaseOfUseCharacteristic"/>
                            <rdf:Description rdf:about="https://purl.archive.org/oquo#EfficiencyInUseCharacteristic"/>
                            <rdf:Description rdf:about="https://purl.archive.org/oquo#HelpfulnessCharacteristic"/>
                            <rdf:Description rdf:about="https://purl.archive.org/oquo#IndexingAndLinkingCharacteristic"/>
                            <rdf:Description rdf:about="https://purl.archive.org/oquo#KnowledgeReuseCharacteristic"/>
                            <rdf:Description rdf:about="https://purl.archive.org/oquo#LearnabilityCharacteristic"/>
                        </owl:unionOf>
                    </owl:Class>
                </owl:allValuesFrom>
            </owl:Restriction>
        </rdfs:subClassOf>
        <rdfs:subClassOf>
            <owl:Restriction>
                <owl:onProperty rdf:resource="http://purl.org/net/QualityModel#hasScale"/>
                <owl:hasValue rdf:resource="https://purl.archive.org/oquo#ClassesWithNoDescriptionMetricScale"/>
            </owl:Restriction>
        </rdfs:subClassOf>
        <obo:IAO_0000115>The Percentage of classes lacking a description in the ontology.</obo:IAO_0000115>
        <rdf1:acronym>CWND</rdf1:acronym>
        <rdfs:label>classes with no description metric</rdfs:label>
    </owl:Class>
    


    <!-- https://purl.archive.org/oquo#ClassesWithNoNameMetric -->

    <owl:Class rdf:about="https://purl.archive.org/oquo#ClassesWithNoNameMetric">
        <rdfs:subClassOf rdf:resource="http://purl.org/net/QualityModel#DerivedMeasure"/>
        <rdfs:subClassOf>
            <owl:Restriction>
                <owl:onProperty rdf:resource="http://purl.org/net/QualityModel#hasScale"/>
                <owl:someValuesFrom>
                    <owl:Class>
                        <owl:intersectionOf rdf:parseType="Collection">
                            <rdf:Description rdf:about="https://purl.archive.org/oquo#RawScale"/>
                            <owl:Restriction>
                                <owl:onProperty rdf:resource="http://purl.org/net/QualityModel#hasRankigFunction"/>
                                <owl:hasValue rdf:resource="http://purl.org/net/QualityModel#LowerBest"/>
                            </owl:Restriction>
                        </owl:intersectionOf>
                    </owl:Class>
                </owl:someValuesFrom>
            </owl:Restriction>
        </rdfs:subClassOf>
        <rdfs:subClassOf>
            <owl:Restriction>
                <owl:onProperty rdf:resource="https://purl.archive.org/oquo#measuresCharacteristicNegatively"/>
                <owl:someValuesFrom rdf:resource="https://purl.archive.org/oquo#EaseOfUseCharacteristic"/>
            </owl:Restriction>
        </rdfs:subClassOf>
        <rdfs:subClassOf>
            <owl:Restriction>
                <owl:onProperty rdf:resource="https://purl.archive.org/oquo#measuresCharacteristicNegatively"/>
                <owl:someValuesFrom rdf:resource="https://purl.archive.org/oquo#EfficiencyInUseCharacteristic"/>
            </owl:Restriction>
        </rdfs:subClassOf>
        <rdfs:subClassOf>
            <owl:Restriction>
                <owl:onProperty rdf:resource="https://purl.archive.org/oquo#measuresCharacteristicNegatively"/>
                <owl:someValuesFrom rdf:resource="https://purl.archive.org/oquo#IndexingAndLinkingCharacteristic"/>
            </owl:Restriction>
        </rdfs:subClassOf>
        <rdfs:subClassOf>
            <owl:Restriction>
                <owl:onProperty rdf:resource="https://purl.archive.org/oquo#measuresCharacteristicNegatively"/>
                <owl:someValuesFrom rdf:resource="https://purl.archive.org/oquo#KnowledgeReuseCharacteristic"/>
            </owl:Restriction>
        </rdfs:subClassOf>
        <rdfs:subClassOf>
            <owl:Restriction>
                <owl:onProperty rdf:resource="https://purl.archive.org/oquo#measuresCharacteristicNegatively"/>
                <owl:someValuesFrom rdf:resource="https://purl.archive.org/oquo#TextAnalysisCharacteristic"/>
            </owl:Restriction>
        </rdfs:subClassOf>
        <rdfs:subClassOf>
            <owl:Restriction>
                <owl:onProperty rdf:resource="https://purl.archive.org/oquo#measuresCharacteristicNegatively"/>
                <owl:allValuesFrom>
                    <owl:Class>
                        <owl:unionOf rdf:parseType="Collection">
                            <rdf:Description rdf:about="https://purl.archive.org/oquo#EaseOfUseCharacteristic"/>
                            <rdf:Description rdf:about="https://purl.archive.org/oquo#EfficiencyInUseCharacteristic"/>
                            <rdf:Description rdf:about="https://purl.archive.org/oquo#IndexingAndLinkingCharacteristic"/>
                            <rdf:Description rdf:about="https://purl.archive.org/oquo#KnowledgeReuseCharacteristic"/>
                            <rdf:Description rdf:about="https://purl.archive.org/oquo#TextAnalysisCharacteristic"/>
                        </owl:unionOf>
                    </owl:Class>
                </owl:allValuesFrom>
            </owl:Restriction>
        </rdfs:subClassOf>
        <rdfs:subClassOf>
            <owl:Restriction>
                <owl:onProperty rdf:resource="http://purl.org/net/QualityModel#hasScale"/>
                <owl:hasValue rdf:resource="https://purl.archive.org/oquo#ClassesWithNoNameMetricScale"/>
            </owl:Restriction>
        </rdfs:subClassOf>
        <obo:IAO_0000115>The Percentage of classes lacking a name in the ontology.</obo:IAO_0000115>
        <rdf1:acronym>CWNN</rdf1:acronym>
        <rdfs:label>classes with no name metric</rdfs:label>
    </owl:Class>
    


    <!-- https://purl.archive.org/oquo#ClassesWithNoSynonymMetric -->

    <owl:Class rdf:about="https://purl.archive.org/oquo#ClassesWithNoSynonymMetric">
        <rdfs:subClassOf rdf:resource="http://purl.org/net/QualityModel#DerivedMeasure"/>
        <rdfs:subClassOf>
            <owl:Restriction>
                <owl:onProperty rdf:resource="http://purl.org/net/QualityModel#hasScale"/>
                <owl:someValuesFrom>
                    <owl:Class>
                        <owl:intersectionOf rdf:parseType="Collection">
                            <rdf:Description rdf:about="https://purl.archive.org/oquo#RawScale"/>
                            <owl:Restriction>
                                <owl:onProperty rdf:resource="http://purl.org/net/QualityModel#hasRankigFunction"/>
                                <owl:hasValue rdf:resource="http://purl.org/net/QualityModel#LowerBest"/>
                            </owl:Restriction>
                        </owl:intersectionOf>
                    </owl:Class>
                </owl:someValuesFrom>
            </owl:Restriction>
        </rdfs:subClassOf>
        <rdfs:subClassOf>
            <owl:Restriction>
                <owl:onProperty rdf:resource="https://purl.archive.org/oquo#measuresCharacteristicNegatively"/>
                <owl:someValuesFrom rdf:resource="https://purl.archive.org/oquo#EaseOfUseCharacteristic"/>
            </owl:Restriction>
        </rdfs:subClassOf>
        <rdfs:subClassOf>
            <owl:Restriction>
                <owl:onProperty rdf:resource="https://purl.archive.org/oquo#measuresCharacteristicNegatively"/>
                <owl:someValuesFrom rdf:resource="https://purl.archive.org/oquo#EfficiencyInUseCharacteristic"/>
            </owl:Restriction>
        </rdfs:subClassOf>
        <rdfs:subClassOf>
            <owl:Restriction>
                <owl:onProperty rdf:resource="https://purl.archive.org/oquo#measuresCharacteristicNegatively"/>
                <owl:someValuesFrom rdf:resource="https://purl.archive.org/oquo#IndexingAndLinkingCharacteristic"/>
            </owl:Restriction>
        </rdfs:subClassOf>
        <rdfs:subClassOf>
            <owl:Restriction>
                <owl:onProperty rdf:resource="https://purl.archive.org/oquo#measuresCharacteristicNegatively"/>
                <owl:someValuesFrom rdf:resource="https://purl.archive.org/oquo#KnowledgeReuseCharacteristic"/>
            </owl:Restriction>
        </rdfs:subClassOf>
        <rdfs:subClassOf>
            <owl:Restriction>
                <owl:onProperty rdf:resource="https://purl.archive.org/oquo#measuresCharacteristicNegatively"/>
                <owl:someValuesFrom rdf:resource="https://purl.archive.org/oquo#TextAnalysisCharacteristic"/>
            </owl:Restriction>
        </rdfs:subClassOf>
        <rdfs:subClassOf>
            <owl:Restriction>
                <owl:onProperty rdf:resource="https://purl.archive.org/oquo#measuresCharacteristicNegatively"/>
                <owl:allValuesFrom>
                    <owl:Class>
                        <owl:unionOf rdf:parseType="Collection">
                            <rdf:Description rdf:about="https://purl.archive.org/oquo#EaseOfUseCharacteristic"/>
                            <rdf:Description rdf:about="https://purl.archive.org/oquo#EfficiencyInUseCharacteristic"/>
                            <rdf:Description rdf:about="https://purl.archive.org/oquo#IndexingAndLinkingCharacteristic"/>
                            <rdf:Description rdf:about="https://purl.archive.org/oquo#KnowledgeReuseCharacteristic"/>
                            <rdf:Description rdf:about="https://purl.archive.org/oquo#TextAnalysisCharacteristic"/>
                        </owl:unionOf>
                    </owl:Class>
                </owl:allValuesFrom>
            </owl:Restriction>
        </rdfs:subClassOf>
        <rdfs:subClassOf>
            <owl:Restriction>
                <owl:onProperty rdf:resource="http://purl.org/net/QualityModel#hasScale"/>
                <owl:hasValue rdf:resource="https://purl.archive.org/oquo#ClassesWithNoSynonymMetricScale"/>
            </owl:Restriction>
        </rdfs:subClassOf>
        <obo:IAO_0000115>The Percentage of classes lacking a synonym in the ontology.</obo:IAO_0000115>
        <rdf1:acronym>CWNS</rdf1:acronym>
        <rdfs:label>classes with no synonym metric</rdfs:label>
    </owl:Class>
    



    <!-- https://purl.archive.org/oquo#DataPropertiesWithNoDescriptionMetric -->

    <owl:Class rdf:about="https://purl.archive.org/oquo#DataPropertiesWithNoDescriptionMetric">
        <rdfs:subClassOf rdf:resource="http://purl.org/net/QualityModel#DerivedMeasure"/>
        <rdfs:subClassOf>
            <owl:Restriction>
                <owl:onProperty rdf:resource="http://purl.org/net/QualityModel#hasScale"/>
                <owl:someValuesFrom>
                    <owl:Class>
                        <owl:intersectionOf rdf:parseType="Collection">
                            <rdf:Description rdf:about="https://purl.archive.org/oquo#RawScale"/>
                            <owl:Restriction>
                                <owl:onProperty rdf:resource="http://purl.org/net/QualityModel#hasRankigFunction"/>
                                <owl:hasValue rdf:resource="http://purl.org/net/QualityModel#LowerBest"/>
                            </owl:Restriction>
                        </owl:intersectionOf>
                    </owl:Class>
                </owl:someValuesFrom>
            </owl:Restriction>
        </rdfs:subClassOf>
        <rdfs:subClassOf>
            <owl:Restriction>
                <owl:onProperty rdf:resource="https://purl.archive.org/oquo#measuresCharacteristicNegatively"/>
                <owl:someValuesFrom rdf:resource="https://purl.archive.org/oquo#EaseOfUseCharacteristic"/>
            </owl:Restriction>
        </rdfs:subClassOf>
        <rdfs:subClassOf>
            <owl:Restriction>
                <owl:onProperty rdf:resource="https://purl.archive.org/oquo#measuresCharacteristicNegatively"/>
                <owl:someValuesFrom rdf:resource="https://purl.archive.org/oquo#EfficiencyInUseCharacteristic"/>
            </owl:Restriction>
        </rdfs:subClassOf>
        <rdfs:subClassOf>
            <owl:Restriction>
                <owl:onProperty rdf:resource="https://purl.archive.org/oquo#measuresCharacteristicNegatively"/>
                <owl:someValuesFrom rdf:resource="https://purl.archive.org/oquo#HelpfulnessCharacteristic"/>
            </owl:Restriction>
        </rdfs:subClassOf>
        <rdfs:subClassOf>
            <owl:Restriction>
                <owl:onProperty rdf:resource="https://purl.archive.org/oquo#measuresCharacteristicNegatively"/>
                <owl:someValuesFrom rdf:resource="https://purl.archive.org/oquo#IndexingAndLinkingCharacteristic"/>
            </owl:Restriction>
        </rdfs:subClassOf>
        <rdfs:subClassOf>
            <owl:Restriction>
                <owl:onProperty rdf:resource="https://purl.archive.org/oquo#measuresCharacteristicNegatively"/>
                <owl:someValuesFrom rdf:resource="https://purl.archive.org/oquo#KnowledgeReuseCharacteristic"/>
            </owl:Restriction>
        </rdfs:subClassOf>
        <rdfs:subClassOf>
            <owl:Restriction>
                <owl:onProperty rdf:resource="https://purl.archive.org/oquo#measuresCharacteristicNegatively"/>
                <owl:someValuesFrom rdf:resource="https://purl.archive.org/oquo#LearnabilityCharacteristic"/>
            </owl:Restriction>
        </rdfs:subClassOf>
        <rdfs:subClassOf>
            <owl:Restriction>
                <owl:onProperty rdf:resource="https://purl.archive.org/oquo#measuresCharacteristicNegatively"/>
                <owl:allValuesFrom>
                    <owl:Class>
                        <owl:unionOf rdf:parseType="Collection">
                            <rdf:Description rdf:about="https://purl.archive.org/oquo#EaseOfUseCharacteristic"/>
                            <rdf:Description rdf:about="https://purl.archive.org/oquo#EfficiencyInUseCharacteristic"/>
                            <rdf:Description rdf:about="https://purl.archive.org/oquo#HelpfulnessCharacteristic"/>
                            <rdf:Description rdf:about="https://purl.archive.org/oquo#IndexingAndLinkingCharacteristic"/>
                            <rdf:Description rdf:about="https://purl.archive.org/oquo#KnowledgeReuseCharacteristic"/>
                            <rdf:Description rdf:about="https://purl.archive.org/oquo#LearnabilityCharacteristic"/>
                        </owl:unionOf>
                    </owl:Class>
                </owl:allValuesFrom>
            </owl:Restriction>
        </rdfs:subClassOf>
        <rdfs:subClassOf>
            <owl:Restriction>
                <owl:onProperty rdf:resource="http://purl.org/net/QualityModel#hasScale"/>
                <owl:hasValue rdf:resource="https://purl.archive.org/oquo#DataPropertiesWithNoDescriptionMetricScale"/>
            </owl:Restriction>
        </rdfs:subClassOf>
        <obo:IAO_0000115>The Percentage of data properties lacking a description in the ontology.</obo:IAO_0000115>
        <rdf1:acronym>DPWND</rdf1:acronym>
        <rdfs:label>data properties with no description metric</rdfs:label>
    </owl:Class>
    


    <!-- https://purl.archive.org/oquo#DataPropertiesWithNoNameMetric -->

    <owl:Class rdf:about="https://purl.archive.org/oquo#DataPropertiesWithNoNameMetric">
        <rdfs:subClassOf rdf:resource="http://purl.org/net/QualityModel#DerivedMeasure"/>
        <rdfs:subClassOf>
            <owl:Restriction>
                <owl:onProperty rdf:resource="http://purl.org/net/QualityModel#hasScale"/>
                <owl:someValuesFrom>
                    <owl:Class>
                        <owl:intersectionOf rdf:parseType="Collection">
                            <rdf:Description rdf:about="https://purl.archive.org/oquo#RawScale"/>
                            <owl:Restriction>
                                <owl:onProperty rdf:resource="http://purl.org/net/QualityModel#hasRankigFunction"/>
                                <owl:hasValue rdf:resource="http://purl.org/net/QualityModel#LowerBest"/>
                            </owl:Restriction>
                        </owl:intersectionOf>
                    </owl:Class>
                </owl:someValuesFrom>
            </owl:Restriction>
        </rdfs:subClassOf>
        <rdfs:subClassOf>
            <owl:Restriction>
                <owl:onProperty rdf:resource="https://purl.archive.org/oquo#measuresCharacteristicNegatively"/>
                <owl:someValuesFrom rdf:resource="https://purl.archive.org/oquo#EaseOfUseCharacteristic"/>
            </owl:Restriction>
        </rdfs:subClassOf>
        <rdfs:subClassOf>
            <owl:Restriction>
                <owl:onProperty rdf:resource="https://purl.archive.org/oquo#measuresCharacteristicNegatively"/>
                <owl:someValuesFrom rdf:resource="https://purl.archive.org/oquo#EfficiencyInUseCharacteristic"/>
            </owl:Restriction>
        </rdfs:subClassOf>
        <rdfs:subClassOf>
            <owl:Restriction>
                <owl:onProperty rdf:resource="https://purl.archive.org/oquo#measuresCharacteristicNegatively"/>
                <owl:someValuesFrom rdf:resource="https://purl.archive.org/oquo#IndexingAndLinkingCharacteristic"/>
            </owl:Restriction>
        </rdfs:subClassOf>
        <rdfs:subClassOf>
            <owl:Restriction>
                <owl:onProperty rdf:resource="https://purl.archive.org/oquo#measuresCharacteristicNegatively"/>
                <owl:someValuesFrom rdf:resource="https://purl.archive.org/oquo#KnowledgeReuseCharacteristic"/>
            </owl:Restriction>
        </rdfs:subClassOf>
        <rdfs:subClassOf>
            <owl:Restriction>
                <owl:onProperty rdf:resource="https://purl.archive.org/oquo#measuresCharacteristicNegatively"/>
                <owl:someValuesFrom rdf:resource="https://purl.archive.org/oquo#TextAnalysisCharacteristic"/>
            </owl:Restriction>
        </rdfs:subClassOf>
        <rdfs:subClassOf>
            <owl:Restriction>
                <owl:onProperty rdf:resource="https://purl.archive.org/oquo#measuresCharacteristicNegatively"/>
                <owl:allValuesFrom>
                    <owl:Class>
                        <owl:unionOf rdf:parseType="Collection">
                            <rdf:Description rdf:about="https://purl.archive.org/oquo#EaseOfUseCharacteristic"/>
                            <rdf:Description rdf:about="https://purl.archive.org/oquo#EfficiencyInUseCharacteristic"/>
                            <rdf:Description rdf:about="https://purl.archive.org/oquo#IndexingAndLinkingCharacteristic"/>
                            <rdf:Description rdf:about="https://purl.archive.org/oquo#KnowledgeReuseCharacteristic"/>
                            <rdf:Description rdf:about="https://purl.archive.org/oquo#TextAnalysisCharacteristic"/>
                        </owl:unionOf>
                    </owl:Class>
                </owl:allValuesFrom>
            </owl:Restriction>
        </rdfs:subClassOf>
        <rdfs:subClassOf>
            <owl:Restriction>
                <owl:onProperty rdf:resource="http://purl.org/net/QualityModel#hasScale"/>
                <owl:hasValue rdf:resource="https://purl.archive.org/oquo#DataPropertiesWithNoNameMetricScale"/>
            </owl:Restriction>
        </rdfs:subClassOf>
        <obo:IAO_0000115>The Percentage of data properties lacking a name in the ontology.</obo:IAO_0000115>
        <rdf1:acronym>DPWNN</rdf1:acronym>
        <rdfs:label>data properties with no name metric</rdfs:label>
    </owl:Class>
    


    <!-- https://purl.archive.org/oquo#DataPropertiesWithNoSynonymMetric -->

    <owl:Class rdf:about="https://purl.archive.org/oquo#DataPropertiesWithNoSynonymMetric">
        <rdfs:subClassOf rdf:resource="http://purl.org/net/QualityModel#DerivedMeasure"/>
        <rdfs:subClassOf>
            <owl:Restriction>
                <owl:onProperty rdf:resource="http://purl.org/net/QualityModel#hasScale"/>
                <owl:someValuesFrom>
                    <owl:Class>
                        <owl:intersectionOf rdf:parseType="Collection">
                            <rdf:Description rdf:about="https://purl.archive.org/oquo#RawScale"/>
                            <owl:Restriction>
                                <owl:onProperty rdf:resource="http://purl.org/net/QualityModel#hasRankigFunction"/>
                                <owl:hasValue rdf:resource="http://purl.org/net/QualityModel#LowerBest"/>
                            </owl:Restriction>
                        </owl:intersectionOf>
                    </owl:Class>
                </owl:someValuesFrom>
            </owl:Restriction>
        </rdfs:subClassOf>
        <rdfs:subClassOf>
            <owl:Restriction>
                <owl:onProperty rdf:resource="https://purl.archive.org/oquo#measuresCharacteristicNegatively"/>
                <owl:someValuesFrom rdf:resource="https://purl.archive.org/oquo#EaseOfUseCharacteristic"/>
            </owl:Restriction>
        </rdfs:subClassOf>
        <rdfs:subClassOf>
            <owl:Restriction>
                <owl:onProperty rdf:resource="https://purl.archive.org/oquo#measuresCharacteristicNegatively"/>
                <owl:someValuesFrom rdf:resource="https://purl.archive.org/oquo#EfficiencyInUseCharacteristic"/>
            </owl:Restriction>
        </rdfs:subClassOf>
        <rdfs:subClassOf>
            <owl:Restriction>
                <owl:onProperty rdf:resource="https://purl.archive.org/oquo#measuresCharacteristicNegatively"/>
                <owl:someValuesFrom rdf:resource="https://purl.archive.org/oquo#IndexingAndLinkingCharacteristic"/>
            </owl:Restriction>
        </rdfs:subClassOf>
        <rdfs:subClassOf>
            <owl:Restriction>
                <owl:onProperty rdf:resource="https://purl.archive.org/oquo#measuresCharacteristicNegatively"/>
                <owl:someValuesFrom rdf:resource="https://purl.archive.org/oquo#KnowledgeReuseCharacteristic"/>
            </owl:Restriction>
        </rdfs:subClassOf>
        <rdfs:subClassOf>
            <owl:Restriction>
                <owl:onProperty rdf:resource="https://purl.archive.org/oquo#measuresCharacteristicNegatively"/>
                <owl:someValuesFrom rdf:resource="https://purl.archive.org/oquo#TextAnalysisCharacteristic"/>
            </owl:Restriction>
        </rdfs:subClassOf>
        <rdfs:subClassOf>
            <owl:Restriction>
                <owl:onProperty rdf:resource="https://purl.archive.org/oquo#measuresCharacteristicNegatively"/>
                <owl:allValuesFrom>
                    <owl:Class>
                        <owl:unionOf rdf:parseType="Collection">
                            <rdf:Description rdf:about="https://purl.archive.org/oquo#EaseOfUseCharacteristic"/>
                            <rdf:Description rdf:about="https://purl.archive.org/oquo#EfficiencyInUseCharacteristic"/>
                            <rdf:Description rdf:about="https://purl.archive.org/oquo#IndexingAndLinkingCharacteristic"/>
                            <rdf:Description rdf:about="https://purl.archive.org/oquo#KnowledgeReuseCharacteristic"/>
                            <rdf:Description rdf:about="https://purl.archive.org/oquo#TextAnalysisCharacteristic"/>
                        </owl:unionOf>
                    </owl:Class>
                </owl:allValuesFrom>
            </owl:Restriction>
        </rdfs:subClassOf>
        <rdfs:subClassOf>
            <owl:Restriction>
                <owl:onProperty rdf:resource="http://purl.org/net/QualityModel#hasScale"/>
                <owl:hasValue rdf:resource="https://purl.archive.org/oquo#DataPropertiesWithNoSynonymMetricScale"/>
            </owl:Restriction>
        </rdfs:subClassOf>
        <obo:IAO_0000115>The Percentage of data properties lacking a synonym in the ontology.</obo:IAO_0000115>
        <rdf1:acronym>DPWNS</rdf1:acronym>
        <rdfs:label>data properties with no synonym metric</rdfs:label>
    </owl:Class>
    




    <!-- https://purl.archive.org/oquo#DescriptionsPerAnnotationPropertyMetric -->

    <owl:Class rdf:about="https://purl.archive.org/oquo#DescriptionsPerAnnotationPropertyMetric">
        <rdfs:subClassOf rdf:resource="http://purl.org/net/QualityModel#DerivedMeasure"/>
        <rdfs:subClassOf>
            <owl:Restriction>
                <owl:onProperty rdf:resource="http://purl.org/net/QualityModel#hasScale"/>
                <owl:someValuesFrom>
                    <owl:Class>
                        <owl:intersectionOf rdf:parseType="Collection">
                            <rdf:Description rdf:about="https://purl.archive.org/oquo#RawScale"/>
                            <owl:Restriction>
                                <owl:onProperty rdf:resource="http://purl.org/net/QualityModel#hasRankigFunction"/>
                                <owl:hasValue rdf:resource="http://purl.org/net/QualityModel#HigherBest"/>
                            </owl:Restriction>
                        </owl:intersectionOf>
                    </owl:Class>
                </owl:someValuesFrom>
            </owl:Restriction>
        </rdfs:subClassOf>
        <rdfs:subClassOf>
            <owl:Restriction>
                <owl:onProperty rdf:resource="https://purl.archive.org/oquo#measuresCharacteristicPositively"/>
                <owl:someValuesFrom rdf:resource="https://purl.archive.org/oquo#EaseOfUseCharacteristic"/>
            </owl:Restriction>
        </rdfs:subClassOf>
        <rdfs:subClassOf>
            <owl:Restriction>
                <owl:onProperty rdf:resource="https://purl.archive.org/oquo#measuresCharacteristicPositively"/>
                <owl:someValuesFrom rdf:resource="https://purl.archive.org/oquo#EfficiencyInUseCharacteristic"/>
            </owl:Restriction>
        </rdfs:subClassOf>
        <rdfs:subClassOf>
            <owl:Restriction>
                <owl:onProperty rdf:resource="https://purl.archive.org/oquo#measuresCharacteristicPositively"/>
                <owl:someValuesFrom rdf:resource="https://purl.archive.org/oquo#HelpfulnessCharacteristic"/>
            </owl:Restriction>
        </rdfs:subClassOf>
        <rdfs:subClassOf>
            <owl:Restriction>
                <owl:onProperty rdf:resource="https://purl.archive.org/oquo#measuresCharacteristicPositively"/>
                <owl:someValuesFrom rdf:resource="https://purl.archive.org/oquo#IndexingAndLinkingCharacteristic"/>
            </owl:Restriction>
        </rdfs:subClassOf>
        <rdfs:subClassOf>
            <owl:Restriction>
                <owl:onProperty rdf:resource="https://purl.archive.org/oquo#measuresCharacteristicPositively"/>
                <owl:someValuesFrom rdf:resource="https://purl.archive.org/oquo#KnowledgeReuseCharacteristic"/>
            </owl:Restriction>
        </rdfs:subClassOf>
        <rdfs:subClassOf>
            <owl:Restriction>
                <owl:onProperty rdf:resource="https://purl.archive.org/oquo#measuresCharacteristicPositively"/>
                <owl:someValuesFrom rdf:resource="https://purl.archive.org/oquo#LearnabilityCharacteristic"/>
            </owl:Restriction>
        </rdfs:subClassOf>
        <rdfs:subClassOf>
            <owl:Restriction>
                <owl:onProperty rdf:resource="https://purl.archive.org/oquo#measuresCharacteristicPositively"/>
                <owl:allValuesFrom>
                    <owl:Class>
                        <owl:unionOf rdf:parseType="Collection">
                            <rdf:Description rdf:about="https://purl.archive.org/oquo#EaseOfUseCharacteristic"/>
                            <rdf:Description rdf:about="https://purl.archive.org/oquo#EfficiencyInUseCharacteristic"/>
                            <rdf:Description rdf:about="https://purl.archive.org/oquo#HelpfulnessCharacteristic"/>
                            <rdf:Description rdf:about="https://purl.archive.org/oquo#IndexingAndLinkingCharacteristic"/>
                            <rdf:Description rdf:about="https://purl.archive.org/oquo#KnowledgeReuseCharacteristic"/>
                            <rdf:Description rdf:about="https://purl.archive.org/oquo#LearnabilityCharacteristic"/>
                        </owl:unionOf>
                    </owl:Class>
                </owl:allValuesFrom>
            </owl:Restriction>
        </rdfs:subClassOf>
        <rdfs:subClassOf>
            <owl:Restriction>
                <owl:onProperty rdf:resource="http://purl.org/net/QualityModel#hasScale"/>
                <owl:hasValue rdf:resource="https://purl.archive.org/oquo#DescriptionsPerAnnotationPropertyMetricScale"/>
            </owl:Restriction>
        </rdfs:subClassOf>
        <obo:IAO_0000115 xml:lang="en">This metric accounts for the number of descriptions associated with annotation properties, which can also be provided by using different annotation properties used by the community to include descriptions (rdfs:comment, skos:definition, dcterms:description, etc.). This metric is calculated as the total number of descriptions associated with ontology annotation properties divided by the total number of annotation properties in the ontology. The range of the value of this metric is the set of real positive numbers.</obo:IAO_0000115>
        <rdf1:acronym>DxAP</rdf1:acronym>
        <rdfs:comment>The total number of annotation property descriptions over the total number of annotation properties.</rdfs:comment>
        <rdfs:label>descriptions per annotation property metric</rdfs:label>
    </owl:Class>
    


    <!-- https://purl.archive.org/oquo#DescriptionsPerClassMetric -->

    <owl:Class rdf:about="https://purl.archive.org/oquo#DescriptionsPerClassMetric">
        <rdfs:subClassOf rdf:resource="http://purl.org/net/QualityModel#DerivedMeasure"/>
        <rdfs:subClassOf>
            <owl:Restriction>
                <owl:onProperty rdf:resource="http://purl.org/net/QualityModel#hasScale"/>
                <owl:someValuesFrom>
                    <owl:Class>
                        <owl:intersectionOf rdf:parseType="Collection">
                            <rdf:Description rdf:about="https://purl.archive.org/oquo#RawScale"/>
                            <owl:Restriction>
                                <owl:onProperty rdf:resource="http://purl.org/net/QualityModel#hasRankigFunction"/>
                                <owl:hasValue rdf:resource="http://purl.org/net/QualityModel#HigherBest"/>
                            </owl:Restriction>
                        </owl:intersectionOf>
                    </owl:Class>
                </owl:someValuesFrom>
            </owl:Restriction>
        </rdfs:subClassOf>
        <rdfs:subClassOf>
            <owl:Restriction>
                <owl:onProperty rdf:resource="https://purl.archive.org/oquo#measuresCharacteristicPositively"/>
                <owl:someValuesFrom rdf:resource="https://purl.archive.org/oquo#EaseOfUseCharacteristic"/>
            </owl:Restriction>
        </rdfs:subClassOf>
        <rdfs:subClassOf>
            <owl:Restriction>
                <owl:onProperty rdf:resource="https://purl.archive.org/oquo#measuresCharacteristicPositively"/>
                <owl:someValuesFrom rdf:resource="https://purl.archive.org/oquo#EfficiencyInUseCharacteristic"/>
            </owl:Restriction>
        </rdfs:subClassOf>
        <rdfs:subClassOf>
            <owl:Restriction>
                <owl:onProperty rdf:resource="https://purl.archive.org/oquo#measuresCharacteristicPositively"/>
                <owl:someValuesFrom rdf:resource="https://purl.archive.org/oquo#HelpfulnessCharacteristic"/>
            </owl:Restriction>
        </rdfs:subClassOf>
        <rdfs:subClassOf>
            <owl:Restriction>
                <owl:onProperty rdf:resource="https://purl.archive.org/oquo#measuresCharacteristicPositively"/>
                <owl:someValuesFrom rdf:resource="https://purl.archive.org/oquo#IndexingAndLinkingCharacteristic"/>
            </owl:Restriction>
        </rdfs:subClassOf>
        <rdfs:subClassOf>
            <owl:Restriction>
                <owl:onProperty rdf:resource="https://purl.archive.org/oquo#measuresCharacteristicPositively"/>
                <owl:someValuesFrom rdf:resource="https://purl.archive.org/oquo#KnowledgeReuseCharacteristic"/>
            </owl:Restriction>
        </rdfs:subClassOf>
        <rdfs:subClassOf>
            <owl:Restriction>
                <owl:onProperty rdf:resource="https://purl.archive.org/oquo#measuresCharacteristicPositively"/>
                <owl:someValuesFrom rdf:resource="https://purl.archive.org/oquo#LearnabilityCharacteristic"/>
            </owl:Restriction>
        </rdfs:subClassOf>
        <rdfs:subClassOf>
            <owl:Restriction>
                <owl:onProperty rdf:resource="https://purl.archive.org/oquo#measuresCharacteristicPositively"/>
                <owl:allValuesFrom>
                    <owl:Class>
                        <owl:unionOf rdf:parseType="Collection">
                            <rdf:Description rdf:about="https://purl.archive.org/oquo#EaseOfUseCharacteristic"/>
                            <rdf:Description rdf:about="https://purl.archive.org/oquo#EfficiencyInUseCharacteristic"/>
                            <rdf:Description rdf:about="https://purl.archive.org/oquo#HelpfulnessCharacteristic"/>
                            <rdf:Description rdf:about="https://purl.archive.org/oquo#IndexingAndLinkingCharacteristic"/>
                            <rdf:Description rdf:about="https://purl.archive.org/oquo#KnowledgeReuseCharacteristic"/>
                            <rdf:Description rdf:about="https://purl.archive.org/oquo#LearnabilityCharacteristic"/>
                        </owl:unionOf>
                    </owl:Class>
                </owl:allValuesFrom>
            </owl:Restriction>
        </rdfs:subClassOf>
        <rdfs:subClassOf>
            <owl:Restriction>
                <owl:onProperty rdf:resource="http://purl.org/net/QualityModel#hasScale"/>
                <owl:hasValue rdf:resource="https://purl.archive.org/oquo#DescriptionsPerClassMetricScale"/>
            </owl:Restriction>
        </rdfs:subClassOf>
        <obo:IAO_0000115 xml:lang="en">This metric accounts for the number of descriptions associated with classes, which can also be provided by using different annotation properties used by the community to include descriptions (rdfs:comment, skos:definition, dcterms:description, etc.). This metric is calculated as the total number of descriptions associated with ontology classes divided by the total number of classes in the ontology. The range of the value of this metric is the set of real positive numbers.</obo:IAO_0000115>
        <rdf1:acronym>DxC</rdf1:acronym>
        <rdfs:comment>The total number of class descriptions over the total number of classes.</rdfs:comment>
        <rdfs:label>descriptions per class metric</rdfs:label>
    </owl:Class>
    


    <!-- https://purl.archive.org/oquo#DescriptionsPerDataPropertyMetric -->

    <owl:Class rdf:about="https://purl.archive.org/oquo#DescriptionsPerDataPropertyMetric">
        <rdfs:subClassOf rdf:resource="http://purl.org/net/QualityModel#DerivedMeasure"/>
        <rdfs:subClassOf>
            <owl:Restriction>
                <owl:onProperty rdf:resource="http://purl.org/net/QualityModel#hasScale"/>
                <owl:someValuesFrom>
                    <owl:Class>
                        <owl:intersectionOf rdf:parseType="Collection">
                            <rdf:Description rdf:about="https://purl.archive.org/oquo#RawScale"/>
                            <owl:Restriction>
                                <owl:onProperty rdf:resource="http://purl.org/net/QualityModel#hasRankigFunction"/>
                                <owl:hasValue rdf:resource="http://purl.org/net/QualityModel#HigherBest"/>
                            </owl:Restriction>
                        </owl:intersectionOf>
                    </owl:Class>
                </owl:someValuesFrom>
            </owl:Restriction>
        </rdfs:subClassOf>
        <rdfs:subClassOf>
            <owl:Restriction>
                <owl:onProperty rdf:resource="https://purl.archive.org/oquo#measuresCharacteristicPositively"/>
                <owl:someValuesFrom rdf:resource="https://purl.archive.org/oquo#EaseOfUseCharacteristic"/>
            </owl:Restriction>
        </rdfs:subClassOf>
        <rdfs:subClassOf>
            <owl:Restriction>
                <owl:onProperty rdf:resource="https://purl.archive.org/oquo#measuresCharacteristicPositively"/>
                <owl:someValuesFrom rdf:resource="https://purl.archive.org/oquo#EfficiencyInUseCharacteristic"/>
            </owl:Restriction>
        </rdfs:subClassOf>
        <rdfs:subClassOf>
            <owl:Restriction>
                <owl:onProperty rdf:resource="https://purl.archive.org/oquo#measuresCharacteristicPositively"/>
                <owl:someValuesFrom rdf:resource="https://purl.archive.org/oquo#HelpfulnessCharacteristic"/>
            </owl:Restriction>
        </rdfs:subClassOf>
        <rdfs:subClassOf>
            <owl:Restriction>
                <owl:onProperty rdf:resource="https://purl.archive.org/oquo#measuresCharacteristicPositively"/>
                <owl:someValuesFrom rdf:resource="https://purl.archive.org/oquo#IndexingAndLinkingCharacteristic"/>
            </owl:Restriction>
        </rdfs:subClassOf>
        <rdfs:subClassOf>
            <owl:Restriction>
                <owl:onProperty rdf:resource="https://purl.archive.org/oquo#measuresCharacteristicPositively"/>
                <owl:someValuesFrom rdf:resource="https://purl.archive.org/oquo#KnowledgeReuseCharacteristic"/>
            </owl:Restriction>
        </rdfs:subClassOf>
        <rdfs:subClassOf>
            <owl:Restriction>
                <owl:onProperty rdf:resource="https://purl.archive.org/oquo#measuresCharacteristicPositively"/>
                <owl:someValuesFrom rdf:resource="https://purl.archive.org/oquo#LearnabilityCharacteristic"/>
            </owl:Restriction>
        </rdfs:subClassOf>
        <rdfs:subClassOf>
            <owl:Restriction>
                <owl:onProperty rdf:resource="https://purl.archive.org/oquo#measuresCharacteristicPositively"/>
                <owl:allValuesFrom>
                    <owl:Class>
                        <owl:unionOf rdf:parseType="Collection">
                            <rdf:Description rdf:about="https://purl.archive.org/oquo#EaseOfUseCharacteristic"/>
                            <rdf:Description rdf:about="https://purl.archive.org/oquo#EfficiencyInUseCharacteristic"/>
                            <rdf:Description rdf:about="https://purl.archive.org/oquo#HelpfulnessCharacteristic"/>
                            <rdf:Description rdf:about="https://purl.archive.org/oquo#IndexingAndLinkingCharacteristic"/>
                            <rdf:Description rdf:about="https://purl.archive.org/oquo#KnowledgeReuseCharacteristic"/>
                            <rdf:Description rdf:about="https://purl.archive.org/oquo#LearnabilityCharacteristic"/>
                        </owl:unionOf>
                    </owl:Class>
                </owl:allValuesFrom>
            </owl:Restriction>
        </rdfs:subClassOf>
        <rdfs:subClassOf>
            <owl:Restriction>
                <owl:onProperty rdf:resource="http://purl.org/net/QualityModel#hasScale"/>
                <owl:hasValue rdf:resource="https://purl.archive.org/oquo#DescriptionsPerDataPropertyMetricScale"/>
            </owl:Restriction>
        </rdfs:subClassOf>
        <obo:IAO_0000115 xml:lang="en">This metric accounts for the number of descriptions associated with data type properties, which can also be provided by using different annotation properties used by the community to include descriptions (rdfs:comment, skos:definition, dcterms:description, etc.). This metric is calculated as the total number of descriptions associated with ontology data type properties divided by the total number of data type properties in the ontology. The range of the value of this metric is the set of real positive numbers.</obo:IAO_0000115>
        <rdf1:acronym>DxDP</rdf1:acronym>
        <rdfs:comment>The total number of data property descriptions over the total number of data properties.</rdfs:comment>
        <rdfs:label>descriptions per data property metric</rdfs:label>
    </owl:Class>
    


    <!-- https://purl.archive.org/oquo#DescriptionsPerObjectPropertyMetric -->

    <owl:Class rdf:about="https://purl.archive.org/oquo#DescriptionsPerObjectPropertyMetric">
        <rdfs:subClassOf rdf:resource="http://purl.org/net/QualityModel#DerivedMeasure"/>
        <rdfs:subClassOf>
            <owl:Restriction>
                <owl:onProperty rdf:resource="http://purl.org/net/QualityModel#hasScale"/>
                <owl:someValuesFrom>
                    <owl:Class>
                        <owl:intersectionOf rdf:parseType="Collection">
                            <rdf:Description rdf:about="https://purl.archive.org/oquo#RawScale"/>
                            <owl:Restriction>
                                <owl:onProperty rdf:resource="http://purl.org/net/QualityModel#hasRankigFunction"/>
                                <owl:hasValue rdf:resource="http://purl.org/net/QualityModel#HigherBest"/>
                            </owl:Restriction>
                        </owl:intersectionOf>
                    </owl:Class>
                </owl:someValuesFrom>
            </owl:Restriction>
        </rdfs:subClassOf>
        <rdfs:subClassOf>
            <owl:Restriction>
                <owl:onProperty rdf:resource="https://purl.archive.org/oquo#measuresCharacteristicPositively"/>
                <owl:someValuesFrom rdf:resource="https://purl.archive.org/oquo#EaseOfUseCharacteristic"/>
            </owl:Restriction>
        </rdfs:subClassOf>
        <rdfs:subClassOf>
            <owl:Restriction>
                <owl:onProperty rdf:resource="https://purl.archive.org/oquo#measuresCharacteristicPositively"/>
                <owl:someValuesFrom rdf:resource="https://purl.archive.org/oquo#EfficiencyInUseCharacteristic"/>
            </owl:Restriction>
        </rdfs:subClassOf>
        <rdfs:subClassOf>
            <owl:Restriction>
                <owl:onProperty rdf:resource="https://purl.archive.org/oquo#measuresCharacteristicPositively"/>
                <owl:someValuesFrom rdf:resource="https://purl.archive.org/oquo#HelpfulnessCharacteristic"/>
            </owl:Restriction>
        </rdfs:subClassOf>
        <rdfs:subClassOf>
            <owl:Restriction>
                <owl:onProperty rdf:resource="https://purl.archive.org/oquo#measuresCharacteristicPositively"/>
                <owl:someValuesFrom rdf:resource="https://purl.archive.org/oquo#IndexingAndLinkingCharacteristic"/>
            </owl:Restriction>
        </rdfs:subClassOf>
        <rdfs:subClassOf>
            <owl:Restriction>
                <owl:onProperty rdf:resource="https://purl.archive.org/oquo#measuresCharacteristicPositively"/>
                <owl:someValuesFrom rdf:resource="https://purl.archive.org/oquo#KnowledgeReuseCharacteristic"/>
            </owl:Restriction>
        </rdfs:subClassOf>
        <rdfs:subClassOf>
            <owl:Restriction>
                <owl:onProperty rdf:resource="https://purl.archive.org/oquo#measuresCharacteristicPositively"/>
                <owl:someValuesFrom rdf:resource="https://purl.archive.org/oquo#LearnabilityCharacteristic"/>
            </owl:Restriction>
        </rdfs:subClassOf>
        <rdfs:subClassOf>
            <owl:Restriction>
                <owl:onProperty rdf:resource="https://purl.archive.org/oquo#measuresCharacteristicPositively"/>
                <owl:allValuesFrom>
                    <owl:Class>
                        <owl:unionOf rdf:parseType="Collection">
                            <rdf:Description rdf:about="https://purl.archive.org/oquo#EaseOfUseCharacteristic"/>
                            <rdf:Description rdf:about="https://purl.archive.org/oquo#EfficiencyInUseCharacteristic"/>
                            <rdf:Description rdf:about="https://purl.archive.org/oquo#HelpfulnessCharacteristic"/>
                            <rdf:Description rdf:about="https://purl.archive.org/oquo#IndexingAndLinkingCharacteristic"/>
                            <rdf:Description rdf:about="https://purl.archive.org/oquo#KnowledgeReuseCharacteristic"/>
                            <rdf:Description rdf:about="https://purl.archive.org/oquo#LearnabilityCharacteristic"/>
                        </owl:unionOf>
                    </owl:Class>
                </owl:allValuesFrom>
            </owl:Restriction>
        </rdfs:subClassOf>
        <rdfs:subClassOf>
            <owl:Restriction>
                <owl:onProperty rdf:resource="http://purl.org/net/QualityModel#hasScale"/>
                <owl:hasValue rdf:resource="https://purl.archive.org/oquo#DescriptionsPerObjectPropertyMetricScale"/>
            </owl:Restriction>
        </rdfs:subClassOf>
        <obo:IAO_0000115 xml:lang="en">This metric accounts for the number of descriptions associated with object properties, which can also be provided by using different annotation properties used by the community to include descriptions (rdfs:comment, skos:definition, dcterms:description, etc.). This metric is calculated as the total number of descriptions associated with ontology object properties divided by the total number of object properties in the ontology. The range of the value of this metric is the set of real positive numbers.</obo:IAO_0000115>
        <rdf1:acronym>DxOP</rdf1:acronym>
        <rdfs:comment>The total number of object property descriptions over the total number of object properties.</rdfs:comment>
        <rdfs:label>descriptions per object property metric</rdfs:label>
    </owl:Class>
    


    <!-- https://purl.archive.org/oquo#DescriptionsPerPropertyMetric -->

    <owl:Class rdf:about="https://purl.archive.org/oquo#DescriptionsPerPropertyMetric">
        <rdfs:subClassOf rdf:resource="http://purl.org/net/QualityModel#DerivedMeasure"/>
        <rdfs:subClassOf>
            <owl:Restriction>
                <owl:onProperty rdf:resource="http://purl.org/net/QualityModel#hasScale"/>
                <owl:someValuesFrom>
                    <owl:Class>
                        <owl:intersectionOf rdf:parseType="Collection">
                            <rdf:Description rdf:about="https://purl.archive.org/oquo#RawScale"/>
                            <owl:Restriction>
                                <owl:onProperty rdf:resource="http://purl.org/net/QualityModel#hasRankigFunction"/>
                                <owl:hasValue rdf:resource="http://purl.org/net/QualityModel#HigherBest"/>
                            </owl:Restriction>
                        </owl:intersectionOf>
                    </owl:Class>
                </owl:someValuesFrom>
            </owl:Restriction>
        </rdfs:subClassOf>
        <rdfs:subClassOf>
            <owl:Restriction>
                <owl:onProperty rdf:resource="https://purl.archive.org/oquo#measuresCharacteristicPositively"/>
                <owl:someValuesFrom rdf:resource="https://purl.archive.org/oquo#EaseOfUseCharacteristic"/>
            </owl:Restriction>
        </rdfs:subClassOf>
        <rdfs:subClassOf>
            <owl:Restriction>
                <owl:onProperty rdf:resource="https://purl.archive.org/oquo#measuresCharacteristicPositively"/>
                <owl:someValuesFrom rdf:resource="https://purl.archive.org/oquo#EfficiencyInUseCharacteristic"/>
            </owl:Restriction>
        </rdfs:subClassOf>
        <rdfs:subClassOf>
            <owl:Restriction>
                <owl:onProperty rdf:resource="https://purl.archive.org/oquo#measuresCharacteristicPositively"/>
                <owl:someValuesFrom rdf:resource="https://purl.archive.org/oquo#HelpfulnessCharacteristic"/>
            </owl:Restriction>
        </rdfs:subClassOf>
        <rdfs:subClassOf>
            <owl:Restriction>
                <owl:onProperty rdf:resource="https://purl.archive.org/oquo#measuresCharacteristicPositively"/>
                <owl:someValuesFrom rdf:resource="https://purl.archive.org/oquo#IndexingAndLinkingCharacteristic"/>
            </owl:Restriction>
        </rdfs:subClassOf>
        <rdfs:subClassOf>
            <owl:Restriction>
                <owl:onProperty rdf:resource="https://purl.archive.org/oquo#measuresCharacteristicPositively"/>
                <owl:someValuesFrom rdf:resource="https://purl.archive.org/oquo#KnowledgeReuseCharacteristic"/>
            </owl:Restriction>
        </rdfs:subClassOf>
        <rdfs:subClassOf>
            <owl:Restriction>
                <owl:onProperty rdf:resource="https://purl.archive.org/oquo#measuresCharacteristicPositively"/>
                <owl:someValuesFrom rdf:resource="https://purl.archive.org/oquo#LearnabilityCharacteristic"/>
            </owl:Restriction>
        </rdfs:subClassOf>
        <rdfs:subClassOf>
            <owl:Restriction>
                <owl:onProperty rdf:resource="https://purl.archive.org/oquo#measuresCharacteristicPositively"/>
                <owl:allValuesFrom>
                    <owl:Class>
                        <owl:unionOf rdf:parseType="Collection">
                            <rdf:Description rdf:about="https://purl.archive.org/oquo#EaseOfUseCharacteristic"/>
                            <rdf:Description rdf:about="https://purl.archive.org/oquo#EfficiencyInUseCharacteristic"/>
                            <rdf:Description rdf:about="https://purl.archive.org/oquo#HelpfulnessCharacteristic"/>
                            <rdf:Description rdf:about="https://purl.archive.org/oquo#IndexingAndLinkingCharacteristic"/>
                            <rdf:Description rdf:about="https://purl.archive.org/oquo#KnowledgeReuseCharacteristic"/>
                            <rdf:Description rdf:about="https://purl.archive.org/oquo#LearnabilityCharacteristic"/>
                        </owl:unionOf>
                    </owl:Class>
                </owl:allValuesFrom>
            </owl:Restriction>
        </rdfs:subClassOf>
        <rdfs:subClassOf>
            <owl:Restriction>
                <owl:onProperty rdf:resource="http://purl.org/net/QualityModel#hasScale"/>
                <owl:hasValue rdf:resource="https://purl.archive.org/oquo#DescriptionsPerPropertyMetricScale"/>
            </owl:Restriction>
        </rdfs:subClassOf>
        <obo:IAO_0000115 xml:lang="en">This metric accounts for the number of descriptions associated with properties, which can also be provided by using different annotation properties used by the community to include descriptions (rdfs:comment, skos:definition, dcterms:description, etc.). This metric is calculated as the total number of descriptions associated with ontology properties (including annotation, data, and object properties) divided by the total number of properties in the ontology. The range of the value of this metric is the set of real positive numbers.</obo:IAO_0000115>
        <rdf1:acronym>DxP</rdf1:acronym>
        <rdfs:label>descriptions per property metric</rdfs:label>
    </owl:Class>
    


    <!-- https://purl.archive.org/oquo#LexicalRegularitiesPerClassMetric -->

    <owl:Class rdf:about="https://purl.archive.org/oquo#LexicalRegularitiesPerClassMetric">
        <rdfs:subClassOf rdf:resource="http://purl.org/net/QualityModel#DerivedMeasure"/>
        <rdfs:subClassOf>
            <owl:Restriction>
                <owl:onProperty rdf:resource="http://purl.org/net/QualityModel#hasScale"/>
                <owl:someValuesFrom>
                    <owl:Class>
                        <owl:intersectionOf rdf:parseType="Collection">
                            <rdf:Description rdf:about="https://purl.archive.org/oquo#RawScale"/>
                            <owl:Restriction>
                                <owl:onProperty rdf:resource="http://purl.org/net/QualityModel#hasRankigFunction"/>
                                <owl:hasValue rdf:resource="http://purl.org/net/QualityModel#HigherBest"/>
                            </owl:Restriction>
                        </owl:intersectionOf>
                    </owl:Class>
                </owl:someValuesFrom>
            </owl:Restriction>
        </rdfs:subClassOf>
        <rdfs:subClassOf>
            <owl:Restriction>
                <owl:onProperty rdf:resource="https://purl.archive.org/oquo#measuresCharacteristicPositively"/>
                <owl:someValuesFrom rdf:resource="https://purl.archive.org/oquo#StructuralAccuracyCharacteristic"/>
            </owl:Restriction>
        </rdfs:subClassOf>
        <rdfs:subClassOf>
            <owl:Restriction>
                <owl:onProperty rdf:resource="https://purl.archive.org/oquo#measuresCharacteristicPositively"/>
                <owl:someValuesFrom rdf:resource="https://purl.archive.org/oquo#TextAnalysisCharacteristic"/>
            </owl:Restriction>
        </rdfs:subClassOf>
        <rdfs:subClassOf>
            <owl:Restriction>
                <owl:onProperty rdf:resource="https://purl.archive.org/oquo#measuresCharacteristicPositively"/>
                <owl:allValuesFrom>
                    <owl:Class>
                        <owl:unionOf rdf:parseType="Collection">
                            <rdf:Description rdf:about="https://purl.archive.org/oquo#StructuralAccuracyCharacteristic"/>
                            <rdf:Description rdf:about="https://purl.archive.org/oquo#TextAnalysisCharacteristic"/>
                        </owl:unionOf>
                    </owl:Class>
                </owl:allValuesFrom>
            </owl:Restriction>
        </rdfs:subClassOf>
        <rdfs:subClassOf>
            <owl:Restriction>
                <owl:onProperty rdf:resource="http://purl.org/net/QualityModel#hasScale"/>
                <owl:hasValue rdf:resource="https://purl.archive.org/oquo#LexicalRegularitiesPerClassMetricScale"/>
            </owl:Restriction>
        </rdfs:subClassOf>
        <obo:IAO_0000115 xml:lang="en">This metric measures the proportion between the total number of lexical regularities appearing in the ontology and the total number of classes. This metric can measure whether the ontology is using genus-differentia naming style.</obo:IAO_0000115>
        <rdf1:acronym>LRsxC</rdf1:acronym>
        <rdfs:comment>The number of lexical regularities appearing in the ontology over the number of classes.</rdfs:comment>
        <rdfs:label>lexical regularities per class metric</rdfs:label>
    </owl:Class>
    


    <!-- https://purl.archive.org/oquo#LexicalRegularityClassPercentageMetric -->

    <owl:Class rdf:about="https://purl.archive.org/oquo#LexicalRegularityClassPercentageMetric">
        <rdfs:subClassOf rdf:resource="http://purl.org/net/QualityModel#DerivedMeasure"/>
        <rdfs:subClassOf>
            <owl:Restriction>
                <owl:onProperty rdf:resource="http://purl.org/net/QualityModel#hasScale"/>
                <owl:someValuesFrom>
                    <owl:Class>
                        <owl:intersectionOf rdf:parseType="Collection">
                            <rdf:Description rdf:about="https://purl.archive.org/oquo#RawScale"/>
                            <owl:Restriction>
                                <owl:onProperty rdf:resource="http://purl.org/net/QualityModel#hasRankigFunction"/>
                                <owl:hasValue rdf:resource="http://purl.org/net/QualityModel#HigherBest"/>
                            </owl:Restriction>
                        </owl:intersectionOf>
                    </owl:Class>
                </owl:someValuesFrom>
            </owl:Restriction>
        </rdfs:subClassOf>
        <rdfs:subClassOf>
            <owl:Restriction>
                <owl:onProperty rdf:resource="https://purl.archive.org/oquo#measuresCharacteristicPositively"/>
                <owl:someValuesFrom rdf:resource="https://purl.archive.org/oquo#StructuralAccuracyCharacteristic"/>
            </owl:Restriction>
        </rdfs:subClassOf>
        <rdfs:subClassOf>
            <owl:Restriction>
                <owl:onProperty rdf:resource="https://purl.archive.org/oquo#measuresCharacteristicPositively"/>
                <owl:someValuesFrom rdf:resource="https://purl.archive.org/oquo#TextAnalysisCharacteristic"/>
            </owl:Restriction>
        </rdfs:subClassOf>
        <rdfs:subClassOf>
            <owl:Restriction>
                <owl:onProperty rdf:resource="https://purl.archive.org/oquo#measuresCharacteristicPositively"/>
                <owl:allValuesFrom>
                    <owl:Class>
                        <owl:unionOf rdf:parseType="Collection">
                            <rdf:Description rdf:about="https://purl.archive.org/oquo#StructuralAccuracyCharacteristic"/>
                            <rdf:Description rdf:about="https://purl.archive.org/oquo#TextAnalysisCharacteristic"/>
                        </owl:unionOf>
                    </owl:Class>
                </owl:allValuesFrom>
            </owl:Restriction>
        </rdfs:subClassOf>
        <rdfs:subClassOf>
            <owl:Restriction>
                <owl:onProperty rdf:resource="http://purl.org/net/QualityModel#hasScale"/>
                <owl:hasValue rdf:resource="https://purl.archive.org/oquo#LexicalRegularityClassPercentageMetricScale"/>
            </owl:Restriction>
        </rdfs:subClassOf>
        <obo:IAO_0000115 xml:lang="en">The percentage of classes in the ontology that are LR classes. In other words, the percentage of classes whose complete name is a lexical regularity.</obo:IAO_0000115>
        <rdf1:acronym>LRClassPCT</rdf1:acronym>
        <rdfs:comment>The percentage of classes in the ontology that are LR classes.</rdfs:comment>
        <rdfs:label>lexical regularity class percentage metric</rdfs:label>
    </owl:Class>
    


    <!-- https://purl.archive.org/oquo#LexicallySuggestLogicallyDefineMetric -->

    <owl:Class rdf:about="https://purl.archive.org/oquo#LexicallySuggestLogicallyDefineMetric">
        <rdfs:subClassOf rdf:resource="http://purl.org/net/QualityModel#DerivedMeasure"/>
        <rdfs:subClassOf>
            <owl:Restriction>
                <owl:onProperty rdf:resource="http://purl.org/net/QualityModel#hasScale"/>
                <owl:someValuesFrom>
                    <owl:Class>
                        <owl:intersectionOf rdf:parseType="Collection">
                            <rdf:Description rdf:about="https://purl.archive.org/oquo#RawScale"/>
                            <owl:Restriction>
                                <owl:onProperty rdf:resource="http://purl.org/net/QualityModel#hasRankigFunction"/>
                                <owl:hasValue rdf:resource="http://purl.org/net/QualityModel#HigherBest"/>
                            </owl:Restriction>
                        </owl:intersectionOf>
                    </owl:Class>
                </owl:someValuesFrom>
            </owl:Restriction>
        </rdfs:subClassOf>
        <rdfs:subClassOf>
            <owl:Restriction>
                <owl:onProperty rdf:resource="https://purl.archive.org/oquo#measuresCharacteristicPositively"/>
                <owl:someValuesFrom rdf:resource="https://purl.archive.org/oquo#StructuralAccuracyCharacteristic"/>
            </owl:Restriction>
        </rdfs:subClassOf>
        <rdfs:subClassOf>
            <owl:Restriction>
                <owl:onProperty rdf:resource="https://purl.archive.org/oquo#measuresCharacteristicPositively"/>
                <owl:someValuesFrom rdf:resource="https://purl.archive.org/oquo#TextAnalysisCharacteristic"/>
            </owl:Restriction>
        </rdfs:subClassOf>
        <rdfs:subClassOf>
            <owl:Restriction>
                <owl:onProperty rdf:resource="https://purl.archive.org/oquo#measuresCharacteristicPositively"/>
                <owl:allValuesFrom>
                    <owl:Class>
                        <owl:unionOf rdf:parseType="Collection">
                            <rdf:Description rdf:about="https://purl.archive.org/oquo#StructuralAccuracyCharacteristic"/>
                            <rdf:Description rdf:about="https://purl.archive.org/oquo#TextAnalysisCharacteristic"/>
                        </owl:unionOf>
                    </owl:Class>
                </owl:allValuesFrom>
            </owl:Restriction>
        </rdfs:subClassOf>
        <rdfs:subClassOf>
            <owl:Restriction>
                <owl:onProperty rdf:resource="http://purl.org/net/QualityModel#hasScale"/>
                <owl:hasValue rdf:resource="https://purl.archive.org/oquo#LexicallySuggestLogicallyDefineMetricScale"/>
            </owl:Restriction>
        </rdfs:subClassOf>
        <obo:IAO_0000115 xml:lang="en">This metric is related to the design principle of the same name, which we interpret as follows: what is expressed in natural language for humans should be expressed as logical axioms for the machine. It is calculated as the ratio in which an LR class is semantically related to other classes exhibiting its lexical regularity. Here, two classes are semantically related if there exist a path of an arbitrary length between them through the axioms in the ontology (i.e. subclass of, equivalency, or domain/range property). For computational reasons, we limited the length of the path between classes up to 5 steps; thus, classes semantically related between them through longer paths will be considered as not semantically related. In this case, positive cases are classes exhibiting a lexical regularity and that are semantically linked with the corresponding LR class. Negative cases are classes exhibiting a lexical regularity and that are not semantically linked with the corresponding LR class. The value of the metric is calculated by dividing the positive cases by the total number of cases. This metric is calculated for each LR class. The final value of the metric for an ontology is calculated as the sum of all the positive cases divided by the sum of all the positive and negative cases obtained by each LR class in the ontology. The value is in the range [0, 1], the highest values representing the best values for the metric.</obo:IAO_0000115>
        <rdf1:acronym>LSLD</rdf1:acronym>
        <rdfs:comment>The degree in which LR classes are semantically linked to the classes exhibiting the corresponding lexical regularity.</rdfs:comment>
        <rdfs:label>lexically suggest logically define metric</rdfs:label>
    </owl:Class>
    


    <!-- https://purl.archive.org/oquo#NamesPerAnnotationPropertyMetric -->

    <owl:Class rdf:about="https://purl.archive.org/oquo#NamesPerAnnotationPropertyMetric">
        <rdfs:subClassOf rdf:resource="http://purl.org/net/QualityModel#DerivedMeasure"/>
        <rdfs:subClassOf>
            <owl:Restriction>
                <owl:onProperty rdf:resource="http://purl.org/net/QualityModel#hasScale"/>
                <owl:someValuesFrom>
                    <owl:Class>
                        <owl:intersectionOf rdf:parseType="Collection">
                            <rdf:Description rdf:about="https://purl.archive.org/oquo#RawScale"/>
                            <owl:Restriction>
                                <owl:onProperty rdf:resource="http://purl.org/net/QualityModel#hasRankigFunction"/>
                                <owl:hasValue rdf:resource="http://purl.org/net/QualityModel#HigherBest"/>
                            </owl:Restriction>
                        </owl:intersectionOf>
                    </owl:Class>
                </owl:someValuesFrom>
            </owl:Restriction>
        </rdfs:subClassOf>
        <rdfs:subClassOf>
            <owl:Restriction>
                <owl:onProperty rdf:resource="https://purl.archive.org/oquo#measuresCharacteristicPositively"/>
                <owl:someValuesFrom rdf:resource="https://purl.archive.org/oquo#EaseOfUseCharacteristic"/>
            </owl:Restriction>
        </rdfs:subClassOf>
        <rdfs:subClassOf>
            <owl:Restriction>
                <owl:onProperty rdf:resource="https://purl.archive.org/oquo#measuresCharacteristicPositively"/>
                <owl:someValuesFrom rdf:resource="https://purl.archive.org/oquo#EfficiencyInUseCharacteristic"/>
            </owl:Restriction>
        </rdfs:subClassOf>
        <rdfs:subClassOf>
            <owl:Restriction>
                <owl:onProperty rdf:resource="https://purl.archive.org/oquo#measuresCharacteristicPositively"/>
                <owl:someValuesFrom rdf:resource="https://purl.archive.org/oquo#IndexingAndLinkingCharacteristic"/>
            </owl:Restriction>
        </rdfs:subClassOf>
        <rdfs:subClassOf>
            <owl:Restriction>
                <owl:onProperty rdf:resource="https://purl.archive.org/oquo#measuresCharacteristicPositively"/>
                <owl:someValuesFrom rdf:resource="https://purl.archive.org/oquo#KnowledgeReuseCharacteristic"/>
            </owl:Restriction>
        </rdfs:subClassOf>
        <rdfs:subClassOf>
            <owl:Restriction>
                <owl:onProperty rdf:resource="https://purl.archive.org/oquo#measuresCharacteristicPositively"/>
                <owl:someValuesFrom rdf:resource="https://purl.archive.org/oquo#TextAnalysisCharacteristic"/>
            </owl:Restriction>
        </rdfs:subClassOf>
        <rdfs:subClassOf>
            <owl:Restriction>
                <owl:onProperty rdf:resource="https://purl.archive.org/oquo#measuresCharacteristicPositively"/>
                <owl:allValuesFrom>
                    <owl:Class>
                        <owl:unionOf rdf:parseType="Collection">
                            <rdf:Description rdf:about="https://purl.archive.org/oquo#EaseOfUseCharacteristic"/>
                            <rdf:Description rdf:about="https://purl.archive.org/oquo#EfficiencyInUseCharacteristic"/>
                            <rdf:Description rdf:about="https://purl.archive.org/oquo#IndexingAndLinkingCharacteristic"/>
                            <rdf:Description rdf:about="https://purl.archive.org/oquo#KnowledgeReuseCharacteristic"/>
                            <rdf:Description rdf:about="https://purl.archive.org/oquo#TextAnalysisCharacteristic"/>
                        </owl:unionOf>
                    </owl:Class>
                </owl:allValuesFrom>
            </owl:Restriction>
        </rdfs:subClassOf>
        <rdfs:subClassOf>
            <owl:Restriction>
                <owl:onProperty rdf:resource="http://purl.org/net/QualityModel#hasScale"/>
                <owl:hasValue rdf:resource="https://purl.archive.org/oquo#NamesPerAnnotationPropertyMetricScale"/>
            </owl:Restriction>
        </rdfs:subClassOf>
        <obo:IAO_0000115 xml:lang="en">This metric accounts for the number of names associated with annotation properties, and uses the list of annotation properties used by the community for names (rdfs:label, skos:prefLabel, foaf:name, etc.). Then, this metric is calculated as the number of names associated with ontology annotation properties divided by the total number of annotation properties in the ontology. The range of the value of this metric is the set of real positive numbers. Values lower than one mean that there are annotation properties without any name in the ontology. Contrariwise, a value greater than 1 indicates that there are annotation properties with multiple names; possibly caused by the inclusion of multilingual names or by some design decision.</obo:IAO_0000115>
        <rdf1:acronym>NxAP</rdf1:acronym>
        <rdfs:comment>The total number of annotation property names over the total number of annotation properties.</rdfs:comment>
        <rdfs:label>names per annotation property metric</rdfs:label>
    </owl:Class>
    


    <!-- https://purl.archive.org/oquo#NamesPerClassMetric -->

    <owl:Class rdf:about="https://purl.archive.org/oquo#NamesPerClassMetric">
        <rdfs:subClassOf rdf:resource="http://purl.org/net/QualityModel#DerivedMeasure"/>
        <rdfs:subClassOf>
            <owl:Restriction>
                <owl:onProperty rdf:resource="http://purl.org/net/QualityModel#hasScale"/>
                <owl:someValuesFrom>
                    <owl:Class>
                        <owl:intersectionOf rdf:parseType="Collection">
                            <rdf:Description rdf:about="https://purl.archive.org/oquo#RawScale"/>
                            <owl:Restriction>
                                <owl:onProperty rdf:resource="http://purl.org/net/QualityModel#hasRankigFunction"/>
                                <owl:hasValue rdf:resource="http://purl.org/net/QualityModel#HigherBest"/>
                            </owl:Restriction>
                        </owl:intersectionOf>
                    </owl:Class>
                </owl:someValuesFrom>
            </owl:Restriction>
        </rdfs:subClassOf>
        <rdfs:subClassOf>
            <owl:Restriction>
                <owl:onProperty rdf:resource="https://purl.archive.org/oquo#measuresCharacteristicPositively"/>
                <owl:someValuesFrom rdf:resource="https://purl.archive.org/oquo#EaseOfUseCharacteristic"/>
            </owl:Restriction>
        </rdfs:subClassOf>
        <rdfs:subClassOf>
            <owl:Restriction>
                <owl:onProperty rdf:resource="https://purl.archive.org/oquo#measuresCharacteristicPositively"/>
                <owl:someValuesFrom rdf:resource="https://purl.archive.org/oquo#EfficiencyInUseCharacteristic"/>
            </owl:Restriction>
        </rdfs:subClassOf>
        <rdfs:subClassOf>
            <owl:Restriction>
                <owl:onProperty rdf:resource="https://purl.archive.org/oquo#measuresCharacteristicPositively"/>
                <owl:someValuesFrom rdf:resource="https://purl.archive.org/oquo#IndexingAndLinkingCharacteristic"/>
            </owl:Restriction>
        </rdfs:subClassOf>
        <rdfs:subClassOf>
            <owl:Restriction>
                <owl:onProperty rdf:resource="https://purl.archive.org/oquo#measuresCharacteristicPositively"/>
                <owl:someValuesFrom rdf:resource="https://purl.archive.org/oquo#KnowledgeReuseCharacteristic"/>
            </owl:Restriction>
        </rdfs:subClassOf>
        <rdfs:subClassOf>
            <owl:Restriction>
                <owl:onProperty rdf:resource="https://purl.archive.org/oquo#measuresCharacteristicPositively"/>
                <owl:someValuesFrom rdf:resource="https://purl.archive.org/oquo#TextAnalysisCharacteristic"/>
            </owl:Restriction>
        </rdfs:subClassOf>
        <rdfs:subClassOf>
            <owl:Restriction>
                <owl:onProperty rdf:resource="https://purl.archive.org/oquo#measuresCharacteristicPositively"/>
                <owl:allValuesFrom>
                    <owl:Class>
                        <owl:unionOf rdf:parseType="Collection">
                            <rdf:Description rdf:about="https://purl.archive.org/oquo#EaseOfUseCharacteristic"/>
                            <rdf:Description rdf:about="https://purl.archive.org/oquo#EfficiencyInUseCharacteristic"/>
                            <rdf:Description rdf:about="https://purl.archive.org/oquo#IndexingAndLinkingCharacteristic"/>
                            <rdf:Description rdf:about="https://purl.archive.org/oquo#KnowledgeReuseCharacteristic"/>
                            <rdf:Description rdf:about="https://purl.archive.org/oquo#TextAnalysisCharacteristic"/>
                        </owl:unionOf>
                    </owl:Class>
                </owl:allValuesFrom>
            </owl:Restriction>
        </rdfs:subClassOf>
        <rdfs:subClassOf>
            <owl:Restriction>
                <owl:onProperty rdf:resource="http://purl.org/net/QualityModel#hasScale"/>
                <owl:hasValue rdf:resource="https://purl.archive.org/oquo#NamesPerClassMetricScale"/>
            </owl:Restriction>
        </rdfs:subClassOf>
        <obo:IAO_0000115 xml:lang="en">This metric accounts for the number of names associated with classes, and uses the list of annotation properties used by the community for names (rdfs:label, skos:prefLabel, foaf:name, etc.). Then, this metric is calculated as the number of names associated with ontology classes divided by the total number of classes in the ontology. The range of the value of this metric is the set of real positive numbers. Values lower than one mean that there are classes without any name in the ontology. Contrariwise, a value greater than 1 indicates that there are classes with multiple names; possibly caused by the inclusion of multilingual names or by some design decision.</obo:IAO_0000115>
        <rdf1:acronym>NxC</rdf1:acronym>
        <rdfs:comment>The total number of class names over the total number of classes.</rdfs:comment>
        <rdfs:label>names per class metric</rdfs:label>
    </owl:Class>
    


    <!-- https://purl.archive.org/oquo#NamesPerDataPropertyMetric -->

    <owl:Class rdf:about="https://purl.archive.org/oquo#NamesPerDataPropertyMetric">
        <rdfs:subClassOf rdf:resource="http://purl.org/net/QualityModel#DerivedMeasure"/>
        <rdfs:subClassOf>
            <owl:Restriction>
                <owl:onProperty rdf:resource="http://purl.org/net/QualityModel#hasScale"/>
                <owl:someValuesFrom>
                    <owl:Class>
                        <owl:intersectionOf rdf:parseType="Collection">
                            <rdf:Description rdf:about="https://purl.archive.org/oquo#RawScale"/>
                            <owl:Restriction>
                                <owl:onProperty rdf:resource="http://purl.org/net/QualityModel#hasRankigFunction"/>
                                <owl:hasValue rdf:resource="http://purl.org/net/QualityModel#HigherBest"/>
                            </owl:Restriction>
                        </owl:intersectionOf>
                    </owl:Class>
                </owl:someValuesFrom>
            </owl:Restriction>
        </rdfs:subClassOf>
        <rdfs:subClassOf>
            <owl:Restriction>
                <owl:onProperty rdf:resource="https://purl.archive.org/oquo#measuresCharacteristicPositively"/>
                <owl:someValuesFrom rdf:resource="https://purl.archive.org/oquo#EaseOfUseCharacteristic"/>
            </owl:Restriction>
        </rdfs:subClassOf>
        <rdfs:subClassOf>
            <owl:Restriction>
                <owl:onProperty rdf:resource="https://purl.archive.org/oquo#measuresCharacteristicPositively"/>
                <owl:someValuesFrom rdf:resource="https://purl.archive.org/oquo#EfficiencyInUseCharacteristic"/>
            </owl:Restriction>
        </rdfs:subClassOf>
        <rdfs:subClassOf>
            <owl:Restriction>
                <owl:onProperty rdf:resource="https://purl.archive.org/oquo#measuresCharacteristicPositively"/>
                <owl:someValuesFrom rdf:resource="https://purl.archive.org/oquo#IndexingAndLinkingCharacteristic"/>
            </owl:Restriction>
        </rdfs:subClassOf>
        <rdfs:subClassOf>
            <owl:Restriction>
                <owl:onProperty rdf:resource="https://purl.archive.org/oquo#measuresCharacteristicPositively"/>
                <owl:someValuesFrom rdf:resource="https://purl.archive.org/oquo#KnowledgeReuseCharacteristic"/>
            </owl:Restriction>
        </rdfs:subClassOf>
        <rdfs:subClassOf>
            <owl:Restriction>
                <owl:onProperty rdf:resource="https://purl.archive.org/oquo#measuresCharacteristicPositively"/>
                <owl:someValuesFrom rdf:resource="https://purl.archive.org/oquo#TextAnalysisCharacteristic"/>
            </owl:Restriction>
        </rdfs:subClassOf>
        <rdfs:subClassOf>
            <owl:Restriction>
                <owl:onProperty rdf:resource="https://purl.archive.org/oquo#measuresCharacteristicPositively"/>
                <owl:allValuesFrom>
                    <owl:Class>
                        <owl:unionOf rdf:parseType="Collection">
                            <rdf:Description rdf:about="https://purl.archive.org/oquo#EaseOfUseCharacteristic"/>
                            <rdf:Description rdf:about="https://purl.archive.org/oquo#EfficiencyInUseCharacteristic"/>
                            <rdf:Description rdf:about="https://purl.archive.org/oquo#IndexingAndLinkingCharacteristic"/>
                            <rdf:Description rdf:about="https://purl.archive.org/oquo#KnowledgeReuseCharacteristic"/>
                            <rdf:Description rdf:about="https://purl.archive.org/oquo#TextAnalysisCharacteristic"/>
                        </owl:unionOf>
                    </owl:Class>
                </owl:allValuesFrom>
            </owl:Restriction>
        </rdfs:subClassOf>
        <rdfs:subClassOf>
            <owl:Restriction>
                <owl:onProperty rdf:resource="http://purl.org/net/QualityModel#hasScale"/>
                <owl:hasValue rdf:resource="https://purl.archive.org/oquo#NamesPerDataPropertyMetricScale"/>
            </owl:Restriction>
        </rdfs:subClassOf>
        <obo:IAO_0000115 xml:lang="en">This metric accounts for the number of names associated with data type properties, and uses the list of annotation properties used by the community for names (rdfs:label, skos:prefLabel, foaf:name, etc.). Then, this metric is calculated as the number of names associated with ontology data type properties divided by the total number of data type properties in the ontology. The range of the value of this metric is the set of real positive numbers. Values lower than one mean that there are data type properties without any name in the ontology. Contrariwise, a value greater than 1 indicates that there are data type properties with multiple names; possibly caused by the inclusion of multilingual names or by some design decision.</obo:IAO_0000115>
        <rdf1:acronym>NxDP</rdf1:acronym>
        <rdfs:comment>The total number of data property names over the total number of data properties.</rdfs:comment>
        <rdfs:label>names per data property metric</rdfs:label>
    </owl:Class>
    


    <!-- https://purl.archive.org/oquo#NamesPerObjectPropertyMetric -->

    <owl:Class rdf:about="https://purl.archive.org/oquo#NamesPerObjectPropertyMetric">
        <rdfs:subClassOf rdf:resource="http://purl.org/net/QualityModel#DerivedMeasure"/>
        <rdfs:subClassOf>
            <owl:Restriction>
                <owl:onProperty rdf:resource="http://purl.org/net/QualityModel#hasScale"/>
                <owl:someValuesFrom>
                    <owl:Class>
                        <owl:intersectionOf rdf:parseType="Collection">
                            <rdf:Description rdf:about="https://purl.archive.org/oquo#RawScale"/>
                            <owl:Restriction>
                                <owl:onProperty rdf:resource="http://purl.org/net/QualityModel#hasRankigFunction"/>
                                <owl:hasValue rdf:resource="http://purl.org/net/QualityModel#HigherBest"/>
                            </owl:Restriction>
                        </owl:intersectionOf>
                    </owl:Class>
                </owl:someValuesFrom>
            </owl:Restriction>
        </rdfs:subClassOf>
        <rdfs:subClassOf>
            <owl:Restriction>
                <owl:onProperty rdf:resource="https://purl.archive.org/oquo#measuresCharacteristicPositively"/>
                <owl:someValuesFrom rdf:resource="https://purl.archive.org/oquo#EaseOfUseCharacteristic"/>
            </owl:Restriction>
        </rdfs:subClassOf>
        <rdfs:subClassOf>
            <owl:Restriction>
                <owl:onProperty rdf:resource="https://purl.archive.org/oquo#measuresCharacteristicPositively"/>
                <owl:someValuesFrom rdf:resource="https://purl.archive.org/oquo#EfficiencyInUseCharacteristic"/>
            </owl:Restriction>
        </rdfs:subClassOf>
        <rdfs:subClassOf>
            <owl:Restriction>
                <owl:onProperty rdf:resource="https://purl.archive.org/oquo#measuresCharacteristicPositively"/>
                <owl:someValuesFrom rdf:resource="https://purl.archive.org/oquo#IndexingAndLinkingCharacteristic"/>
            </owl:Restriction>
        </rdfs:subClassOf>
        <rdfs:subClassOf>
            <owl:Restriction>
                <owl:onProperty rdf:resource="https://purl.archive.org/oquo#measuresCharacteristicPositively"/>
                <owl:someValuesFrom rdf:resource="https://purl.archive.org/oquo#KnowledgeReuseCharacteristic"/>
            </owl:Restriction>
        </rdfs:subClassOf>
        <rdfs:subClassOf>
            <owl:Restriction>
                <owl:onProperty rdf:resource="https://purl.archive.org/oquo#measuresCharacteristicPositively"/>
                <owl:someValuesFrom rdf:resource="https://purl.archive.org/oquo#TextAnalysisCharacteristic"/>
            </owl:Restriction>
        </rdfs:subClassOf>
        <rdfs:subClassOf>
            <owl:Restriction>
                <owl:onProperty rdf:resource="https://purl.archive.org/oquo#measuresCharacteristicPositively"/>
                <owl:allValuesFrom>
                    <owl:Class>
                        <owl:unionOf rdf:parseType="Collection">
                            <rdf:Description rdf:about="https://purl.archive.org/oquo#EaseOfUseCharacteristic"/>
                            <rdf:Description rdf:about="https://purl.archive.org/oquo#EfficiencyInUseCharacteristic"/>
                            <rdf:Description rdf:about="https://purl.archive.org/oquo#IndexingAndLinkingCharacteristic"/>
                            <rdf:Description rdf:about="https://purl.archive.org/oquo#KnowledgeReuseCharacteristic"/>
                            <rdf:Description rdf:about="https://purl.archive.org/oquo#TextAnalysisCharacteristic"/>
                        </owl:unionOf>
                    </owl:Class>
                </owl:allValuesFrom>
            </owl:Restriction>
        </rdfs:subClassOf>
        <rdfs:subClassOf>
            <owl:Restriction>
                <owl:onProperty rdf:resource="http://purl.org/net/QualityModel#hasScale"/>
                <owl:hasValue rdf:resource="https://purl.archive.org/oquo#NamesPerObjectPropertyMetricScale"/>
            </owl:Restriction>
        </rdfs:subClassOf>
        <obo:IAO_0000115 xml:lang="en">This metric accounts for the number of names associated with object properties, and uses the list of annotation properties used by the community for names (rdfs:label, skos:prefLabel, foaf:name, etc.). Then, this metric is calculated as the number of names associated with ontology object properties divided by the total number of object properties in the ontology. The range of the value of this metric is the set of real positive numbers. Values lower than one mean that there are object properties without any name in the ontology. Contrariwise, a value greater than 1 indicates that there are object properties with multiple names; possibly caused by the inclusion of multilingual names or by some design decision.</obo:IAO_0000115>
        <rdf1:acronym>NxOP</rdf1:acronym>
        <rdfs:comment>The total number of object property names over the total number of object properties.</rdfs:comment>
        <rdfs:label>names per object property metric</rdfs:label>
    </owl:Class>
    


    <!-- https://purl.archive.org/oquo#NamesPerPropertyMetric -->

    <owl:Class rdf:about="https://purl.archive.org/oquo#NamesPerPropertyMetric">
        <rdfs:subClassOf rdf:resource="http://purl.org/net/QualityModel#DerivedMeasure"/>
        <rdfs:subClassOf>
            <owl:Restriction>
                <owl:onProperty rdf:resource="http://purl.org/net/QualityModel#hasScale"/>
                <owl:someValuesFrom>
                    <owl:Class>
                        <owl:intersectionOf rdf:parseType="Collection">
                            <rdf:Description rdf:about="https://purl.archive.org/oquo#RawScale"/>
                            <owl:Restriction>
                                <owl:onProperty rdf:resource="http://purl.org/net/QualityModel#hasRankigFunction"/>
                                <owl:hasValue rdf:resource="http://purl.org/net/QualityModel#HigherBest"/>
                            </owl:Restriction>
                        </owl:intersectionOf>
                    </owl:Class>
                </owl:someValuesFrom>
            </owl:Restriction>
        </rdfs:subClassOf>
        <rdfs:subClassOf>
            <owl:Restriction>
                <owl:onProperty rdf:resource="https://purl.archive.org/oquo#measuresCharacteristicPositively"/>
                <owl:someValuesFrom rdf:resource="https://purl.archive.org/oquo#EaseOfUseCharacteristic"/>
            </owl:Restriction>
        </rdfs:subClassOf>
        <rdfs:subClassOf>
            <owl:Restriction>
                <owl:onProperty rdf:resource="https://purl.archive.org/oquo#measuresCharacteristicPositively"/>
                <owl:someValuesFrom rdf:resource="https://purl.archive.org/oquo#EfficiencyInUseCharacteristic"/>
            </owl:Restriction>
        </rdfs:subClassOf>
        <rdfs:subClassOf>
            <owl:Restriction>
                <owl:onProperty rdf:resource="https://purl.archive.org/oquo#measuresCharacteristicPositively"/>
                <owl:someValuesFrom rdf:resource="https://purl.archive.org/oquo#HelpfulnessCharacteristic"/>
            </owl:Restriction>
        </rdfs:subClassOf>
        <rdfs:subClassOf>
            <owl:Restriction>
                <owl:onProperty rdf:resource="https://purl.archive.org/oquo#measuresCharacteristicPositively"/>
                <owl:someValuesFrom rdf:resource="https://purl.archive.org/oquo#IndexingAndLinkingCharacteristic"/>
            </owl:Restriction>
        </rdfs:subClassOf>
        <rdfs:subClassOf>
            <owl:Restriction>
                <owl:onProperty rdf:resource="https://purl.archive.org/oquo#measuresCharacteristicPositively"/>
                <owl:someValuesFrom rdf:resource="https://purl.archive.org/oquo#KnowledgeReuseCharacteristic"/>
            </owl:Restriction>
        </rdfs:subClassOf>
        <rdfs:subClassOf>
            <owl:Restriction>
                <owl:onProperty rdf:resource="https://purl.archive.org/oquo#measuresCharacteristicPositively"/>
                <owl:someValuesFrom rdf:resource="https://purl.archive.org/oquo#LearnabilityCharacteristic"/>
            </owl:Restriction>
        </rdfs:subClassOf>
        <rdfs:subClassOf>
            <owl:Restriction>
                <owl:onProperty rdf:resource="https://purl.archive.org/oquo#measuresCharacteristicPositively"/>
                <owl:allValuesFrom>
                    <owl:Class>
                        <owl:unionOf rdf:parseType="Collection">
                            <rdf:Description rdf:about="https://purl.archive.org/oquo#EaseOfUseCharacteristic"/>
                            <rdf:Description rdf:about="https://purl.archive.org/oquo#EfficiencyInUseCharacteristic"/>
                            <rdf:Description rdf:about="https://purl.archive.org/oquo#HelpfulnessCharacteristic"/>
                            <rdf:Description rdf:about="https://purl.archive.org/oquo#IndexingAndLinkingCharacteristic"/>
                            <rdf:Description rdf:about="https://purl.archive.org/oquo#KnowledgeReuseCharacteristic"/>
                            <rdf:Description rdf:about="https://purl.archive.org/oquo#LearnabilityCharacteristic"/>
                        </owl:unionOf>
                    </owl:Class>
                </owl:allValuesFrom>
            </owl:Restriction>
        </rdfs:subClassOf>
        <rdfs:subClassOf>
            <owl:Restriction>
                <owl:onProperty rdf:resource="http://purl.org/net/QualityModel#hasScale"/>
                <owl:hasValue rdf:resource="https://purl.archive.org/oquo#NamesPerPropertyMetricScale"/>
            </owl:Restriction>
        </rdfs:subClassOf>
        <obo:IAO_0000115 xml:lang="en">This metric accounts for the number of names associated with properties, which can also be provided by using different annotation properties used by the community to include names (rdfs:label, skos:prefLabel, foaf:name, etc.). This metric is calculated as the total number of names associated with ontology properties (including annotation, data, and object properties) divided by the total number of properties in the ontology. The range of the value of this metric is the set of real positive numbers.</obo:IAO_0000115>
        <rdf1:acronym>DxP</rdf1:acronym>
        <rdfs:label>names per property metric</rdfs:label>
    </owl:Class>


    <!-- https://purl.archive.org/oquo#NumberOfClassesMetric -->

    <owl:Class rdf:about="https://purl.archive.org/oquo#NumberOfClassesMetric">
        <rdfs:subClassOf rdf:resource="http://purl.org/net/QualityModel#BaseMeasure"/>
        <obo:IAO_0000115>This metric calculates the number of classes asserted in the ontology.</obo:IAO_0000115>
        <rdf1:acronym>NCLASSES</rdf1:acronym>
        <rdfs:label>number of classes metric</rdfs:label>
    </owl:Class>
    


    <!-- https://purl.archive.org/oquo#NumberOfLexicalRegularitiesMetric -->

    <owl:Class rdf:about="https://purl.archive.org/oquo#NumberOfLexicalRegularitiesMetric">
        <rdfs:subClassOf rdf:resource="http://purl.org/net/QualityModel#DerivedMeasure"/>
        <rdfs:subClassOf>
            <owl:Restriction>
                <owl:onProperty rdf:resource="http://purl.org/net/QualityModel#hasScale"/>
                <owl:someValuesFrom>
                    <owl:Class>
                        <owl:intersectionOf rdf:parseType="Collection">
                            <rdf:Description rdf:about="https://purl.archive.org/oquo#RawScale"/>
                            <owl:Restriction>
                                <owl:onProperty rdf:resource="http://purl.org/net/QualityModel#hasRankigFunction"/>
                                <owl:hasValue rdf:resource="http://purl.org/net/QualityModel#HigherBest"/>
                            </owl:Restriction>
                        </owl:intersectionOf>
                    </owl:Class>
                </owl:someValuesFrom>
            </owl:Restriction>
        </rdfs:subClassOf>
        <rdfs:subClassOf>
            <owl:Restriction>
                <owl:onProperty rdf:resource="https://purl.archive.org/oquo#measuresCharacteristicPositively"/>
                <owl:someValuesFrom rdf:resource="https://purl.archive.org/oquo#ControlledVocabularyCharacteristic"/>
            </owl:Restriction>
        </rdfs:subClassOf>
        <rdfs:subClassOf>
            <owl:Restriction>
                <owl:onProperty rdf:resource="https://purl.archive.org/oquo#measuresCharacteristicPositively"/>
                <owl:allValuesFrom>
                    <owl:Class>
                        <owl:unionOf rdf:parseType="Collection">
                            <rdf:Description rdf:about="https://purl.archive.org/oquo#ControlledVocabularyCharacteristic"/>
                        </owl:unionOf>
                    </owl:Class>
                </owl:allValuesFrom>
            </owl:Restriction>
        </rdfs:subClassOf>
        <rdfs:subClassOf>
            <owl:Restriction>
                <owl:onProperty rdf:resource="http://purl.org/net/QualityModel#hasScale"/>
                <owl:hasValue rdf:resource="https://purl.archive.org/oquo#NumberOfLexicalRegularitiesMetricScale"/>
            </owl:Restriction>
        </rdfs:subClassOf>
        <obo:IAO_0000115 xml:lang="en">This metric examines the names of the ontology classes, stabished by using &apos;rdfs:label&apos;, and identifies the number of lexical regularities appearing in the ontology.</obo:IAO_0000115>
        <rdf1:acronym>NLR</rdf1:acronym>
        <rdfs:comment>The number of lexical regularities found in the ontology.</rdfs:comment>
        <rdfs:label>number of lexical regularities metric</rdfs:label>
    </owl:Class>
    


    <!-- https://purl.archive.org/oquo#NumberOfLexicalRegularityClassesMetric -->

    <owl:Class rdf:about="https://purl.archive.org/oquo#NumberOfLexicalRegularityClassesMetric">
        <rdfs:subClassOf rdf:resource="http://purl.org/net/QualityModel#DerivedMeasure"/>
        <rdfs:subClassOf>
            <owl:Restriction>
                <owl:onProperty rdf:resource="http://purl.org/net/QualityModel#hasScale"/>
                <owl:someValuesFrom>
                    <owl:Class>
                        <owl:intersectionOf rdf:parseType="Collection">
                            <rdf:Description rdf:about="https://purl.archive.org/oquo#RawScale"/>
                            <owl:Restriction>
                                <owl:onProperty rdf:resource="http://purl.org/net/QualityModel#hasRankigFunction"/>
                                <owl:hasValue rdf:resource="http://purl.org/net/QualityModel#HigherBest"/>
                            </owl:Restriction>
                        </owl:intersectionOf>
                    </owl:Class>
                </owl:someValuesFrom>
            </owl:Restriction>
        </rdfs:subClassOf>
        <rdfs:subClassOf>
            <owl:Restriction>
                <owl:onProperty rdf:resource="https://purl.archive.org/oquo#measuresCharacteristicPositively"/>
                <owl:someValuesFrom rdf:resource="https://purl.archive.org/oquo#ControlledVocabularyCharacteristic"/>
            </owl:Restriction>
        </rdfs:subClassOf>
        <rdfs:subClassOf>
            <owl:Restriction>
                <owl:onProperty rdf:resource="https://purl.archive.org/oquo#measuresCharacteristicPositively"/>
                <owl:allValuesFrom>
                    <owl:Class>
                        <owl:unionOf rdf:parseType="Collection">
                            <rdf:Description rdf:about="https://purl.archive.org/oquo#ControlledVocabularyCharacteristic"/>
                        </owl:unionOf>
                    </owl:Class>
                </owl:allValuesFrom>
            </owl:Restriction>
        </rdfs:subClassOf>
        <rdfs:subClassOf>
            <owl:Restriction>
                <owl:onProperty rdf:resource="http://purl.org/net/QualityModel#hasScale"/>
                <owl:hasValue rdf:resource="https://purl.archive.org/oquo#NumberOfLexicalRegularityClassesMetricScale"/>
            </owl:Restriction>
        </rdfs:subClassOf>
        <obo:IAO_0000115 xml:lang="en">This metric returns the number of ontology classes whose complete name, set by using &apos;rdfs:label&apos;, is a lexical regularity.</obo:IAO_0000115>
        <rdf1:acronym>NLRC</rdf1:acronym>
        <rdfs:comment>The number of ontology classes whose name is a lexical regularity.</rdfs:comment>
        <rdfs:label>number of lexical regularity classes metric</rdfs:label>
    </owl:Class>
    


    <!-- https://purl.archive.org/oquo#ObjectPropertiesWithNoDescriptionMetric -->

    <owl:Class rdf:about="https://purl.archive.org/oquo#ObjectPropertiesWithNoDescriptionMetric">
        <rdfs:subClassOf rdf:resource="http://purl.org/net/QualityModel#DerivedMeasure"/>
        <rdfs:subClassOf>
            <owl:Restriction>
                <owl:onProperty rdf:resource="http://purl.org/net/QualityModel#hasScale"/>
                <owl:someValuesFrom>
                    <owl:Class>
                        <owl:intersectionOf rdf:parseType="Collection">
                            <rdf:Description rdf:about="https://purl.archive.org/oquo#RawScale"/>
                            <owl:Restriction>
                                <owl:onProperty rdf:resource="http://purl.org/net/QualityModel#hasRankigFunction"/>
                                <owl:hasValue rdf:resource="http://purl.org/net/QualityModel#LowerBest"/>
                            </owl:Restriction>
                        </owl:intersectionOf>
                    </owl:Class>
                </owl:someValuesFrom>
            </owl:Restriction>
        </rdfs:subClassOf>
        <rdfs:subClassOf>
            <owl:Restriction>
                <owl:onProperty rdf:resource="https://purl.archive.org/oquo#measuresCharacteristicNegatively"/>
                <owl:someValuesFrom rdf:resource="https://purl.archive.org/oquo#EaseOfUseCharacteristic"/>
            </owl:Restriction>
        </rdfs:subClassOf>
        <rdfs:subClassOf>
            <owl:Restriction>
                <owl:onProperty rdf:resource="https://purl.archive.org/oquo#measuresCharacteristicNegatively"/>
                <owl:someValuesFrom rdf:resource="https://purl.archive.org/oquo#EfficiencyInUseCharacteristic"/>
            </owl:Restriction>
        </rdfs:subClassOf>
        <rdfs:subClassOf>
            <owl:Restriction>
                <owl:onProperty rdf:resource="https://purl.archive.org/oquo#measuresCharacteristicNegatively"/>
                <owl:someValuesFrom rdf:resource="https://purl.archive.org/oquo#HelpfulnessCharacteristic"/>
            </owl:Restriction>
        </rdfs:subClassOf>
        <rdfs:subClassOf>
            <owl:Restriction>
                <owl:onProperty rdf:resource="https://purl.archive.org/oquo#measuresCharacteristicNegatively"/>
                <owl:someValuesFrom rdf:resource="https://purl.archive.org/oquo#IndexingAndLinkingCharacteristic"/>
            </owl:Restriction>
        </rdfs:subClassOf>
        <rdfs:subClassOf>
            <owl:Restriction>
                <owl:onProperty rdf:resource="https://purl.archive.org/oquo#measuresCharacteristicNegatively"/>
                <owl:someValuesFrom rdf:resource="https://purl.archive.org/oquo#KnowledgeReuseCharacteristic"/>
            </owl:Restriction>
        </rdfs:subClassOf>
        <rdfs:subClassOf>
            <owl:Restriction>
                <owl:onProperty rdf:resource="https://purl.archive.org/oquo#measuresCharacteristicNegatively"/>
                <owl:someValuesFrom rdf:resource="https://purl.archive.org/oquo#LearnabilityCharacteristic"/>
            </owl:Restriction>
        </rdfs:subClassOf>
        <rdfs:subClassOf>
            <owl:Restriction>
                <owl:onProperty rdf:resource="https://purl.archive.org/oquo#measuresCharacteristicNegatively"/>
                <owl:allValuesFrom>
                    <owl:Class>
                        <owl:unionOf rdf:parseType="Collection">
                            <rdf:Description rdf:about="https://purl.archive.org/oquo#EaseOfUseCharacteristic"/>
                            <rdf:Description rdf:about="https://purl.archive.org/oquo#EfficiencyInUseCharacteristic"/>
                            <rdf:Description rdf:about="https://purl.archive.org/oquo#HelpfulnessCharacteristic"/>
                            <rdf:Description rdf:about="https://purl.archive.org/oquo#IndexingAndLinkingCharacteristic"/>
                            <rdf:Description rdf:about="https://purl.archive.org/oquo#KnowledgeReuseCharacteristic"/>
                            <rdf:Description rdf:about="https://purl.archive.org/oquo#LearnabilityCharacteristic"/>
                        </owl:unionOf>
                    </owl:Class>
                </owl:allValuesFrom>
            </owl:Restriction>
        </rdfs:subClassOf>
        <rdfs:subClassOf>
            <owl:Restriction>
                <owl:onProperty rdf:resource="http://purl.org/net/QualityModel#hasScale"/>
                <owl:hasValue rdf:resource="https://purl.archive.org/oquo#ObjectPropertiesWithNoDescriptionMetricScale"/>
            </owl:Restriction>
        </rdfs:subClassOf>
        <obo:IAO_0000115>The Percentage of object properties lacking a description in the ontology.</obo:IAO_0000115>
        <rdf1:acronym>OPWND</rdf1:acronym>
        <rdfs:label>object properties with no description metric</rdfs:label>
    </owl:Class>
    


    <!-- https://purl.archive.org/oquo#ObjectPropertiesWithNoNameMetric -->

    <owl:Class rdf:about="https://purl.archive.org/oquo#ObjectPropertiesWithNoNameMetric">
        <rdfs:subClassOf rdf:resource="http://purl.org/net/QualityModel#DerivedMeasure"/>
        <rdfs:subClassOf>
            <owl:Restriction>
                <owl:onProperty rdf:resource="http://purl.org/net/QualityModel#hasScale"/>
                <owl:someValuesFrom>
                    <owl:Class>
                        <owl:intersectionOf rdf:parseType="Collection">
                            <rdf:Description rdf:about="https://purl.archive.org/oquo#RawScale"/>
                            <owl:Restriction>
                                <owl:onProperty rdf:resource="http://purl.org/net/QualityModel#hasRankigFunction"/>
                                <owl:hasValue rdf:resource="http://purl.org/net/QualityModel#LowerBest"/>
                            </owl:Restriction>
                        </owl:intersectionOf>
                    </owl:Class>
                </owl:someValuesFrom>
            </owl:Restriction>
        </rdfs:subClassOf>
        <rdfs:subClassOf>
            <owl:Restriction>
                <owl:onProperty rdf:resource="https://purl.archive.org/oquo#measuresCharacteristicNegatively"/>
                <owl:someValuesFrom rdf:resource="https://purl.archive.org/oquo#EaseOfUseCharacteristic"/>
            </owl:Restriction>
        </rdfs:subClassOf>
        <rdfs:subClassOf>
            <owl:Restriction>
                <owl:onProperty rdf:resource="https://purl.archive.org/oquo#measuresCharacteristicNegatively"/>
                <owl:someValuesFrom rdf:resource="https://purl.archive.org/oquo#EfficiencyInUseCharacteristic"/>
            </owl:Restriction>
        </rdfs:subClassOf>
        <rdfs:subClassOf>
            <owl:Restriction>
                <owl:onProperty rdf:resource="https://purl.archive.org/oquo#measuresCharacteristicNegatively"/>
                <owl:someValuesFrom rdf:resource="https://purl.archive.org/oquo#IndexingAndLinkingCharacteristic"/>
            </owl:Restriction>
        </rdfs:subClassOf>
        <rdfs:subClassOf>
            <owl:Restriction>
                <owl:onProperty rdf:resource="https://purl.archive.org/oquo#measuresCharacteristicNegatively"/>
                <owl:someValuesFrom rdf:resource="https://purl.archive.org/oquo#KnowledgeReuseCharacteristic"/>
            </owl:Restriction>
        </rdfs:subClassOf>
        <rdfs:subClassOf>
            <owl:Restriction>
                <owl:onProperty rdf:resource="https://purl.archive.org/oquo#measuresCharacteristicNegatively"/>
                <owl:someValuesFrom rdf:resource="https://purl.archive.org/oquo#TextAnalysisCharacteristic"/>
            </owl:Restriction>
        </rdfs:subClassOf>
        <rdfs:subClassOf>
            <owl:Restriction>
                <owl:onProperty rdf:resource="https://purl.archive.org/oquo#measuresCharacteristicNegatively"/>
                <owl:allValuesFrom>
                    <owl:Class>
                        <owl:unionOf rdf:parseType="Collection">
                            <rdf:Description rdf:about="https://purl.archive.org/oquo#EaseOfUseCharacteristic"/>
                            <rdf:Description rdf:about="https://purl.archive.org/oquo#EfficiencyInUseCharacteristic"/>
                            <rdf:Description rdf:about="https://purl.archive.org/oquo#IndexingAndLinkingCharacteristic"/>
                            <rdf:Description rdf:about="https://purl.archive.org/oquo#KnowledgeReuseCharacteristic"/>
                            <rdf:Description rdf:about="https://purl.archive.org/oquo#TextAnalysisCharacteristic"/>
                        </owl:unionOf>
                    </owl:Class>
                </owl:allValuesFrom>
            </owl:Restriction>
        </rdfs:subClassOf>
        <rdfs:subClassOf>
            <owl:Restriction>
                <owl:onProperty rdf:resource="http://purl.org/net/QualityModel#hasScale"/>
                <owl:hasValue rdf:resource="https://purl.archive.org/oquo#ObjectPropertiesWithNoNameMetricScale"/>
            </owl:Restriction>
        </rdfs:subClassOf>
        <obo:IAO_0000115>The Percentage of object properties lacking a name in the ontology.</obo:IAO_0000115>
        <rdf1:acronym>OPWNN</rdf1:acronym>
        <rdfs:label>object properties with no name metric</rdfs:label>
    </owl:Class>
    


    <!-- https://purl.archive.org/oquo#ObjectPropertiesWithNoSynonymMetric -->

    <owl:Class rdf:about="https://purl.archive.org/oquo#ObjectPropertiesWithNoSynonymMetric">
        <rdfs:subClassOf rdf:resource="http://purl.org/net/QualityModel#DerivedMeasure"/>
        <rdfs:subClassOf>
            <owl:Restriction>
                <owl:onProperty rdf:resource="http://purl.org/net/QualityModel#hasScale"/>
                <owl:someValuesFrom>
                    <owl:Class>
                        <owl:intersectionOf rdf:parseType="Collection">
                            <rdf:Description rdf:about="https://purl.archive.org/oquo#RawScale"/>
                            <owl:Restriction>
                                <owl:onProperty rdf:resource="http://purl.org/net/QualityModel#hasRankigFunction"/>
                                <owl:hasValue rdf:resource="http://purl.org/net/QualityModel#LowerBest"/>
                            </owl:Restriction>
                        </owl:intersectionOf>
                    </owl:Class>
                </owl:someValuesFrom>
            </owl:Restriction>
        </rdfs:subClassOf>
        <rdfs:subClassOf>
            <owl:Restriction>
                <owl:onProperty rdf:resource="https://purl.archive.org/oquo#measuresCharacteristicNegatively"/>
                <owl:someValuesFrom rdf:resource="https://purl.archive.org/oquo#EaseOfUseCharacteristic"/>
            </owl:Restriction>
        </rdfs:subClassOf>
        <rdfs:subClassOf>
            <owl:Restriction>
                <owl:onProperty rdf:resource="https://purl.archive.org/oquo#measuresCharacteristicNegatively"/>
                <owl:someValuesFrom rdf:resource="https://purl.archive.org/oquo#EfficiencyInUseCharacteristic"/>
            </owl:Restriction>
        </rdfs:subClassOf>
        <rdfs:subClassOf>
            <owl:Restriction>
                <owl:onProperty rdf:resource="https://purl.archive.org/oquo#measuresCharacteristicNegatively"/>
                <owl:someValuesFrom rdf:resource="https://purl.archive.org/oquo#IndexingAndLinkingCharacteristic"/>
            </owl:Restriction>
        </rdfs:subClassOf>
        <rdfs:subClassOf>
            <owl:Restriction>
                <owl:onProperty rdf:resource="https://purl.archive.org/oquo#measuresCharacteristicNegatively"/>
                <owl:someValuesFrom rdf:resource="https://purl.archive.org/oquo#KnowledgeReuseCharacteristic"/>
            </owl:Restriction>
        </rdfs:subClassOf>
        <rdfs:subClassOf>
            <owl:Restriction>
                <owl:onProperty rdf:resource="https://purl.archive.org/oquo#measuresCharacteristicNegatively"/>
                <owl:someValuesFrom rdf:resource="https://purl.archive.org/oquo#TextAnalysisCharacteristic"/>
            </owl:Restriction>
        </rdfs:subClassOf>
        <rdfs:subClassOf>
            <owl:Restriction>
                <owl:onProperty rdf:resource="https://purl.archive.org/oquo#measuresCharacteristicNegatively"/>
                <owl:allValuesFrom>
                    <owl:Class>
                        <owl:unionOf rdf:parseType="Collection">
                            <rdf:Description rdf:about="https://purl.archive.org/oquo#EaseOfUseCharacteristic"/>
                            <rdf:Description rdf:about="https://purl.archive.org/oquo#EfficiencyInUseCharacteristic"/>
                            <rdf:Description rdf:about="https://purl.archive.org/oquo#IndexingAndLinkingCharacteristic"/>
                            <rdf:Description rdf:about="https://purl.archive.org/oquo#KnowledgeReuseCharacteristic"/>
                            <rdf:Description rdf:about="https://purl.archive.org/oquo#TextAnalysisCharacteristic"/>
                        </owl:unionOf>
                    </owl:Class>
                </owl:allValuesFrom>
            </owl:Restriction>
        </rdfs:subClassOf>
        <rdfs:subClassOf>
            <owl:Restriction>
                <owl:onProperty rdf:resource="http://purl.org/net/QualityModel#hasScale"/>
                <owl:hasValue rdf:resource="https://purl.archive.org/oquo#ObjectPropertiesWithNoSynonymMetricScale"/>
            </owl:Restriction>
        </rdfs:subClassOf>
        <obo:IAO_0000115>The Percentage of object properties lacking a synonym in the ontology.</obo:IAO_0000115>
        <rdf1:acronym>OPWNS</rdf1:acronym>
        <rdfs:label>object properties with no synonym metric</rdfs:label>
    </owl:Class>
    


    <!-- https://purl.archive.org/oquo#SynonymsPerAnnotationPropertyMetric -->

    <owl:Class rdf:about="https://purl.archive.org/oquo#SynonymsPerAnnotationPropertyMetric">
        <rdfs:subClassOf rdf:resource="http://purl.org/net/QualityModel#DerivedMeasure"/>
        <rdfs:subClassOf>
            <owl:Restriction>
                <owl:onProperty rdf:resource="http://purl.org/net/QualityModel#hasScale"/>
                <owl:someValuesFrom>
                    <owl:Class>
                        <owl:intersectionOf rdf:parseType="Collection">
                            <rdf:Description rdf:about="https://purl.archive.org/oquo#RawScale"/>
                            <owl:Restriction>
                                <owl:onProperty rdf:resource="http://purl.org/net/QualityModel#hasRankigFunction"/>
                                <owl:hasValue rdf:resource="http://purl.org/net/QualityModel#HigherBest"/>
                            </owl:Restriction>
                        </owl:intersectionOf>
                    </owl:Class>
                </owl:someValuesFrom>
            </owl:Restriction>
        </rdfs:subClassOf>
        <rdfs:subClassOf>
            <owl:Restriction>
                <owl:onProperty rdf:resource="https://purl.archive.org/oquo#measuresCharacteristicPositively"/>
                <owl:someValuesFrom rdf:resource="https://purl.archive.org/oquo#EaseOfUseCharacteristic"/>
            </owl:Restriction>
        </rdfs:subClassOf>
        <rdfs:subClassOf>
            <owl:Restriction>
                <owl:onProperty rdf:resource="https://purl.archive.org/oquo#measuresCharacteristicPositively"/>
                <owl:someValuesFrom rdf:resource="https://purl.archive.org/oquo#EfficiencyInUseCharacteristic"/>
            </owl:Restriction>
        </rdfs:subClassOf>
        <rdfs:subClassOf>
            <owl:Restriction>
                <owl:onProperty rdf:resource="https://purl.archive.org/oquo#measuresCharacteristicPositively"/>
                <owl:someValuesFrom rdf:resource="https://purl.archive.org/oquo#IndexingAndLinkingCharacteristic"/>
            </owl:Restriction>
        </rdfs:subClassOf>
        <rdfs:subClassOf>
            <owl:Restriction>
                <owl:onProperty rdf:resource="https://purl.archive.org/oquo#measuresCharacteristicPositively"/>
                <owl:someValuesFrom rdf:resource="https://purl.archive.org/oquo#KnowledgeReuseCharacteristic"/>
            </owl:Restriction>
        </rdfs:subClassOf>
        <rdfs:subClassOf>
            <owl:Restriction>
                <owl:onProperty rdf:resource="https://purl.archive.org/oquo#measuresCharacteristicPositively"/>
                <owl:someValuesFrom rdf:resource="https://purl.archive.org/oquo#TextAnalysisCharacteristic"/>
            </owl:Restriction>
        </rdfs:subClassOf>
        <rdfs:subClassOf>
            <owl:Restriction>
                <owl:onProperty rdf:resource="https://purl.archive.org/oquo#measuresCharacteristicPositively"/>
                <owl:allValuesFrom>
                    <owl:Class>
                        <owl:unionOf rdf:parseType="Collection">
                            <rdf:Description rdf:about="https://purl.archive.org/oquo#EaseOfUseCharacteristic"/>
                            <rdf:Description rdf:about="https://purl.archive.org/oquo#EfficiencyInUseCharacteristic"/>
                            <rdf:Description rdf:about="https://purl.archive.org/oquo#IndexingAndLinkingCharacteristic"/>
                            <rdf:Description rdf:about="https://purl.archive.org/oquo#KnowledgeReuseCharacteristic"/>
                            <rdf:Description rdf:about="https://purl.archive.org/oquo#TextAnalysisCharacteristic"/>
                        </owl:unionOf>
                    </owl:Class>
                </owl:allValuesFrom>
            </owl:Restriction>
        </rdfs:subClassOf>
        <rdfs:subClassOf>
            <owl:Restriction>
                <owl:onProperty rdf:resource="http://purl.org/net/QualityModel#hasScale"/>
                <owl:hasValue rdf:resource="https://purl.archive.org/oquo#SynonymsPerAnnotationPropertyMetricScale"/>
            </owl:Restriction>
        </rdfs:subClassOf>
        <obo:IAO_0000115 xml:lang="en">This metric accounts for the number of synonyms associated with annotation properties, which can also be provided by using different annotation properties used by the community to include synonyms (oboInOwl:hasExactSynonym, skos:altLabel, iao:0000118, etc.). This metric is calculated as the number of synonyms associated with annotation properties divided by the total number of annotation properties in the ontology. The range of the value of this metric is the set of real positive numbers.</obo:IAO_0000115>
        <rdf1:acronym>SxAP</rdf1:acronym>
        <rdfs:comment>The total number of annotation property synonyms over the total number of annotation properties.</rdfs:comment>
        <rdfs:label>synonyms per annotation property metric</rdfs:label>
    </owl:Class>
    


    <!-- https://purl.archive.org/oquo#SynonymsPerClassMetric -->

    <owl:Class rdf:about="https://purl.archive.org/oquo#SynonymsPerClassMetric">
        <rdfs:subClassOf rdf:resource="http://purl.org/net/QualityModel#DerivedMeasure"/>
        <rdfs:subClassOf>
            <owl:Restriction>
                <owl:onProperty rdf:resource="http://purl.org/net/QualityModel#hasScale"/>
                <owl:someValuesFrom>
                    <owl:Class>
                        <owl:intersectionOf rdf:parseType="Collection">
                            <rdf:Description rdf:about="https://purl.archive.org/oquo#RawScale"/>
                            <owl:Restriction>
                                <owl:onProperty rdf:resource="http://purl.org/net/QualityModel#hasRankigFunction"/>
                                <owl:hasValue rdf:resource="http://purl.org/net/QualityModel#HigherBest"/>
                            </owl:Restriction>
                        </owl:intersectionOf>
                    </owl:Class>
                </owl:someValuesFrom>
            </owl:Restriction>
        </rdfs:subClassOf>
        <rdfs:subClassOf>
            <owl:Restriction>
                <owl:onProperty rdf:resource="https://purl.archive.org/oquo#measuresCharacteristicPositively"/>
                <owl:someValuesFrom rdf:resource="https://purl.archive.org/oquo#EaseOfUseCharacteristic"/>
            </owl:Restriction>
        </rdfs:subClassOf>
        <rdfs:subClassOf>
            <owl:Restriction>
                <owl:onProperty rdf:resource="https://purl.archive.org/oquo#measuresCharacteristicPositively"/>
                <owl:someValuesFrom rdf:resource="https://purl.archive.org/oquo#EfficiencyInUseCharacteristic"/>
            </owl:Restriction>
        </rdfs:subClassOf>
        <rdfs:subClassOf>
            <owl:Restriction>
                <owl:onProperty rdf:resource="https://purl.archive.org/oquo#measuresCharacteristicPositively"/>
                <owl:someValuesFrom rdf:resource="https://purl.archive.org/oquo#IndexingAndLinkingCharacteristic"/>
            </owl:Restriction>
        </rdfs:subClassOf>
        <rdfs:subClassOf>
            <owl:Restriction>
                <owl:onProperty rdf:resource="https://purl.archive.org/oquo#measuresCharacteristicPositively"/>
                <owl:someValuesFrom rdf:resource="https://purl.archive.org/oquo#KnowledgeReuseCharacteristic"/>
            </owl:Restriction>
        </rdfs:subClassOf>
        <rdfs:subClassOf>
            <owl:Restriction>
                <owl:onProperty rdf:resource="https://purl.archive.org/oquo#measuresCharacteristicPositively"/>
                <owl:someValuesFrom rdf:resource="https://purl.archive.org/oquo#TextAnalysisCharacteristic"/>
            </owl:Restriction>
        </rdfs:subClassOf>
        <rdfs:subClassOf>
            <owl:Restriction>
                <owl:onProperty rdf:resource="https://purl.archive.org/oquo#measuresCharacteristicPositively"/>
                <owl:allValuesFrom>
                    <owl:Class>
                        <owl:unionOf rdf:parseType="Collection">
                            <rdf:Description rdf:about="https://purl.archive.org/oquo#EaseOfUseCharacteristic"/>
                            <rdf:Description rdf:about="https://purl.archive.org/oquo#EfficiencyInUseCharacteristic"/>
                            <rdf:Description rdf:about="https://purl.archive.org/oquo#IndexingAndLinkingCharacteristic"/>
                            <rdf:Description rdf:about="https://purl.archive.org/oquo#KnowledgeReuseCharacteristic"/>
                            <rdf:Description rdf:about="https://purl.archive.org/oquo#TextAnalysisCharacteristic"/>
                        </owl:unionOf>
                    </owl:Class>
                </owl:allValuesFrom>
            </owl:Restriction>
        </rdfs:subClassOf>
        <rdfs:subClassOf>
            <owl:Restriction>
                <owl:onProperty rdf:resource="http://purl.org/net/QualityModel#hasScale"/>
                <owl:hasValue rdf:resource="https://purl.archive.org/oquo#SynonymsPerClassMetricScale"/>
            </owl:Restriction>
        </rdfs:subClassOf>
        <obo:IAO_0000115 xml:lang="en">This metric accounts for the number of synonyms associated with classes, which can also be provided by using different annotation properties used by the community to include synonyms (oboInOwl:hasExactSynonym, skos:altLabel, iao:0000118, etc.). This metric is calculated as the number of synonyms associated with classes divided by the total number of classes in the ontology. The range of the value of this metric is the set of real positive numbers.</obo:IAO_0000115>
        <rdf1:acronym>SxC</rdf1:acronym>
        <rdfs:comment>The total number of class synonyms over the total number of classes.</rdfs:comment>
        <rdfs:label>synonyms per class metric</rdfs:label>
    </owl:Class>
    


    <!-- https://purl.archive.org/oquo#SynonymsPerDataPropertyMetric -->

    <owl:Class rdf:about="https://purl.archive.org/oquo#SynonymsPerDataPropertyMetric">
        <rdfs:subClassOf rdf:resource="http://purl.org/net/QualityModel#DerivedMeasure"/>
        <rdfs:subClassOf>
            <owl:Restriction>
                <owl:onProperty rdf:resource="http://purl.org/net/QualityModel#hasScale"/>
                <owl:someValuesFrom>
                    <owl:Class>
                        <owl:intersectionOf rdf:parseType="Collection">
                            <rdf:Description rdf:about="https://purl.archive.org/oquo#RawScale"/>
                            <owl:Restriction>
                                <owl:onProperty rdf:resource="http://purl.org/net/QualityModel#hasRankigFunction"/>
                                <owl:hasValue rdf:resource="http://purl.org/net/QualityModel#HigherBest"/>
                            </owl:Restriction>
                        </owl:intersectionOf>
                    </owl:Class>
                </owl:someValuesFrom>
            </owl:Restriction>
        </rdfs:subClassOf>
        <rdfs:subClassOf>
            <owl:Restriction>
                <owl:onProperty rdf:resource="https://purl.archive.org/oquo#measuresCharacteristicPositively"/>
                <owl:someValuesFrom rdf:resource="https://purl.archive.org/oquo#EaseOfUseCharacteristic"/>
            </owl:Restriction>
        </rdfs:subClassOf>
        <rdfs:subClassOf>
            <owl:Restriction>
                <owl:onProperty rdf:resource="https://purl.archive.org/oquo#measuresCharacteristicPositively"/>
                <owl:someValuesFrom rdf:resource="https://purl.archive.org/oquo#EfficiencyInUseCharacteristic"/>
            </owl:Restriction>
        </rdfs:subClassOf>
        <rdfs:subClassOf>
            <owl:Restriction>
                <owl:onProperty rdf:resource="https://purl.archive.org/oquo#measuresCharacteristicPositively"/>
                <owl:someValuesFrom rdf:resource="https://purl.archive.org/oquo#IndexingAndLinkingCharacteristic"/>
            </owl:Restriction>
        </rdfs:subClassOf>
        <rdfs:subClassOf>
            <owl:Restriction>
                <owl:onProperty rdf:resource="https://purl.archive.org/oquo#measuresCharacteristicPositively"/>
                <owl:someValuesFrom rdf:resource="https://purl.archive.org/oquo#KnowledgeReuseCharacteristic"/>
            </owl:Restriction>
        </rdfs:subClassOf>
        <rdfs:subClassOf>
            <owl:Restriction>
                <owl:onProperty rdf:resource="https://purl.archive.org/oquo#measuresCharacteristicPositively"/>
                <owl:someValuesFrom rdf:resource="https://purl.archive.org/oquo#TextAnalysisCharacteristic"/>
            </owl:Restriction>
        </rdfs:subClassOf>
        <rdfs:subClassOf>
            <owl:Restriction>
                <owl:onProperty rdf:resource="https://purl.archive.org/oquo#measuresCharacteristicPositively"/>
                <owl:allValuesFrom>
                    <owl:Class>
                        <owl:unionOf rdf:parseType="Collection">
                            <rdf:Description rdf:about="https://purl.archive.org/oquo#EaseOfUseCharacteristic"/>
                            <rdf:Description rdf:about="https://purl.archive.org/oquo#EfficiencyInUseCharacteristic"/>
                            <rdf:Description rdf:about="https://purl.archive.org/oquo#IndexingAndLinkingCharacteristic"/>
                            <rdf:Description rdf:about="https://purl.archive.org/oquo#KnowledgeReuseCharacteristic"/>
                            <rdf:Description rdf:about="https://purl.archive.org/oquo#TextAnalysisCharacteristic"/>
                        </owl:unionOf>
                    </owl:Class>
                </owl:allValuesFrom>
            </owl:Restriction>
        </rdfs:subClassOf>
        <rdfs:subClassOf>
            <owl:Restriction>
                <owl:onProperty rdf:resource="http://purl.org/net/QualityModel#hasScale"/>
                <owl:hasValue rdf:resource="https://purl.archive.org/oquo#SynonymsPerDataPropertyMetricScale"/>
            </owl:Restriction>
        </rdfs:subClassOf>
        <obo:IAO_0000115 xml:lang="en">This metric accounts for the number of synonyms associated with data type properties, which can also be provided by using different annotation properties used by the community to include synonyms (oboInOwl:hasExactSynonym, skos:altLabel, iao:0000118, etc.). This metric is calculated as the number of synonyms associated with data type properties divided by the total number of data type properties in the ontology. The range of the value of this metric is the set of real positive numbers.</obo:IAO_0000115>
        <rdf1:acronym>SxDP</rdf1:acronym>
        <rdfs:comment>The total number of data property synonyms over the total number of data properties.</rdfs:comment>
        <rdfs:label>synonyms per data property metric</rdfs:label>
    </owl:Class>
    


    <!-- https://purl.archive.org/oquo#SynonymsPerObjectPropertyMetric -->

    <owl:Class rdf:about="https://purl.archive.org/oquo#SynonymsPerObjectPropertyMetric">
        <rdfs:subClassOf rdf:resource="http://purl.org/net/QualityModel#DerivedMeasure"/>
        <rdfs:subClassOf>
            <owl:Restriction>
                <owl:onProperty rdf:resource="http://purl.org/net/QualityModel#hasScale"/>
                <owl:someValuesFrom>
                    <owl:Class>
                        <owl:intersectionOf rdf:parseType="Collection">
                            <rdf:Description rdf:about="https://purl.archive.org/oquo#RawScale"/>
                            <owl:Restriction>
                                <owl:onProperty rdf:resource="http://purl.org/net/QualityModel#hasRankigFunction"/>
                                <owl:hasValue rdf:resource="http://purl.org/net/QualityModel#HigherBest"/>
                            </owl:Restriction>
                        </owl:intersectionOf>
                    </owl:Class>
                </owl:someValuesFrom>
            </owl:Restriction>
        </rdfs:subClassOf>
        <rdfs:subClassOf>
            <owl:Restriction>
                <owl:onProperty rdf:resource="https://purl.archive.org/oquo#measuresCharacteristicPositively"/>
                <owl:someValuesFrom rdf:resource="https://purl.archive.org/oquo#EaseOfUseCharacteristic"/>
            </owl:Restriction>
        </rdfs:subClassOf>
        <rdfs:subClassOf>
            <owl:Restriction>
                <owl:onProperty rdf:resource="https://purl.archive.org/oquo#measuresCharacteristicPositively"/>
                <owl:someValuesFrom rdf:resource="https://purl.archive.org/oquo#EfficiencyInUseCharacteristic"/>
            </owl:Restriction>
        </rdfs:subClassOf>
        <rdfs:subClassOf>
            <owl:Restriction>
                <owl:onProperty rdf:resource="https://purl.archive.org/oquo#measuresCharacteristicPositively"/>
                <owl:someValuesFrom rdf:resource="https://purl.archive.org/oquo#IndexingAndLinkingCharacteristic"/>
            </owl:Restriction>
        </rdfs:subClassOf>
        <rdfs:subClassOf>
            <owl:Restriction>
                <owl:onProperty rdf:resource="https://purl.archive.org/oquo#measuresCharacteristicPositively"/>
                <owl:someValuesFrom rdf:resource="https://purl.archive.org/oquo#KnowledgeReuseCharacteristic"/>
            </owl:Restriction>
        </rdfs:subClassOf>
        <rdfs:subClassOf>
            <owl:Restriction>
                <owl:onProperty rdf:resource="https://purl.archive.org/oquo#measuresCharacteristicPositively"/>
                <owl:someValuesFrom rdf:resource="https://purl.archive.org/oquo#TextAnalysisCharacteristic"/>
            </owl:Restriction>
        </rdfs:subClassOf>
        <rdfs:subClassOf>
            <owl:Restriction>
                <owl:onProperty rdf:resource="https://purl.archive.org/oquo#measuresCharacteristicPositively"/>
                <owl:allValuesFrom>
                    <owl:Class>
                        <owl:unionOf rdf:parseType="Collection">
                            <rdf:Description rdf:about="https://purl.archive.org/oquo#EaseOfUseCharacteristic"/>
                            <rdf:Description rdf:about="https://purl.archive.org/oquo#EfficiencyInUseCharacteristic"/>
                            <rdf:Description rdf:about="https://purl.archive.org/oquo#IndexingAndLinkingCharacteristic"/>
                            <rdf:Description rdf:about="https://purl.archive.org/oquo#KnowledgeReuseCharacteristic"/>
                            <rdf:Description rdf:about="https://purl.archive.org/oquo#TextAnalysisCharacteristic"/>
                        </owl:unionOf>
                    </owl:Class>
                </owl:allValuesFrom>
            </owl:Restriction>
        </rdfs:subClassOf>
        <rdfs:subClassOf>
            <owl:Restriction>
                <owl:onProperty rdf:resource="http://purl.org/net/QualityModel#hasScale"/>
                <owl:hasValue rdf:resource="https://purl.archive.org/oquo#SynonymsPerObjectPropertyMetricScale"/>
            </owl:Restriction>
        </rdfs:subClassOf>
        <obo:IAO_0000115 xml:lang="en">This metric accounts for the number of synonyms associated with object properties, which can also be provided by using different annotation properties used by the community to include synonyms (oboInOwl:hasExactSynonym, skos:altLabel, iao:0000118, etc.). This metric is calculated as the number of synonyms associated with object properties divided by the total number of object properties in the ontology. The range of the value of this metric is the set of real positive numbers.</obo:IAO_0000115>
        <rdf1:acronym>SxOP</rdf1:acronym>
        <rdfs:comment>The total number of object property synonyms over the total number of object properties.</rdfs:comment>
        <rdfs:label>synonyms per object property metric</rdfs:label>
    </owl:Class>
    


    <!-- https://purl.archive.org/oquo#SynonymsPerPropertyMetric -->

    <owl:Class rdf:about="https://purl.archive.org/oquo#SynonymsPerPropertyMetric">
        <rdfs:subClassOf rdf:resource="http://purl.org/net/QualityModel#DerivedMeasure"/>
        <rdfs:subClassOf>
            <owl:Restriction>
                <owl:onProperty rdf:resource="http://purl.org/net/QualityModel#hasScale"/>
                <owl:someValuesFrom>
                    <owl:Class>
                        <owl:intersectionOf rdf:parseType="Collection">
                            <rdf:Description rdf:about="https://purl.archive.org/oquo#RawScale"/>
                            <owl:Restriction>
                                <owl:onProperty rdf:resource="http://purl.org/net/QualityModel#hasRankigFunction"/>
                                <owl:hasValue rdf:resource="http://purl.org/net/QualityModel#HigherBest"/>
                            </owl:Restriction>
                        </owl:intersectionOf>
                    </owl:Class>
                </owl:someValuesFrom>
            </owl:Restriction>
        </rdfs:subClassOf>
        <rdfs:subClassOf>
            <owl:Restriction>
                <owl:onProperty rdf:resource="https://purl.archive.org/oquo#measuresCharacteristicPositively"/>
                <owl:someValuesFrom rdf:resource="https://purl.archive.org/oquo#EaseOfUseCharacteristic"/>
            </owl:Restriction>
        </rdfs:subClassOf>
        <rdfs:subClassOf>
            <owl:Restriction>
                <owl:onProperty rdf:resource="https://purl.archive.org/oquo#measuresCharacteristicPositively"/>
                <owl:someValuesFrom rdf:resource="https://purl.archive.org/oquo#EfficiencyInUseCharacteristic"/>
            </owl:Restriction>
        </rdfs:subClassOf>
        <rdfs:subClassOf>
            <owl:Restriction>
                <owl:onProperty rdf:resource="https://purl.archive.org/oquo#measuresCharacteristicPositively"/>
                <owl:someValuesFrom rdf:resource="https://purl.archive.org/oquo#IndexingAndLinkingCharacteristic"/>
            </owl:Restriction>
        </rdfs:subClassOf>
        <rdfs:subClassOf>
            <owl:Restriction>
                <owl:onProperty rdf:resource="https://purl.archive.org/oquo#measuresCharacteristicPositively"/>
                <owl:someValuesFrom rdf:resource="https://purl.archive.org/oquo#KnowledgeReuseCharacteristic"/>
            </owl:Restriction>
        </rdfs:subClassOf>
        <rdfs:subClassOf>
            <owl:Restriction>
                <owl:onProperty rdf:resource="https://purl.archive.org/oquo#measuresCharacteristicPositively"/>
                <owl:someValuesFrom rdf:resource="https://purl.archive.org/oquo#TextAnalysisCharacteristic"/>
            </owl:Restriction>
        </rdfs:subClassOf>
        <rdfs:subClassOf>
            <owl:Restriction>
                <owl:onProperty rdf:resource="https://purl.archive.org/oquo#measuresCharacteristicPositively"/>
                <owl:allValuesFrom>
                    <owl:Class>
                        <owl:unionOf rdf:parseType="Collection">
                            <rdf:Description rdf:about="https://purl.archive.org/oquo#EaseOfUseCharacteristic"/>
                            <rdf:Description rdf:about="https://purl.archive.org/oquo#EfficiencyInUseCharacteristic"/>
                            <rdf:Description rdf:about="https://purl.archive.org/oquo#IndexingAndLinkingCharacteristic"/>
                            <rdf:Description rdf:about="https://purl.archive.org/oquo#KnowledgeReuseCharacteristic"/>
                            <rdf:Description rdf:about="https://purl.archive.org/oquo#TextAnalysisCharacteristic"/>
                        </owl:unionOf>
                    </owl:Class>
                </owl:allValuesFrom>
            </owl:Restriction>
        </rdfs:subClassOf>
        <rdfs:subClassOf>
            <owl:Restriction>
                <owl:onProperty rdf:resource="http://purl.org/net/QualityModel#hasScale"/>
                <owl:hasValue rdf:resource="https://purl.archive.org/oquo#SynonymsPerPropertyMetricScale"/>
            </owl:Restriction>
        </rdfs:subClassOf>
        <obo:IAO_0000115 xml:lang="en">This metric accounts for the number of synonyms associated with properties, which can also be provided by using different annotation properties used by the community to include synonyms (oboInOwl:hasExactSynonym, skos:altLabel, iao:0000118, etc.). This metric is calculated as the number of synonyms associated with properties (including annotation, data, and object properties) divided by the total number of properties in the ontology. The range of the value of this metric is the set of real positive numbers.</obo:IAO_0000115>
        <rdf1:acronym>SxC</rdf1:acronym>
        <rdfs:comment>The total number of property synonyms over the total number of properties, including data, object and annotation properties.</rdfs:comment>
        <rdfs:label>synonyms per property metric</rdfs:label>
    </owl:Class>
    


    <!-- https://purl.archive.org/oquo#SystematicNamingMetric -->

    <owl:Class rdf:about="https://purl.archive.org/oquo#SystematicNamingMetric">
        <rdfs:subClassOf rdf:resource="http://purl.org/net/QualityModel#DerivedMeasure"/>
        <rdfs:subClassOf>
            <owl:Restriction>
                <owl:onProperty rdf:resource="http://purl.org/net/QualityModel#hasScale"/>
                <owl:someValuesFrom>
                    <owl:Class>
                        <owl:intersectionOf rdf:parseType="Collection">
                            <rdf:Description rdf:about="https://purl.archive.org/oquo#RawScale"/>
                            <owl:Restriction>
                                <owl:onProperty rdf:resource="http://purl.org/net/QualityModel#hasRankigFunction"/>
                                <owl:hasValue rdf:resource="http://purl.org/net/QualityModel#HigherBest"/>
                            </owl:Restriction>
                        </owl:intersectionOf>
                    </owl:Class>
                </owl:someValuesFrom>
            </owl:Restriction>
        </rdfs:subClassOf>
        <rdfs:subClassOf>
            <owl:Restriction>
                <owl:onProperty rdf:resource="https://purl.archive.org/oquo#measuresCharacteristicPositively"/>
                <owl:someValuesFrom rdf:resource="https://purl.archive.org/oquo#StructuralAccuracyCharacteristic"/>
            </owl:Restriction>
        </rdfs:subClassOf>
        <rdfs:subClassOf>
            <owl:Restriction>
                <owl:onProperty rdf:resource="https://purl.archive.org/oquo#measuresCharacteristicPositively"/>
                <owl:someValuesFrom rdf:resource="https://purl.archive.org/oquo#TextAnalysisCharacteristic"/>
            </owl:Restriction>
        </rdfs:subClassOf>
        <rdfs:subClassOf>
            <owl:Restriction>
                <owl:onProperty rdf:resource="https://purl.archive.org/oquo#measuresCharacteristicPositively"/>
                <owl:allValuesFrom>
                    <owl:Class>
                        <owl:unionOf rdf:parseType="Collection">
                            <rdf:Description rdf:about="https://purl.archive.org/oquo#StructuralAccuracyCharacteristic"/>
                            <rdf:Description rdf:about="https://purl.archive.org/oquo#TextAnalysisCharacteristic"/>
                        </owl:unionOf>
                    </owl:Class>
                </owl:allValuesFrom>
            </owl:Restriction>
        </rdfs:subClassOf>
        <rdfs:subClassOf>
            <owl:Restriction>
                <owl:onProperty rdf:resource="http://purl.org/net/QualityModel#hasScale"/>
                <owl:hasValue rdf:resource="https://purl.archive.org/oquo#SystematicNamingMetricScale"/>
            </owl:Restriction>
        </rdfs:subClassOf>
        <obo:IAO_0000115 xml:lang="en">This metric is related to the ontology design principle that states that classes in the same taxonomy should share part of their name, since subclasses are specializations of the parent class. In other words, class names should follow a genus-differentia style. This metric is calculated as the ratio of subclasses of an LR class that exhibit the lexical regularity of the parent class. This requires to calculate how many subclasses of a given LR class exhibit the lexical regularity in their name (positive cases) and how many do not (negative cases). The value of the metric is calculated by dividing the positive cases by the total number of cases. It is calculated for each LR class. The final value of the metric for an ontology is calculated as the sum of all the positive cases divided by the sum of all the positive and negative cases obtained by each LR class in the ontology. The value is in the range [0, 1], the highest values representing the best values for the metric.</obo:IAO_0000115>
        <rdf1:acronym>SYSNAM</rdf1:acronym>
        <rdfs:comment>The degree in which hierarchies under LR classes exhibit the lexical regularity of the parent class.</rdfs:comment>
        <rdfs:label>systematic naming metric</rdfs:label>
    </owl:Class>
    


    <!-- 
    ///////////////////////////////////////////////////////////////////////////////////////
    //
    // Individuals
    //
    ///////////////////////////////////////////////////////////////////////////////////////
     -->
    


    <!-- https://purl.archive.org/oquo#AnnotationPropertiesWithNoDescriptionMetricScale -->

    <owl:NamedIndividual rdf:about="https://purl.archive.org/oquo#AnnotationPropertiesWithNoDescriptionMetricScale">
        <rdf:type rdf:resource="http://www.wurvoc.org/vocabularies/om-1.8/Ratio_scale"/>
        <rdf:type rdf:resource="https://purl.archive.org/oquo#RawScale"/>
        <QualityModel:hasRankigFunction rdf:resource="http://purl.org/net/QualityModel#LowerBest"/>
        <obo:IAO_0000115>The number of annotation properties lacking a description over the number of the annotation properties considered.</obo:IAO_0000115>
        <rdfs:label>annotation properties with no description metric scale</rdfs:label>
    </owl:NamedIndividual>
    


    <!-- https://purl.archive.org/oquo#AnnotationPropertiesWithNoNameMetricScale -->

    <owl:NamedIndividual rdf:about="https://purl.archive.org/oquo#AnnotationPropertiesWithNoNameMetricScale">
        <rdf:type rdf:resource="http://www.wurvoc.org/vocabularies/om-1.8/Ratio_scale"/>
        <rdf:type rdf:resource="https://purl.archive.org/oquo#RawScale"/>
        <QualityModel:hasRankigFunction rdf:resource="http://purl.org/net/QualityModel#LowerBest"/>
        <obo:IAO_0000115>The numberof annotation properties lacking a name over the number of annotation properties considered.</obo:IAO_0000115>
        <rdfs:label>annotation properties with no name metric scale</rdfs:label>
    </owl:NamedIndividual>
    


    <!-- https://purl.archive.org/oquo#AnnotationPropertiesWithNoSynonymMetricScale -->

    <owl:NamedIndividual rdf:about="https://purl.archive.org/oquo#AnnotationPropertiesWithNoSynonymMetricScale">
        <rdf:type rdf:resource="http://www.wurvoc.org/vocabularies/om-1.8/Ratio_scale"/>
        <rdf:type rdf:resource="https://purl.archive.org/oquo#RawScale"/>
        <QualityModel:hasRankigFunction rdf:resource="http://purl.org/net/QualityModel#LowerBest"/>
        <obo:IAO_0000115>The number of annotation properties lacking synonyms over the annotation properties considered.</obo:IAO_0000115>
        <rdfs:label>annotation properties with no synonym metric scale</rdfs:label>
    </owl:NamedIndividual>


    


    <!-- https://purl.archive.org/oquo#ClassesWithNoDescriptionMetricScale -->

    <owl:NamedIndividual rdf:about="https://purl.archive.org/oquo#ClassesWithNoDescriptionMetricScale">
        <rdf:type rdf:resource="http://www.wurvoc.org/vocabularies/om-1.8/Ratio_scale"/>
        <rdf:type rdf:resource="https://purl.archive.org/oquo#RawScale"/>
        <QualityModel:hasRankigFunction rdf:resource="http://purl.org/net/QualityModel#LowerBest"/>
        <obo:IAO_0000115>The number of classes lacking a description over the number of classes considered.</obo:IAO_0000115>
        <rdfs:label>classes with no description metric scale</rdfs:label>
    </owl:NamedIndividual>
    


    <!-- https://purl.archive.org/oquo#ClassesWithNoNameMetricScale -->

    <owl:NamedIndividual rdf:about="https://purl.archive.org/oquo#ClassesWithNoNameMetricScale">
        <rdf:type rdf:resource="http://www.wurvoc.org/vocabularies/om-1.8/Ratio_scale"/>
        <rdf:type rdf:resource="https://purl.archive.org/oquo#RawScale"/>
        <QualityModel:hasRankigFunction rdf:resource="http://purl.org/net/QualityModel#LowerBest"/>
        <obo:IAO_0000115>The number of classes lacking a name over the number of classes considered.</obo:IAO_0000115>
        <rdfs:label>classes with no name metric scale</rdfs:label>
    </owl:NamedIndividual>
    


    <!-- https://purl.archive.org/oquo#ClassesWithNoSynonymMetricScale -->

    <owl:NamedIndividual rdf:about="https://purl.archive.org/oquo#ClassesWithNoSynonymMetricScale">
        <rdf:type rdf:resource="http://www.wurvoc.org/vocabularies/om-1.8/Ratio_scale"/>
        <rdf:type rdf:resource="https://purl.archive.org/oquo#RawScale"/>
        <QualityModel:hasRankigFunction rdf:resource="http://purl.org/net/QualityModel#LowerBest"/>
        <obo:IAO_0000115>The number of classes lacking synonyms over the number of classes considered.</obo:IAO_0000115>
        <rdfs:label>classes with no synonym metric scale</rdfs:label>
    </owl:NamedIndividual>
    

    


    <!-- https://purl.archive.org/oquo#DataPropertiesWithNoDescriptionMetricScale -->

    <owl:NamedIndividual rdf:about="https://purl.archive.org/oquo#DataPropertiesWithNoDescriptionMetricScale">
        <rdf:type rdf:resource="http://www.wurvoc.org/vocabularies/om-1.8/Ratio_scale"/>
        <rdf:type rdf:resource="https://purl.archive.org/oquo#RawScale"/>
        <QualityModel:hasRankigFunction rdf:resource="http://purl.org/net/QualityModel#LowerBest"/>
        <obo:IAO_0000115>The number of data properties lacking a description over the number of data properties considered.</obo:IAO_0000115>
        <rdfs:label>data properties with no description metric scale</rdfs:label>
    </owl:NamedIndividual>
    


    <!-- https://purl.archive.org/oquo#DataPropertiesWithNoNameMetricScale -->

    <owl:NamedIndividual rdf:about="https://purl.archive.org/oquo#DataPropertiesWithNoNameMetricScale">
        <rdf:type rdf:resource="http://www.wurvoc.org/vocabularies/om-1.8/Ratio_scale"/>
        <rdf:type rdf:resource="https://purl.archive.org/oquo#RawScale"/>
        <QualityModel:hasRankigFunction rdf:resource="http://purl.org/net/QualityModel#LowerBest"/>
        <obo:IAO_0000115>The number of data properties lacking a name over the number of data properties considered.</obo:IAO_0000115>
        <rdfs:label>data properties with no name metric scale</rdfs:label>
    </owl:NamedIndividual>
    


    <!-- https://purl.archive.org/oquo#DataPropertiesWithNoSynonymMetricScale -->

    <owl:NamedIndividual rdf:about="https://purl.archive.org/oquo#DataPropertiesWithNoSynonymMetricScale">
        <rdf:type rdf:resource="http://www.wurvoc.org/vocabularies/om-1.8/Ratio_scale"/>
        <rdf:type rdf:resource="https://purl.archive.org/oquo#RawScale"/>
        <QualityModel:hasRankigFunction rdf:resource="http://purl.org/net/QualityModel#LowerBest"/>
        <obo:IAO_0000115>The number of data properties lacking synonyms over the number of data properties considered.</obo:IAO_0000115>
        <rdfs:label>data properties with no synonym metric scale</rdfs:label>
    </owl:NamedIndividual>

    


    <!-- https://purl.archive.org/oquo#DescriptionsPerAnnotationPropertyMetricScale -->

    <owl:NamedIndividual rdf:about="https://purl.archive.org/oquo#DescriptionsPerAnnotationPropertyMetricScale">
        <rdf:type rdf:resource="http://www.wurvoc.org/vocabularies/om-1.8/Ratio_scale"/>
        <rdf:type rdf:resource="https://purl.archive.org/oquo#RawScale"/>
        <QualityModel:hasRankigFunction rdf:resource="http://purl.org/net/QualityModel#HigherBest"/>
        <obo:IAO_0000115>The total number of annotation property descriptions over the total number of annotation properties.</obo:IAO_0000115>
        <rdfs:label>descriptions per annotation property metric scale</rdfs:label>
    </owl:NamedIndividual>
    


    <!-- https://purl.archive.org/oquo#DescriptionsPerClassMetricScale -->

    <owl:NamedIndividual rdf:about="https://purl.archive.org/oquo#DescriptionsPerClassMetricScale">
        <rdf:type rdf:resource="http://www.wurvoc.org/vocabularies/om-1.8/Ratio_scale"/>
        <rdf:type rdf:resource="https://purl.archive.org/oquo#RawScale"/>
        <QualityModel:hasRankigFunction rdf:resource="http://purl.org/net/QualityModel#HigherBest"/>
        <obo:IAO_0000115>The total number of class descriptions over the total number of classes.</obo:IAO_0000115>
        <rdfs:label>descriptions per class metric scale</rdfs:label>
    </owl:NamedIndividual>
    


    <!-- https://purl.archive.org/oquo#DescriptionsPerDataPropertyMetricScale -->

    <owl:NamedIndividual rdf:about="https://purl.archive.org/oquo#DescriptionsPerDataPropertyMetricScale">
        <rdf:type rdf:resource="http://www.wurvoc.org/vocabularies/om-1.8/Ratio_scale"/>
        <rdf:type rdf:resource="https://purl.archive.org/oquo#RawScale"/>
        <QualityModel:hasRankigFunction rdf:resource="http://purl.org/net/QualityModel#HigherBest"/>
        <obo:IAO_0000115>The total number of data property descriptions over the total number of data properties.</obo:IAO_0000115>
        <rdfs:label>descriptions per data property metric scale</rdfs:label>
    </owl:NamedIndividual>
    


    <!-- https://purl.archive.org/oquo#DescriptionsPerObjectPropertyMetricScale -->

    <owl:NamedIndividual rdf:about="https://purl.archive.org/oquo#DescriptionsPerObjectPropertyMetricScale">
        <rdf:type rdf:resource="http://www.wurvoc.org/vocabularies/om-1.8/Ratio_scale"/>
        <rdf:type rdf:resource="https://purl.archive.org/oquo#RawScale"/>
        <QualityModel:hasRankigFunction rdf:resource="http://purl.org/net/QualityModel#HigherBest"/>
        <obo:IAO_0000115>The total number of object property descriptions over the total number of object properties.</obo:IAO_0000115>
        <rdfs:label>descriptions per object property metric scale</rdfs:label>
    </owl:NamedIndividual>
    


    <!-- https://purl.archive.org/oquo#DescriptionsPerPropertyMetricScale -->

    <owl:NamedIndividual rdf:about="https://purl.archive.org/oquo#DescriptionsPerPropertyMetricScale">
        <rdf:type rdf:resource="http://www.wurvoc.org/vocabularies/om-1.8/Ratio_scale"/>
        <rdf:type rdf:resource="https://purl.archive.org/oquo#RawScale"/>
        <QualityModel:hasRankigFunction rdf:resource="http://purl.org/net/QualityModel#HigherBest"/>
        <obo:IAO_0000115>The total property descriptions over the total number of properties.</obo:IAO_0000115>
        <rdfs:label>descriptions per property metric scale</rdfs:label>
    </owl:NamedIndividual>
    


    <!-- https://purl.archive.org/oquo#LexicalRegularitiesPerClassMetricScale -->

    <owl:NamedIndividual rdf:about="https://purl.archive.org/oquo#LexicalRegularitiesPerClassMetricScale">
        <rdf:type rdf:resource="http://www.wurvoc.org/vocabularies/om-1.8/Ratio_scale"/>
        <rdf:type rdf:resource="https://purl.archive.org/oquo#RawScale"/>
        <QualityModel:hasRankigFunction rdf:resource="http://purl.org/net/QualityModel#HigherBest"/>
        <obo:IAO_0000115>The number of lexical regularities appearing in the ontology over the number of classes.</obo:IAO_0000115>
        <rdfs:label>lexical regularities per class metric scale</rdfs:label>
    </owl:NamedIndividual>
    


    <!-- https://purl.archive.org/oquo#LexicalRegularityClassPercentageMetricScale -->

    <owl:NamedIndividual rdf:about="https://purl.archive.org/oquo#LexicalRegularityClassPercentageMetricScale">
        <rdf:type rdf:resource="http://www.wurvoc.org/vocabularies/om-1.8/Ratio_scale"/>
        <rdf:type rdf:resource="https://purl.archive.org/oquo#RawScale"/>
        <QualityModel:hasRankigFunction rdf:resource="http://purl.org/net/QualityModel#HigherBest"/>
        <obo:IAO_0000115>The percentage of classes in the ontology that are LR classes.</obo:IAO_0000115>
        <rdfs:label>lexical resularity class percentage metric scale</rdfs:label>
    </owl:NamedIndividual>
    


    <!-- https://purl.archive.org/oquo#LexicallySuggestLogicallyDefineMetricScale -->

    <owl:NamedIndividual rdf:about="https://purl.archive.org/oquo#LexicallySuggestLogicallyDefineMetricScale">
        <rdf:type rdf:resource="http://www.wurvoc.org/vocabularies/om-1.8/Ratio_scale"/>
        <rdf:type rdf:resource="https://purl.archive.org/oquo#RawScale"/>
        <QualityModel:hasRankigFunction rdf:resource="http://purl.org/net/QualityModel#HigherBest"/>
        <obo:IAO_0000115>The degree in which LR classes are semantically linked to the classes exhibiting the corresponding lexical regularity.</obo:IAO_0000115>
        <rdfs:label>lexically suggest logically define metric scale</rdfs:label>
    </owl:NamedIndividual>
    


    <!-- https://purl.archive.org/oquo#NamesPerAnnotationPropertyMetricScale -->

    <owl:NamedIndividual rdf:about="https://purl.archive.org/oquo#NamesPerAnnotationPropertyMetricScale">
        <rdf:type rdf:resource="http://www.wurvoc.org/vocabularies/om-1.8/Ratio_scale"/>
        <rdf:type rdf:resource="https://purl.archive.org/oquo#RawScale"/>
        <QualityModel:hasRankigFunction rdf:resource="http://purl.org/net/QualityModel#HigherBest"/>
        <obo:IAO_0000115>The total number of annotation property names over the total number of annotation properties.</obo:IAO_0000115>
        <rdfs:label>names per annotation property metrics scale</rdfs:label>
    </owl:NamedIndividual>
    


    <!-- https://purl.archive.org/oquo#NamesPerClassMetricScale -->

    <owl:NamedIndividual rdf:about="https://purl.archive.org/oquo#NamesPerClassMetricScale">
        <rdf:type rdf:resource="http://www.wurvoc.org/vocabularies/om-1.8/Ratio_scale"/>
        <rdf:type rdf:resource="https://purl.archive.org/oquo#RawScale"/>
        <QualityModel:hasRankigFunction rdf:resource="http://purl.org/net/QualityModel#HigherBest"/>
        <obo:IAO_0000115>The total number of class names over the total number of classes.</obo:IAO_0000115>
        <rdfs:label>names per class metric scale</rdfs:label>
    </owl:NamedIndividual>
    


    <!-- https://purl.archive.org/oquo#NamesPerDataPropertyMetricScale -->

    <owl:NamedIndividual rdf:about="https://purl.archive.org/oquo#NamesPerDataPropertyMetricScale">
        <rdf:type rdf:resource="http://www.wurvoc.org/vocabularies/om-1.8/Ratio_scale"/>
        <rdf:type rdf:resource="https://purl.archive.org/oquo#RawScale"/>
        <QualityModel:hasRankigFunction rdf:resource="http://purl.org/net/QualityModel#HigherBest"/>
        <obo:IAO_0000115>The total number of data property names over the total number of data properties.</obo:IAO_0000115>
        <rdfs:label>names per data property metric scale</rdfs:label>
    </owl:NamedIndividual>
    


    <!-- https://purl.archive.org/oquo#NamesPerObjectPropertyMetricScale -->

    <owl:NamedIndividual rdf:about="https://purl.archive.org/oquo#NamesPerObjectPropertyMetricScale">
        <rdf:type rdf:resource="http://www.wurvoc.org/vocabularies/om-1.8/Ratio_scale"/>
        <rdf:type rdf:resource="https://purl.archive.org/oquo#RawScale"/>
        <QualityModel:hasRankigFunction rdf:resource="http://purl.org/net/QualityModel#HigherBest"/>
        <obo:IAO_0000115>The total number of object property names over the total number of object properties.</obo:IAO_0000115>
        <rdfs:label>names per object property metric scale</rdfs:label>
    </owl:NamedIndividual>
    


    <!-- https://purl.archive.org/oquo#NamesPerPropertyMetricScale -->

    <owl:NamedIndividual rdf:about="https://purl.archive.org/oquo#NamesPerPropertyMetricScale">
        <rdf:type rdf:resource="http://www.wurvoc.org/vocabularies/om-1.8/Ratio_scale"/>
        <rdf:type rdf:resource="https://purl.archive.org/oquo#RawScale"/>
        <QualityModel:hasRankigFunction rdf:resource="http://purl.org/net/QualityModel#HigherBest"/>
        <obo:IAO_0000115>The total number of property names over the total number of properties.</obo:IAO_0000115>
        <rdfs:label>names per property metric scale</rdfs:label>
    </owl:NamedIndividual>
    

    

    


    <!-- https://purl.archive.org/oquo#NumberOfClassesMetricScale -->

    <owl:NamedIndividual rdf:about="https://purl.archive.org/oquo#NumberOfClassesMetricScale">
        <rdf:type rdf:resource="http://www.wurvoc.org/vocabularies/om-1.8/Ratio_scale"/>
        <rdf:type rdf:resource="https://purl.archive.org/oquo#RawScale"/>
        <obo:IAO_0000115>The number of classes in the ontology.</obo:IAO_0000115>
        <rdfs:label>number of classes metric scale</rdfs:label>
    </owl:NamedIndividual>
    


    <!-- https://purl.archive.org/oquo#NumberOfLexicalRegularitiesMetricScale -->

    <owl:NamedIndividual rdf:about="https://purl.archive.org/oquo#NumberOfLexicalRegularitiesMetricScale">
        <rdf:type rdf:resource="http://www.wurvoc.org/vocabularies/om-1.8/Ratio_scale"/>
        <rdf:type rdf:resource="https://purl.archive.org/oquo#RawScale"/>
        <QualityModel:hasRankigFunction rdf:resource="http://purl.org/net/QualityModel#HigherBest"/>
        <obo:IAO_0000115>The number of lexical regularities found in the ontology.</obo:IAO_0000115>
        <rdfs:label>number of lexical regularities metric scale</rdfs:label>
    </owl:NamedIndividual>
    


    <!-- https://purl.archive.org/oquo#NumberOfLexicalRegularityClassesMetricScale -->

    <owl:NamedIndividual rdf:about="https://purl.archive.org/oquo#NumberOfLexicalRegularityClassesMetricScale">
        <rdf:type rdf:resource="http://www.wurvoc.org/vocabularies/om-1.8/Ratio_scale"/>
        <rdf:type rdf:resource="https://purl.archive.org/oquo#RawScale"/>
        <QualityModel:hasRankigFunction rdf:resource="http://purl.org/net/QualityModel#HigherBest"/>
        <obo:IAO_0000115>The number of ontology classes whose name is a lexical regularity.</obo:IAO_0000115>
        <rdfs:label>number of lexical regularity classes metric scale</rdfs:label>
    </owl:NamedIndividual>
    
    


    <!-- https://purl.archive.org/oquo#ObjectPropertiesWithNoDescriptionMetricScale -->

    <owl:NamedIndividual rdf:about="https://purl.archive.org/oquo#ObjectPropertiesWithNoDescriptionMetricScale">
        <rdf:type rdf:resource="http://www.wurvoc.org/vocabularies/om-1.8/Ratio_scale"/>
        <rdf:type rdf:resource="https://purl.archive.org/oquo#RawScale"/>
        <QualityModel:hasRankigFunction rdf:resource="http://purl.org/net/QualityModel#LowerBest"/>
        <obo:IAO_0000115>The number  of object properties lacking a description over the number of object properties considered.</obo:IAO_0000115>
        <rdfs:label>object properties with no description metric scale</rdfs:label>
    </owl:NamedIndividual>
    


    <!-- https://purl.archive.org/oquo#ObjectPropertiesWithNoNameMetricScale -->

    <owl:NamedIndividual rdf:about="https://purl.archive.org/oquo#ObjectPropertiesWithNoNameMetricScale">
        <rdf:type rdf:resource="http://www.wurvoc.org/vocabularies/om-1.8/Ratio_scale"/>
        <rdf:type rdf:resource="https://purl.archive.org/oquo#RawScale"/>
        <QualityModel:hasRankigFunction rdf:resource="http://purl.org/net/QualityModel#LowerBest"/>
        <obo:IAO_0000115>The number of object properties lacking a name over the number of object properties considered.</obo:IAO_0000115>
        <rdfs:label>object properties with no name metric scale</rdfs:label>
    </owl:NamedIndividual>
    


    <!-- https://purl.archive.org/oquo#ObjectPropertiesWithNoSynonymMetricScale -->

    <owl:NamedIndividual rdf:about="https://purl.archive.org/oquo#ObjectPropertiesWithNoSynonymMetricScale">
        <rdf:type rdf:resource="http://www.wurvoc.org/vocabularies/om-1.8/Ratio_scale"/>
        <rdf:type rdf:resource="https://purl.archive.org/oquo#RawScale"/>
        <QualityModel:hasRankigFunction rdf:resource="http://purl.org/net/QualityModel#LowerBest"/>
        <obo:IAO_0000115>The number of object properties lacking a synonym over the number of object properties considered.</obo:IAO_0000115>
        <rdfs:label>object properties with no synonym metric scale</rdfs:label>
    </owl:NamedIndividual>
    


    



    <!-- https://purl.archive.org/oquo#SynonymsPerAnnotationPropertyMetricScale -->

    <owl:NamedIndividual rdf:about="https://purl.archive.org/oquo#SynonymsPerAnnotationPropertyMetricScale">
        <rdf:type rdf:resource="http://www.wurvoc.org/vocabularies/om-1.8/Ratio_scale"/>
        <rdf:type rdf:resource="https://purl.archive.org/oquo#RawScale"/>
        <QualityModel:hasRankigFunction rdf:resource="http://purl.org/net/QualityModel#HigherBest"/>
        <obo:IAO_0000115>The total number of annotation property synonyms over the total number of annotation properties.</obo:IAO_0000115>
        <rdfs:label>synonyms per annotation property metric scale</rdfs:label>
    </owl:NamedIndividual>
    


    <!-- https://purl.archive.org/oquo#SynonymsPerClassMetricScale -->

    <owl:NamedIndividual rdf:about="https://purl.archive.org/oquo#SynonymsPerClassMetricScale">
        <rdf:type rdf:resource="http://www.wurvoc.org/vocabularies/om-1.8/Ratio_scale"/>
        <rdf:type rdf:resource="https://purl.archive.org/oquo#RawScale"/>
        <QualityModel:hasRankigFunction rdf:resource="http://purl.org/net/QualityModel#HigherBest"/>
        <obo:IAO_0000115>The total number of class synonyms over the total number of classes.</obo:IAO_0000115>
        <rdfs:label>synonyms per class metric scale</rdfs:label>
    </owl:NamedIndividual>
    


    <!-- https://purl.archive.org/oquo#SynonymsPerDataPropertyMetricScale -->

    <owl:NamedIndividual rdf:about="https://purl.archive.org/oquo#SynonymsPerDataPropertyMetricScale">
        <rdf:type rdf:resource="http://www.wurvoc.org/vocabularies/om-1.8/Ratio_scale"/>
        <rdf:type rdf:resource="https://purl.archive.org/oquo#RawScale"/>
        <QualityModel:hasRankigFunction rdf:resource="http://purl.org/net/QualityModel#HigherBest"/>
        <obo:IAO_0000115>The total number of data property synonyms over the total number of data properties.</obo:IAO_0000115>
        <rdfs:label>synonyms per data property metric scale</rdfs:label>
    </owl:NamedIndividual>
    


    <!-- https://purl.archive.org/oquo#SynonymsPerObjectPropertyMetricScale -->

    <owl:NamedIndividual rdf:about="https://purl.archive.org/oquo#SynonymsPerObjectPropertyMetricScale">
        <rdf:type rdf:resource="http://www.wurvoc.org/vocabularies/om-1.8/Ratio_scale"/>
        <rdf:type rdf:resource="https://purl.archive.org/oquo#RawScale"/>
        <QualityModel:hasRankigFunction rdf:resource="http://purl.org/net/QualityModel#HigherBest"/>
        <obo:IAO_0000115>The total number of object property synonyms over the total number of object properties.</obo:IAO_0000115>
        <rdfs:label>synonyms per object property metric scale</rdfs:label>
    </owl:NamedIndividual>
    


    <!-- https://purl.archive.org/oquo#SynonymsPerPropertyMetricScale -->

    <owl:NamedIndividual rdf:about="https://purl.archive.org/oquo#SynonymsPerPropertyMetricScale">
        <rdf:type rdf:resource="http://www.wurvoc.org/vocabularies/om-1.8/Ratio_scale"/>
        <rdf:type rdf:resource="https://purl.archive.org/oquo#RawScale"/>
        <QualityModel:hasRankigFunction rdf:resource="http://purl.org/net/QualityModel#HigherBest"/>
        <obo:IAO_0000115>The total number of property synonyms over the total number of properties, including data, object and annotation properties.</obo:IAO_0000115>
        <rdfs:label>synonyms per property metric scale</rdfs:label>
    </owl:NamedIndividual>
    


    <!-- https://purl.archive.org/oquo#SystematicNamingMetricScale -->

    <owl:NamedIndividual rdf:about="https://purl.archive.org/oquo#SystematicNamingMetricScale">
        <rdf:type rdf:resource="http://www.wurvoc.org/vocabularies/om-1.8/Ratio_scale"/>
        <rdf:type rdf:resource="https://purl.archive.org/oquo#RawScale"/>
        <QualityModel:hasRankigFunction rdf:resource="http://purl.org/net/QualityModel#HigherBest"/>
        <obo:IAO_0000115>The degree in which hierarchies under LR classes exhibit the lexical regularity of the parent class.</obo:IAO_0000115>
        <rdfs:label>systematic naming metric scale</rdfs:label>
    </owl:NamedIndividual>
    



    


    <!-- 
    ///////////////////////////////////////////////////////////////////////////////////////
    //
    // General axioms
    //
    ///////////////////////////////////////////////////////////////////////////////////////
     -->

    <rdf:Description>
        <rdf:type rdf:resource="http://www.w3.org/2002/07/owl#AllDisjointClasses"/>
        <owl:members rdf:parseType="Collection">
            <rdf:Description rdf:about="https://purl.archive.org/oquo#AnnotationPropertiesWithNoDescriptionMetric"/>
            <rdf:Description rdf:about="https://purl.archive.org/oquo#AnnotationPropertiesWithNoNameMetric"/>
            <rdf:Description rdf:about="https://purl.archive.org/oquo#AnnotationPropertiesWithNoSynonymMetric"/>
            <rdf:Description rdf:about="https://purl.archive.org/oquo#ClassesWithNoDescriptionMetric"/>
            <rdf:Description rdf:about="https://purl.archive.org/oquo#ClassesWithNoNameMetric"/>
            <rdf:Description rdf:about="https://purl.archive.org/oquo#ClassesWithNoSynonymMetric"/>
            <rdf:Description rdf:about="https://purl.archive.org/oquo#DataPropertiesWithNoDescriptionMetric"/>
            <rdf:Description rdf:about="https://purl.archive.org/oquo#DataPropertiesWithNoNameMetric"/>
            <rdf:Description rdf:about="https://purl.archive.org/oquo#DataPropertiesWithNoSynonymMetric"/>
            <rdf:Description rdf:about="https://purl.archive.org/oquo#DescriptionsPerAnnotationPropertyMetric"/>
            <rdf:Description rdf:about="https://purl.archive.org/oquo#DescriptionsPerClassMetric"/>
            <rdf:Description rdf:about="https://purl.archive.org/oquo#DescriptionsPerDataPropertyMetric"/>
            <rdf:Description rdf:about="https://purl.archive.org/oquo#DescriptionsPerObjectPropertyMetric"/>
            <rdf:Description rdf:about="https://purl.archive.org/oquo#DescriptionsPerPropertyMetric"/>
            <rdf:Description rdf:about="https://purl.archive.org/oquo#LexicalRegularitiesPerClassMetric"/>
            <rdf:Description rdf:about="https://purl.archive.org/oquo#LexicalRegularityClassPercentageMetric"/>
            <rdf:Description rdf:about="https://purl.archive.org/oquo#LexicallySuggestLogicallyDefineMetric"/>
            <rdf:Description rdf:about="https://purl.archive.org/oquo#NamesPerAnnotationPropertyMetric"/>
            <rdf:Description rdf:about="https://purl.archive.org/oquo#NamesPerClassMetric"/>
            <rdf:Description rdf:about="https://purl.archive.org/oquo#NamesPerDataPropertyMetric"/>
            <rdf:Description rdf:about="https://purl.archive.org/oquo#NamesPerObjectPropertyMetric"/>
            <rdf:Description rdf:about="https://purl.archive.org/oquo#NamesPerPropertyMetric"/>
            <rdf:Description rdf:about="https://purl.archive.org/oquo#NumberOfLexicalRegularitiesMetric"/>
            <rdf:Description rdf:about="https://purl.archive.org/oquo#NumberOfLexicalRegularityClassesMetric"/>
            <rdf:Description rdf:about="https://purl.archive.org/oquo#ObjectPropertiesWithNoDescriptionMetric"/>
            <rdf:Description rdf:about="https://purl.archive.org/oquo#ObjectPropertiesWithNoNameMetric"/>
            <rdf:Description rdf:about="https://purl.archive.org/oquo#ObjectPropertiesWithNoSynonymMetric"/>
            <rdf:Description rdf:about="https://purl.archive.org/oquo#SynonymsPerAnnotationPropertyMetric"/>
            <rdf:Description rdf:about="https://purl.archive.org/oquo#SynonymsPerClassMetric"/>
            <rdf:Description rdf:about="https://purl.archive.org/oquo#SynonymsPerDataPropertyMetric"/>
            <rdf:Description rdf:about="https://purl.archive.org/oquo#SynonymsPerObjectPropertyMetric"/>
            <rdf:Description rdf:about="https://purl.archive.org/oquo#SynonymsPerPropertyMetric"/>
            <rdf:Description rdf:about="https://purl.archive.org/oquo#SystematicNamingMetric"/>
        </owl:members>
    </rdf:Description>
</rdf:RDF>



<!-- Generated by the OWL API (version 4.5.9.2019-02-01T07:24:44Z) https://github.com/owlcs/owlapi -->

